<?xml version="1.0"?>
<rdf:RDF xmlns="https://raw.githubusercontent.com/sustainable-processes/ontology/refs/heads/main/OntoCAPE/supporting_concepts/geometry/geometry.owl#"
     xml:base="https://raw.githubusercontent.com/sustainable-processes/ontology/refs/heads/main/OntoCAPE/supporting_concepts/geometry/geometry.owl"
     xmlns:owl="http://www.w3.org/2002/07/owl#"
     xmlns:rdf="http://www.w3.org/1999/02/22-rdf-syntax-ns#"
     xmlns:xml="http://www.w3.org/XML/1998/namespace"
     xmlns:xsd="http://www.w3.org/2001/XMLSchema#"
     xmlns:rdfs="http://www.w3.org/2000/01/rdf-schema#"
     xmlns:root="https://raw.githubusercontent.com/sustainable-processes/ontology/refs/heads/main/OntoCAPE/"
     xmlns:terms="http://purl.org/dc/terms/"
     xmlns:system="https://raw.githubusercontent.com/sustainable-processes/ontology/refs/heads/main/OntoCAPE/upper_level/system.owl#"
     xmlns:der_dim="https://raw.githubusercontent.com/sustainable-processes/ontology/refs/heads/main/OntoCAPE/supporting_concepts/physical_dimension/derived_dimensions.owl#"
     xmlns:geometry="https://raw.githubusercontent.com/sustainable-processes/ontology/refs/heads/main/OntoCAPE/supporting_concepts/geometry/geometry.owl"
     xmlns:phys_dim="https://raw.githubusercontent.com/sustainable-processes/ontology/refs/heads/main/OntoCAPE/supporting_concepts/physical_dimension/physical_dimension.owl">
    <owl:Ontology rdf:about="https://raw.githubusercontent.com/sustainable-processes/ontology/refs/heads/main/OntoCAPE/supporting_concepts/geometry/geometry.owl">
        <owl:imports rdf:resource="https://raw.githubusercontent.com/sustainable-processes/ontology/refs/heads/main/OntoCAPE/supporting_concepts/physical_dimension/derived_dimensions.owl"/>
        <terms:license>Copyright (C) [2009] [Andreas Wiesner]
                This program is free software; you can redistribute it and/or modify it under the terms of the GNU General Public License as published by the Free Software Foundation; either version 3 of the License, or (at your option) any later version.
                This program is distributed in the hope that it will be useful, but WITHOUT ANY WARRANTY; without even the implied warranty of MERCHANTABILITY or FITNESS FOR A PARTICULAR PURPOSE. See the GNU General Public License for more details.
                You should have received a copy of the GNU General Public License along with this program; if not, see &lt;http://www.gnu.org/licenses/&gt;.
</terms:license>
        <rdfs:comment>The ontology module &apos;geometry&apos; introduces some  geometric concpets for the representation of surfaces and geometric solids.
The following classes, relations, and individuals from other ontology modules are used within &apos;geometry&apos;:

&lt;owl:Class rdf:about=&quot;https://raw.githubusercontent.com/sustainable-processes/ontology/refs/heads/main/OntoCAPE/upper_level/system.owl#PhysicalQuantity&quot;/&gt;
&lt;owl:Class rdf:about=&quot;https://raw.githubusercontent.com/sustainable-processes/ontology/refs/heads/main/OntoCAPE/upper_level/system.owl#ScalarQuantity&quot;/&gt;
&lt;owl:Class rdf:about=&quot;https://raw.githubusercontent.com/sustainable-processes/ontology/refs/heads/main/OntoCAPE/upper_level/system.owl#System&quot;/&gt;

&lt;owl:ObjectProperty rdf:about=&quot;https://raw.githubusercontent.com/sustainable-processes/ontology/refs/heads/main/OntoCAPE/upper_level/system.owl#hasAspectSystem&quot;/&gt;
&lt;owl:ObjectProperty rdf:about=&quot;https://raw.githubusercontent.com/sustainable-processes/ontology/refs/heads/main/OntoCAPE/upper_level/system.owl#hasDimension&quot;/&gt;
&lt;owl:ObjectProperty rdf:about=&quot;https://raw.githubusercontent.com/sustainable-processes/ontology/refs/heads/main/OntoCAPE/upper_level/system.owl#hasProperty&quot;/&gt;
&lt;owl:ObjectProperty rdf:about=&quot;https://raw.githubusercontent.com/sustainable-processes/ontology/refs/heads/main/OntoCAPE/upper_level/system.owl#isPropertyOf&quot;/&gt;
&lt;owl:ObjectProperty rdf:about=&quot;https://raw.githubusercontent.com/sustainable-processes/ontology/refs/heads/main/OntoCAPE/upper_level/system.owl#representsAspectOf&quot;/&gt;

&lt;der_dim:SpaceAndTime    rdf:about=&quot;https://raw.githubusercontent.com/sustainable-processes/ontology/refs/heads/main/OntoCAPE/supporting_concepts/physical_dimension/derived_dimensions.owl#area&quot;/&gt;
&lt;der_dim:SpaceAndTime    rdf:about=&quot;https://raw.githubusercontent.com/sustainable-processes/ontology/refs/heads/main/OntoCAPE/supporting_concepts/physical_dimension/derived_dimensions.owl#volume&quot;/&gt;
&lt;phys_dim:BaseDimension  rdf:about=&quot;https://raw.githubusercontent.com/sustainable-processes/ontology/refs/heads/main/OntoCAPE/supporting_concepts/physical_dimension/physical_dimension.owl#length&quot;/&gt;</rdfs:comment>
        <owl:versionInfo>2.0</owl:versionInfo>
    </owl:Ontology>
    


    <!-- 
    ///////////////////////////////////////////////////////////////////////////////////////
    //
    // Annotation properties
    //
    ///////////////////////////////////////////////////////////////////////////////////////
     -->

    


    <!-- http://purl.org/dc/terms/license -->

    <owl:AnnotationProperty rdf:about="http://purl.org/dc/terms/license"/>
    


    <!-- 
    ///////////////////////////////////////////////////////////////////////////////////////
    //
    // Object Properties
    //
    ///////////////////////////////////////////////////////////////////////////////////////
     -->

    


    <!-- https://raw.githubusercontent.com/sustainable-processes/ontology/refs/heads/main/OntoCAPE/supporting_concepts/geometry/geometry.owl#hasShapeRepresentation -->

    <owl:ObjectProperty rdf:about="https://raw.githubusercontent.com/sustainable-processes/ontology/refs/heads/main/OntoCAPE/supporting_concepts/geometry/geometry.owl#hasShapeRepresentation">
        <rdfs:subPropertyOf rdf:resource="https://raw.githubusercontent.com/sustainable-processes/ontology/refs/heads/main/OntoCAPE/upper_level/system.owl#hasAspectSystem"/>
        <owl:inverseOf rdf:resource="https://raw.githubusercontent.com/sustainable-processes/ontology/refs/heads/main/OntoCAPE/supporting_concepts/geometry/geometry.owl#representsShapeOf"/>
        <rdfs:range rdf:resource="https://raw.githubusercontent.com/sustainable-processes/ontology/refs/heads/main/OntoCAPE/supporting_concepts/geometry/geometry.owl#Solid"/>
        <rdfs:comment>points from a System to the Solid that represents its geometry</rdfs:comment>
    </owl:ObjectProperty>
    


    <!-- https://raw.githubusercontent.com/sustainable-processes/ontology/refs/heads/main/OntoCAPE/supporting_concepts/geometry/geometry.owl#hasSurfaceGeometry -->

    <owl:ObjectProperty rdf:about="https://raw.githubusercontent.com/sustainable-processes/ontology/refs/heads/main/OntoCAPE/supporting_concepts/geometry/geometry.owl#hasSurfaceGeometry">
        <rdfs:subPropertyOf rdf:resource="https://raw.githubusercontent.com/sustainable-processes/ontology/refs/heads/main/OntoCAPE/upper_level/system.owl#hasAspectSystem"/>
        <owl:inverseOf rdf:resource="https://raw.githubusercontent.com/sustainable-processes/ontology/refs/heads/main/OntoCAPE/supporting_concepts/geometry/geometry.owl#representsSurfaceGeometryOf"/>
        <rdfs:range rdf:resource="https://raw.githubusercontent.com/sustainable-processes/ontology/refs/heads/main/OntoCAPE/supporting_concepts/geometry/geometry.owl#Surface"/>
        <rdfs:comment>points from a System to the Surface that represents its geometry</rdfs:comment>
    </owl:ObjectProperty>
    


    <!-- https://raw.githubusercontent.com/sustainable-processes/ontology/refs/heads/main/OntoCAPE/supporting_concepts/geometry/geometry.owl#has_area -->

    <owl:ObjectProperty rdf:about="https://raw.githubusercontent.com/sustainable-processes/ontology/refs/heads/main/OntoCAPE/supporting_concepts/geometry/geometry.owl#has_area">
        <rdfs:subPropertyOf rdf:resource="https://raw.githubusercontent.com/sustainable-processes/ontology/refs/heads/main/OntoCAPE/upper_level/system.owl#hasProperty"/>
        <rdfs:domain>
            <owl:Class>
                <owl:unionOf rdf:parseType="Collection">
                    <rdf:Description rdf:about="https://raw.githubusercontent.com/sustainable-processes/ontology/refs/heads/main/OntoCAPE/supporting_concepts/geometry/geometry.owl#Solid"/>
                    <rdf:Description rdf:about="https://raw.githubusercontent.com/sustainable-processes/ontology/refs/heads/main/OntoCAPE/supporting_concepts/geometry/geometry.owl#Surface"/>
                </owl:unionOf>
            </owl:Class>
        </rdfs:domain>
        <rdfs:range rdf:resource="https://raw.githubusercontent.com/sustainable-processes/ontology/refs/heads/main/OntoCAPE/supporting_concepts/geometry/geometry.owl#SurfaceArea"/>
        <rdfs:comment>workaround for QCR which is a feature of modeling currently not available from OWL.</rdfs:comment>
    </owl:ObjectProperty>
    


    <!-- https://raw.githubusercontent.com/sustainable-processes/ontology/refs/heads/main/OntoCAPE/supporting_concepts/geometry/geometry.owl#has_length -->

    <owl:ObjectProperty rdf:about="https://raw.githubusercontent.com/sustainable-processes/ontology/refs/heads/main/OntoCAPE/supporting_concepts/geometry/geometry.owl#has_length">
        <rdfs:subPropertyOf rdf:resource="https://raw.githubusercontent.com/sustainable-processes/ontology/refs/heads/main/OntoCAPE/upper_level/system.owl#hasProperty"/>
        <rdfs:domain>
            <owl:Class>
                <owl:unionOf rdf:parseType="Collection">
                    <rdf:Description rdf:about="https://raw.githubusercontent.com/sustainable-processes/ontology/refs/heads/main/OntoCAPE/supporting_concepts/geometry/geometry.owl#Solid"/>
                    <rdf:Description rdf:about="https://raw.githubusercontent.com/sustainable-processes/ontology/refs/heads/main/OntoCAPE/supporting_concepts/geometry/geometry.owl#Surface"/>
                </owl:unionOf>
            </owl:Class>
        </rdfs:domain>
        <rdfs:range>
            <owl:Class>
                <owl:unionOf rdf:parseType="Collection">
                    <rdf:Description rdf:about="https://raw.githubusercontent.com/sustainable-processes/ontology/refs/heads/main/OntoCAPE/supporting_concepts/geometry/geometry.owl#Diameter"/>
                    <rdf:Description rdf:about="https://raw.githubusercontent.com/sustainable-processes/ontology/refs/heads/main/OntoCAPE/supporting_concepts/geometry/geometry.owl#EdgeLength"/>
                    <rdf:Description rdf:about="https://raw.githubusercontent.com/sustainable-processes/ontology/refs/heads/main/OntoCAPE/supporting_concepts/geometry/geometry.owl#Height"/>
                    <rdf:Description rdf:about="https://raw.githubusercontent.com/sustainable-processes/ontology/refs/heads/main/OntoCAPE/supporting_concepts/geometry/geometry.owl#Radius"/>
                </owl:unionOf>
            </owl:Class>
        </rdfs:range>
        <rdfs:comment>workaround for QCR which is a feature of modeling currently not available from OWL.</rdfs:comment>
    </owl:ObjectProperty>
    


    <!-- https://raw.githubusercontent.com/sustainable-processes/ontology/refs/heads/main/OntoCAPE/supporting_concepts/geometry/geometry.owl#has_volume -->

    <owl:ObjectProperty rdf:about="https://raw.githubusercontent.com/sustainable-processes/ontology/refs/heads/main/OntoCAPE/supporting_concepts/geometry/geometry.owl#has_volume">
        <rdfs:subPropertyOf rdf:resource="https://raw.githubusercontent.com/sustainable-processes/ontology/refs/heads/main/OntoCAPE/upper_level/system.owl#hasProperty"/>
        <rdfs:domain rdf:resource="https://raw.githubusercontent.com/sustainable-processes/ontology/refs/heads/main/OntoCAPE/supporting_concepts/geometry/geometry.owl#Solid"/>
        <rdfs:range rdf:resource="https://raw.githubusercontent.com/sustainable-processes/ontology/refs/heads/main/OntoCAPE/supporting_concepts/geometry/geometry.owl#Volume"/>
        <rdfs:comment>workaround for QCR which is a feature of modeling currently not available from OWL.</rdfs:comment>
    </owl:ObjectProperty>
    


    <!-- https://raw.githubusercontent.com/sustainable-processes/ontology/refs/heads/main/OntoCAPE/supporting_concepts/geometry/geometry.owl#representsShapeOf -->

    <owl:ObjectProperty rdf:about="https://raw.githubusercontent.com/sustainable-processes/ontology/refs/heads/main/OntoCAPE/supporting_concepts/geometry/geometry.owl#representsShapeOf">
        <rdfs:subPropertyOf rdf:resource="https://raw.githubusercontent.com/sustainable-processes/ontology/refs/heads/main/OntoCAPE/upper_level/system.owl#representsAspectOf"/>
        <rdfs:domain rdf:resource="https://raw.githubusercontent.com/sustainable-processes/ontology/refs/heads/main/OntoCAPE/supporting_concepts/geometry/geometry.owl#Solid"/>
        <rdfs:comment>points from a Solid to the System whose geometry the Solid represents</rdfs:comment>
    </owl:ObjectProperty>
    


    <!-- https://raw.githubusercontent.com/sustainable-processes/ontology/refs/heads/main/OntoCAPE/supporting_concepts/geometry/geometry.owl#representsSurfaceGeometryOf -->

    <owl:ObjectProperty rdf:about="https://raw.githubusercontent.com/sustainable-processes/ontology/refs/heads/main/OntoCAPE/supporting_concepts/geometry/geometry.owl#representsSurfaceGeometryOf">
        <rdfs:subPropertyOf rdf:resource="https://raw.githubusercontent.com/sustainable-processes/ontology/refs/heads/main/OntoCAPE/upper_level/system.owl#representsAspectOf"/>
        <rdfs:domain rdf:resource="https://raw.githubusercontent.com/sustainable-processes/ontology/refs/heads/main/OntoCAPE/supporting_concepts/geometry/geometry.owl#Surface"/>
        <rdfs:comment>points from a Surface to the System whose geometry the Surface represents</rdfs:comment>
    </owl:ObjectProperty>
    


    <!-- https://raw.githubusercontent.com/sustainable-processes/ontology/refs/heads/main/OntoCAPE/upper_level/system.owl#hasAspectSystem -->

    <owl:ObjectProperty rdf:about="https://raw.githubusercontent.com/sustainable-processes/ontology/refs/heads/main/OntoCAPE/upper_level/system.owl#hasAspectSystem"/>
    


    <!-- https://raw.githubusercontent.com/sustainable-processes/ontology/refs/heads/main/OntoCAPE/upper_level/system.owl#hasDimension -->

    <owl:ObjectProperty rdf:about="https://raw.githubusercontent.com/sustainable-processes/ontology/refs/heads/main/OntoCAPE/upper_level/system.owl#hasDimension"/>
    


    <!-- https://raw.githubusercontent.com/sustainable-processes/ontology/refs/heads/main/OntoCAPE/upper_level/system.owl#hasProperty -->

    <owl:ObjectProperty rdf:about="https://raw.githubusercontent.com/sustainable-processes/ontology/refs/heads/main/OntoCAPE/upper_level/system.owl#hasProperty"/>
    


    <!-- https://raw.githubusercontent.com/sustainable-processes/ontology/refs/heads/main/OntoCAPE/upper_level/system.owl#isPropertyOf -->

    <owl:ObjectProperty rdf:about="https://raw.githubusercontent.com/sustainable-processes/ontology/refs/heads/main/OntoCAPE/upper_level/system.owl#isPropertyOf"/>
    


    <!-- https://raw.githubusercontent.com/sustainable-processes/ontology/refs/heads/main/OntoCAPE/upper_level/system.owl#representsAspectOf -->

    <owl:ObjectProperty rdf:about="https://raw.githubusercontent.com/sustainable-processes/ontology/refs/heads/main/OntoCAPE/upper_level/system.owl#representsAspectOf"/>
    


    <!-- 
    ///////////////////////////////////////////////////////////////////////////////////////
    //
    // Classes
    //
    ///////////////////////////////////////////////////////////////////////////////////////
     -->

    


    <!-- https://raw.githubusercontent.com/sustainable-processes/ontology/refs/heads/main/OntoCAPE/supporting_concepts/geometry/geometry.owl#BaseArea -->

    <owl:Class rdf:about="https://raw.githubusercontent.com/sustainable-processes/ontology/refs/heads/main/OntoCAPE/supporting_concepts/geometry/geometry.owl#BaseArea">
        <rdfs:subClassOf rdf:resource="https://raw.githubusercontent.com/sustainable-processes/ontology/refs/heads/main/OntoCAPE/supporting_concepts/geometry/geometry.owl#SideArea"/>
        <owl:disjointWith rdf:resource="https://raw.githubusercontent.com/sustainable-processes/ontology/refs/heads/main/OntoCAPE/supporting_concepts/geometry/geometry.owl#LateralSurfaceArea"/>
        <rdfs:comment>The base is the bottom of a solid. If the top is parallel to the bottom (as in a trapezoid or prism), both the top and bottom are called bases. The BaseArea is the SurfaceArea of (one of) the base(s).</rdfs:comment>
    </owl:Class>
    


    <!-- https://raw.githubusercontent.com/sustainable-processes/ontology/refs/heads/main/OntoCAPE/supporting_concepts/geometry/geometry.owl#Cone -->

    <owl:Class rdf:about="https://raw.githubusercontent.com/sustainable-processes/ontology/refs/heads/main/OntoCAPE/supporting_concepts/geometry/geometry.owl#Cone">
        <rdfs:subClassOf rdf:resource="https://raw.githubusercontent.com/sustainable-processes/ontology/refs/heads/main/OntoCAPE/supporting_concepts/geometry/geometry.owl#Solid"/>
        <rdfs:subClassOf>
            <owl:Restriction>
                <owl:onProperty rdf:resource="https://raw.githubusercontent.com/sustainable-processes/ontology/refs/heads/main/OntoCAPE/supporting_concepts/geometry/geometry.owl#has_area"/>
                <owl:someValuesFrom rdf:resource="https://raw.githubusercontent.com/sustainable-processes/ontology/refs/heads/main/OntoCAPE/supporting_concepts/geometry/geometry.owl#BaseArea"/>
            </owl:Restriction>
        </rdfs:subClassOf>
        <rdfs:subClassOf>
            <owl:Restriction>
                <owl:onProperty rdf:resource="https://raw.githubusercontent.com/sustainable-processes/ontology/refs/heads/main/OntoCAPE/supporting_concepts/geometry/geometry.owl#has_area"/>
                <owl:someValuesFrom rdf:resource="https://raw.githubusercontent.com/sustainable-processes/ontology/refs/heads/main/OntoCAPE/supporting_concepts/geometry/geometry.owl#LateralSurfaceArea"/>
            </owl:Restriction>
        </rdfs:subClassOf>
        <rdfs:subClassOf>
            <owl:Restriction>
                <owl:onProperty rdf:resource="https://raw.githubusercontent.com/sustainable-processes/ontology/refs/heads/main/OntoCAPE/supporting_concepts/geometry/geometry.owl#has_length"/>
                <owl:someValuesFrom rdf:resource="https://raw.githubusercontent.com/sustainable-processes/ontology/refs/heads/main/OntoCAPE/supporting_concepts/geometry/geometry.owl#Height"/>
            </owl:Restriction>
        </rdfs:subClassOf>
        <rdfs:subClassOf>
            <owl:Restriction>
                <owl:onProperty rdf:resource="https://raw.githubusercontent.com/sustainable-processes/ontology/refs/heads/main/OntoCAPE/supporting_concepts/geometry/geometry.owl#has_area"/>
                <owl:allValuesFrom>
                    <owl:Class>
                        <owl:unionOf rdf:parseType="Collection">
                            <rdf:Description rdf:about="https://raw.githubusercontent.com/sustainable-processes/ontology/refs/heads/main/OntoCAPE/supporting_concepts/geometry/geometry.owl#BaseArea"/>
                            <rdf:Description rdf:about="https://raw.githubusercontent.com/sustainable-processes/ontology/refs/heads/main/OntoCAPE/supporting_concepts/geometry/geometry.owl#LateralSurfaceArea"/>
                        </owl:unionOf>
                    </owl:Class>
                </owl:allValuesFrom>
            </owl:Restriction>
        </rdfs:subClassOf>
        <owl:disjointWith rdf:resource="https://raw.githubusercontent.com/sustainable-processes/ontology/refs/heads/main/OntoCAPE/supporting_concepts/geometry/geometry.owl#Cuboid"/>
        <owl:disjointWith rdf:resource="https://raw.githubusercontent.com/sustainable-processes/ontology/refs/heads/main/OntoCAPE/supporting_concepts/geometry/geometry.owl#Cylinder"/>
        <owl:disjointWith rdf:resource="https://raw.githubusercontent.com/sustainable-processes/ontology/refs/heads/main/OntoCAPE/supporting_concepts/geometry/geometry.owl#Sphere"/>
        <rdfs:comment>A three dimensional figure with a single base tapering to an apex. The base can be any simple closed curve. [http://www.mathwords.com/c/cone.htm]</rdfs:comment>
    </owl:Class>
    


    <!-- https://raw.githubusercontent.com/sustainable-processes/ontology/refs/heads/main/OntoCAPE/supporting_concepts/geometry/geometry.owl#Cuboid -->

    <owl:Class rdf:about="https://raw.githubusercontent.com/sustainable-processes/ontology/refs/heads/main/OntoCAPE/supporting_concepts/geometry/geometry.owl#Cuboid">
        <rdfs:subClassOf rdf:resource="https://raw.githubusercontent.com/sustainable-processes/ontology/refs/heads/main/OntoCAPE/supporting_concepts/geometry/geometry.owl#Solid"/>
        <rdfs:subClassOf>
            <owl:Restriction>
                <owl:onProperty rdf:resource="https://raw.githubusercontent.com/sustainable-processes/ontology/refs/heads/main/OntoCAPE/supporting_concepts/geometry/geometry.owl#has_area"/>
                <owl:someValuesFrom rdf:resource="https://raw.githubusercontent.com/sustainable-processes/ontology/refs/heads/main/OntoCAPE/supporting_concepts/geometry/geometry.owl#SideArea"/>
            </owl:Restriction>
        </rdfs:subClassOf>
        <rdfs:subClassOf>
            <owl:Restriction>
                <owl:onProperty rdf:resource="https://raw.githubusercontent.com/sustainable-processes/ontology/refs/heads/main/OntoCAPE/supporting_concepts/geometry/geometry.owl#has_length"/>
                <owl:someValuesFrom rdf:resource="https://raw.githubusercontent.com/sustainable-processes/ontology/refs/heads/main/OntoCAPE/supporting_concepts/geometry/geometry.owl#EdgeLength"/>
            </owl:Restriction>
        </rdfs:subClassOf>
        <rdfs:subClassOf>
            <owl:Restriction>
                <owl:onProperty rdf:resource="https://raw.githubusercontent.com/sustainable-processes/ontology/refs/heads/main/OntoCAPE/supporting_concepts/geometry/geometry.owl#has_area"/>
                <owl:allValuesFrom rdf:resource="https://raw.githubusercontent.com/sustainable-processes/ontology/refs/heads/main/OntoCAPE/supporting_concepts/geometry/geometry.owl#SideArea"/>
            </owl:Restriction>
        </rdfs:subClassOf>
        <rdfs:subClassOf>
            <owl:Restriction>
                <owl:onProperty rdf:resource="https://raw.githubusercontent.com/sustainable-processes/ontology/refs/heads/main/OntoCAPE/supporting_concepts/geometry/geometry.owl#has_length"/>
                <owl:allValuesFrom rdf:resource="https://raw.githubusercontent.com/sustainable-processes/ontology/refs/heads/main/OntoCAPE/supporting_concepts/geometry/geometry.owl#EdgeLength"/>
            </owl:Restriction>
        </rdfs:subClassOf>
        <rdfs:subClassOf>
            <owl:Restriction>
                <owl:onProperty rdf:resource="https://raw.githubusercontent.com/sustainable-processes/ontology/refs/heads/main/OntoCAPE/supporting_concepts/geometry/geometry.owl#has_area"/>
                <owl:cardinality rdf:datatype="http://www.w3.org/2001/XMLSchema#nonNegativeInteger">3</owl:cardinality>
            </owl:Restriction>
        </rdfs:subClassOf>
        <rdfs:subClassOf>
            <owl:Restriction>
                <owl:onProperty rdf:resource="https://raw.githubusercontent.com/sustainable-processes/ontology/refs/heads/main/OntoCAPE/supporting_concepts/geometry/geometry.owl#has_length"/>
                <owl:cardinality rdf:datatype="http://www.w3.org/2001/XMLSchema#nonNegativeInteger">3</owl:cardinality>
            </owl:Restriction>
        </rdfs:subClassOf>
        <owl:disjointWith rdf:resource="https://raw.githubusercontent.com/sustainable-processes/ontology/refs/heads/main/OntoCAPE/supporting_concepts/geometry/geometry.owl#Cylinder"/>
        <owl:disjointWith rdf:resource="https://raw.githubusercontent.com/sustainable-processes/ontology/refs/heads/main/OntoCAPE/supporting_concepts/geometry/geometry.owl#Sphere"/>
        <rdfs:comment>A closed box composed of three pairs of rectangular faces placed opposite each other and joined at right angles to each other, also known as a rectangular parallelepiped. [Weisstein, Eric W. &quot;Cuboid.&quot; From MathWorld--A Wolfram Web Resource. http://mathworld.wolfram.com/Cuboid.html]</rdfs:comment>
    </owl:Class>
    


    <!-- https://raw.githubusercontent.com/sustainable-processes/ontology/refs/heads/main/OntoCAPE/supporting_concepts/geometry/geometry.owl#Cylinder -->

    <owl:Class rdf:about="https://raw.githubusercontent.com/sustainable-processes/ontology/refs/heads/main/OntoCAPE/supporting_concepts/geometry/geometry.owl#Cylinder">
        <rdfs:subClassOf rdf:resource="https://raw.githubusercontent.com/sustainable-processes/ontology/refs/heads/main/OntoCAPE/supporting_concepts/geometry/geometry.owl#Solid"/>
        <rdfs:subClassOf>
            <owl:Restriction>
                <owl:onProperty rdf:resource="https://raw.githubusercontent.com/sustainable-processes/ontology/refs/heads/main/OntoCAPE/supporting_concepts/geometry/geometry.owl#has_area"/>
                <owl:someValuesFrom rdf:resource="https://raw.githubusercontent.com/sustainable-processes/ontology/refs/heads/main/OntoCAPE/supporting_concepts/geometry/geometry.owl#BaseArea"/>
            </owl:Restriction>
        </rdfs:subClassOf>
        <rdfs:subClassOf>
            <owl:Restriction>
                <owl:onProperty rdf:resource="https://raw.githubusercontent.com/sustainable-processes/ontology/refs/heads/main/OntoCAPE/supporting_concepts/geometry/geometry.owl#has_area"/>
                <owl:someValuesFrom rdf:resource="https://raw.githubusercontent.com/sustainable-processes/ontology/refs/heads/main/OntoCAPE/supporting_concepts/geometry/geometry.owl#LateralSurfaceArea"/>
            </owl:Restriction>
        </rdfs:subClassOf>
        <rdfs:subClassOf>
            <owl:Restriction>
                <owl:onProperty rdf:resource="https://raw.githubusercontent.com/sustainable-processes/ontology/refs/heads/main/OntoCAPE/supporting_concepts/geometry/geometry.owl#has_length"/>
                <owl:someValuesFrom rdf:resource="https://raw.githubusercontent.com/sustainable-processes/ontology/refs/heads/main/OntoCAPE/supporting_concepts/geometry/geometry.owl#Height"/>
            </owl:Restriction>
        </rdfs:subClassOf>
        <rdfs:subClassOf>
            <owl:Restriction>
                <owl:onProperty rdf:resource="https://raw.githubusercontent.com/sustainable-processes/ontology/refs/heads/main/OntoCAPE/supporting_concepts/geometry/geometry.owl#has_area"/>
                <owl:allValuesFrom>
                    <owl:Class>
                        <owl:unionOf rdf:parseType="Collection">
                            <rdf:Description rdf:about="https://raw.githubusercontent.com/sustainable-processes/ontology/refs/heads/main/OntoCAPE/supporting_concepts/geometry/geometry.owl#BaseArea"/>
                            <rdf:Description rdf:about="https://raw.githubusercontent.com/sustainable-processes/ontology/refs/heads/main/OntoCAPE/supporting_concepts/geometry/geometry.owl#LateralSurfaceArea"/>
                        </owl:unionOf>
                    </owl:Class>
                </owl:allValuesFrom>
            </owl:Restriction>
        </rdfs:subClassOf>
        <rdfs:subClassOf>
            <owl:Restriction>
                <owl:onProperty rdf:resource="https://raw.githubusercontent.com/sustainable-processes/ontology/refs/heads/main/OntoCAPE/supporting_concepts/geometry/geometry.owl#has_area"/>
                <owl:minCardinality rdf:datatype="http://www.w3.org/2001/XMLSchema#nonNegativeInteger">3</owl:minCardinality>
            </owl:Restriction>
        </rdfs:subClassOf>
        <owl:disjointWith rdf:resource="https://raw.githubusercontent.com/sustainable-processes/ontology/refs/heads/main/OntoCAPE/supporting_concepts/geometry/geometry.owl#Sphere"/>
        <rdfs:comment>A Solid with parallel congruent bases. The bases can be shaped like any closed plane figure (not necessarily a circle) and must be oriented identically. [http://www.mathwords.com/c/cylinder.htm]</rdfs:comment>
    </owl:Class>
    


    <!-- https://raw.githubusercontent.com/sustainable-processes/ontology/refs/heads/main/OntoCAPE/supporting_concepts/geometry/geometry.owl#Diameter -->

    <owl:Class rdf:about="https://raw.githubusercontent.com/sustainable-processes/ontology/refs/heads/main/OntoCAPE/supporting_concepts/geometry/geometry.owl#Diameter">
        <rdfs:subClassOf rdf:resource="https://raw.githubusercontent.com/sustainable-processes/ontology/refs/heads/main/OntoCAPE/upper_level/system.owl#ScalarQuantity"/>
        <rdfs:subClassOf>
            <owl:Restriction>
                <owl:onProperty rdf:resource="https://raw.githubusercontent.com/sustainable-processes/ontology/refs/heads/main/OntoCAPE/upper_level/system.owl#hasDimension"/>
                <owl:hasValue rdf:resource="https://raw.githubusercontent.com/sustainable-processes/ontology/refs/heads/main/OntoCAPE/supporting_concepts/physical_dimension/physical_dimension.owl#length"/>
            </owl:Restriction>
        </rdfs:subClassOf>
        <owl:disjointWith rdf:resource="https://raw.githubusercontent.com/sustainable-processes/ontology/refs/heads/main/OntoCAPE/supporting_concepts/geometry/geometry.owl#EdgeLength"/>
        <owl:disjointWith rdf:resource="https://raw.githubusercontent.com/sustainable-processes/ontology/refs/heads/main/OntoCAPE/supporting_concepts/geometry/geometry.owl#Height"/>
        <owl:disjointWith rdf:resource="https://raw.githubusercontent.com/sustainable-processes/ontology/refs/heads/main/OntoCAPE/supporting_concepts/geometry/geometry.owl#Radius"/>
        <owl:disjointWith rdf:resource="https://raw.githubusercontent.com/sustainable-processes/ontology/refs/heads/main/OntoCAPE/supporting_concepts/geometry/geometry.owl#TotalSurfaceArea"/>
        <owl:disjointWith rdf:resource="https://raw.githubusercontent.com/sustainable-processes/ontology/refs/heads/main/OntoCAPE/supporting_concepts/geometry/geometry.owl#Volume"/>
        <rdfs:comment>The length of a line segment between two points on a Disk or Sphere which passes through the center of the Disk or Sphere.</rdfs:comment>
    </owl:Class>
    


    <!-- https://raw.githubusercontent.com/sustainable-processes/ontology/refs/heads/main/OntoCAPE/supporting_concepts/geometry/geometry.owl#Disk -->

    <owl:Class rdf:about="https://raw.githubusercontent.com/sustainable-processes/ontology/refs/heads/main/OntoCAPE/supporting_concepts/geometry/geometry.owl#Disk">
        <rdfs:subClassOf rdf:resource="https://raw.githubusercontent.com/sustainable-processes/ontology/refs/heads/main/OntoCAPE/supporting_concepts/geometry/geometry.owl#Surface"/>
        <rdfs:subClassOf>
            <owl:Restriction>
                <owl:onProperty rdf:resource="https://raw.githubusercontent.com/sustainable-processes/ontology/refs/heads/main/OntoCAPE/supporting_concepts/geometry/geometry.owl#has_length"/>
                <owl:someValuesFrom>
                    <owl:Class>
                        <owl:unionOf rdf:parseType="Collection">
                            <rdf:Description rdf:about="https://raw.githubusercontent.com/sustainable-processes/ontology/refs/heads/main/OntoCAPE/supporting_concepts/geometry/geometry.owl#Diameter"/>
                            <rdf:Description rdf:about="https://raw.githubusercontent.com/sustainable-processes/ontology/refs/heads/main/OntoCAPE/supporting_concepts/geometry/geometry.owl#Radius"/>
                        </owl:unionOf>
                    </owl:Class>
                </owl:someValuesFrom>
            </owl:Restriction>
        </rdfs:subClassOf>
        <rdfs:subClassOf>
            <owl:Restriction>
                <owl:onProperty rdf:resource="https://raw.githubusercontent.com/sustainable-processes/ontology/refs/heads/main/OntoCAPE/supporting_concepts/geometry/geometry.owl#has_length"/>
                <owl:allValuesFrom>
                    <owl:Class>
                        <owl:unionOf rdf:parseType="Collection">
                            <rdf:Description rdf:about="https://raw.githubusercontent.com/sustainable-processes/ontology/refs/heads/main/OntoCAPE/supporting_concepts/geometry/geometry.owl#Diameter"/>
                            <rdf:Description rdf:about="https://raw.githubusercontent.com/sustainable-processes/ontology/refs/heads/main/OntoCAPE/supporting_concepts/geometry/geometry.owl#Radius"/>
                        </owl:unionOf>
                    </owl:Class>
                </owl:allValuesFrom>
            </owl:Restriction>
        </rdfs:subClassOf>
        <rdfs:subClassOf>
            <owl:Restriction>
                <owl:onProperty rdf:resource="https://raw.githubusercontent.com/sustainable-processes/ontology/refs/heads/main/OntoCAPE/supporting_concepts/geometry/geometry.owl#has_length"/>
                <owl:cardinality rdf:datatype="http://www.w3.org/2001/XMLSchema#nonNegativeInteger">1</owl:cardinality>
            </owl:Restriction>
        </rdfs:subClassOf>
        <owl:disjointWith rdf:resource="https://raw.githubusercontent.com/sustainable-processes/ontology/refs/heads/main/OntoCAPE/supporting_concepts/geometry/geometry.owl#Rectangle"/>
        <rdfs:comment>A Disk is the union of a circle and its interior [http://www.mathwords.com/d/disk.htm]. A circle is given by the set of points in a plane that are equidistant from a given point.</rdfs:comment>
    </owl:Class>
    


    <!-- https://raw.githubusercontent.com/sustainable-processes/ontology/refs/heads/main/OntoCAPE/supporting_concepts/geometry/geometry.owl#EdgeLength -->

    <owl:Class rdf:about="https://raw.githubusercontent.com/sustainable-processes/ontology/refs/heads/main/OntoCAPE/supporting_concepts/geometry/geometry.owl#EdgeLength">
        <rdfs:subClassOf rdf:resource="https://raw.githubusercontent.com/sustainable-processes/ontology/refs/heads/main/OntoCAPE/upper_level/system.owl#ScalarQuantity"/>
        <rdfs:subClassOf>
            <owl:Restriction>
                <owl:onProperty rdf:resource="https://raw.githubusercontent.com/sustainable-processes/ontology/refs/heads/main/OntoCAPE/upper_level/system.owl#hasDimension"/>
                <owl:hasValue rdf:resource="https://raw.githubusercontent.com/sustainable-processes/ontology/refs/heads/main/OntoCAPE/supporting_concepts/physical_dimension/physical_dimension.owl#length"/>
            </owl:Restriction>
        </rdfs:subClassOf>
        <owl:disjointWith rdf:resource="https://raw.githubusercontent.com/sustainable-processes/ontology/refs/heads/main/OntoCAPE/supporting_concepts/geometry/geometry.owl#Height"/>
        <owl:disjointWith rdf:resource="https://raw.githubusercontent.com/sustainable-processes/ontology/refs/heads/main/OntoCAPE/supporting_concepts/geometry/geometry.owl#Radius"/>
        <owl:disjointWith rdf:resource="https://raw.githubusercontent.com/sustainable-processes/ontology/refs/heads/main/OntoCAPE/supporting_concepts/geometry/geometry.owl#SurfaceArea"/>
        <owl:disjointWith rdf:resource="https://raw.githubusercontent.com/sustainable-processes/ontology/refs/heads/main/OntoCAPE/supporting_concepts/geometry/geometry.owl#TotalSurfaceArea"/>
        <owl:disjointWith rdf:resource="https://raw.githubusercontent.com/sustainable-processes/ontology/refs/heads/main/OntoCAPE/supporting_concepts/geometry/geometry.owl#Volume"/>
        <rdfs:comment>The length of a (straight) edge of a Surface or Solid</rdfs:comment>
    </owl:Class>
    


    <!-- https://raw.githubusercontent.com/sustainable-processes/ontology/refs/heads/main/OntoCAPE/supporting_concepts/geometry/geometry.owl#Height -->

    <owl:Class rdf:about="https://raw.githubusercontent.com/sustainable-processes/ontology/refs/heads/main/OntoCAPE/supporting_concepts/geometry/geometry.owl#Height">
        <rdfs:subClassOf rdf:resource="https://raw.githubusercontent.com/sustainable-processes/ontology/refs/heads/main/OntoCAPE/upper_level/system.owl#ScalarQuantity"/>
        <rdfs:subClassOf>
            <owl:Restriction>
                <owl:onProperty rdf:resource="https://raw.githubusercontent.com/sustainable-processes/ontology/refs/heads/main/OntoCAPE/upper_level/system.owl#hasDimension"/>
                <owl:hasValue rdf:resource="https://raw.githubusercontent.com/sustainable-processes/ontology/refs/heads/main/OntoCAPE/supporting_concepts/physical_dimension/physical_dimension.owl#length"/>
            </owl:Restriction>
        </rdfs:subClassOf>
        <owl:disjointWith rdf:resource="https://raw.githubusercontent.com/sustainable-processes/ontology/refs/heads/main/OntoCAPE/supporting_concepts/geometry/geometry.owl#Radius"/>
        <owl:disjointWith rdf:resource="https://raw.githubusercontent.com/sustainable-processes/ontology/refs/heads/main/OntoCAPE/supporting_concepts/geometry/geometry.owl#TotalSurfaceArea"/>
        <owl:disjointWith rdf:resource="https://raw.githubusercontent.com/sustainable-processes/ontology/refs/heads/main/OntoCAPE/supporting_concepts/geometry/geometry.owl#Volume"/>
        <rdfs:comment>The shortest distance between the base of a geometric figure and its top, whether that top is an opposite vertex, an apex, or another base.
[http://www.mathwords.com/a/altitude.htm]</rdfs:comment>
    </owl:Class>
    


    <!-- https://raw.githubusercontent.com/sustainable-processes/ontology/refs/heads/main/OntoCAPE/supporting_concepts/geometry/geometry.owl#LateralSurfaceArea -->

    <owl:Class rdf:about="https://raw.githubusercontent.com/sustainable-processes/ontology/refs/heads/main/OntoCAPE/supporting_concepts/geometry/geometry.owl#LateralSurfaceArea">
        <rdfs:subClassOf rdf:resource="https://raw.githubusercontent.com/sustainable-processes/ontology/refs/heads/main/OntoCAPE/supporting_concepts/geometry/geometry.owl#SideArea"/>
        <rdfs:comment>The SurfaceArea of a single lateral surface of a solid (i.e., any SideArea that is not a BaseArea).</rdfs:comment>
    </owl:Class>
    


    <!-- https://raw.githubusercontent.com/sustainable-processes/ontology/refs/heads/main/OntoCAPE/supporting_concepts/geometry/geometry.owl#Radius -->

    <owl:Class rdf:about="https://raw.githubusercontent.com/sustainable-processes/ontology/refs/heads/main/OntoCAPE/supporting_concepts/geometry/geometry.owl#Radius">
        <rdfs:subClassOf rdf:resource="https://raw.githubusercontent.com/sustainable-processes/ontology/refs/heads/main/OntoCAPE/upper_level/system.owl#ScalarQuantity"/>
        <rdfs:subClassOf>
            <owl:Restriction>
                <owl:onProperty rdf:resource="https://raw.githubusercontent.com/sustainable-processes/ontology/refs/heads/main/OntoCAPE/upper_level/system.owl#hasDimension"/>
                <owl:hasValue rdf:resource="https://raw.githubusercontent.com/sustainable-processes/ontology/refs/heads/main/OntoCAPE/supporting_concepts/physical_dimension/physical_dimension.owl#length"/>
            </owl:Restriction>
        </rdfs:subClassOf>
        <owl:disjointWith rdf:resource="https://raw.githubusercontent.com/sustainable-processes/ontology/refs/heads/main/OntoCAPE/supporting_concepts/geometry/geometry.owl#SurfaceArea"/>
        <owl:disjointWith rdf:resource="https://raw.githubusercontent.com/sustainable-processes/ontology/refs/heads/main/OntoCAPE/supporting_concepts/geometry/geometry.owl#TotalSurfaceArea"/>
        <owl:disjointWith rdf:resource="https://raw.githubusercontent.com/sustainable-processes/ontology/refs/heads/main/OntoCAPE/supporting_concepts/geometry/geometry.owl#Volume"/>
        <rdfs:comment>The length of the line segment between the center and a point on a circle or Sphere.</rdfs:comment>
    </owl:Class>
    


    <!-- https://raw.githubusercontent.com/sustainable-processes/ontology/refs/heads/main/OntoCAPE/supporting_concepts/geometry/geometry.owl#Rectangle -->

    <owl:Class rdf:about="https://raw.githubusercontent.com/sustainable-processes/ontology/refs/heads/main/OntoCAPE/supporting_concepts/geometry/geometry.owl#Rectangle">
        <rdfs:subClassOf rdf:resource="https://raw.githubusercontent.com/sustainable-processes/ontology/refs/heads/main/OntoCAPE/supporting_concepts/geometry/geometry.owl#Surface"/>
        <rdfs:subClassOf>
            <owl:Restriction>
                <owl:onProperty rdf:resource="https://raw.githubusercontent.com/sustainable-processes/ontology/refs/heads/main/OntoCAPE/supporting_concepts/geometry/geometry.owl#has_length"/>
                <owl:someValuesFrom rdf:resource="https://raw.githubusercontent.com/sustainable-processes/ontology/refs/heads/main/OntoCAPE/supporting_concepts/geometry/geometry.owl#EdgeLength"/>
            </owl:Restriction>
        </rdfs:subClassOf>
        <rdfs:subClassOf>
            <owl:Restriction>
                <owl:onProperty rdf:resource="https://raw.githubusercontent.com/sustainable-processes/ontology/refs/heads/main/OntoCAPE/supporting_concepts/geometry/geometry.owl#has_length"/>
                <owl:allValuesFrom rdf:resource="https://raw.githubusercontent.com/sustainable-processes/ontology/refs/heads/main/OntoCAPE/supporting_concepts/geometry/geometry.owl#EdgeLength"/>
            </owl:Restriction>
        </rdfs:subClassOf>
        <rdfs:subClassOf>
            <owl:Restriction>
                <owl:onProperty rdf:resource="https://raw.githubusercontent.com/sustainable-processes/ontology/refs/heads/main/OntoCAPE/supporting_concepts/geometry/geometry.owl#has_length"/>
                <owl:cardinality rdf:datatype="http://www.w3.org/2001/XMLSchema#nonNegativeInteger">2</owl:cardinality>
            </owl:Restriction>
        </rdfs:subClassOf>
        <rdfs:comment>A box shape on a plane. Formally, a rectangle is a quadrilateral with four congruent angles (all 90°). [http://www.mathwords.com/r/rectangle.htm]</rdfs:comment>
    </owl:Class>
    


    <!-- https://raw.githubusercontent.com/sustainable-processes/ontology/refs/heads/main/OntoCAPE/supporting_concepts/geometry/geometry.owl#RightCircularCone -->

    <owl:Class rdf:about="https://raw.githubusercontent.com/sustainable-processes/ontology/refs/heads/main/OntoCAPE/supporting_concepts/geometry/geometry.owl#RightCircularCone">
        <rdfs:subClassOf rdf:resource="https://raw.githubusercontent.com/sustainable-processes/ontology/refs/heads/main/OntoCAPE/supporting_concepts/geometry/geometry.owl#RightCone"/>
        <rdfs:subClassOf>
            <owl:Restriction>
                <owl:onProperty rdf:resource="https://raw.githubusercontent.com/sustainable-processes/ontology/refs/heads/main/OntoCAPE/supporting_concepts/geometry/geometry.owl#has_length"/>
                <owl:allValuesFrom rdf:resource="https://raw.githubusercontent.com/sustainable-processes/ontology/refs/heads/main/OntoCAPE/supporting_concepts/geometry/geometry.owl#Height"/>
            </owl:Restriction>
        </rdfs:subClassOf>
        <rdfs:subClassOf>
            <owl:Restriction>
                <owl:onProperty rdf:resource="https://raw.githubusercontent.com/sustainable-processes/ontology/refs/heads/main/OntoCAPE/supporting_concepts/geometry/geometry.owl#has_area"/>
                <owl:cardinality rdf:datatype="http://www.w3.org/2001/XMLSchema#nonNegativeInteger">2</owl:cardinality>
            </owl:Restriction>
        </rdfs:subClassOf>
        <rdfs:subClassOf>
            <owl:Restriction>
                <owl:onProperty rdf:resource="https://raw.githubusercontent.com/sustainable-processes/ontology/refs/heads/main/OntoCAPE/supporting_concepts/geometry/geometry.owl#has_length"/>
                <owl:cardinality rdf:datatype="http://www.w3.org/2001/XMLSchema#nonNegativeInteger">1</owl:cardinality>
            </owl:Restriction>
        </rdfs:subClassOf>
        <rdfs:comment>A RightCone with a base that is a circle.</rdfs:comment>
    </owl:Class>
    


    <!-- https://raw.githubusercontent.com/sustainable-processes/ontology/refs/heads/main/OntoCAPE/supporting_concepts/geometry/geometry.owl#RightCircularCylinder -->

    <owl:Class rdf:about="https://raw.githubusercontent.com/sustainable-processes/ontology/refs/heads/main/OntoCAPE/supporting_concepts/geometry/geometry.owl#RightCircularCylinder">
        <rdfs:subClassOf rdf:resource="https://raw.githubusercontent.com/sustainable-processes/ontology/refs/heads/main/OntoCAPE/supporting_concepts/geometry/geometry.owl#RightCylinder"/>
        <rdfs:subClassOf>
            <owl:Restriction>
                <owl:onProperty rdf:resource="https://raw.githubusercontent.com/sustainable-processes/ontology/refs/heads/main/OntoCAPE/supporting_concepts/geometry/geometry.owl#has_length"/>
                <owl:someValuesFrom>
                    <owl:Class>
                        <owl:unionOf rdf:parseType="Collection">
                            <rdf:Description rdf:about="https://raw.githubusercontent.com/sustainable-processes/ontology/refs/heads/main/OntoCAPE/supporting_concepts/geometry/geometry.owl#Diameter"/>
                            <rdf:Description rdf:about="https://raw.githubusercontent.com/sustainable-processes/ontology/refs/heads/main/OntoCAPE/supporting_concepts/geometry/geometry.owl#Radius"/>
                        </owl:unionOf>
                    </owl:Class>
                </owl:someValuesFrom>
            </owl:Restriction>
        </rdfs:subClassOf>
        <rdfs:subClassOf>
            <owl:Restriction>
                <owl:onProperty rdf:resource="https://raw.githubusercontent.com/sustainable-processes/ontology/refs/heads/main/OntoCAPE/supporting_concepts/geometry/geometry.owl#has_length"/>
                <owl:allValuesFrom>
                    <owl:Class>
                        <owl:unionOf rdf:parseType="Collection">
                            <rdf:Description rdf:about="https://raw.githubusercontent.com/sustainable-processes/ontology/refs/heads/main/OntoCAPE/supporting_concepts/geometry/geometry.owl#Diameter"/>
                            <rdf:Description rdf:about="https://raw.githubusercontent.com/sustainable-processes/ontology/refs/heads/main/OntoCAPE/supporting_concepts/geometry/geometry.owl#Height"/>
                            <rdf:Description rdf:about="https://raw.githubusercontent.com/sustainable-processes/ontology/refs/heads/main/OntoCAPE/supporting_concepts/geometry/geometry.owl#Radius"/>
                        </owl:unionOf>
                    </owl:Class>
                </owl:allValuesFrom>
            </owl:Restriction>
        </rdfs:subClassOf>
        <rdfs:subClassOf>
            <owl:Restriction>
                <owl:onProperty rdf:resource="https://raw.githubusercontent.com/sustainable-processes/ontology/refs/heads/main/OntoCAPE/supporting_concepts/geometry/geometry.owl#has_area"/>
                <owl:cardinality rdf:datatype="http://www.w3.org/2001/XMLSchema#nonNegativeInteger">3</owl:cardinality>
            </owl:Restriction>
        </rdfs:subClassOf>
        <rdfs:subClassOf>
            <owl:Restriction>
                <owl:onProperty rdf:resource="https://raw.githubusercontent.com/sustainable-processes/ontology/refs/heads/main/OntoCAPE/supporting_concepts/geometry/geometry.owl#has_length"/>
                <owl:cardinality rdf:datatype="http://www.w3.org/2001/XMLSchema#nonNegativeInteger">2</owl:cardinality>
            </owl:Restriction>
        </rdfs:subClassOf>
        <rdfs:comment>A RightCylinder with bases that are circles [http://www.mathwords.com/r/right_circular_cylinder.htm]</rdfs:comment>
    </owl:Class>
    


    <!-- https://raw.githubusercontent.com/sustainable-processes/ontology/refs/heads/main/OntoCAPE/supporting_concepts/geometry/geometry.owl#RightCone -->

    <owl:Class rdf:about="https://raw.githubusercontent.com/sustainable-processes/ontology/refs/heads/main/OntoCAPE/supporting_concepts/geometry/geometry.owl#RightCone">
        <rdfs:subClassOf rdf:resource="https://raw.githubusercontent.com/sustainable-processes/ontology/refs/heads/main/OntoCAPE/supporting_concepts/geometry/geometry.owl#Cone"/>
        <rdfs:comment>A Cone that has its apex aligned directly above the center of its base [http://www.mathwords.com/r/right_cone.htm].</rdfs:comment>
    </owl:Class>
    


    <!-- https://raw.githubusercontent.com/sustainable-processes/ontology/refs/heads/main/OntoCAPE/supporting_concepts/geometry/geometry.owl#RightCylinder -->

    <owl:Class rdf:about="https://raw.githubusercontent.com/sustainable-processes/ontology/refs/heads/main/OntoCAPE/supporting_concepts/geometry/geometry.owl#RightCylinder">
        <rdfs:subClassOf rdf:resource="https://raw.githubusercontent.com/sustainable-processes/ontology/refs/heads/main/OntoCAPE/supporting_concepts/geometry/geometry.owl#Cylinder"/>
        <rdfs:comment>A Cylinder which has bases aligned one directly above the other [http://www.mathwords.com/r/right_cylinder.htm]</rdfs:comment>
    </owl:Class>
    


    <!-- https://raw.githubusercontent.com/sustainable-processes/ontology/refs/heads/main/OntoCAPE/supporting_concepts/geometry/geometry.owl#SideArea -->

    <owl:Class rdf:about="https://raw.githubusercontent.com/sustainable-processes/ontology/refs/heads/main/OntoCAPE/supporting_concepts/geometry/geometry.owl#SideArea">
        <rdfs:subClassOf rdf:resource="https://raw.githubusercontent.com/sustainable-processes/ontology/refs/heads/main/OntoCAPE/supporting_concepts/geometry/geometry.owl#SurfaceArea"/>
        <rdfs:subClassOf>
            <owl:Restriction>
                <owl:onProperty rdf:resource="https://raw.githubusercontent.com/sustainable-processes/ontology/refs/heads/main/OntoCAPE/upper_level/system.owl#isPropertyOf"/>
                <owl:allValuesFrom rdf:resource="https://raw.githubusercontent.com/sustainable-processes/ontology/refs/heads/main/OntoCAPE/supporting_concepts/geometry/geometry.owl#Solid"/>
            </owl:Restriction>
        </rdfs:subClassOf>
        <owl:disjointWith rdf:resource="https://raw.githubusercontent.com/sustainable-processes/ontology/refs/heads/main/OntoCAPE/supporting_concepts/geometry/geometry.owl#TotalSurfaceArea"/>
        <rdfs:comment>The area of one particular exterior surface of a Solid. This concept should be applied only if the Solid has several distinguishable exterior surfaces. Otherwise (e.g., for a Sphere) use TotalSufaceArea
A SideArea can either be a ScalarQuantity or a VectorQuantity. In case of the latter, the vector is perpendicular to the surface (i.e., it has the same orientation as the surface normal), and its Euclidean norm equals the area of the surface.</rdfs:comment>
    </owl:Class>
    


    <!-- https://raw.githubusercontent.com/sustainable-processes/ontology/refs/heads/main/OntoCAPE/supporting_concepts/geometry/geometry.owl#Solid -->

    <owl:Class rdf:about="https://raw.githubusercontent.com/sustainable-processes/ontology/refs/heads/main/OntoCAPE/supporting_concepts/geometry/geometry.owl#Solid">
        <rdfs:subClassOf rdf:resource="https://raw.githubusercontent.com/sustainable-processes/ontology/refs/heads/main/OntoCAPE/upper_level/system.owl#System"/>
        <rdfs:subClassOf>
            <owl:Restriction>
                <owl:onProperty rdf:resource="https://raw.githubusercontent.com/sustainable-processes/ontology/refs/heads/main/OntoCAPE/supporting_concepts/geometry/geometry.owl#has_area"/>
                <owl:someValuesFrom rdf:resource="https://raw.githubusercontent.com/sustainable-processes/ontology/refs/heads/main/OntoCAPE/supporting_concepts/geometry/geometry.owl#SurfaceArea"/>
            </owl:Restriction>
        </rdfs:subClassOf>
        <rdfs:subClassOf>
            <owl:Restriction>
                <owl:onProperty rdf:resource="https://raw.githubusercontent.com/sustainable-processes/ontology/refs/heads/main/OntoCAPE/supporting_concepts/geometry/geometry.owl#has_volume"/>
                <owl:someValuesFrom rdf:resource="https://raw.githubusercontent.com/sustainable-processes/ontology/refs/heads/main/OntoCAPE/supporting_concepts/geometry/geometry.owl#Volume"/>
            </owl:Restriction>
        </rdfs:subClassOf>
        <rdfs:subClassOf>
            <owl:Restriction>
                <owl:onProperty rdf:resource="https://raw.githubusercontent.com/sustainable-processes/ontology/refs/heads/main/OntoCAPE/supporting_concepts/geometry/geometry.owl#has_area"/>
                <owl:allValuesFrom rdf:resource="https://raw.githubusercontent.com/sustainable-processes/ontology/refs/heads/main/OntoCAPE/supporting_concepts/geometry/geometry.owl#SurfaceArea"/>
            </owl:Restriction>
        </rdfs:subClassOf>
        <rdfs:subClassOf>
            <owl:Restriction>
                <owl:onProperty rdf:resource="https://raw.githubusercontent.com/sustainable-processes/ontology/refs/heads/main/OntoCAPE/supporting_concepts/geometry/geometry.owl#has_volume"/>
                <owl:allValuesFrom rdf:resource="https://raw.githubusercontent.com/sustainable-processes/ontology/refs/heads/main/OntoCAPE/supporting_concepts/geometry/geometry.owl#Volume"/>
            </owl:Restriction>
        </rdfs:subClassOf>
        <rdfs:subClassOf>
            <owl:Restriction>
                <owl:onProperty rdf:resource="https://raw.githubusercontent.com/sustainable-processes/ontology/refs/heads/main/OntoCAPE/supporting_concepts/geometry/geometry.owl#has_volume"/>
                <owl:cardinality rdf:datatype="http://www.w3.org/2001/XMLSchema#nonNegativeInteger">1</owl:cardinality>
            </owl:Restriction>
        </rdfs:subClassOf>
        <rdfs:comment>Solid (aka Geometric Solid or Solid Geometric Figure) is a collective term for all bounded three-dimensional geometric figures. This includes polyhedra, pyramids, prisms, cylinders, cones, spheres, ellipsoids, etc. [http://www.mathwords.com/s/solid.htm]</rdfs:comment>
    </owl:Class>
    


    <!-- https://raw.githubusercontent.com/sustainable-processes/ontology/refs/heads/main/OntoCAPE/supporting_concepts/geometry/geometry.owl#Sphere -->

    <owl:Class rdf:about="https://raw.githubusercontent.com/sustainable-processes/ontology/refs/heads/main/OntoCAPE/supporting_concepts/geometry/geometry.owl#Sphere">
        <rdfs:subClassOf rdf:resource="https://raw.githubusercontent.com/sustainable-processes/ontology/refs/heads/main/OntoCAPE/supporting_concepts/geometry/geometry.owl#Solid"/>
        <rdfs:subClassOf>
            <owl:Restriction>
                <owl:onProperty rdf:resource="https://raw.githubusercontent.com/sustainable-processes/ontology/refs/heads/main/OntoCAPE/supporting_concepts/geometry/geometry.owl#has_length"/>
                <owl:someValuesFrom>
                    <owl:Class>
                        <owl:unionOf rdf:parseType="Collection">
                            <rdf:Description rdf:about="https://raw.githubusercontent.com/sustainable-processes/ontology/refs/heads/main/OntoCAPE/supporting_concepts/geometry/geometry.owl#Diameter"/>
                            <rdf:Description rdf:about="https://raw.githubusercontent.com/sustainable-processes/ontology/refs/heads/main/OntoCAPE/supporting_concepts/geometry/geometry.owl#Radius"/>
                        </owl:unionOf>
                    </owl:Class>
                </owl:someValuesFrom>
            </owl:Restriction>
        </rdfs:subClassOf>
        <rdfs:subClassOf>
            <owl:Restriction>
                <owl:onProperty rdf:resource="https://raw.githubusercontent.com/sustainable-processes/ontology/refs/heads/main/OntoCAPE/supporting_concepts/geometry/geometry.owl#has_area"/>
                <owl:allValuesFrom rdf:resource="https://raw.githubusercontent.com/sustainable-processes/ontology/refs/heads/main/OntoCAPE/supporting_concepts/geometry/geometry.owl#TotalSurfaceArea"/>
            </owl:Restriction>
        </rdfs:subClassOf>
        <rdfs:subClassOf>
            <owl:Restriction>
                <owl:onProperty rdf:resource="https://raw.githubusercontent.com/sustainable-processes/ontology/refs/heads/main/OntoCAPE/supporting_concepts/geometry/geometry.owl#has_length"/>
                <owl:allValuesFrom>
                    <owl:Class>
                        <owl:unionOf rdf:parseType="Collection">
                            <rdf:Description rdf:about="https://raw.githubusercontent.com/sustainable-processes/ontology/refs/heads/main/OntoCAPE/supporting_concepts/geometry/geometry.owl#Diameter"/>
                            <rdf:Description rdf:about="https://raw.githubusercontent.com/sustainable-processes/ontology/refs/heads/main/OntoCAPE/supporting_concepts/geometry/geometry.owl#Radius"/>
                        </owl:unionOf>
                    </owl:Class>
                </owl:allValuesFrom>
            </owl:Restriction>
        </rdfs:subClassOf>
        <rdfs:subClassOf>
            <owl:Restriction>
                <owl:onProperty rdf:resource="https://raw.githubusercontent.com/sustainable-processes/ontology/refs/heads/main/OntoCAPE/supporting_concepts/geometry/geometry.owl#has_area"/>
                <owl:cardinality rdf:datatype="http://www.w3.org/2001/XMLSchema#nonNegativeInteger">1</owl:cardinality>
            </owl:Restriction>
        </rdfs:subClassOf>
        <rdfs:subClassOf>
            <owl:Restriction>
                <owl:onProperty rdf:resource="https://raw.githubusercontent.com/sustainable-processes/ontology/refs/heads/main/OntoCAPE/supporting_concepts/geometry/geometry.owl#has_length"/>
                <owl:cardinality rdf:datatype="http://www.w3.org/2001/XMLSchema#nonNegativeInteger">1</owl:cardinality>
            </owl:Restriction>
        </rdfs:subClassOf>
        <rdfs:comment>A Solid consisting of all points equidistant from a given point. This point is the center of the sphere. [http://www.mathwords.com/s/sphere.htm]</rdfs:comment>
    </owl:Class>
    


    <!-- https://raw.githubusercontent.com/sustainable-processes/ontology/refs/heads/main/OntoCAPE/supporting_concepts/geometry/geometry.owl#Surface -->

    <owl:Class rdf:about="https://raw.githubusercontent.com/sustainable-processes/ontology/refs/heads/main/OntoCAPE/supporting_concepts/geometry/geometry.owl#Surface">
        <rdfs:subClassOf rdf:resource="https://raw.githubusercontent.com/sustainable-processes/ontology/refs/heads/main/OntoCAPE/upper_level/system.owl#System"/>
        <rdfs:subClassOf>
            <owl:Restriction>
                <owl:onProperty rdf:resource="https://raw.githubusercontent.com/sustainable-processes/ontology/refs/heads/main/OntoCAPE/supporting_concepts/geometry/geometry.owl#has_area"/>
                <owl:someValuesFrom rdf:resource="https://raw.githubusercontent.com/sustainable-processes/ontology/refs/heads/main/OntoCAPE/supporting_concepts/geometry/geometry.owl#SurfaceArea"/>
            </owl:Restriction>
        </rdfs:subClassOf>
        <rdfs:subClassOf>
            <owl:Restriction>
                <owl:onProperty rdf:resource="https://raw.githubusercontent.com/sustainable-processes/ontology/refs/heads/main/OntoCAPE/supporting_concepts/geometry/geometry.owl#has_area"/>
                <owl:allValuesFrom rdf:resource="https://raw.githubusercontent.com/sustainable-processes/ontology/refs/heads/main/OntoCAPE/supporting_concepts/geometry/geometry.owl#SurfaceArea"/>
            </owl:Restriction>
        </rdfs:subClassOf>
        <rdfs:subClassOf>
            <owl:Restriction>
                <owl:onProperty rdf:resource="https://raw.githubusercontent.com/sustainable-processes/ontology/refs/heads/main/OntoCAPE/supporting_concepts/geometry/geometry.owl#has_area"/>
                <owl:cardinality rdf:datatype="http://www.w3.org/2001/XMLSchema#nonNegativeInteger">1</owl:cardinality>
            </owl:Restriction>
        </rdfs:subClassOf>
        <rdfs:comment>a two-dimensional submanifold of three-dimensional Euclidean space</rdfs:comment>
    </owl:Class>
    


    <!-- https://raw.githubusercontent.com/sustainable-processes/ontology/refs/heads/main/OntoCAPE/supporting_concepts/geometry/geometry.owl#SurfaceArea -->

    <owl:Class rdf:about="https://raw.githubusercontent.com/sustainable-processes/ontology/refs/heads/main/OntoCAPE/supporting_concepts/geometry/geometry.owl#SurfaceArea">
        <owl:equivalentClass>
            <owl:Class>
                <owl:unionOf rdf:parseType="Collection">
                    <rdf:Description rdf:about="https://raw.githubusercontent.com/sustainable-processes/ontology/refs/heads/main/OntoCAPE/supporting_concepts/geometry/geometry.owl#SideArea"/>
                    <rdf:Description rdf:about="https://raw.githubusercontent.com/sustainable-processes/ontology/refs/heads/main/OntoCAPE/supporting_concepts/geometry/geometry.owl#TotalSurfaceArea"/>
                </owl:unionOf>
            </owl:Class>
        </owl:equivalentClass>
        <rdfs:subClassOf rdf:resource="https://raw.githubusercontent.com/sustainable-processes/ontology/refs/heads/main/OntoCAPE/upper_level/system.owl#PhysicalQuantity"/>
        <rdfs:subClassOf>
            <owl:Restriction>
                <owl:onProperty rdf:resource="https://raw.githubusercontent.com/sustainable-processes/ontology/refs/heads/main/OntoCAPE/upper_level/system.owl#hasDimension"/>
                <owl:hasValue rdf:resource="https://raw.githubusercontent.com/sustainable-processes/ontology/refs/heads/main/OntoCAPE/supporting_concepts/physical_dimension/derived_dimensions.owl#area"/>
            </owl:Restriction>
        </rdfs:subClassOf>
        <rdfs:comment>The area of a Surface or of (one of) the exterior surface(s) of a Solid. 
More precisely, the class alternatively denotes
- the area of a Surface, or
- the area of a single exterior surface of a Solid, or
- the total area of the exterior surface(s) of a Solid.</rdfs:comment>
    </owl:Class>
    


    <!-- https://raw.githubusercontent.com/sustainable-processes/ontology/refs/heads/main/OntoCAPE/supporting_concepts/geometry/geometry.owl#TotalSurfaceArea -->

    <owl:Class rdf:about="https://raw.githubusercontent.com/sustainable-processes/ontology/refs/heads/main/OntoCAPE/supporting_concepts/geometry/geometry.owl#TotalSurfaceArea">
        <rdfs:subClassOf rdf:resource="https://raw.githubusercontent.com/sustainable-processes/ontology/refs/heads/main/OntoCAPE/supporting_concepts/geometry/geometry.owl#SurfaceArea"/>
        <rdfs:subClassOf rdf:resource="https://raw.githubusercontent.com/sustainable-processes/ontology/refs/heads/main/OntoCAPE/upper_level/system.owl#ScalarQuantity"/>
        <owl:disjointWith rdf:resource="https://raw.githubusercontent.com/sustainable-processes/ontology/refs/heads/main/OntoCAPE/supporting_concepts/geometry/geometry.owl#Volume"/>
        <rdfs:comment>The total area of a Surface or of (all) the exterior surface(s) of a Solid.</rdfs:comment>
    </owl:Class>
    


    <!-- https://raw.githubusercontent.com/sustainable-processes/ontology/refs/heads/main/OntoCAPE/supporting_concepts/geometry/geometry.owl#Volume -->

    <owl:Class rdf:about="https://raw.githubusercontent.com/sustainable-processes/ontology/refs/heads/main/OntoCAPE/supporting_concepts/geometry/geometry.owl#Volume">
        <rdfs:subClassOf rdf:resource="https://raw.githubusercontent.com/sustainable-processes/ontology/refs/heads/main/OntoCAPE/upper_level/system.owl#ScalarQuantity"/>
        <rdfs:subClassOf>
            <owl:Restriction>
                <owl:onProperty rdf:resource="https://raw.githubusercontent.com/sustainable-processes/ontology/refs/heads/main/OntoCAPE/upper_level/system.owl#hasDimension"/>
                <owl:hasValue rdf:resource="https://raw.githubusercontent.com/sustainable-processes/ontology/refs/heads/main/OntoCAPE/supporting_concepts/physical_dimension/derived_dimensions.owl#volume"/>
            </owl:Restriction>
        </rdfs:subClassOf>
        <rdfs:comment>The total amount of space enclosed in a Solid [http://www.mathwords.com/v/volume.htm]</rdfs:comment>
    </owl:Class>
    


    <!-- https://raw.githubusercontent.com/sustainable-processes/ontology/refs/heads/main/OntoCAPE/upper_level/system.owl#PhysicalQuantity -->

    <owl:Class rdf:about="https://raw.githubusercontent.com/sustainable-processes/ontology/refs/heads/main/OntoCAPE/upper_level/system.owl#PhysicalQuantity"/>
    


    <!-- https://raw.githubusercontent.com/sustainable-processes/ontology/refs/heads/main/OntoCAPE/upper_level/system.owl#ScalarQuantity -->

    <owl:Class rdf:about="https://raw.githubusercontent.com/sustainable-processes/ontology/refs/heads/main/OntoCAPE/upper_level/system.owl#ScalarQuantity"/>
    


    <!-- https://raw.githubusercontent.com/sustainable-processes/ontology/refs/heads/main/OntoCAPE/upper_level/system.owl#System -->

    <owl:Class rdf:about="https://raw.githubusercontent.com/sustainable-processes/ontology/refs/heads/main/OntoCAPE/upper_level/system.owl#System"/>
    


    <!-- 
    ///////////////////////////////////////////////////////////////////////////////////////
    //
    // Individuals
    //
    ///////////////////////////////////////////////////////////////////////////////////////
     -->

    


    <!-- https://raw.githubusercontent.com/sustainable-processes/ontology/refs/heads/main/OntoCAPE/supporting_concepts/physical_dimension/derived_dimensions.owl#area -->

    <owl:NamedIndividual rdf:about="https://raw.githubusercontent.com/sustainable-processes/ontology/refs/heads/main/OntoCAPE/supporting_concepts/physical_dimension/derived_dimensions.owl#area"/>
    


    <!-- https://raw.githubusercontent.com/sustainable-processes/ontology/refs/heads/main/OntoCAPE/supporting_concepts/physical_dimension/derived_dimensions.owl#volume -->

    <owl:NamedIndividual rdf:about="https://raw.githubusercontent.com/sustainable-processes/ontology/refs/heads/main/OntoCAPE/supporting_concepts/physical_dimension/derived_dimensions.owl#volume"/>
    


    <!-- https://raw.githubusercontent.com/sustainable-processes/ontology/refs/heads/main/OntoCAPE/supporting_concepts/physical_dimension/physical_dimension.owl#length -->

    <owl:NamedIndividual rdf:about="https://raw.githubusercontent.com/sustainable-processes/ontology/refs/heads/main/OntoCAPE/supporting_concepts/physical_dimension/physical_dimension.owl#length"/>
</rdf:RDF>



<!-- Generated by the OWL API (version 4.5.26.2023-07-17T20:34:13Z) https://github.com/owlcs/owlapi -->

