<?xml version="1.0"?>
<rdf:RDF xmlns="https://github.com/sustainable-processes/ontology/OntoCAPE/model/equation_system.owl#"
     xml:base="https://github.com/sustainable-processes/ontology/OntoCAPE/model/equation_system.owl"
     xmlns:owl="http://www.w3.org/2002/07/owl#"
     xmlns:rdf="http://www.w3.org/1999/02/22-rdf-syntax-ns#"
     xmlns:xml="http://www.w3.org/XML/1998/namespace"
     xmlns:xsd="http://www.w3.org/2001/XMLSchema#"
     xmlns:rdfs="http://www.w3.org/2000/01/rdf-schema#"
     xmlns:root="https://github.com/sustainable-processes/ontology/OntoCAPE/"
     xmlns:terms="http://purl.org/dc/terms/"
     xmlns:system="https://github.com/sustainable-processes/ontology/OntoCAPE/upper_level/system.owl#"
     xmlns:equation_system="https://github.com/sustainable-processes/ontology/OntoCAPE/model/equation_system.owl"
     xmlns:mathematical_model="https://github.com/sustainable-processes/ontology/OntoCAPE/model/mathematical_model.owl#">
    <owl:Ontology rdf:about="https://github.com/sustainable-processes/ontology/OntoCAPE/model/equation_system.owl">
        <owl:imports rdf:resource="https://github.com/sustainable-processes/ontology/OntoCAPE/model/mathematical_model.owl"/>
        <terms:license>Copyright (C) [2009] [Andreas Wiesner]
                This program is free software; you can redistribute it and/or modify it under the terms of the GNU General Public License as published by the Free Software Foundation; either version 3 of the License, or (at your option) any later version.
                This program is distributed in the hope that it will be useful, but WITHOUT ANY WARRANTY; without even the implied warranty of MERCHANTABILITY or FITNESS FOR A PARTICULAR PURPOSE. See the GNU General Public License for more details.
                You should have received a copy of the GNU General Public License along with this program; if not, see &lt;http://www.gnu.org/licenses/&gt;.
    </terms:license>
        <rdfs:comment>The ontolog module &apos;equation_system&apos; provides concepts for the description of the model equations that constitute a mathematical model. 
The following classes and relations from other ontology modules are used within &apos;equation_system&apos;:

&lt;owl:Class rdf:about=&quot;https://github.com/sustainable-processes/ontology/OntoCAPE/model/mathematical_model.owl#MathematicalModel&quot;/&gt;
&lt;owl:Class rdf:about=&quot;https://github.com/sustainable-processes/ontology/OntoCAPE/upper_level/system.owl#FixedValueSet&quot;/&gt;

&lt;owl:ObjectProperty rdf:about=&quot;https://github.com/sustainable-processes/ontology/OntoCAPE/upper_level/system.owl#hasCharacteristic&quot;/&gt;
    </rdfs:comment>
        <owl:versionInfo>2.0</owl:versionInfo>
    </owl:Ontology>
    


    <!-- 
    ///////////////////////////////////////////////////////////////////////////////////////
    //
    // Object Properties
    //
    ///////////////////////////////////////////////////////////////////////////////////////
     -->

    


    <!-- https://github.com/sustainable-processes/ontology/OntoCAPE/model/equation_system.owl#hasDAE_Explicitness -->

    <owl:ObjectProperty rdf:about="https://github.com/sustainable-processes/ontology/OntoCAPE/model/equation_system.owl#hasDAE_Explicitness">
        <rdfs:subPropertyOf rdf:resource="https://github.com/sustainable-processes/ontology/OntoCAPE/upper_level/system.owl#hasCharacteristic"/>
        <rdfs:domain rdf:resource="https://github.com/sustainable-processes/ontology/OntoCAPE/model/equation_system.owl#DifferentialAlgebraicEquationSystem"/>
        <rdfs:range rdf:resource="https://github.com/sustainable-processes/ontology/OntoCAPE/model/equation_system.owl#DAE_Explicitness"/>
        <rdfs:comment>Indicates an EquationSystemCharacteristic of type DAE_explicitness.</rdfs:comment>
    </owl:ObjectProperty>
    


    <!-- https://github.com/sustainable-processes/ontology/OntoCAPE/model/equation_system.owl#hasLinearity -->

    <owl:ObjectProperty rdf:about="https://github.com/sustainable-processes/ontology/OntoCAPE/model/equation_system.owl#hasLinearity">
        <rdfs:subPropertyOf rdf:resource="https://github.com/sustainable-processes/ontology/OntoCAPE/upper_level/system.owl#hasCharacteristic"/>
        <rdfs:domain>
            <owl:Class>
                <owl:unionOf rdf:parseType="Collection">
                    <rdf:Description rdf:about="https://github.com/sustainable-processes/ontology/OntoCAPE/model/equation_system.owl#AlgebraicEquationSystem"/>
                    <rdf:Description rdf:about="https://github.com/sustainable-processes/ontology/OntoCAPE/model/equation_system.owl#DifferentialAlgebraicEquationSystem"/>
                </owl:unionOf>
            </owl:Class>
        </rdfs:domain>
        <rdfs:range rdf:resource="https://github.com/sustainable-processes/ontology/OntoCAPE/model/equation_system.owl#Linearity"/>
        <rdfs:comment>Indicates an EquationSystemCharacteristic of type Linearity</rdfs:comment>
    </owl:ObjectProperty>
    


    <!-- https://github.com/sustainable-processes/ontology/OntoCAPE/model/equation_system.owl#hasModelRepresentationForm -->

    <owl:ObjectProperty rdf:about="https://github.com/sustainable-processes/ontology/OntoCAPE/model/equation_system.owl#hasModelRepresentationForm">
        <rdfs:subPropertyOf rdf:resource="https://github.com/sustainable-processes/ontology/OntoCAPE/upper_level/system.owl#hasCharacteristic"/>
        <rdfs:domain rdf:resource="https://github.com/sustainable-processes/ontology/OntoCAPE/model/mathematical_model.owl#MathematicalModel"/>
        <rdfs:range rdf:resource="https://github.com/sustainable-processes/ontology/OntoCAPE/model/equation_system.owl#ModelRepresentationForm"/>
        <rdfs:comment>Indicates an EquationSystemCharacteristic of type ModelRepresentationForm</rdfs:comment>
    </owl:ObjectProperty>
    


    <!-- https://github.com/sustainable-processes/ontology/OntoCAPE/model/equation_system.owl#hasNumericalStiffness -->

    <owl:ObjectProperty rdf:about="https://github.com/sustainable-processes/ontology/OntoCAPE/model/equation_system.owl#hasNumericalStiffness">
        <rdfs:subPropertyOf rdf:resource="https://github.com/sustainable-processes/ontology/OntoCAPE/upper_level/system.owl#hasCharacteristic"/>
        <rdfs:domain rdf:resource="https://github.com/sustainable-processes/ontology/OntoCAPE/model/equation_system.owl#OrdinaryDifferentialEquationSystem"/>
        <rdfs:range rdf:resource="https://github.com/sustainable-processes/ontology/OntoCAPE/model/equation_system.owl#NumericalStiffness"/>
        <rdfs:comment>Indicates an EquationSystemCharacteristic of type NumericalStiffness</rdfs:comment>
    </owl:ObjectProperty>
    


    <!-- https://github.com/sustainable-processes/ontology/OntoCAPE/model/equation_system.owl#hasODE_explicitness -->

    <owl:ObjectProperty rdf:about="https://github.com/sustainable-processes/ontology/OntoCAPE/model/equation_system.owl#hasODE_explicitness">
        <rdfs:subPropertyOf rdf:resource="https://github.com/sustainable-processes/ontology/OntoCAPE/upper_level/system.owl#hasCharacteristic"/>
        <rdfs:domain rdf:resource="https://github.com/sustainable-processes/ontology/OntoCAPE/model/equation_system.owl#OrdinaryDifferentialEquationSystem"/>
        <rdfs:range rdf:resource="https://github.com/sustainable-processes/ontology/OntoCAPE/model/equation_system.owl#ODE_Explicitness"/>
        <rdfs:comment>Indicates an EquationSystemCharacteristic of type ODE_Explicitness.</rdfs:comment>
    </owl:ObjectProperty>
    


    <!-- https://github.com/sustainable-processes/ontology/OntoCAPE/model/equation_system.owl#hasVariablesType -->

    <owl:ObjectProperty rdf:about="https://github.com/sustainable-processes/ontology/OntoCAPE/model/equation_system.owl#hasVariablesType">
        <rdfs:subPropertyOf rdf:resource="https://github.com/sustainable-processes/ontology/OntoCAPE/upper_level/system.owl#hasCharacteristic"/>
        <rdfs:domain rdf:resource="https://github.com/sustainable-processes/ontology/OntoCAPE/model/mathematical_model.owl#MathematicalModel"/>
        <rdfs:range rdf:resource="https://github.com/sustainable-processes/ontology/OntoCAPE/model/equation_system.owl#VariablesType"/>
        <rdfs:comment>Indicates an EquationSystemCharacteristic of type VariablesType</rdfs:comment>
    </owl:ObjectProperty>
    


    <!-- https://github.com/sustainable-processes/ontology/OntoCAPE/upper_level/system.owl#hasCharacteristic -->

    <owl:ObjectProperty rdf:about="https://github.com/sustainable-processes/ontology/OntoCAPE/upper_level/system.owl#hasCharacteristic"/>
    


    <!-- 
    ///////////////////////////////////////////////////////////////////////////////////////
    //
    // Data properties
    //
    ///////////////////////////////////////////////////////////////////////////////////////
     -->

    


    <!-- https://github.com/sustainable-processes/ontology/OntoCAPE/model/equation_system.owl#differentialIndex -->

    <owl:DatatypeProperty rdf:about="https://github.com/sustainable-processes/ontology/OntoCAPE/model/equation_system.owl#differentialIndex">
        <rdfs:domain rdf:resource="https://github.com/sustainable-processes/ontology/OntoCAPE/model/equation_system.owl#DifferentialAlgebraicEquationSystem"/>
        <rdfs:range rdf:resource="http://www.w3.org/2001/XMLSchema#int"/>
        <rdfs:comment>The attribute represents the differential index of a DAE system, as defined by Gear &amp; Petzold (1984).</rdfs:comment>
    </owl:DatatypeProperty>
    


    <!-- https://github.com/sustainable-processes/ontology/OntoCAPE/model/equation_system.owl#differentialOrder -->

    <owl:DatatypeProperty rdf:about="https://github.com/sustainable-processes/ontology/OntoCAPE/model/equation_system.owl#differentialOrder">
        <rdfs:domain rdf:resource="https://github.com/sustainable-processes/ontology/OntoCAPE/model/equation_system.owl#DifferentialEquationSystem"/>
        <rdfs:range rdf:resource="http://www.w3.org/2001/XMLSchema#int"/>
        <rdfs:comment>The attribute differentialOrder denotes the order of a differential equation, which is defined as the order of the highest derivative of a ModelVariable appearing in the differential equation</rdfs:comment>
    </owl:DatatypeProperty>
    


    <!-- 
    ///////////////////////////////////////////////////////////////////////////////////////
    //
    // Classes
    //
    ///////////////////////////////////////////////////////////////////////////////////////
     -->

    


    <!-- https://github.com/sustainable-processes/ontology/OntoCAPE/model/equation_system.owl#AlgebraicEquationSystem -->

    <owl:Class rdf:about="https://github.com/sustainable-processes/ontology/OntoCAPE/model/equation_system.owl#AlgebraicEquationSystem">
        <owl:equivalentClass>
            <owl:Class>
                <owl:unionOf rdf:parseType="Collection">
                    <rdf:Description rdf:about="https://github.com/sustainable-processes/ontology/OntoCAPE/model/equation_system.owl#LinearAlgebraicSystem"/>
                    <rdf:Description rdf:about="https://github.com/sustainable-processes/ontology/OntoCAPE/model/equation_system.owl#NonlinearAlgebraicSystem"/>
                </owl:unionOf>
            </owl:Class>
        </owl:equivalentClass>
        <rdfs:subClassOf rdf:resource="https://github.com/sustainable-processes/ontology/OntoCAPE/model/mathematical_model.owl#MathematicalModel"/>
        <rdfs:subClassOf>
            <owl:Restriction>
                <owl:onProperty rdf:resource="https://github.com/sustainable-processes/ontology/OntoCAPE/model/equation_system.owl#hasLinearity"/>
                <owl:someValuesFrom rdf:resource="https://github.com/sustainable-processes/ontology/OntoCAPE/model/equation_system.owl#Linearity"/>
            </owl:Restriction>
        </rdfs:subClassOf>
        <rdfs:subClassOf>
            <owl:Restriction>
                <owl:onProperty rdf:resource="https://github.com/sustainable-processes/ontology/OntoCAPE/model/equation_system.owl#hasLinearity"/>
                <owl:allValuesFrom rdf:resource="https://github.com/sustainable-processes/ontology/OntoCAPE/model/equation_system.owl#Linearity"/>
            </owl:Restriction>
        </rdfs:subClassOf>
        <rdfs:subClassOf>
            <owl:Restriction>
                <owl:onProperty rdf:resource="https://github.com/sustainable-processes/ontology/OntoCAPE/model/equation_system.owl#hasLinearity"/>
                <owl:cardinality rdf:datatype="http://www.w3.org/2001/XMLSchema#nonNegativeInteger">1</owl:cardinality>
            </owl:Restriction>
        </rdfs:subClassOf>
        <owl:disjointWith rdf:resource="https://github.com/sustainable-processes/ontology/OntoCAPE/model/equation_system.owl#DifferentialAlgebraicEquationSystem"/>
        <owl:disjointWith rdf:resource="https://github.com/sustainable-processes/ontology/OntoCAPE/model/equation_system.owl#DifferentialEquationSystem"/>
        <rdfs:comment>An AlgebraicEquationSystem is a MathematicalModel which solely consists of algebraic equations.</rdfs:comment>
    </owl:Class>
    


    <!-- https://github.com/sustainable-processes/ontology/OntoCAPE/model/equation_system.owl#DAE_Explicitness -->

    <owl:Class rdf:about="https://github.com/sustainable-processes/ontology/OntoCAPE/model/equation_system.owl#DAE_Explicitness">
        <owl:equivalentClass>
            <owl:Class>
                <owl:oneOf rdf:parseType="Collection">
                    <rdf:Description rdf:about="https://github.com/sustainable-processes/ontology/OntoCAPE/model/equation_system.owl#fully_implicit"/>
                    <rdf:Description rdf:about="https://github.com/sustainable-processes/ontology/OntoCAPE/model/equation_system.owl#semi-explicit"/>
                </owl:oneOf>
            </owl:Class>
        </owl:equivalentClass>
        <rdfs:subClassOf rdf:resource="https://github.com/sustainable-processes/ontology/OntoCAPE/model/equation_system.owl#EquationSystemCharacteristics"/>
        <owl:disjointWith rdf:resource="https://github.com/sustainable-processes/ontology/OntoCAPE/model/equation_system.owl#Linearity"/>
        <owl:disjointWith rdf:resource="https://github.com/sustainable-processes/ontology/OntoCAPE/model/equation_system.owl#ModelRepresentationForm"/>
        <owl:disjointWith rdf:resource="https://github.com/sustainable-processes/ontology/OntoCAPE/model/equation_system.owl#NumericalStiffness"/>
        <owl:disjointWith rdf:resource="https://github.com/sustainable-processes/ontology/OntoCAPE/model/equation_system.owl#ODE_Explicitness"/>
        <owl:disjointWith rdf:resource="https://github.com/sustainable-processes/ontology/OntoCAPE/model/equation_system.owl#VariablesType"/>
        <rdfs:comment>Characterizes the explicitness of a DAE system</rdfs:comment>
    </owl:Class>
    


    <!-- https://github.com/sustainable-processes/ontology/OntoCAPE/model/equation_system.owl#DifferentialAlgebraicEquationSystem -->

    <owl:Class rdf:about="https://github.com/sustainable-processes/ontology/OntoCAPE/model/equation_system.owl#DifferentialAlgebraicEquationSystem">
        <owl:equivalentClass>
            <owl:Class>
                <owl:unionOf rdf:parseType="Collection">
                    <rdf:Description rdf:about="https://github.com/sustainable-processes/ontology/OntoCAPE/model/equation_system.owl#OrdinaryDifferentialAlgebraicSystem"/>
                    <rdf:Description rdf:about="https://github.com/sustainable-processes/ontology/OntoCAPE/model/equation_system.owl#PartialDifferentialAlgebraicSystem"/>
                </owl:unionOf>
            </owl:Class>
        </owl:equivalentClass>
        <rdfs:subClassOf rdf:resource="https://github.com/sustainable-processes/ontology/OntoCAPE/model/mathematical_model.owl#MathematicalModel"/>
        <rdfs:subClassOf>
            <owl:Restriction>
                <owl:onProperty rdf:resource="https://github.com/sustainable-processes/ontology/OntoCAPE/model/equation_system.owl#hasDAE_Explicitness"/>
                <owl:someValuesFrom rdf:resource="https://github.com/sustainable-processes/ontology/OntoCAPE/model/equation_system.owl#DAE_Explicitness"/>
            </owl:Restriction>
        </rdfs:subClassOf>
        <rdfs:subClassOf>
            <owl:Restriction>
                <owl:onProperty rdf:resource="https://github.com/sustainable-processes/ontology/OntoCAPE/model/equation_system.owl#hasLinearity"/>
                <owl:someValuesFrom rdf:resource="https://github.com/sustainable-processes/ontology/OntoCAPE/model/equation_system.owl#Linearity"/>
            </owl:Restriction>
        </rdfs:subClassOf>
        <rdfs:subClassOf>
            <owl:Restriction>
                <owl:onProperty rdf:resource="https://github.com/sustainable-processes/ontology/OntoCAPE/model/equation_system.owl#hasDAE_Explicitness"/>
                <owl:allValuesFrom rdf:resource="https://github.com/sustainable-processes/ontology/OntoCAPE/model/equation_system.owl#DAE_Explicitness"/>
            </owl:Restriction>
        </rdfs:subClassOf>
        <rdfs:subClassOf>
            <owl:Restriction>
                <owl:onProperty rdf:resource="https://github.com/sustainable-processes/ontology/OntoCAPE/model/equation_system.owl#hasLinearity"/>
                <owl:allValuesFrom rdf:resource="https://github.com/sustainable-processes/ontology/OntoCAPE/model/equation_system.owl#Linearity"/>
            </owl:Restriction>
        </rdfs:subClassOf>
        <rdfs:subClassOf>
            <owl:Restriction>
                <owl:onProperty rdf:resource="https://github.com/sustainable-processes/ontology/OntoCAPE/model/equation_system.owl#hasDAE_Explicitness"/>
                <owl:cardinality rdf:datatype="http://www.w3.org/2001/XMLSchema#nonNegativeInteger">1</owl:cardinality>
            </owl:Restriction>
        </rdfs:subClassOf>
        <rdfs:subClassOf>
            <owl:Restriction>
                <owl:onProperty rdf:resource="https://github.com/sustainable-processes/ontology/OntoCAPE/model/equation_system.owl#hasLinearity"/>
                <owl:cardinality rdf:datatype="http://www.w3.org/2001/XMLSchema#nonNegativeInteger">1</owl:cardinality>
            </owl:Restriction>
        </rdfs:subClassOf>
        <rdfs:subClassOf>
            <owl:Restriction>
                <owl:onProperty rdf:resource="https://github.com/sustainable-processes/ontology/OntoCAPE/model/equation_system.owl#differentialIndex"/>
                <owl:cardinality rdf:datatype="http://www.w3.org/2001/XMLSchema#nonNegativeInteger">1</owl:cardinality>
            </owl:Restriction>
        </rdfs:subClassOf>
        <owl:disjointWith rdf:resource="https://github.com/sustainable-processes/ontology/OntoCAPE/model/equation_system.owl#DifferentialEquationSystem"/>
        <rdfs:comment>A DifferentialAlgebraicEquationSystem (DAE system) is a MathematicalModel that comprises both algebraic and differential equations.</rdfs:comment>
    </owl:Class>
    


    <!-- https://github.com/sustainable-processes/ontology/OntoCAPE/model/equation_system.owl#DifferentialEquationSystem -->

    <owl:Class rdf:about="https://github.com/sustainable-processes/ontology/OntoCAPE/model/equation_system.owl#DifferentialEquationSystem">
        <owl:equivalentClass>
            <owl:Class>
                <owl:unionOf rdf:parseType="Collection">
                    <rdf:Description rdf:about="https://github.com/sustainable-processes/ontology/OntoCAPE/model/equation_system.owl#OrdinaryDifferentialEquationSystem"/>
                    <rdf:Description rdf:about="https://github.com/sustainable-processes/ontology/OntoCAPE/model/equation_system.owl#PartialDifferentialEquationSystem"/>
                </owl:unionOf>
            </owl:Class>
        </owl:equivalentClass>
        <rdfs:subClassOf rdf:resource="https://github.com/sustainable-processes/ontology/OntoCAPE/model/mathematical_model.owl#MathematicalModel"/>
        <rdfs:subClassOf>
            <owl:Restriction>
                <owl:onProperty rdf:resource="https://github.com/sustainable-processes/ontology/OntoCAPE/model/equation_system.owl#differentialOrder"/>
                <owl:cardinality rdf:datatype="http://www.w3.org/2001/XMLSchema#nonNegativeInteger">1</owl:cardinality>
            </owl:Restriction>
        </rdfs:subClassOf>
        <rdfs:comment>A DifferentialEquationSystem is a MathematicalModel that solely consists of differential equations.</rdfs:comment>
    </owl:Class>
    


    <!-- https://github.com/sustainable-processes/ontology/OntoCAPE/model/equation_system.owl#EquationSystemCharacteristics -->

    <owl:Class rdf:about="https://github.com/sustainable-processes/ontology/OntoCAPE/model/equation_system.owl#EquationSystemCharacteristics">
        <rdfs:subClassOf rdf:resource="https://github.com/sustainable-processes/ontology/OntoCAPE/upper_level/system.owl#FixedValueSet"/>
        <rdfs:comment>The EquationSystemCharacteristics characterize the model equations of a MathematicalModel.</rdfs:comment>
    </owl:Class>
    


    <!-- https://github.com/sustainable-processes/ontology/OntoCAPE/model/equation_system.owl#LinearAlgebraicSystem -->

    <owl:Class rdf:about="https://github.com/sustainable-processes/ontology/OntoCAPE/model/equation_system.owl#LinearAlgebraicSystem">
        <owl:equivalentClass>
            <owl:Class>
                <owl:intersectionOf rdf:parseType="Collection">
                    <rdf:Description rdf:about="https://github.com/sustainable-processes/ontology/OntoCAPE/model/equation_system.owl#AlgebraicEquationSystem"/>
                    <owl:Restriction>
                        <owl:onProperty rdf:resource="https://github.com/sustainable-processes/ontology/OntoCAPE/model/equation_system.owl#hasLinearity"/>
                        <owl:hasValue rdf:resource="https://github.com/sustainable-processes/ontology/OntoCAPE/model/equation_system.owl#linear"/>
                    </owl:Restriction>
                </owl:intersectionOf>
            </owl:Class>
        </owl:equivalentClass>
        <owl:disjointWith rdf:resource="https://github.com/sustainable-processes/ontology/OntoCAPE/model/equation_system.owl#NonlinearAlgebraicSystem"/>
        <rdfs:comment>A LinearAlgebraicSystem is an AlgebraicSystem which contains only linear equations.</rdfs:comment>
    </owl:Class>
    


    <!-- https://github.com/sustainable-processes/ontology/OntoCAPE/model/equation_system.owl#Linearity -->

    <owl:Class rdf:about="https://github.com/sustainable-processes/ontology/OntoCAPE/model/equation_system.owl#Linearity">
        <owl:equivalentClass>
            <owl:Class>
                <owl:oneOf rdf:parseType="Collection">
                    <rdf:Description rdf:about="https://github.com/sustainable-processes/ontology/OntoCAPE/model/equation_system.owl#linear"/>
                    <rdf:Description rdf:about="https://github.com/sustainable-processes/ontology/OntoCAPE/model/equation_system.owl#nonlinear"/>
                </owl:oneOf>
            </owl:Class>
        </owl:equivalentClass>
        <rdfs:subClassOf rdf:resource="https://github.com/sustainable-processes/ontology/OntoCAPE/model/equation_system.owl#EquationSystemCharacteristics"/>
        <owl:disjointWith rdf:resource="https://github.com/sustainable-processes/ontology/OntoCAPE/model/equation_system.owl#ModelRepresentationForm"/>
        <owl:disjointWith rdf:resource="https://github.com/sustainable-processes/ontology/OntoCAPE/model/equation_system.owl#NumericalStiffness"/>
        <owl:disjointWith rdf:resource="https://github.com/sustainable-processes/ontology/OntoCAPE/model/equation_system.owl#ODE_Explicitness"/>
        <owl:disjointWith rdf:resource="https://github.com/sustainable-processes/ontology/OntoCAPE/model/equation_system.owl#VariablesType"/>
        <rdfs:comment>Characterizes the linearity of a (Differential)AlgebrailEquationSystem.</rdfs:comment>
    </owl:Class>
    


    <!-- https://github.com/sustainable-processes/ontology/OntoCAPE/model/equation_system.owl#ModelRepresentationForm -->

    <owl:Class rdf:about="https://github.com/sustainable-processes/ontology/OntoCAPE/model/equation_system.owl#ModelRepresentationForm">
        <owl:equivalentClass>
            <owl:Class>
                <owl:oneOf rdf:parseType="Collection">
                    <rdf:Description rdf:about="https://github.com/sustainable-processes/ontology/OntoCAPE/model/equation_system.owl#closed_form"/>
                    <rdf:Description rdf:about="https://github.com/sustainable-processes/ontology/OntoCAPE/model/equation_system.owl#open_form"/>
                </owl:oneOf>
            </owl:Class>
        </owl:equivalentClass>
        <rdfs:subClassOf rdf:resource="https://github.com/sustainable-processes/ontology/OntoCAPE/model/equation_system.owl#EquationSystemCharacteristics"/>
        <owl:disjointWith rdf:resource="https://github.com/sustainable-processes/ontology/OntoCAPE/model/equation_system.owl#NumericalStiffness"/>
        <owl:disjointWith rdf:resource="https://github.com/sustainable-processes/ontology/OntoCAPE/model/equation_system.owl#ODE_Explicitness"/>
        <owl:disjointWith rdf:resource="https://github.com/sustainable-processes/ontology/OntoCAPE/model/equation_system.owl#VariablesType"/>
        <rdfs:comment>A MathematicalModel may appear in two forms, as indicated by the ModelRepresentationForm: 
- An open-form model is solved by an external algorithm. One can freely choose the inputs and outputs of the open-form model.
- A closed-form model includes an underlying numerical algorithm that solves the model equations. The algorithm accepts only a fixed set of input variables, and consequently returns only a fixed set of output variables.</rdfs:comment>
    </owl:Class>
    


    <!-- https://github.com/sustainable-processes/ontology/OntoCAPE/model/equation_system.owl#NonlinearAlgebraicSystem -->

    <owl:Class rdf:about="https://github.com/sustainable-processes/ontology/OntoCAPE/model/equation_system.owl#NonlinearAlgebraicSystem">
        <owl:equivalentClass>
            <owl:Class>
                <owl:intersectionOf rdf:parseType="Collection">
                    <rdf:Description rdf:about="https://github.com/sustainable-processes/ontology/OntoCAPE/model/equation_system.owl#AlgebraicEquationSystem"/>
                    <owl:Restriction>
                        <owl:onProperty rdf:resource="https://github.com/sustainable-processes/ontology/OntoCAPE/model/equation_system.owl#hasLinearity"/>
                        <owl:hasValue rdf:resource="https://github.com/sustainable-processes/ontology/OntoCAPE/model/equation_system.owl#nonlinear"/>
                    </owl:Restriction>
                </owl:intersectionOf>
            </owl:Class>
        </owl:equivalentClass>
        <rdfs:comment>A NonlinearAlgebraicSystem is an AlgebraicEquationSystem that is characterized as nonlinear.</rdfs:comment>
    </owl:Class>
    


    <!-- https://github.com/sustainable-processes/ontology/OntoCAPE/model/equation_system.owl#NumericalStiffness -->

    <owl:Class rdf:about="https://github.com/sustainable-processes/ontology/OntoCAPE/model/equation_system.owl#NumericalStiffness">
        <owl:equivalentClass>
            <owl:Class>
                <owl:oneOf rdf:parseType="Collection">
                    <rdf:Description rdf:about="https://github.com/sustainable-processes/ontology/OntoCAPE/model/equation_system.owl#nonstiff"/>
                    <rdf:Description rdf:about="https://github.com/sustainable-processes/ontology/OntoCAPE/model/equation_system.owl#stiff"/>
                </owl:oneOf>
            </owl:Class>
        </owl:equivalentClass>
        <rdfs:subClassOf rdf:resource="https://github.com/sustainable-processes/ontology/OntoCAPE/model/equation_system.owl#EquationSystemCharacteristics"/>
        <owl:disjointWith rdf:resource="https://github.com/sustainable-processes/ontology/OntoCAPE/model/equation_system.owl#ODE_Explicitness"/>
        <owl:disjointWith rdf:resource="https://github.com/sustainable-processes/ontology/OntoCAPE/model/equation_system.owl#VariablesType"/>
        <rdfs:comment>In mathematics, a stiff equation is a differential equation for which certain numerical methods for solving the equation are numerically unstable, unless the step size is taken to be extremely small. It has proved difficult to formulate a precise definition of stiffness, but the main idea is that the equation includes some terms that can lead to rapid variation in the solution (Wikipedia, 2007).</rdfs:comment>
    </owl:Class>
    


    <!-- https://github.com/sustainable-processes/ontology/OntoCAPE/model/equation_system.owl#ODE_Explicitness -->

    <owl:Class rdf:about="https://github.com/sustainable-processes/ontology/OntoCAPE/model/equation_system.owl#ODE_Explicitness">
        <owl:equivalentClass>
            <owl:Class>
                <owl:oneOf rdf:parseType="Collection">
                    <rdf:Description rdf:about="https://github.com/sustainable-processes/ontology/OntoCAPE/model/equation_system.owl#explicit_formulation"/>
                    <rdf:Description rdf:about="https://github.com/sustainable-processes/ontology/OntoCAPE/model/equation_system.owl#implicit_formulation"/>
                </owl:oneOf>
            </owl:Class>
        </owl:equivalentClass>
        <rdfs:subClassOf rdf:resource="https://github.com/sustainable-processes/ontology/OntoCAPE/model/equation_system.owl#EquationSystemCharacteristics"/>
        <owl:disjointWith rdf:resource="https://github.com/sustainable-processes/ontology/OntoCAPE/model/equation_system.owl#VariablesType"/>
        <rdfs:comment>Characterizes the explicitness of an OrdinaryDifferentialEquationSystem, which can be given in implicit_formulation or explicit_formulation.</rdfs:comment>
    </owl:Class>
    


    <!-- https://github.com/sustainable-processes/ontology/OntoCAPE/model/equation_system.owl#OrdinaryDifferentialAlgebraicSystem -->

    <owl:Class rdf:about="https://github.com/sustainable-processes/ontology/OntoCAPE/model/equation_system.owl#OrdinaryDifferentialAlgebraicSystem">
        <rdfs:subClassOf rdf:resource="https://github.com/sustainable-processes/ontology/OntoCAPE/model/equation_system.owl#DifferentialAlgebraicEquationSystem"/>
        <owl:disjointWith rdf:resource="https://github.com/sustainable-processes/ontology/OntoCAPE/model/equation_system.owl#PartialDifferentialAlgebraicSystem"/>
        <rdfs:comment>An OrdinaryDifferentialAlgebraicSystem is a DifferentialAlgebraicSystem system which comprises ordinary differential equations as well as algebraic equations.</rdfs:comment>
    </owl:Class>
    


    <!-- https://github.com/sustainable-processes/ontology/OntoCAPE/model/equation_system.owl#OrdinaryDifferentialEquationSystem -->

    <owl:Class rdf:about="https://github.com/sustainable-processes/ontology/OntoCAPE/model/equation_system.owl#OrdinaryDifferentialEquationSystem">
        <rdfs:subClassOf rdf:resource="https://github.com/sustainable-processes/ontology/OntoCAPE/model/equation_system.owl#DifferentialEquationSystem"/>
        <rdfs:subClassOf>
            <owl:Restriction>
                <owl:onProperty rdf:resource="https://github.com/sustainable-processes/ontology/OntoCAPE/model/equation_system.owl#hasNumericalStiffness"/>
                <owl:someValuesFrom rdf:resource="https://github.com/sustainable-processes/ontology/OntoCAPE/model/equation_system.owl#NumericalStiffness"/>
            </owl:Restriction>
        </rdfs:subClassOf>
        <rdfs:subClassOf>
            <owl:Restriction>
                <owl:onProperty rdf:resource="https://github.com/sustainable-processes/ontology/OntoCAPE/model/equation_system.owl#hasODE_explicitness"/>
                <owl:someValuesFrom rdf:resource="https://github.com/sustainable-processes/ontology/OntoCAPE/model/equation_system.owl#ODE_Explicitness"/>
            </owl:Restriction>
        </rdfs:subClassOf>
        <rdfs:subClassOf>
            <owl:Restriction>
                <owl:onProperty rdf:resource="https://github.com/sustainable-processes/ontology/OntoCAPE/model/equation_system.owl#hasNumericalStiffness"/>
                <owl:allValuesFrom rdf:resource="https://github.com/sustainable-processes/ontology/OntoCAPE/model/equation_system.owl#NumericalStiffness"/>
            </owl:Restriction>
        </rdfs:subClassOf>
        <rdfs:subClassOf>
            <owl:Restriction>
                <owl:onProperty rdf:resource="https://github.com/sustainable-processes/ontology/OntoCAPE/model/equation_system.owl#hasODE_explicitness"/>
                <owl:allValuesFrom rdf:resource="https://github.com/sustainable-processes/ontology/OntoCAPE/model/equation_system.owl#ODE_Explicitness"/>
            </owl:Restriction>
        </rdfs:subClassOf>
        <rdfs:subClassOf>
            <owl:Restriction>
                <owl:onProperty rdf:resource="https://github.com/sustainable-processes/ontology/OntoCAPE/model/equation_system.owl#hasNumericalStiffness"/>
                <owl:cardinality rdf:datatype="http://www.w3.org/2001/XMLSchema#nonNegativeInteger">1</owl:cardinality>
            </owl:Restriction>
        </rdfs:subClassOf>
        <rdfs:subClassOf>
            <owl:Restriction>
                <owl:onProperty rdf:resource="https://github.com/sustainable-processes/ontology/OntoCAPE/model/equation_system.owl#hasODE_explicitness"/>
                <owl:cardinality rdf:datatype="http://www.w3.org/2001/XMLSchema#nonNegativeInteger">1</owl:cardinality>
            </owl:Restriction>
        </rdfs:subClassOf>
        <owl:disjointWith rdf:resource="https://github.com/sustainable-processes/ontology/OntoCAPE/model/equation_system.owl#PartialDifferentialEquationSystem"/>
        <rdfs:comment>An OrdinaryDifferentialEquationSystem (ODE system) is a DifferentialEquationSystem which solely consists of ordinary differential equations.</rdfs:comment>
    </owl:Class>
    


    <!-- https://github.com/sustainable-processes/ontology/OntoCAPE/model/equation_system.owl#PartialDifferentialAlgebraicSystem -->

    <owl:Class rdf:about="https://github.com/sustainable-processes/ontology/OntoCAPE/model/equation_system.owl#PartialDifferentialAlgebraicSystem">
        <rdfs:subClassOf rdf:resource="https://github.com/sustainable-processes/ontology/OntoCAPE/model/equation_system.owl#DifferentialAlgebraicEquationSystem"/>
        <rdfs:comment>A PartialDifferentialAlgebraicSystem comprises both partial differential equations and algebraic equations.</rdfs:comment>
    </owl:Class>
    


    <!-- https://github.com/sustainable-processes/ontology/OntoCAPE/model/equation_system.owl#PartialDifferentialEquationSystem -->

    <owl:Class rdf:about="https://github.com/sustainable-processes/ontology/OntoCAPE/model/equation_system.owl#PartialDifferentialEquationSystem">
        <rdfs:subClassOf rdf:resource="https://github.com/sustainable-processes/ontology/OntoCAPE/model/equation_system.owl#DifferentialEquationSystem"/>
        <rdfs:comment>A PartialDifferentialEquationSystem (PDE system) is a DifferentialEquationSystem which consists of partial differential equations.</rdfs:comment>
    </owl:Class>
    


    <!-- https://github.com/sustainable-processes/ontology/OntoCAPE/model/equation_system.owl#VariablesType -->

    <owl:Class rdf:about="https://github.com/sustainable-processes/ontology/OntoCAPE/model/equation_system.owl#VariablesType">
        <owl:equivalentClass>
            <owl:Class>
                <owl:oneOf rdf:parseType="Collection">
                    <rdf:Description rdf:about="https://github.com/sustainable-processes/ontology/OntoCAPE/model/equation_system.owl#continuous_model"/>
                    <rdf:Description rdf:about="https://github.com/sustainable-processes/ontology/OntoCAPE/model/equation_system.owl#discrete_model"/>
                    <rdf:Description rdf:about="https://github.com/sustainable-processes/ontology/OntoCAPE/model/equation_system.owl#mixed_model"/>
                </owl:oneOf>
            </owl:Class>
        </owl:equivalentClass>
        <rdfs:subClassOf rdf:resource="https://github.com/sustainable-processes/ontology/OntoCAPE/model/equation_system.owl#EquationSystemCharacteristics"/>
        <rdfs:comment>A VariablesType indicates whether the ModelVariables of a MathematicalModel are all continuous, all discrete, or partly continuous and partly discrete:
-   A continuous_model denotes a MathematicalModel in which all the ModelVariables are continuous.
-   A discrete_model denotes a MathematicalModel in which all the ModelVariables are discrete. An example of a mixed_model is an integer model.
-   A mixed_model denotes a MathematicalModel in which some of the model variables are discrete while the others are continuous. An example of a mixed_model is a mixed integer model.</rdfs:comment>
    </owl:Class>
    


    <!-- https://github.com/sustainable-processes/ontology/OntoCAPE/model/mathematical_model.owl#MathematicalModel -->

    <owl:Class rdf:about="https://github.com/sustainable-processes/ontology/OntoCAPE/model/mathematical_model.owl#MathematicalModel">
        <rdfs:subClassOf>
            <owl:Restriction>
                <owl:onProperty rdf:resource="https://github.com/sustainable-processes/ontology/OntoCAPE/model/equation_system.owl#hasModelRepresentationForm"/>
                <owl:someValuesFrom rdf:resource="https://github.com/sustainable-processes/ontology/OntoCAPE/model/equation_system.owl#ModelRepresentationForm"/>
            </owl:Restriction>
        </rdfs:subClassOf>
        <rdfs:subClassOf>
            <owl:Restriction>
                <owl:onProperty rdf:resource="https://github.com/sustainable-processes/ontology/OntoCAPE/model/equation_system.owl#hasVariablesType"/>
                <owl:someValuesFrom rdf:resource="https://github.com/sustainable-processes/ontology/OntoCAPE/model/equation_system.owl#VariablesType"/>
            </owl:Restriction>
        </rdfs:subClassOf>
        <rdfs:subClassOf>
            <owl:Restriction>
                <owl:onProperty rdf:resource="https://github.com/sustainable-processes/ontology/OntoCAPE/model/equation_system.owl#hasModelRepresentationForm"/>
                <owl:allValuesFrom rdf:resource="https://github.com/sustainable-processes/ontology/OntoCAPE/model/equation_system.owl#ModelRepresentationForm"/>
            </owl:Restriction>
        </rdfs:subClassOf>
        <rdfs:subClassOf>
            <owl:Restriction>
                <owl:onProperty rdf:resource="https://github.com/sustainable-processes/ontology/OntoCAPE/model/equation_system.owl#hasVariablesType"/>
                <owl:allValuesFrom rdf:resource="https://github.com/sustainable-processes/ontology/OntoCAPE/model/equation_system.owl#VariablesType"/>
            </owl:Restriction>
        </rdfs:subClassOf>
        <rdfs:subClassOf>
            <owl:Restriction>
                <owl:onProperty rdf:resource="https://github.com/sustainable-processes/ontology/OntoCAPE/model/equation_system.owl#hasModelRepresentationForm"/>
                <owl:cardinality rdf:datatype="http://www.w3.org/2001/XMLSchema#nonNegativeInteger">1</owl:cardinality>
            </owl:Restriction>
        </rdfs:subClassOf>
        <rdfs:subClassOf>
            <owl:Restriction>
                <owl:onProperty rdf:resource="https://github.com/sustainable-processes/ontology/OntoCAPE/model/equation_system.owl#hasVariablesType"/>
                <owl:cardinality rdf:datatype="http://www.w3.org/2001/XMLSchema#nonNegativeInteger">1</owl:cardinality>
            </owl:Restriction>
        </rdfs:subClassOf>
    </owl:Class>
    


    <!-- https://github.com/sustainable-processes/ontology/OntoCAPE/upper_level/system.owl#FixedValueSet -->

    <owl:Class rdf:about="https://github.com/sustainable-processes/ontology/OntoCAPE/upper_level/system.owl#FixedValueSet"/>
    


    <!-- 
    ///////////////////////////////////////////////////////////////////////////////////////
    //
    // Individuals
    //
    ///////////////////////////////////////////////////////////////////////////////////////
     -->

    


    <!-- https://github.com/sustainable-processes/ontology/OntoCAPE/model/equation_system.owl#closed_form -->

    <owl:NamedIndividual rdf:about="https://github.com/sustainable-processes/ontology/OntoCAPE/model/equation_system.owl#closed_form">
        <rdf:type rdf:resource="https://github.com/sustainable-processes/ontology/OntoCAPE/model/equation_system.owl#ModelRepresentationForm"/>
        <owl:differentFrom rdf:resource="https://github.com/sustainable-processes/ontology/OntoCAPE/model/equation_system.owl#open_form"/>
        <rdfs:comment>A closed-form model includes an underlying numerical algorithm that solves the model equations. The algorithm accepts only a fixed set of input variables, and consequently returns only a fixed set of output variables.</rdfs:comment>
    </owl:NamedIndividual>
    


    <!-- https://github.com/sustainable-processes/ontology/OntoCAPE/model/equation_system.owl#continuous_model -->

    <owl:NamedIndividual rdf:about="https://github.com/sustainable-processes/ontology/OntoCAPE/model/equation_system.owl#continuous_model">
        <rdf:type rdf:resource="https://github.com/sustainable-processes/ontology/OntoCAPE/model/equation_system.owl#VariablesType"/>
        <owl:differentFrom rdf:resource="https://github.com/sustainable-processes/ontology/OntoCAPE/model/equation_system.owl#discrete_model"/>
        <owl:differentFrom rdf:resource="https://github.com/sustainable-processes/ontology/OntoCAPE/model/equation_system.owl#mixed_model"/>
        <rdfs:comment>A continuous_model denotes a MathematicalModel in which all the ModelVariables are continuous.</rdfs:comment>
    </owl:NamedIndividual>
    


    <!-- https://github.com/sustainable-processes/ontology/OntoCAPE/model/equation_system.owl#discrete_model -->

    <owl:NamedIndividual rdf:about="https://github.com/sustainable-processes/ontology/OntoCAPE/model/equation_system.owl#discrete_model">
        <rdf:type rdf:resource="https://github.com/sustainable-processes/ontology/OntoCAPE/model/equation_system.owl#VariablesType"/>
        <owl:differentFrom rdf:resource="https://github.com/sustainable-processes/ontology/OntoCAPE/model/equation_system.owl#mixed_model"/>
        <rdfs:comment>A discrete_model denotes a MathematicalModel in which all the ModelVariables are discrete. An example of a discrete_model is an integer model.</rdfs:comment>
    </owl:NamedIndividual>
    


    <!-- https://github.com/sustainable-processes/ontology/OntoCAPE/model/equation_system.owl#explicit_formulation -->

    <owl:NamedIndividual rdf:about="https://github.com/sustainable-processes/ontology/OntoCAPE/model/equation_system.owl#explicit_formulation">
        <rdf:type rdf:resource="https://github.com/sustainable-processes/ontology/OntoCAPE/model/equation_system.owl#ODE_Explicitness"/>
        <owl:differentFrom rdf:resource="https://github.com/sustainable-processes/ontology/OntoCAPE/model/equation_system.owl#implicit_formulation"/>
        <rdfs:comment>In an explicit_formulation, the OrdinaryDifferentialAlgebraicSystem is explicitly solved for the highest-order derivative y^(n), i.e., F(x, y, y&apos;, y&apos;&apos;, ...  y^(n-1) ) = y^(n)</rdfs:comment>
    </owl:NamedIndividual>
    


    <!-- https://github.com/sustainable-processes/ontology/OntoCAPE/model/equation_system.owl#fully_implicit -->

    <owl:NamedIndividual rdf:about="https://github.com/sustainable-processes/ontology/OntoCAPE/model/equation_system.owl#fully_implicit">
        <rdf:type rdf:resource="https://github.com/sustainable-processes/ontology/OntoCAPE/model/equation_system.owl#DAE_Explicitness"/>
        <owl:differentFrom rdf:resource="https://github.com/sustainable-processes/ontology/OntoCAPE/model/equation_system.owl#semi-explicit"/>
        <rdfs:comment>A DifferentialAlgebraicEquationSystem is fully_implicit if it has the form
  F(x, x&apos;, u, t) = 0</rdfs:comment>
    </owl:NamedIndividual>
    


    <!-- https://github.com/sustainable-processes/ontology/OntoCAPE/model/equation_system.owl#implicit_formulation -->

    <owl:NamedIndividual rdf:about="https://github.com/sustainable-processes/ontology/OntoCAPE/model/equation_system.owl#implicit_formulation">
        <rdf:type rdf:resource="https://github.com/sustainable-processes/ontology/OntoCAPE/model/equation_system.owl#ODE_Explicitness"/>
        <rdfs:comment>In an implicit_formulation, the ordinary differential algebraic system is not solved for the highest-order derivative, i.e., F(x, y, y&apos;, y&apos;&apos;, y&apos;&apos;&apos; ...) = 0</rdfs:comment>
    </owl:NamedIndividual>
    


    <!-- https://github.com/sustainable-processes/ontology/OntoCAPE/model/equation_system.owl#linear -->

    <owl:NamedIndividual rdf:about="https://github.com/sustainable-processes/ontology/OntoCAPE/model/equation_system.owl#linear">
        <rdf:type rdf:resource="https://github.com/sustainable-processes/ontology/OntoCAPE/model/equation_system.owl#Linearity"/>
        <owl:differentFrom rdf:resource="https://github.com/sustainable-processes/ontology/OntoCAPE/model/equation_system.owl#nonlinear"/>
        <rdfs:comment>Characterizes a linear equation system</rdfs:comment>
    </owl:NamedIndividual>
    


    <!-- https://github.com/sustainable-processes/ontology/OntoCAPE/model/equation_system.owl#mixed_model -->

    <owl:NamedIndividual rdf:about="https://github.com/sustainable-processes/ontology/OntoCAPE/model/equation_system.owl#mixed_model">
        <rdf:type rdf:resource="https://github.com/sustainable-processes/ontology/OntoCAPE/model/equation_system.owl#VariablesType"/>
        <rdfs:comment>A  mixed_model denotes a MathematicalModel in which some of the ModelVariables are discrete while the others are continuous. An example of a mixed_model is a mixed integer model.</rdfs:comment>
    </owl:NamedIndividual>
    


    <!-- https://github.com/sustainable-processes/ontology/OntoCAPE/model/equation_system.owl#nonlinear -->

    <owl:NamedIndividual rdf:about="https://github.com/sustainable-processes/ontology/OntoCAPE/model/equation_system.owl#nonlinear">
        <rdf:type rdf:resource="https://github.com/sustainable-processes/ontology/OntoCAPE/model/equation_system.owl#Linearity"/>
        <rdfs:comment>Characterizes a nonlinear equation system</rdfs:comment>
    </owl:NamedIndividual>
    


    <!-- https://github.com/sustainable-processes/ontology/OntoCAPE/model/equation_system.owl#nonstiff -->

    <owl:NamedIndividual rdf:about="https://github.com/sustainable-processes/ontology/OntoCAPE/model/equation_system.owl#nonstiff">
        <rdf:type rdf:resource="https://github.com/sustainable-processes/ontology/OntoCAPE/model/equation_system.owl#NumericalStiffness"/>
        <owl:differentFrom rdf:resource="https://github.com/sustainable-processes/ontology/OntoCAPE/model/equation_system.owl#stiff"/>
        <rdfs:comment>Characterizes a nonstiff differential equation.</rdfs:comment>
    </owl:NamedIndividual>
    


    <!-- https://github.com/sustainable-processes/ontology/OntoCAPE/model/equation_system.owl#open_form -->

    <owl:NamedIndividual rdf:about="https://github.com/sustainable-processes/ontology/OntoCAPE/model/equation_system.owl#open_form">
        <rdf:type rdf:resource="https://github.com/sustainable-processes/ontology/OntoCAPE/model/equation_system.owl#ModelRepresentationForm"/>
        <rdfs:comment>An open-form model is solved by an external algorithm. One can freely choose the inputs and outputs of the open-form model.</rdfs:comment>
    </owl:NamedIndividual>
    


    <!-- https://github.com/sustainable-processes/ontology/OntoCAPE/model/equation_system.owl#semi-explicit -->

    <owl:NamedIndividual rdf:about="https://github.com/sustainable-processes/ontology/OntoCAPE/model/equation_system.owl#semi-explicit">
        <rdf:type rdf:resource="https://github.com/sustainable-processes/ontology/OntoCAPE/model/equation_system.owl#DAE_Explicitness"/>
        <rdfs:comment>A DifferentialAlgebraicEquationSystem is semi-explict if it has the form
  f(x, u, t) = x&apos;
  g(x, u, t) = 0</rdfs:comment>
    </owl:NamedIndividual>
    


    <!-- https://github.com/sustainable-processes/ontology/OntoCAPE/model/equation_system.owl#stiff -->

    <owl:NamedIndividual rdf:about="https://github.com/sustainable-processes/ontology/OntoCAPE/model/equation_system.owl#stiff">
        <rdf:type rdf:resource="https://github.com/sustainable-processes/ontology/OntoCAPE/model/equation_system.owl#NumericalStiffness"/>
        <rdfs:comment>Characterizes a stiff differential equation.</rdfs:comment>
    </owl:NamedIndividual>
</rdf:RDF>



<!-- Generated by the OWL API (version 4.5.26.2023-07-17T20:34:13Z) https://github.com/owlcs/owlapi -->

