<?xml version="1.0"?>
<rdf:RDF xmlns="https://github.com/sustainable-processes/ontology/OntoCAPE/model/laws.owl#"
     xml:base="https://github.com/sustainable-processes/ontology/OntoCAPE/model/laws.owl"
     xmlns:owl="http://www.w3.org/2002/07/owl#"
     xmlns:rdf="http://www.w3.org/1999/02/22-rdf-syntax-ns#"
     xmlns:xml="http://www.w3.org/XML/1998/namespace"
     xmlns:xsd="http://www.w3.org/2001/XMLSchema#"
     xmlns:laws="https://github.com/sustainable-processes/ontology/OntoCAPE/model/laws.owl#"
     xmlns:rdfs="http://www.w3.org/2000/01/rdf-schema#"
     xmlns:array="https://github.com/sustainable-processes/ontology/meta_model/data_structures/array.owl#"
     xmlns:terms="http://purl.org/dc/terms/"
     xmlns:owl2xml="http://www.w3.org/2006/12/owl2-xml#"
     xmlns:behavior="https://github.com/sustainable-processes/ontology/OntoCAPE/chemical_process_system/CPS_behavior/behavior.owl#"
     xmlns:multiset="https://github.com/sustainable-processes/ontology/meta_model/data_structures/multiset.owl#"
     xmlns:process_model="https://github.com/sustainable-processes/ontology/OntoCAPE/model/process_model.owl#"
     xmlns:fundamental_concepts="https://github.com/sustainable-processes/ontology/meta_model/fundamental_concepts/fundamental_concepts.owl#"
     xmlns:mathematical_relation="https://github.com/sustainable-processes/ontology/OntoCAPE/supporting_concepts/mathematical_relation/mathematical_relation.owl#">
    <owl:Ontology rdf:about="https://github.com/sustainable-processes/ontology/OntoCAPE/model/laws.owl">
        <owl:imports rdf:resource="https://github.com/sustainable-processes/ontology/OntoCAPE/model/process_model.owl"/>
        <terms:license>Copyright (C) [2009] [Andreas Wiesner]
                This program is free software; you can redistribute it and/or modify it under the terms of the GNU General Public License as published by the Free Software Foundation; either version 3 of the License, or (at your option) any later version.
                This program is distributed in the hope that it will be useful, but WITHOUT ANY WARRANTY; without even the implied warranty of MERCHANTABILITY or FITNESS FOR A PARTICULAR PURPOSE. See the GNU General Public License for more details.
                You should have received a copy of the GNU General Public License along with this program; if not, see &lt;http://www.gnu.org/licenses/&gt;.</terms:license>
        <rdfs:comment>The ontolog module &apos;laws&apos; provides a collection of laws that are frequently used in process modeling.
The following classes, relations, and individuals from other ontology modules are used within &apos;laws&apos;:

&lt;owl:Class rdf:about=&quot;https://github.com/sustainable-processes/ontology/OntoCAPE/chemical_process_system/CPS_behavior/behavior.owl#Accumulation&quot;/&gt;
&lt;owl:Class rdf:about=&quot;https://github.com/sustainable-processes/ontology/OntoCAPE/model/process_model.owl#Law&quot;/&gt;
&lt;owl:Class rdf:about=&quot;https://github.com/sustainable-processes/ontology/OntoCAPE/chemical_process_system/CPS_behavior/behavior.owl#MolecularTransportPhenomenon&quot;/&gt;
&lt;owl:Class rdf:about=&quot;https://github.com/sustainable-processes/ontology/OntoCAPE/chemical_process_system/CPS_behavior/behavior.owl#ParticlePhenomenon&quot;/&gt;
&lt;owl:Class rdf:about=&quot;https://github.com/sustainable-processes/ontology/OntoCAPE/chemical_process_system/CPS_behavior/behavior.owl#PhysicalEquilibriumPhenomenon&quot;/&gt;

&lt;owl:ObjectProperty rdf:about=&quot;https://github.com/sustainable-processes/ontology/OntoCAPE/model/process_model.owl#isAssociatedWith&quot;/&gt;

&lt;behavior:Accumulation rdf:about=&quot;https://github.com/sustainable-processes/ontology/OntoCAPE/chemical_process_system/CPS_behavior/behavior.owl#energy_accumulation&quot;/&gt;
&lt;behavior:Accumulation rdf:about=&quot;https://github.com/sustainable-processes/ontology/OntoCAPE/chemical_process_system/CPS_behavior/behavior.owl#mass_accumulation&quot;/&gt;
&lt;behavior:Accumulation rdf:about=&quot;https://github.com/sustainable-processes/ontology/OntoCAPE/chemical_process_system/CPS_behavior/behavior.owl#momentum_accumulation&quot;/&gt;
&lt;behavior:AdsorptionPhenomenon rdf:about=&quot;https://github.com/sustainable-processes/ontology/OntoCAPE/chemical_process_system/CPS_behavior/behavior.owl#equilibrium_adsorption&quot;/&gt;
&lt;behavior:AdsorptionPhenomenon rdf:about=&quot;https://github.com/sustainable-processes/ontology/OntoCAPE/chemical_process_system/CPS_behavior/behavior.owl#non-equilibrium_adsorption&quot;/&gt;
&lt;behavior:ChemicalReactionPhenomenon rdf:about=&quot;https://github.com/sustainable-processes/ontology/OntoCAPE/chemical_process_system/CPS_behavior/behavior.owl#chemical_reaction_equilibrium&quot;/&gt;
&lt;behavior:InterfaceMolecularTransportPhenomenon rdf:about=&quot;https://github.com/sustainable-processes/ontology/OntoCAPE/chemical_process_system/CPS_behavior/behavior.owl#interface_heat_conduction&quot;/&gt;
&lt;behavior:InterfaceMolecularTransportPhenomenon rdf:about=&quot;https://github.com/sustainable-processes/ontology/OntoCAPE/chemical_process_system/CPS_behavior/behavior.owl#interface_mass_diffusion&quot;/&gt;
&lt;behavior:InterfaceMolecularTransportPhenomenon rdf:about=&quot;https://github.com/sustainable-processes/ontology/OntoCAPE/chemical_process_system/CPS_behavior/behavior.owl#phase_interface_viscous_momentum_transport&quot;/&gt;
&lt;behavior:MaterialAmountConnectionPhenomenon rdf:about=&quot;https://github.com/sustainable-processes/ontology/OntoCAPE/chemical_process_system/CPS_behavior/behavior.owl#convective_material_flow&quot;/&gt;
&lt;behavior:MaterialAmountConnectionPhenomenon rdf:about=&quot;https://github.com/sustainable-processes/ontology/OntoCAPE/chemical_process_system/CPS_behavior/behavior.owl#heat_radiation&quot;/&gt;
&lt;behavior:MolecularTransportPhenomenon rdf:about=&quot;https://github.com/sustainable-processes/ontology/OntoCAPE/chemical_process_system/CPS_behavior/behavior.owl#heat_conduction&quot;/&gt;
&lt;behavior:MolecularTransportPhenomenon rdf:about=&quot;https://github.com/sustainable-processes/ontology/OntoCAPE/chemical_process_system/CPS_behavior/behavior.owl#mass_diffusion&quot;/&gt;
&lt;behavior:MolecularTransportPhenomenon rdf:about=&quot;https://github.com/sustainable-processes/ontology/OntoCAPE/chemical_process_system/CPS_behavior/behavior.owl#viscous_momentum_transport&quot;/&gt;
&lt;behavior:ParticlePhenomenon rdf:about=&quot;https://github.com/sustainable-processes/ontology/OntoCAPE/chemical_process_system/CPS_behavior/behavior.owl#agglomeration&quot;/&gt;
&lt;behavior:ParticlePhenomenon rdf:about=&quot;https://github.com/sustainable-processes/ontology/OntoCAPE/chemical_process_system/CPS_behavior/behavior.owl#breakage&quot;/&gt;
&lt;behavior:ParticlePhenomenon rdf:about=&quot;https://github.com/sustainable-processes/ontology/OntoCAPE/chemical_process_system/CPS_behavior/behavior.owl#growth&quot;/&gt;
&lt;behavior:ParticlePhenomenon rdf:about=&quot;https://github.com/sustainable-processes/ontology/OntoCAPE/chemical_process_system/CPS_behavior/behavior.owl#nucleation&quot;/&gt;
&lt;behavior:ParticlePhenomenon rdf:about=&quot;https://github.com/sustainable-processes/ontology/OntoCAPE/chemical_process_system/CPS_behavior/behavior.owl#particle_population_accumulation&quot;/&gt;
&lt;behavior:PhysicalEquilibriumPhenomenon rdf:about=&quot;https://github.com/sustainable-processes/ontology/OntoCAPE/chemical_process_system/CPS_behavior/behavior.owl#mechanical_equilibrium&quot;/&gt;
&lt;behavior:PhysicalEquilibriumPhenomenon rdf:about=&quot;https://github.com/sustainable-processes/ontology/OntoCAPE/chemical_process_system/CPS_behavior/behavior.owl#phase_equilibrium&quot;/&gt;
&lt;behavior:PhysicalEquilibriumPhenomenon rdf:about=&quot;https://github.com/sustainable-processes/ontology/OntoCAPE/chemical_process_system/CPS_behavior/behavior.owl#thermal_equilibrium&quot;/&gt;
&lt;behavior:SurfacePhenomenon rdf:about=&quot;https://github.com/sustainable-processes/ontology/OntoCAPE/chemical_process_system/CPS_behavior/behavior.owl#surface_mass_diffusion&quot;/&gt;</rdfs:comment>
        <owl:versionInfo>2.0</owl:versionInfo>
    </owl:Ontology>
    


    <!-- 
    ///////////////////////////////////////////////////////////////////////////////////////
    //
    // Annotation properties
    //
    ///////////////////////////////////////////////////////////////////////////////////////
     -->

    


    <!-- http://purl.org/dc/terms/license -->

    <owl:AnnotationProperty rdf:about="http://purl.org/dc/terms/license"/>
    


    <!-- 
    ///////////////////////////////////////////////////////////////////////////////////////
    //
    // Object Properties
    //
    ///////////////////////////////////////////////////////////////////////////////////////
     -->

    


    <!-- https://github.com/sustainable-processes/ontology/OntoCAPE/model/process_model.owl#isAssociatedWith -->

    <owl:ObjectProperty rdf:about="https://github.com/sustainable-processes/ontology/OntoCAPE/model/process_model.owl#isAssociatedWith"/>
    


    <!-- 
    ///////////////////////////////////////////////////////////////////////////////////////
    //
    // Classes
    //
    ///////////////////////////////////////////////////////////////////////////////////////
     -->

    


    <!-- https://github.com/sustainable-processes/ontology/OntoCAPE/chemical_process_system/CPS_behavior/behavior.owl#Accumulation -->

    <owl:Class rdf:about="https://github.com/sustainable-processes/ontology/OntoCAPE/chemical_process_system/CPS_behavior/behavior.owl#Accumulation"/>
    


    <!-- https://github.com/sustainable-processes/ontology/OntoCAPE/chemical_process_system/CPS_behavior/behavior.owl#MolecularTransportPhenomenon -->

    <owl:Class rdf:about="https://github.com/sustainable-processes/ontology/OntoCAPE/chemical_process_system/CPS_behavior/behavior.owl#MolecularTransportPhenomenon">
        <rdfs:comment>A law that is associated with a phenomenon of inter- or intra-phase transport.</rdfs:comment>
    </owl:Class>
    


    <!-- https://github.com/sustainable-processes/ontology/OntoCAPE/chemical_process_system/CPS_behavior/behavior.owl#ParticlePhenomenon -->

    <owl:Class rdf:about="https://github.com/sustainable-processes/ontology/OntoCAPE/chemical_process_system/CPS_behavior/behavior.owl#ParticlePhenomenon"/>
    


    <!-- https://github.com/sustainable-processes/ontology/OntoCAPE/chemical_process_system/CPS_behavior/behavior.owl#PhysicalEquilibriumPhenomenon -->

    <owl:Class rdf:about="https://github.com/sustainable-processes/ontology/OntoCAPE/chemical_process_system/CPS_behavior/behavior.owl#PhysicalEquilibriumPhenomenon"/>
    


    <!-- https://github.com/sustainable-processes/ontology/OntoCAPE/model/laws.owl#AccumulationLaw -->

    <owl:Class rdf:about="https://github.com/sustainable-processes/ontology/OntoCAPE/model/laws.owl#AccumulationLaw">
        <rdfs:subClassOf rdf:resource="https://github.com/sustainable-processes/ontology/OntoCAPE/model/laws.owl#GeneralizedFluxLaw"/>
    </owl:Class>
    


    <!-- https://github.com/sustainable-processes/ontology/OntoCAPE/model/laws.owl#AdsorptionEquilibriumConstraint -->

    <owl:Class rdf:about="https://github.com/sustainable-processes/ontology/OntoCAPE/model/laws.owl#AdsorptionEquilibriumConstraint">
        <rdfs:subClassOf rdf:resource="https://github.com/sustainable-processes/ontology/OntoCAPE/model/laws.owl#EquilibriumConstraint"/>
        <rdfs:subClassOf>
            <owl:Restriction>
                <owl:onProperty rdf:resource="https://github.com/sustainable-processes/ontology/OntoCAPE/model/process_model.owl#isAssociatedWith"/>
                <owl:hasValue rdf:resource="https://github.com/sustainable-processes/ontology/OntoCAPE/chemical_process_system/CPS_behavior/behavior.owl#equilibrium_adsorption"/>
            </owl:Restriction>
        </rdfs:subClassOf>
        <owl:disjointWith rdf:resource="https://github.com/sustainable-processes/ontology/OntoCAPE/model/laws.owl#ChemicalReactionEquilibriumConstraint"/>
        <owl:disjointWith rdf:resource="https://github.com/sustainable-processes/ontology/OntoCAPE/model/laws.owl#MechanicalEquilibriumConstraint"/>
        <owl:disjointWith rdf:resource="https://github.com/sustainable-processes/ontology/OntoCAPE/model/laws.owl#PhaseEquilibriumConstraint"/>
        <owl:disjointWith rdf:resource="https://github.com/sustainable-processes/ontology/OntoCAPE/model/laws.owl#ThermalEquilibriumConstraint"/>
        <rdfs:comment>A Law that is associated with the phenomenon of equilibrium_adsorption.</rdfs:comment>
    </owl:Class>
    


    <!-- https://github.com/sustainable-processes/ontology/OntoCAPE/model/laws.owl#AdsorptionKineticsLaw -->

    <owl:Class rdf:about="https://github.com/sustainable-processes/ontology/OntoCAPE/model/laws.owl#AdsorptionKineticsLaw">
        <rdfs:subClassOf rdf:resource="https://github.com/sustainable-processes/ontology/OntoCAPE/model/laws.owl#SourceLaw"/>
        <rdfs:subClassOf>
            <owl:Restriction>
                <owl:onProperty rdf:resource="https://github.com/sustainable-processes/ontology/OntoCAPE/model/process_model.owl#isAssociatedWith"/>
                <owl:hasValue rdf:resource="https://github.com/sustainable-processes/ontology/OntoCAPE/chemical_process_system/CPS_behavior/behavior.owl#non-equilibrium_adsorption"/>
            </owl:Restriction>
        </rdfs:subClassOf>
        <owl:disjointWith rdf:resource="https://github.com/sustainable-processes/ontology/OntoCAPE/model/laws.owl#ReactionKineticsLaw"/>
        <rdfs:comment>A Law that is associated with the phenomenon of non-equilibrium_adsorption.</rdfs:comment>
    </owl:Class>
    


    <!-- https://github.com/sustainable-processes/ontology/OntoCAPE/model/laws.owl#AgglomerationLaw -->

    <owl:Class rdf:about="https://github.com/sustainable-processes/ontology/OntoCAPE/model/laws.owl#AgglomerationLaw">
        <rdfs:subClassOf rdf:resource="https://github.com/sustainable-processes/ontology/OntoCAPE/model/laws.owl#ParticleKineticsLaw"/>
        <rdfs:subClassOf>
            <owl:Restriction>
                <owl:onProperty rdf:resource="https://github.com/sustainable-processes/ontology/OntoCAPE/model/process_model.owl#isAssociatedWith"/>
                <owl:hasValue rdf:resource="https://github.com/sustainable-processes/ontology/OntoCAPE/chemical_process_system/CPS_behavior/behavior.owl#agglomeration"/>
            </owl:Restriction>
        </rdfs:subClassOf>
        <owl:disjointWith rdf:resource="https://github.com/sustainable-processes/ontology/OntoCAPE/model/laws.owl#BreakageLaw"/>
        <owl:disjointWith rdf:resource="https://github.com/sustainable-processes/ontology/OntoCAPE/model/laws.owl#GrowthLaw"/>
        <owl:disjointWith rdf:resource="https://github.com/sustainable-processes/ontology/OntoCAPE/model/laws.owl#NucleationLaw"/>
        <rdfs:comment>A Law that is associated with the phenomenon of agglomeration (of particles).</rdfs:comment>
    </owl:Class>
    


    <!-- https://github.com/sustainable-processes/ontology/OntoCAPE/model/laws.owl#BalanceLaw -->

    <owl:Class rdf:about="https://github.com/sustainable-processes/ontology/OntoCAPE/model/laws.owl#BalanceLaw">
        <rdfs:subClassOf rdf:resource="https://github.com/sustainable-processes/ontology/OntoCAPE/model/process_model.owl#Law"/>
        <rdfs:subClassOf>
            <owl:Restriction>
                <owl:onProperty rdf:resource="https://github.com/sustainable-processes/ontology/OntoCAPE/model/process_model.owl#isAssociatedWith"/>
                <owl:someValuesFrom rdf:resource="https://github.com/sustainable-processes/ontology/OntoCAPE/chemical_process_system/CPS_behavior/behavior.owl#Accumulation"/>
            </owl:Restriction>
        </rdfs:subClassOf>
        <rdfs:subClassOf>
            <owl:Restriction>
                <owl:onProperty rdf:resource="https://github.com/sustainable-processes/ontology/OntoCAPE/model/process_model.owl#isAssociatedWith"/>
                <owl:allValuesFrom rdf:resource="https://github.com/sustainable-processes/ontology/OntoCAPE/chemical_process_system/CPS_behavior/behavior.owl#Accumulation"/>
            </owl:Restriction>
        </rdfs:subClassOf>
        <owl:disjointWith rdf:resource="https://github.com/sustainable-processes/ontology/OntoCAPE/model/laws.owl#ConstitutiveLaw"/>
        <owl:disjointWith rdf:resource="https://github.com/sustainable-processes/ontology/OntoCAPE/model/laws.owl#EquilibriumConstraint"/>
        <rdfs:comment>A Law that is associated with an Accumulation phenomenon.</rdfs:comment>
    </owl:Class>
    


    <!-- https://github.com/sustainable-processes/ontology/OntoCAPE/model/laws.owl#BreakageLaw -->

    <owl:Class rdf:about="https://github.com/sustainable-processes/ontology/OntoCAPE/model/laws.owl#BreakageLaw">
        <rdfs:subClassOf rdf:resource="https://github.com/sustainable-processes/ontology/OntoCAPE/model/laws.owl#ParticleKineticsLaw"/>
        <rdfs:subClassOf>
            <owl:Restriction>
                <owl:onProperty rdf:resource="https://github.com/sustainable-processes/ontology/OntoCAPE/model/process_model.owl#isAssociatedWith"/>
                <owl:hasValue rdf:resource="https://github.com/sustainable-processes/ontology/OntoCAPE/chemical_process_system/CPS_behavior/behavior.owl#breakage"/>
            </owl:Restriction>
        </rdfs:subClassOf>
        <owl:disjointWith rdf:resource="https://github.com/sustainable-processes/ontology/OntoCAPE/model/laws.owl#GrowthLaw"/>
        <owl:disjointWith rdf:resource="https://github.com/sustainable-processes/ontology/OntoCAPE/model/laws.owl#NucleationLaw"/>
        <rdfs:comment>A Law that is associated with the phenomenon of breakage (of particles).</rdfs:comment>
    </owl:Class>
    


    <!-- https://github.com/sustainable-processes/ontology/OntoCAPE/model/laws.owl#ChemicalKineticsLaw -->

    <owl:Class rdf:about="https://github.com/sustainable-processes/ontology/OntoCAPE/model/laws.owl#ChemicalKineticsLaw">
        <rdfs:subClassOf rdf:resource="https://github.com/sustainable-processes/ontology/OntoCAPE/model/laws.owl#ConstitutiveLaw"/>
        <owl:disjointWith rdf:resource="https://github.com/sustainable-processes/ontology/OntoCAPE/model/laws.owl#ParticleKineticsLaw"/>
        <owl:disjointWith rdf:resource="https://github.com/sustainable-processes/ontology/OntoCAPE/model/laws.owl#TransportLaw"/>
        <rdfs:comment>A Law that is associated with some kinetic phenomenon, such as non-equilibrium reaction or adsorption.</rdfs:comment>
    </owl:Class>
    


    <!-- https://github.com/sustainable-processes/ontology/OntoCAPE/model/laws.owl#ChemicalReactionEquilibriumConstraint -->

    <owl:Class rdf:about="https://github.com/sustainable-processes/ontology/OntoCAPE/model/laws.owl#ChemicalReactionEquilibriumConstraint">
        <rdfs:subClassOf rdf:resource="https://github.com/sustainable-processes/ontology/OntoCAPE/model/laws.owl#EquilibriumConstraint"/>
        <rdfs:subClassOf>
            <owl:Restriction>
                <owl:onProperty rdf:resource="https://github.com/sustainable-processes/ontology/OntoCAPE/model/process_model.owl#isAssociatedWith"/>
                <owl:hasValue rdf:resource="https://github.com/sustainable-processes/ontology/OntoCAPE/chemical_process_system/CPS_behavior/behavior.owl#chemical_reaction_equilibrium"/>
            </owl:Restriction>
        </rdfs:subClassOf>
        <owl:disjointWith rdf:resource="https://github.com/sustainable-processes/ontology/OntoCAPE/model/laws.owl#MechanicalEquilibriumConstraint"/>
        <owl:disjointWith rdf:resource="https://github.com/sustainable-processes/ontology/OntoCAPE/model/laws.owl#PhaseEquilibriumConstraint"/>
        <owl:disjointWith rdf:resource="https://github.com/sustainable-processes/ontology/OntoCAPE/model/laws.owl#ThermalEquilibriumConstraint"/>
        <rdfs:comment>A Law that is associated with the phenomenon of chemical_reaction_equilibrium.</rdfs:comment>
    </owl:Class>
    


    <!-- https://github.com/sustainable-processes/ontology/OntoCAPE/model/laws.owl#ConstitutiveLaw -->

    <owl:Class rdf:about="https://github.com/sustainable-processes/ontology/OntoCAPE/model/laws.owl#ConstitutiveLaw">
        <rdfs:subClassOf rdf:resource="https://github.com/sustainable-processes/ontology/OntoCAPE/model/process_model.owl#Law"/>
        <owl:disjointWith rdf:resource="https://github.com/sustainable-processes/ontology/OntoCAPE/model/laws.owl#EquilibriumConstraint"/>
        <rdfs:comment>A Law that is associated with some non-equilibrium phenomenon.</rdfs:comment>
    </owl:Class>
    


    <!-- https://github.com/sustainable-processes/ontology/OntoCAPE/model/laws.owl#Constraint -->

    <owl:Class rdf:about="https://github.com/sustainable-processes/ontology/OntoCAPE/model/laws.owl#Constraint">
        <rdfs:subClassOf rdf:resource="https://github.com/sustainable-processes/ontology/OntoCAPE/model/process_model.owl#Law"/>
    </owl:Class>
    


    <!-- https://github.com/sustainable-processes/ontology/OntoCAPE/model/laws.owl#ConvectiveMaterialFlowLaw -->

    <owl:Class rdf:about="https://github.com/sustainable-processes/ontology/OntoCAPE/model/laws.owl#ConvectiveMaterialFlowLaw">
        <rdfs:subClassOf rdf:resource="https://github.com/sustainable-processes/ontology/OntoCAPE/model/laws.owl#TransportLaw"/>
        <rdfs:subClassOf>
            <owl:Restriction>
                <owl:onProperty rdf:resource="https://github.com/sustainable-processes/ontology/OntoCAPE/model/process_model.owl#isAssociatedWith"/>
                <owl:hasValue rdf:resource="https://github.com/sustainable-processes/ontology/OntoCAPE/chemical_process_system/CPS_behavior/behavior.owl#convective_material_flow"/>
            </owl:Restriction>
        </rdfs:subClassOf>
        <owl:disjointWith rdf:resource="https://github.com/sustainable-processes/ontology/OntoCAPE/model/laws.owl#HeatRadiationLaw"/>
        <owl:disjointWith rdf:resource="https://github.com/sustainable-processes/ontology/OntoCAPE/model/laws.owl#InterfaceHeatConductionLaw"/>
        <owl:disjointWith rdf:resource="https://github.com/sustainable-processes/ontology/OntoCAPE/model/laws.owl#InterfaceMassDiffusionLaw"/>
        <owl:disjointWith rdf:resource="https://github.com/sustainable-processes/ontology/OntoCAPE/model/laws.owl#InterfaceViscousMomentumTransportLaw"/>
        <owl:disjointWith rdf:resource="https://github.com/sustainable-processes/ontology/OntoCAPE/model/laws.owl#SurfaceMassDiffusionLaw"/>
        <rdfs:comment>A Law that is associated with the phenomenon of convective_material_flow.</rdfs:comment>
    </owl:Class>
    


    <!-- https://github.com/sustainable-processes/ontology/OntoCAPE/model/laws.owl#EnergyBalanceLaw -->

    <owl:Class rdf:about="https://github.com/sustainable-processes/ontology/OntoCAPE/model/laws.owl#EnergyBalanceLaw">
        <rdfs:subClassOf rdf:resource="https://github.com/sustainable-processes/ontology/OntoCAPE/model/laws.owl#BalanceLaw"/>
        <rdfs:subClassOf>
            <owl:Restriction>
                <owl:onProperty rdf:resource="https://github.com/sustainable-processes/ontology/OntoCAPE/model/process_model.owl#isAssociatedWith"/>
                <owl:hasValue rdf:resource="https://github.com/sustainable-processes/ontology/OntoCAPE/chemical_process_system/CPS_behavior/behavior.owl#energy_accumulation"/>
            </owl:Restriction>
        </rdfs:subClassOf>
        <owl:disjointWith rdf:resource="https://github.com/sustainable-processes/ontology/OntoCAPE/model/laws.owl#MassBalanceLaw"/>
        <owl:disjointWith rdf:resource="https://github.com/sustainable-processes/ontology/OntoCAPE/model/laws.owl#MomentumBalanceLaw"/>
        <owl:disjointWith rdf:resource="https://github.com/sustainable-processes/ontology/OntoCAPE/model/laws.owl#PopulationBalanceLaw"/>
        <rdfs:comment>A Law that is associated with the phenomenon of energy_accumulation.</rdfs:comment>
    </owl:Class>
    


    <!-- https://github.com/sustainable-processes/ontology/OntoCAPE/model/laws.owl#EquilibriumConstraint -->

    <owl:Class rdf:about="https://github.com/sustainable-processes/ontology/OntoCAPE/model/laws.owl#EquilibriumConstraint">
        <rdfs:subClassOf rdf:resource="https://github.com/sustainable-processes/ontology/OntoCAPE/model/laws.owl#Constraint"/>
        <rdfs:subClassOf>
            <owl:Restriction>
                <owl:onProperty rdf:resource="https://github.com/sustainable-processes/ontology/OntoCAPE/model/process_model.owl#isAssociatedWith"/>
                <owl:someValuesFrom rdf:resource="https://github.com/sustainable-processes/ontology/OntoCAPE/chemical_process_system/CPS_behavior/behavior.owl#PhysicalEquilibriumPhenomenon"/>
            </owl:Restriction>
        </rdfs:subClassOf>
        <rdfs:subClassOf>
            <owl:Restriction>
                <owl:onProperty rdf:resource="https://github.com/sustainable-processes/ontology/OntoCAPE/model/process_model.owl#isAssociatedWith"/>
                <owl:allValuesFrom rdf:resource="https://github.com/sustainable-processes/ontology/OntoCAPE/chemical_process_system/CPS_behavior/behavior.owl#PhysicalEquilibriumPhenomenon"/>
            </owl:Restriction>
        </rdfs:subClassOf>
    </owl:Class>
    


    <!-- https://github.com/sustainable-processes/ontology/OntoCAPE/model/laws.owl#ExchangeLaw -->

    <owl:Class rdf:about="https://github.com/sustainable-processes/ontology/OntoCAPE/model/laws.owl#ExchangeLaw">
        <rdfs:subClassOf rdf:resource="https://github.com/sustainable-processes/ontology/OntoCAPE/model/laws.owl#GeneralizedFluxLaw"/>
    </owl:Class>
    


    <!-- https://github.com/sustainable-processes/ontology/OntoCAPE/model/laws.owl#GeneralizedFluxLaw -->

    <owl:Class rdf:about="https://github.com/sustainable-processes/ontology/OntoCAPE/model/laws.owl#GeneralizedFluxLaw">
        <rdfs:subClassOf rdf:resource="https://github.com/sustainable-processes/ontology/OntoCAPE/model/laws.owl#ConstitutiveLaw"/>
    </owl:Class>
    


    <!-- https://github.com/sustainable-processes/ontology/OntoCAPE/model/laws.owl#GrowthLaw -->

    <owl:Class rdf:about="https://github.com/sustainable-processes/ontology/OntoCAPE/model/laws.owl#GrowthLaw">
        <rdfs:subClassOf rdf:resource="https://github.com/sustainable-processes/ontology/OntoCAPE/model/laws.owl#ParticleKineticsLaw"/>
        <rdfs:subClassOf>
            <owl:Restriction>
                <owl:onProperty rdf:resource="https://github.com/sustainable-processes/ontology/OntoCAPE/model/process_model.owl#isAssociatedWith"/>
                <owl:hasValue rdf:resource="https://github.com/sustainable-processes/ontology/OntoCAPE/chemical_process_system/CPS_behavior/behavior.owl#growth"/>
            </owl:Restriction>
        </rdfs:subClassOf>
        <owl:disjointWith rdf:resource="https://github.com/sustainable-processes/ontology/OntoCAPE/model/laws.owl#NucleationLaw"/>
        <rdfs:comment>A Law that is associated with the phenomenon of growth (of particles).</rdfs:comment>
    </owl:Class>
    


    <!-- https://github.com/sustainable-processes/ontology/OntoCAPE/model/laws.owl#HeatRadiationLaw -->

    <owl:Class rdf:about="https://github.com/sustainable-processes/ontology/OntoCAPE/model/laws.owl#HeatRadiationLaw">
        <rdfs:subClassOf rdf:resource="https://github.com/sustainable-processes/ontology/OntoCAPE/model/laws.owl#ExchangeLaw"/>
        <rdfs:subClassOf>
            <owl:Restriction>
                <owl:onProperty rdf:resource="https://github.com/sustainable-processes/ontology/OntoCAPE/model/process_model.owl#isAssociatedWith"/>
                <owl:hasValue rdf:resource="https://github.com/sustainable-processes/ontology/OntoCAPE/chemical_process_system/CPS_behavior/behavior.owl#heat_radiation"/>
            </owl:Restriction>
        </rdfs:subClassOf>
        <owl:disjointWith rdf:resource="https://github.com/sustainable-processes/ontology/OntoCAPE/model/laws.owl#InterfaceHeatConductionLaw"/>
        <owl:disjointWith rdf:resource="https://github.com/sustainable-processes/ontology/OntoCAPE/model/laws.owl#InterfaceMassDiffusionLaw"/>
        <owl:disjointWith rdf:resource="https://github.com/sustainable-processes/ontology/OntoCAPE/model/laws.owl#InterfaceViscousMomentumTransportLaw"/>
        <owl:disjointWith rdf:resource="https://github.com/sustainable-processes/ontology/OntoCAPE/model/laws.owl#SurfaceMassDiffusionLaw"/>
        <rdfs:comment>A Law that is associated with the phenomenon of heat_radiation.</rdfs:comment>
    </owl:Class>
    


    <!-- https://github.com/sustainable-processes/ontology/OntoCAPE/model/laws.owl#InterfaceHeatConductionLaw -->

    <owl:Class rdf:about="https://github.com/sustainable-processes/ontology/OntoCAPE/model/laws.owl#InterfaceHeatConductionLaw">
        <rdfs:subClassOf rdf:resource="https://github.com/sustainable-processes/ontology/OntoCAPE/model/laws.owl#ExchangeLaw"/>
        <rdfs:subClassOf>
            <owl:Restriction>
                <owl:onProperty rdf:resource="https://github.com/sustainable-processes/ontology/OntoCAPE/model/process_model.owl#isAssociatedWith"/>
                <owl:hasValue rdf:resource="https://github.com/sustainable-processes/ontology/OntoCAPE/chemical_process_system/CPS_behavior/behavior.owl#interface_heat_conduction"/>
            </owl:Restriction>
        </rdfs:subClassOf>
        <owl:disjointWith rdf:resource="https://github.com/sustainable-processes/ontology/OntoCAPE/model/laws.owl#InterfaceMassDiffusionLaw"/>
        <owl:disjointWith rdf:resource="https://github.com/sustainable-processes/ontology/OntoCAPE/model/laws.owl#InterfaceViscousMomentumTransportLaw"/>
        <owl:disjointWith rdf:resource="https://github.com/sustainable-processes/ontology/OntoCAPE/model/laws.owl#SurfaceMassDiffusionLaw"/>
        <rdfs:comment>A Law that is associated with the phenomenon of interface_heat_conduction.</rdfs:comment>
    </owl:Class>
    


    <!-- https://github.com/sustainable-processes/ontology/OntoCAPE/model/laws.owl#InterfaceMassDiffusionLaw -->

    <owl:Class rdf:about="https://github.com/sustainable-processes/ontology/OntoCAPE/model/laws.owl#InterfaceMassDiffusionLaw">
        <rdfs:subClassOf rdf:resource="https://github.com/sustainable-processes/ontology/OntoCAPE/model/laws.owl#ExchangeLaw"/>
        <rdfs:subClassOf>
            <owl:Restriction>
                <owl:onProperty rdf:resource="https://github.com/sustainable-processes/ontology/OntoCAPE/model/process_model.owl#isAssociatedWith"/>
                <owl:hasValue rdf:resource="https://github.com/sustainable-processes/ontology/OntoCAPE/chemical_process_system/CPS_behavior/behavior.owl#interface_mass_diffusion"/>
            </owl:Restriction>
        </rdfs:subClassOf>
        <owl:disjointWith rdf:resource="https://github.com/sustainable-processes/ontology/OntoCAPE/model/laws.owl#InterfaceViscousMomentumTransportLaw"/>
        <owl:disjointWith rdf:resource="https://github.com/sustainable-processes/ontology/OntoCAPE/model/laws.owl#SurfaceMassDiffusionLaw"/>
        <rdfs:comment>A Law that is associated with the phenomenon of interface_mass_diffusion.</rdfs:comment>
    </owl:Class>
    


    <!-- https://github.com/sustainable-processes/ontology/OntoCAPE/model/laws.owl#InterfaceViscousMomentumTransportLaw -->

    <owl:Class rdf:about="https://github.com/sustainable-processes/ontology/OntoCAPE/model/laws.owl#InterfaceViscousMomentumTransportLaw">
        <rdfs:subClassOf rdf:resource="https://github.com/sustainable-processes/ontology/OntoCAPE/model/laws.owl#ExchangeLaw"/>
        <rdfs:subClassOf>
            <owl:Restriction>
                <owl:onProperty rdf:resource="https://github.com/sustainable-processes/ontology/OntoCAPE/model/process_model.owl#isAssociatedWith"/>
                <owl:hasValue rdf:resource="https://github.com/sustainable-processes/ontology/OntoCAPE/chemical_process_system/CPS_behavior/behavior.owl#phase_interface_viscous_momentum_transport"/>
            </owl:Restriction>
        </rdfs:subClassOf>
        <owl:disjointWith rdf:resource="https://github.com/sustainable-processes/ontology/OntoCAPE/model/laws.owl#SurfaceMassDiffusionLaw"/>
        <rdfs:comment>A Law that is associated with the phenomenon of interface_.viscous_momentum_transport.</rdfs:comment>
    </owl:Class>
    


    <!-- https://github.com/sustainable-processes/ontology/OntoCAPE/model/laws.owl#IntraphaseHeatConductionLaw -->

    <owl:Class rdf:about="https://github.com/sustainable-processes/ontology/OntoCAPE/model/laws.owl#IntraphaseHeatConductionLaw">
        <rdfs:subClassOf rdf:resource="https://github.com/sustainable-processes/ontology/OntoCAPE/model/laws.owl#TransportLaw"/>
        <rdfs:subClassOf>
            <owl:Restriction>
                <owl:onProperty rdf:resource="https://github.com/sustainable-processes/ontology/OntoCAPE/model/process_model.owl#isAssociatedWith"/>
                <owl:hasValue rdf:resource="https://github.com/sustainable-processes/ontology/OntoCAPE/chemical_process_system/CPS_behavior/behavior.owl#heat_conduction"/>
            </owl:Restriction>
        </rdfs:subClassOf>
        <owl:disjointWith rdf:resource="https://github.com/sustainable-processes/ontology/OntoCAPE/model/laws.owl#IntraphaseMassDiffusionLaw"/>
        <owl:disjointWith rdf:resource="https://github.com/sustainable-processes/ontology/OntoCAPE/model/laws.owl#IntraphaseViscousMomentumTransportLaw"/>
        <rdfs:comment>A Law that is associated with the phenomenon of heat_conduction.</rdfs:comment>
    </owl:Class>
    


    <!-- https://github.com/sustainable-processes/ontology/OntoCAPE/model/laws.owl#IntraphaseMassDiffusionLaw -->

    <owl:Class rdf:about="https://github.com/sustainable-processes/ontology/OntoCAPE/model/laws.owl#IntraphaseMassDiffusionLaw">
        <rdfs:subClassOf rdf:resource="https://github.com/sustainable-processes/ontology/OntoCAPE/model/laws.owl#TransportLaw"/>
        <rdfs:subClassOf>
            <owl:Restriction>
                <owl:onProperty rdf:resource="https://github.com/sustainable-processes/ontology/OntoCAPE/model/process_model.owl#isAssociatedWith"/>
                <owl:hasValue rdf:resource="https://github.com/sustainable-processes/ontology/OntoCAPE/chemical_process_system/CPS_behavior/behavior.owl#mass_diffusion"/>
            </owl:Restriction>
        </rdfs:subClassOf>
        <owl:disjointWith rdf:resource="https://github.com/sustainable-processes/ontology/OntoCAPE/model/laws.owl#IntraphaseViscousMomentumTransportLaw"/>
        <rdfs:comment>A Law that is associated with the phenomenon of mass_diffusion.</rdfs:comment>
    </owl:Class>
    


    <!-- https://github.com/sustainable-processes/ontology/OntoCAPE/model/laws.owl#IntraphaseViscousMomentumTransportLaw -->

    <owl:Class rdf:about="https://github.com/sustainable-processes/ontology/OntoCAPE/model/laws.owl#IntraphaseViscousMomentumTransportLaw">
        <rdfs:subClassOf rdf:resource="https://github.com/sustainable-processes/ontology/OntoCAPE/model/laws.owl#TransportLaw"/>
        <rdfs:subClassOf>
            <owl:Restriction>
                <owl:onProperty rdf:resource="https://github.com/sustainable-processes/ontology/OntoCAPE/model/process_model.owl#isAssociatedWith"/>
                <owl:hasValue rdf:resource="https://github.com/sustainable-processes/ontology/OntoCAPE/chemical_process_system/CPS_behavior/behavior.owl#viscous_momentum_transport"/>
            </owl:Restriction>
        </rdfs:subClassOf>
        <rdfs:comment>A Law that is associated with the phenomenon of viscous_momentum_transport.</rdfs:comment>
    </owl:Class>
    


    <!-- https://github.com/sustainable-processes/ontology/OntoCAPE/model/laws.owl#MassBalanceLaw -->

    <owl:Class rdf:about="https://github.com/sustainable-processes/ontology/OntoCAPE/model/laws.owl#MassBalanceLaw">
        <rdfs:subClassOf rdf:resource="https://github.com/sustainable-processes/ontology/OntoCAPE/model/laws.owl#BalanceLaw"/>
        <rdfs:subClassOf>
            <owl:Restriction>
                <owl:onProperty rdf:resource="https://github.com/sustainable-processes/ontology/OntoCAPE/model/process_model.owl#isAssociatedWith"/>
                <owl:hasValue rdf:resource="https://github.com/sustainable-processes/ontology/OntoCAPE/chemical_process_system/CPS_behavior/behavior.owl#mass_accumulation"/>
            </owl:Restriction>
        </rdfs:subClassOf>
        <owl:disjointWith rdf:resource="https://github.com/sustainable-processes/ontology/OntoCAPE/model/laws.owl#MomentumBalanceLaw"/>
        <owl:disjointWith rdf:resource="https://github.com/sustainable-processes/ontology/OntoCAPE/model/laws.owl#PopulationBalanceLaw"/>
        <rdfs:comment>A Law that is associated with the phenomenon of mass_accumulation.</rdfs:comment>
    </owl:Class>
    


    <!-- https://github.com/sustainable-processes/ontology/OntoCAPE/model/laws.owl#MechanicalEquilibriumConstraint -->

    <owl:Class rdf:about="https://github.com/sustainable-processes/ontology/OntoCAPE/model/laws.owl#MechanicalEquilibriumConstraint">
        <rdfs:subClassOf rdf:resource="https://github.com/sustainable-processes/ontology/OntoCAPE/model/laws.owl#EquilibriumConstraint"/>
        <rdfs:subClassOf>
            <owl:Restriction>
                <owl:onProperty rdf:resource="https://github.com/sustainable-processes/ontology/OntoCAPE/model/process_model.owl#isAssociatedWith"/>
                <owl:hasValue rdf:resource="https://github.com/sustainable-processes/ontology/OntoCAPE/chemical_process_system/CPS_behavior/behavior.owl#mechanical_equilibrium"/>
            </owl:Restriction>
        </rdfs:subClassOf>
        <owl:disjointWith rdf:resource="https://github.com/sustainable-processes/ontology/OntoCAPE/model/laws.owl#PhaseEquilibriumConstraint"/>
        <owl:disjointWith rdf:resource="https://github.com/sustainable-processes/ontology/OntoCAPE/model/laws.owl#ThermalEquilibriumConstraint"/>
        <rdfs:comment>A law that is associated with the phenomenon of mechanical_equilibrium.</rdfs:comment>
    </owl:Class>
    


    <!-- https://github.com/sustainable-processes/ontology/OntoCAPE/model/laws.owl#MomentumBalanceLaw -->

    <owl:Class rdf:about="https://github.com/sustainable-processes/ontology/OntoCAPE/model/laws.owl#MomentumBalanceLaw">
        <rdfs:subClassOf rdf:resource="https://github.com/sustainable-processes/ontology/OntoCAPE/model/laws.owl#BalanceLaw"/>
        <rdfs:subClassOf>
            <owl:Restriction>
                <owl:onProperty rdf:resource="https://github.com/sustainable-processes/ontology/OntoCAPE/model/process_model.owl#isAssociatedWith"/>
                <owl:hasValue rdf:resource="https://github.com/sustainable-processes/ontology/OntoCAPE/chemical_process_system/CPS_behavior/behavior.owl#momentum_accumulation"/>
            </owl:Restriction>
        </rdfs:subClassOf>
        <owl:disjointWith rdf:resource="https://github.com/sustainable-processes/ontology/OntoCAPE/model/laws.owl#PopulationBalanceLaw"/>
        <rdfs:comment>A Law that is associated with the phenomenon of momentum_accumulation.</rdfs:comment>
    </owl:Class>
    


    <!-- https://github.com/sustainable-processes/ontology/OntoCAPE/model/laws.owl#NucleationLaw -->

    <owl:Class rdf:about="https://github.com/sustainable-processes/ontology/OntoCAPE/model/laws.owl#NucleationLaw">
        <rdfs:subClassOf rdf:resource="https://github.com/sustainable-processes/ontology/OntoCAPE/model/laws.owl#ParticleKineticsLaw"/>
        <rdfs:subClassOf>
            <owl:Restriction>
                <owl:onProperty rdf:resource="https://github.com/sustainable-processes/ontology/OntoCAPE/model/process_model.owl#isAssociatedWith"/>
                <owl:hasValue rdf:resource="https://github.com/sustainable-processes/ontology/OntoCAPE/chemical_process_system/CPS_behavior/behavior.owl#nucleation"/>
            </owl:Restriction>
        </rdfs:subClassOf>
        <rdfs:comment>A law that is associated with the phenomenon of nucelation (of particles).</rdfs:comment>
    </owl:Class>
    


    <!-- https://github.com/sustainable-processes/ontology/OntoCAPE/model/laws.owl#ParticleKineticsLaw -->

    <owl:Class rdf:about="https://github.com/sustainable-processes/ontology/OntoCAPE/model/laws.owl#ParticleKineticsLaw">
        <rdfs:subClassOf rdf:resource="https://github.com/sustainable-processes/ontology/OntoCAPE/model/laws.owl#AccumulationLaw"/>
        <rdfs:subClassOf>
            <owl:Restriction>
                <owl:onProperty rdf:resource="https://github.com/sustainable-processes/ontology/OntoCAPE/model/process_model.owl#isAssociatedWith"/>
                <owl:someValuesFrom rdf:resource="https://github.com/sustainable-processes/ontology/OntoCAPE/chemical_process_system/CPS_behavior/behavior.owl#ParticlePhenomenon"/>
            </owl:Restriction>
        </rdfs:subClassOf>
        <rdfs:subClassOf>
            <owl:Restriction>
                <owl:onProperty rdf:resource="https://github.com/sustainable-processes/ontology/OntoCAPE/model/process_model.owl#isAssociatedWith"/>
                <owl:allValuesFrom rdf:resource="https://github.com/sustainable-processes/ontology/OntoCAPE/chemical_process_system/CPS_behavior/behavior.owl#ParticlePhenomenon"/>
            </owl:Restriction>
        </rdfs:subClassOf>
        <owl:disjointWith rdf:resource="https://github.com/sustainable-processes/ontology/OntoCAPE/model/laws.owl#TransportLaw"/>
        <rdfs:comment>A Law that is associated with a ParticlePhenomenon.</rdfs:comment>
    </owl:Class>
    


    <!-- https://github.com/sustainable-processes/ontology/OntoCAPE/model/laws.owl#PhaseEquilibriumConstraint -->

    <owl:Class rdf:about="https://github.com/sustainable-processes/ontology/OntoCAPE/model/laws.owl#PhaseEquilibriumConstraint">
        <rdfs:subClassOf rdf:resource="https://github.com/sustainable-processes/ontology/OntoCAPE/model/laws.owl#EquilibriumConstraint"/>
        <rdfs:subClassOf>
            <owl:Restriction>
                <owl:onProperty rdf:resource="https://github.com/sustainable-processes/ontology/OntoCAPE/model/process_model.owl#isAssociatedWith"/>
                <owl:hasValue rdf:resource="https://github.com/sustainable-processes/ontology/OntoCAPE/chemical_process_system/CPS_behavior/behavior.owl#phase_equilibrium"/>
            </owl:Restriction>
        </rdfs:subClassOf>
        <owl:disjointWith rdf:resource="https://github.com/sustainable-processes/ontology/OntoCAPE/model/laws.owl#ThermalEquilibriumConstraint"/>
        <rdfs:comment>A law that is associated with the phenomenon of phase_equilibrium.</rdfs:comment>
    </owl:Class>
    


    <!-- https://github.com/sustainable-processes/ontology/OntoCAPE/model/laws.owl#PhenomenologicalCoefficientLaw -->

    <owl:Class rdf:about="https://github.com/sustainable-processes/ontology/OntoCAPE/model/laws.owl#PhenomenologicalCoefficientLaw">
        <rdfs:subClassOf rdf:resource="https://github.com/sustainable-processes/ontology/OntoCAPE/model/laws.owl#ConstitutiveLaw"/>
    </owl:Class>
    


    <!-- https://github.com/sustainable-processes/ontology/OntoCAPE/model/laws.owl#PopulationBalanceLaw -->

    <owl:Class rdf:about="https://github.com/sustainable-processes/ontology/OntoCAPE/model/laws.owl#PopulationBalanceLaw">
        <rdfs:subClassOf rdf:resource="https://github.com/sustainable-processes/ontology/OntoCAPE/model/laws.owl#BalanceLaw"/>
        <rdfs:subClassOf>
            <owl:Restriction>
                <owl:onProperty rdf:resource="https://github.com/sustainable-processes/ontology/OntoCAPE/model/process_model.owl#isAssociatedWith"/>
                <owl:hasValue rdf:resource="https://github.com/sustainable-processes/ontology/OntoCAPE/chemical_process_system/CPS_behavior/behavior.owl#particle_population_accumulation"/>
            </owl:Restriction>
        </rdfs:subClassOf>
        <rdfs:comment>A Law that is associated with the phenomenon of particle_population_accumulation.</rdfs:comment>
    </owl:Class>
    


    <!-- https://github.com/sustainable-processes/ontology/OntoCAPE/model/laws.owl#ReactionKineticsLaw -->

    <owl:Class rdf:about="https://github.com/sustainable-processes/ontology/OntoCAPE/model/laws.owl#ReactionKineticsLaw">
        <rdfs:subClassOf rdf:resource="https://github.com/sustainable-processes/ontology/OntoCAPE/model/laws.owl#SourceLaw"/>
        <rdfs:subClassOf>
            <owl:Class>
                <owl:unionOf rdf:parseType="Collection">
                    <owl:Restriction>
                        <owl:onProperty rdf:resource="https://github.com/sustainable-processes/ontology/OntoCAPE/model/process_model.owl#isAssociatedWith"/>
                        <owl:hasValue rdf:resource="https://github.com/sustainable-processes/ontology/OntoCAPE/chemical_process_system/CPS_behavior/behavior.owl#non-equilibrium_chemical_reaction"/>
                    </owl:Restriction>
                    <owl:Restriction>
                        <owl:onProperty rdf:resource="https://github.com/sustainable-processes/ontology/OntoCAPE/model/process_model.owl#isAssociatedWith"/>
                        <owl:hasValue rdf:resource="https://github.com/sustainable-processes/ontology/OntoCAPE/chemical_process_system/CPS_behavior/behavior.owl#non-equilibrium_surface_reaction"/>
                    </owl:Restriction>
                </owl:unionOf>
            </owl:Class>
        </rdfs:subClassOf>
        <rdfs:comment>A ReactionKineticsLaw is associated with some phenomenon of chemical reaction kinetics.</rdfs:comment>
    </owl:Class>
    


    <!-- https://github.com/sustainable-processes/ontology/OntoCAPE/model/laws.owl#SourceLaw -->

    <owl:Class rdf:about="https://github.com/sustainable-processes/ontology/OntoCAPE/model/laws.owl#SourceLaw">
        <rdfs:subClassOf rdf:resource="https://github.com/sustainable-processes/ontology/OntoCAPE/model/laws.owl#GeneralizedFluxLaw"/>
    </owl:Class>
    


    <!-- https://github.com/sustainable-processes/ontology/OntoCAPE/model/laws.owl#SurfaceMassDiffusionLaw -->

    <owl:Class rdf:about="https://github.com/sustainable-processes/ontology/OntoCAPE/model/laws.owl#SurfaceMassDiffusionLaw">
        <rdfs:subClassOf rdf:resource="https://github.com/sustainable-processes/ontology/OntoCAPE/model/laws.owl#ExchangeLaw"/>
        <rdfs:subClassOf>
            <owl:Restriction>
                <owl:onProperty rdf:resource="https://github.com/sustainable-processes/ontology/OntoCAPE/model/process_model.owl#isAssociatedWith"/>
                <owl:hasValue rdf:resource="https://github.com/sustainable-processes/ontology/OntoCAPE/chemical_process_system/CPS_behavior/behavior.owl#surface_mass_diffusion"/>
            </owl:Restriction>
        </rdfs:subClassOf>
        <rdfs:comment>A Law that is associated with the phenomenon of surface_mass_diffusion.</rdfs:comment>
    </owl:Class>
    


    <!-- https://github.com/sustainable-processes/ontology/OntoCAPE/model/laws.owl#ThermalEquilibriumConstraint -->

    <owl:Class rdf:about="https://github.com/sustainable-processes/ontology/OntoCAPE/model/laws.owl#ThermalEquilibriumConstraint">
        <rdfs:subClassOf rdf:resource="https://github.com/sustainable-processes/ontology/OntoCAPE/model/laws.owl#EquilibriumConstraint"/>
        <rdfs:subClassOf>
            <owl:Restriction>
                <owl:onProperty rdf:resource="https://github.com/sustainable-processes/ontology/OntoCAPE/model/process_model.owl#isAssociatedWith"/>
                <owl:hasValue rdf:resource="https://github.com/sustainable-processes/ontology/OntoCAPE/chemical_process_system/CPS_behavior/behavior.owl#thermal_equilibrium"/>
            </owl:Restriction>
        </rdfs:subClassOf>
        <rdfs:comment>A law that is associated with the phenomenon of thermal_equilibrium.</rdfs:comment>
    </owl:Class>
    


    <!-- https://github.com/sustainable-processes/ontology/OntoCAPE/model/laws.owl#ThermodynamicStateFunctionLaw -->

    <owl:Class rdf:about="https://github.com/sustainable-processes/ontology/OntoCAPE/model/laws.owl#ThermodynamicStateFunctionLaw">
        <rdfs:subClassOf rdf:resource="https://github.com/sustainable-processes/ontology/OntoCAPE/model/laws.owl#ConstitutiveLaw"/>
    </owl:Class>
    


    <!-- https://github.com/sustainable-processes/ontology/OntoCAPE/model/laws.owl#TransportLaw -->

    <owl:Class rdf:about="https://github.com/sustainable-processes/ontology/OntoCAPE/model/laws.owl#TransportLaw">
        <rdfs:subClassOf rdf:resource="https://github.com/sustainable-processes/ontology/OntoCAPE/model/laws.owl#GeneralizedFluxLaw"/>
    </owl:Class>
    


    <!-- https://github.com/sustainable-processes/ontology/OntoCAPE/model/process_model.owl#Law -->

    <owl:Class rdf:about="https://github.com/sustainable-processes/ontology/OntoCAPE/model/process_model.owl#Law"/>
</rdf:RDF>



<!-- Generated by the OWL API (version 4.5.26.2023-07-17T20:34:13Z) https://github.com/owlcs/owlapi -->

