<?xml version="1.0"?>
<rdf:RDF xmlns="https://github.com/sustainable-processes/ontology/OntoCAPE/model/numerical_solution_strategy.owl#"
     xml:base="https://github.com/sustainable-processes/ontology/OntoCAPE/model/numerical_solution_strategy.owl"
     xmlns:owl="http://www.w3.org/2002/07/owl#"
     xmlns:rdf="http://www.w3.org/1999/02/22-rdf-syntax-ns#"
     xmlns:xml="http://www.w3.org/XML/1998/namespace"
     xmlns:xsd="http://www.w3.org/2001/XMLSchema#"
     xmlns:rdfs="http://www.w3.org/2000/01/rdf-schema#"
     xmlns:root="https://github.com/sustainable-processes/ontology/OntoCAPE/"
     xmlns:array="https://github.com/sustainable-processes/ontology/meta_model/data_structures/array.owl#"
     xmlns:terms="http://purl.org/dc/terms/"
     xmlns:system="https://github.com/sustainable-processes/ontology/OntoCAPE/upper_level/system.owl"
     xmlns:multiset="https://github.com/sustainable-processes/ontology/meta_model/data_structures/multiset.owl#"
     xmlns:equation_system="https://github.com/sustainable-processes/ontology/OntoCAPE/model/equation_system.owl#"
     xmlns:mathematical_model="https://github.com/sustainable-processes/ontology/OntoCAPE/model/mathematical_model.owl"
     xmlns:fundamental_concepts="https://github.com/sustainable-processes/ontology/meta_model/fundamental_concepts/fundamental_concepts.owl#"
     xmlns:numerical_solution_strategy="https://github.com/sustainable-processes/ontology/OntoCAPE/model/numerical_solution_strategy.owl">
    <owl:Ontology rdf:about="https://github.com/sustainable-processes/ontology/OntoCAPE/model/numerical_solution_strategy.owl">
        <owl:imports rdf:resource="https://github.com/sustainable-processes/ontology/OntoCAPE/model/equation_system.owl"/>
        <terms:license>Copyright (C) [2009] [Andreas Wiesner]
                This program is free software; you can redistribute it and/or modify it under the terms of the GNU General Public License as published by the Free Software Foundation; either version 3 of the License, or (at your option) any later version.
                This program is distributed in the hope that it will be useful, but WITHOUT ANY WARRANTY; without even the implied warranty of MERCHANTABILITY or FITNESS FOR A PARTICULAR PURPOSE. See the GNU General Public License for more details.
                You should have received a copy of the GNU General Public License along with this program; if not, see &lt;http://www.gnu.org/licenses/&gt;.
</terms:license>
        <rdfs:comment>The ontology module &apos;numerical_solution_strategy&apos; gives a classification of numerical solution strategies and specifies the ability of those strategy to solve a particular type of mathematical model.    
The follwoing classes and relations from other ontology modules are used within &apos;numerical_solution_strategy&apos;:

&lt;owl:Class rdf:about=&quot;https://github.com/sustainable-processes/ontology/OntoCAPE/model/equation_system.owl#AlgebraicEquationSystem&quot;/&gt;
&lt;owl:Class rdf:about=&quot;https://github.com/sustainable-processes/ontology/OntoCAPE/model/equation_system.owl#DifferentialAlgebraicEquationSystem&quot;/&gt;
&lt;owl:Class rdf:about=&quot;https://github.com/sustainable-processes/ontology/OntoCAPE/model/equation_system.owl#LinearAlgebraicSystem&quot;/&gt;
&lt;owl:Class rdf:about=&quot;https://github.com/sustainable-processes/ontology/OntoCAPE/model/equation_system.owl#NonlinearAlgebraicSystem&quot;/&gt;mathematical_model;#MathematicalModel&quot;/&gt;
&lt;owl:Class rdf:about=&quot;https://github.com/sustainable-processes/ontology/OntoCAPE/model/equation_system.owl#OrdinaryDifferentialEquationSystem&quot;/&gt;
&lt;owl:Class rdf:about=&quot;https://github.com/sustainable-processes/ontology/OntoCAPE/model/equation_system.owl#PartialDifferentialAlgebraicSystem&quot;/&gt;
&lt;owl:Class rdf:about=&quot;https://github.com/sustainable-processes/ontology/OntoCAPE/upper_level/system.owl#System&quot;/&gt;
&lt;owl:Class rdf:about=&quot;https://github.com/sustainable-processes/ontology/OntoCAPE/upper_level/system.owl#FixedValueSet&quot;/&gt;

&lt;owl:ObjectProperty rdf:about=&quot;https://github.com/sustainable-processes/ontology/OntoCAPE/model/equation_system.owl#hasODE_explicitness&quot;/&gt;
&lt;owl:ObjectProperty rdf:about=&quot;https://github.com/sustainable-processes/ontology/OntoCAPE/upper_level/system.owl#containsDirectly&quot;/&gt;
&lt;owl:ObjectProperty rdf:about=&quot;https://github.com/sustainable-processes/ontology/OntoCAPE/upper_level/system.owl#hasCharacteristic&quot;/&gt;
&lt;owl:ObjectProperty rdf:about=&quot;https://github.com/sustainable-processes/ontology/OntoCAPE/upper_level/system.owl#isRelatedTo&quot;/&gt;

&lt;equation_system:ODE_Explicitness rdf:about=&quot;https://github.com/sustainable-processes/ontology/OntoCAPE/model/equation_system.owl#explicit_formulation&quot;/&gt;
&lt;equation_system:ODE_Explicitness rdf:about=&quot;https://github.com/sustainable-processes/ontology/OntoCAPE/model/equation_system.owl#implicit_formulation&quot;/&gt;
</rdfs:comment>
        <owl:versionInfo>2.0</owl:versionInfo>
    </owl:Ontology>
    


    <!-- 
    ///////////////////////////////////////////////////////////////////////////////////////
    //
    // Object Properties
    //
    ///////////////////////////////////////////////////////////////////////////////////////
     -->

    


    <!-- https://github.com/sustainable-processes/ontology/OntoCAPE/model/numerical_solution_strategy.owl#applies -->

    <owl:ObjectProperty rdf:about="https://github.com/sustainable-processes/ontology/OntoCAPE/model/numerical_solution_strategy.owl#applies">
        <rdfs:subPropertyOf rdf:resource="https://github.com/sustainable-processes/ontology/OntoCAPE/upper_level/system.owl#containsDirectly"/>
        <rdfs:domain rdf:resource="https://github.com/sustainable-processes/ontology/OntoCAPE/model/numerical_solution_strategy.owl#ModelSolutionStrategy"/>
        <rdfs:range rdf:resource="https://github.com/sustainable-processes/ontology/OntoCAPE/model/numerical_solution_strategy.owl#ModelSolutionStrategy"/>
        <rdfs:comment>A ModelSolutionStrategy may apply some other, specialized ModelSolutionStrategy (e.g., for initialization, solving corrector equation, solution of a subproblem, etc.).</rdfs:comment>
    </owl:ObjectProperty>
    


    <!-- https://github.com/sustainable-processes/ontology/OntoCAPE/model/numerical_solution_strategy.owl#hasTypeOfInvolvedSteps -->

    <owl:ObjectProperty rdf:about="https://github.com/sustainable-processes/ontology/OntoCAPE/model/numerical_solution_strategy.owl#hasTypeOfInvolvedSteps">
        <rdfs:subPropertyOf rdf:resource="https://github.com/sustainable-processes/ontology/OntoCAPE/upper_level/system.owl#hasCharacteristic"/>
        <rdf:type rdf:resource="http://www.w3.org/2002/07/owl#FunctionalProperty"/>
        <rdfs:domain rdf:resource="https://github.com/sustainable-processes/ontology/OntoCAPE/model/numerical_solution_strategy.owl#ODE_SolutionStrategy"/>
        <rdfs:range rdf:resource="https://github.com/sustainable-processes/ontology/OntoCAPE/model/numerical_solution_strategy.owl#TypeOfInvolvedSteps"/>
        <rdfs:comment>Indicates the TypeOfInvolvedSteps of an ODE_SolutionStrategy.</rdfs:comment>
    </owl:ObjectProperty>
    


    <!-- https://github.com/sustainable-processes/ontology/OntoCAPE/model/numerical_solution_strategy.owl#solves -->

    <owl:ObjectProperty rdf:about="https://github.com/sustainable-processes/ontology/OntoCAPE/model/numerical_solution_strategy.owl#solves">
        <rdfs:subPropertyOf rdf:resource="https://github.com/sustainable-processes/ontology/OntoCAPE/upper_level/system.owl#isDirectlyRelatedTo"/>
        <rdfs:domain rdf:resource="https://github.com/sustainable-processes/ontology/OntoCAPE/model/numerical_solution_strategy.owl#ModelSolutionStrategy"/>
        <rdfs:range rdf:resource="https://github.com/sustainable-processes/ontology/OntoCAPE/model/mathematical_model.owl#MathematicalModel"/>
        <rdfs:comment>The relation indicates the type of MathematicalModel, for the solution of which a particular ModelSolutionStrategy is designated</rdfs:comment>
    </owl:ObjectProperty>
    


    <!-- 
    ///////////////////////////////////////////////////////////////////////////////////////
    //
    // Data properties
    //
    ///////////////////////////////////////////////////////////////////////////////////////
     -->

    


    <!-- https://github.com/sustainable-processes/ontology/OntoCAPE/model/numerical_solution_strategy.owl#handlesDifferentialIndexUpTo -->

    <owl:DatatypeProperty rdf:about="https://github.com/sustainable-processes/ontology/OntoCAPE/model/numerical_solution_strategy.owl#handlesDifferentialIndexUpTo">
        <rdfs:domain rdf:resource="https://github.com/sustainable-processes/ontology/OntoCAPE/model/numerical_solution_strategy.owl#DAE_SolutionStrategy"/>
        <rdfs:range rdf:resource="http://www.w3.org/2001/XMLSchema#int"/>
        <rdfs:comment>A DAE_SolutionStrategy can only solve DifferentialAlgebraicEquationSystems up to a certain differentialIndex. This restriction is specified through the attribute handlesDifferentialIndexUpTo.</rdfs:comment>
    </owl:DatatypeProperty>
    


    <!-- 
    ///////////////////////////////////////////////////////////////////////////////////////
    //
    // Classes
    //
    ///////////////////////////////////////////////////////////////////////////////////////
     -->

    


    <!-- https://github.com/sustainable-processes/ontology/OntoCAPE/model/numerical_solution_strategy.owl#AlgebraicModelSolutionStrategy -->

    <owl:Class rdf:about="https://github.com/sustainable-processes/ontology/OntoCAPE/model/numerical_solution_strategy.owl#AlgebraicModelSolutionStrategy">
        <rdfs:subClassOf rdf:resource="https://github.com/sustainable-processes/ontology/OntoCAPE/model/numerical_solution_strategy.owl#ModelSolutionStrategy"/>
        <rdfs:subClassOf>
            <owl:Restriction>
                <owl:onProperty rdf:resource="https://github.com/sustainable-processes/ontology/OntoCAPE/model/numerical_solution_strategy.owl#solves"/>
                <owl:allValuesFrom rdf:resource="https://github.com/sustainable-processes/ontology/OntoCAPE/model/equation_system.owl#AlgebraicEquationSystem"/>
            </owl:Restriction>
        </rdfs:subClassOf>
        <owl:disjointWith rdf:resource="https://github.com/sustainable-processes/ontology/OntoCAPE/model/numerical_solution_strategy.owl#DAE_SolutionStrategy"/>
        <owl:disjointWith rdf:resource="https://github.com/sustainable-processes/ontology/OntoCAPE/model/numerical_solution_strategy.owl#ODE_SolutionStrategy"/>
        <owl:disjointWith rdf:resource="https://github.com/sustainable-processes/ontology/OntoCAPE/model/numerical_solution_strategy.owl#PartialDifferentialAlgebraicModelSolutionStrategy"/>
        <rdfs:comment>An AlgebraicModelSolutionStrategy is a ModelSolutionStrategy for solving AlgebraicEquationSystems.</rdfs:comment>
    </owl:Class>
    


    <!-- https://github.com/sustainable-processes/ontology/OntoCAPE/model/numerical_solution_strategy.owl#DAE_SolutionStrategy -->

    <owl:Class rdf:about="https://github.com/sustainable-processes/ontology/OntoCAPE/model/numerical_solution_strategy.owl#DAE_SolutionStrategy">
        <rdfs:subClassOf rdf:resource="https://github.com/sustainable-processes/ontology/OntoCAPE/model/numerical_solution_strategy.owl#ModelSolutionStrategy"/>
        <rdfs:subClassOf>
            <owl:Restriction>
                <owl:onProperty rdf:resource="https://github.com/sustainable-processes/ontology/OntoCAPE/model/numerical_solution_strategy.owl#applies"/>
                <owl:someValuesFrom rdf:resource="https://github.com/sustainable-processes/ontology/OntoCAPE/model/numerical_solution_strategy.owl#AlgebraicModelSolutionStrategy"/>
            </owl:Restriction>
        </rdfs:subClassOf>
        <rdfs:subClassOf>
            <owl:Restriction>
                <owl:onProperty rdf:resource="https://github.com/sustainable-processes/ontology/OntoCAPE/model/numerical_solution_strategy.owl#applies"/>
                <owl:someValuesFrom rdf:resource="https://github.com/sustainable-processes/ontology/OntoCAPE/model/numerical_solution_strategy.owl#ODE_SolutionStrategy"/>
            </owl:Restriction>
        </rdfs:subClassOf>
        <rdfs:subClassOf>
            <owl:Restriction>
                <owl:onProperty rdf:resource="https://github.com/sustainable-processes/ontology/OntoCAPE/model/numerical_solution_strategy.owl#applies"/>
                <owl:allValuesFrom>
                    <owl:Class>
                        <owl:unionOf rdf:parseType="Collection">
                            <rdf:Description rdf:about="https://github.com/sustainable-processes/ontology/OntoCAPE/model/numerical_solution_strategy.owl#AlgebraicModelSolutionStrategy"/>
                            <rdf:Description rdf:about="https://github.com/sustainable-processes/ontology/OntoCAPE/model/numerical_solution_strategy.owl#ODE_SolutionStrategy"/>
                        </owl:unionOf>
                    </owl:Class>
                </owl:allValuesFrom>
            </owl:Restriction>
        </rdfs:subClassOf>
        <rdfs:subClassOf>
            <owl:Restriction>
                <owl:onProperty rdf:resource="https://github.com/sustainable-processes/ontology/OntoCAPE/model/numerical_solution_strategy.owl#solves"/>
                <owl:allValuesFrom rdf:resource="https://github.com/sustainable-processes/ontology/OntoCAPE/model/equation_system.owl#DifferentialAlgebraicEquationSystem"/>
            </owl:Restriction>
        </rdfs:subClassOf>
        <rdfs:subClassOf>
            <owl:Restriction>
                <owl:onProperty rdf:resource="https://github.com/sustainable-processes/ontology/OntoCAPE/model/numerical_solution_strategy.owl#applies"/>
                <owl:cardinality rdf:datatype="http://www.w3.org/2001/XMLSchema#nonNegativeInteger">2</owl:cardinality>
            </owl:Restriction>
        </rdfs:subClassOf>
        <rdfs:subClassOf>
            <owl:Restriction>
                <owl:onProperty rdf:resource="https://github.com/sustainable-processes/ontology/OntoCAPE/model/numerical_solution_strategy.owl#handlesDifferentialIndexUpTo"/>
                <owl:cardinality rdf:datatype="http://www.w3.org/2001/XMLSchema#nonNegativeInteger">1</owl:cardinality>
            </owl:Restriction>
        </rdfs:subClassOf>
        <owl:disjointWith rdf:resource="https://github.com/sustainable-processes/ontology/OntoCAPE/model/numerical_solution_strategy.owl#ODE_SolutionStrategy"/>
        <owl:disjointWith rdf:resource="https://github.com/sustainable-processes/ontology/OntoCAPE/model/numerical_solution_strategy.owl#PartialDifferentialAlgebraicModelSolutionStrategy"/>
        <rdfs:comment>A DAE_SolutionStrategy is a ModelSolutionStrategy for solving DifferentialAlgebraicEquationSystems. Examples are implicit Runge-Kutta, BDF, etc.</rdfs:comment>
    </owl:Class>
    


    <!-- https://github.com/sustainable-processes/ontology/OntoCAPE/model/numerical_solution_strategy.owl#LinearAlgebraicModelSolutionStrategy -->

    <owl:Class rdf:about="https://github.com/sustainable-processes/ontology/OntoCAPE/model/numerical_solution_strategy.owl#LinearAlgebraicModelSolutionStrategy">
        <rdfs:subClassOf rdf:resource="https://github.com/sustainable-processes/ontology/OntoCAPE/model/numerical_solution_strategy.owl#AlgebraicModelSolutionStrategy"/>
        <rdfs:subClassOf>
            <owl:Restriction>
                <owl:onProperty rdf:resource="https://github.com/sustainable-processes/ontology/OntoCAPE/model/numerical_solution_strategy.owl#solves"/>
                <owl:allValuesFrom rdf:resource="https://github.com/sustainable-processes/ontology/OntoCAPE/model/equation_system.owl#LinearAlgebraicSystem"/>
            </owl:Restriction>
        </rdfs:subClassOf>
        <owl:disjointWith rdf:resource="https://github.com/sustainable-processes/ontology/OntoCAPE/model/numerical_solution_strategy.owl#NonlinearAlgebraicModelSolutionStrategy"/>
        <rdfs:comment>A LinearAlgebraicModelSolutionStrategy is ModelSolutionStrategy for solving LinearAlgebraicSystems. An example is Gauss-elimination.</rdfs:comment>
    </owl:Class>
    


    <!-- https://github.com/sustainable-processes/ontology/OntoCAPE/model/numerical_solution_strategy.owl#ModelSolutionStrategy -->

    <owl:Class rdf:about="https://github.com/sustainable-processes/ontology/OntoCAPE/model/numerical_solution_strategy.owl#ModelSolutionStrategy">
        <rdfs:subClassOf rdf:resource="https://github.com/sustainable-processes/ontology/OntoCAPE/upper_level/system.owl#System"/>
        <rdfs:subClassOf>
            <owl:Restriction>
                <owl:onProperty rdf:resource="https://github.com/sustainable-processes/ontology/OntoCAPE/model/numerical_solution_strategy.owl#solves"/>
                <owl:someValuesFrom rdf:resource="https://github.com/sustainable-processes/ontology/OntoCAPE/model/mathematical_model.owl#MathematicalModel"/>
            </owl:Restriction>
        </rdfs:subClassOf>
        <rdfs:subClassOf>
            <owl:Restriction>
                <owl:onProperty rdf:resource="https://github.com/sustainable-processes/ontology/OntoCAPE/model/numerical_solution_strategy.owl#applies"/>
                <owl:allValuesFrom rdf:resource="https://github.com/sustainable-processes/ontology/OntoCAPE/model/numerical_solution_strategy.owl#ModelSolutionStrategy"/>
            </owl:Restriction>
        </rdfs:subClassOf>
        <rdfs:subClassOf>
            <owl:Restriction>
                <owl:onProperty rdf:resource="https://github.com/sustainable-processes/ontology/OntoCAPE/model/numerical_solution_strategy.owl#solves"/>
                <owl:allValuesFrom rdf:resource="https://github.com/sustainable-processes/ontology/OntoCAPE/model/mathematical_model.owl#MathematicalModel"/>
            </owl:Restriction>
        </rdfs:subClassOf>
        <rdfs:comment>A ModelSolutionStrategy is a (typcially numerical) algorithm that can be used to solve mathematical models.</rdfs:comment>
    </owl:Class>
    


    <!-- https://github.com/sustainable-processes/ontology/OntoCAPE/model/numerical_solution_strategy.owl#NonlinearAlgebraicModelSolutionStrategy -->

    <owl:Class rdf:about="https://github.com/sustainable-processes/ontology/OntoCAPE/model/numerical_solution_strategy.owl#NonlinearAlgebraicModelSolutionStrategy">
        <rdfs:subClassOf rdf:resource="https://github.com/sustainable-processes/ontology/OntoCAPE/model/numerical_solution_strategy.owl#AlgebraicModelSolutionStrategy"/>
        <rdfs:subClassOf>
            <owl:Restriction>
                <owl:onProperty rdf:resource="https://github.com/sustainable-processes/ontology/OntoCAPE/model/numerical_solution_strategy.owl#solves"/>
                <owl:allValuesFrom rdf:resource="https://github.com/sustainable-processes/ontology/OntoCAPE/model/equation_system.owl#NonlinearAlgebraicSystem"/>
            </owl:Restriction>
        </rdfs:subClassOf>
        <rdfs:comment>A NonlinearAlgebraicModelSolutionStrategy is a ModelSolutionStrategy for solving NonlinearAlgebraicSystem. An example is the Newton&apos;s method.</rdfs:comment>
    </owl:Class>
    


    <!-- https://github.com/sustainable-processes/ontology/OntoCAPE/model/numerical_solution_strategy.owl#ODE_SolutionStrategy -->

    <owl:Class rdf:about="https://github.com/sustainable-processes/ontology/OntoCAPE/model/numerical_solution_strategy.owl#ODE_SolutionStrategy">
        <rdfs:subClassOf rdf:resource="https://github.com/sustainable-processes/ontology/OntoCAPE/model/numerical_solution_strategy.owl#ModelSolutionStrategy"/>
        <rdfs:subClassOf>
            <owl:Restriction>
                <owl:onProperty rdf:resource="https://github.com/sustainable-processes/ontology/OntoCAPE/model/numerical_solution_strategy.owl#hasTypeOfInvolvedSteps"/>
                <owl:someValuesFrom rdf:resource="https://github.com/sustainable-processes/ontology/OntoCAPE/model/numerical_solution_strategy.owl#TypeOfInvolvedSteps"/>
            </owl:Restriction>
        </rdfs:subClassOf>
        <rdfs:subClassOf>
            <owl:Restriction>
                <owl:onProperty rdf:resource="https://github.com/sustainable-processes/ontology/OntoCAPE/model/numerical_solution_strategy.owl#hasTypeOfInvolvedSteps"/>
                <owl:allValuesFrom rdf:resource="https://github.com/sustainable-processes/ontology/OntoCAPE/model/numerical_solution_strategy.owl#TypeOfInvolvedSteps"/>
            </owl:Restriction>
        </rdfs:subClassOf>
        <rdfs:subClassOf>
            <owl:Restriction>
                <owl:onProperty rdf:resource="https://github.com/sustainable-processes/ontology/OntoCAPE/model/numerical_solution_strategy.owl#solves"/>
                <owl:allValuesFrom rdf:resource="https://github.com/sustainable-processes/ontology/OntoCAPE/model/equation_system.owl#OrdinaryDifferentialEquationSystem"/>
            </owl:Restriction>
        </rdfs:subClassOf>
        <rdfs:subClassOf>
            <owl:Restriction>
                <owl:onProperty rdf:resource="https://github.com/sustainable-processes/ontology/OntoCAPE/model/numerical_solution_strategy.owl#hasTypeOfInvolvedSteps"/>
                <owl:cardinality rdf:datatype="http://www.w3.org/2001/XMLSchema#nonNegativeInteger">1</owl:cardinality>
            </owl:Restriction>
        </rdfs:subClassOf>
        <owl:disjointWith rdf:resource="https://github.com/sustainable-processes/ontology/OntoCAPE/model/numerical_solution_strategy.owl#PartialDifferentialAlgebraicModelSolutionStrategy"/>
        <rdfs:comment>An ODE_SolutionStrategy is a ModelSolutionStrategy for solving OrdinaryDifferentialEquationSystems.</rdfs:comment>
    </owl:Class>
    


    <!-- https://github.com/sustainable-processes/ontology/OntoCAPE/model/numerical_solution_strategy.owl#PartialDifferentialAlgebraicModelSolutionStrategy -->

    <owl:Class rdf:about="https://github.com/sustainable-processes/ontology/OntoCAPE/model/numerical_solution_strategy.owl#PartialDifferentialAlgebraicModelSolutionStrategy">
        <rdfs:subClassOf rdf:resource="https://github.com/sustainable-processes/ontology/OntoCAPE/model/numerical_solution_strategy.owl#ModelSolutionStrategy"/>
        <rdfs:subClassOf>
            <owl:Restriction>
                <owl:onProperty rdf:resource="https://github.com/sustainable-processes/ontology/OntoCAPE/model/numerical_solution_strategy.owl#solves"/>
                <owl:allValuesFrom rdf:resource="https://github.com/sustainable-processes/ontology/OntoCAPE/model/equation_system.owl#PartialDifferentialAlgebraicSystem"/>
            </owl:Restriction>
        </rdfs:subClassOf>
        <rdfs:comment>A PartialDifferentialAlgebraicModelSolutionStrategy is a ModelSolutionStrategy for solving PartialDifferentialAlgebraicSystems.</rdfs:comment>
    </owl:Class>
    


    <!-- https://github.com/sustainable-processes/ontology/OntoCAPE/model/numerical_solution_strategy.owl#SolutionStrategyForExplixcitODEs -->

    <owl:Class rdf:about="https://github.com/sustainable-processes/ontology/OntoCAPE/model/numerical_solution_strategy.owl#SolutionStrategyForExplixcitODEs">
        <rdfs:subClassOf rdf:resource="https://github.com/sustainable-processes/ontology/OntoCAPE/model/numerical_solution_strategy.owl#ODE_SolutionStrategy"/>
        <rdfs:subClassOf>
            <owl:Restriction>
                <owl:onProperty rdf:resource="https://github.com/sustainable-processes/ontology/OntoCAPE/model/numerical_solution_strategy.owl#solves"/>
                <owl:allValuesFrom>
                    <owl:Class>
                        <owl:intersectionOf rdf:parseType="Collection">
                            <rdf:Description rdf:about="https://github.com/sustainable-processes/ontology/OntoCAPE/model/equation_system.owl#OrdinaryDifferentialEquationSystem"/>
                            <owl:Restriction>
                                <owl:onProperty rdf:resource="https://github.com/sustainable-processes/ontology/OntoCAPE/model/equation_system.owl#hasODE_explicitness"/>
                                <owl:hasValue rdf:resource="https://github.com/sustainable-processes/ontology/OntoCAPE/model/equation_system.owl#explicit_formulation"/>
                            </owl:Restriction>
                        </owl:intersectionOf>
                    </owl:Class>
                </owl:allValuesFrom>
            </owl:Restriction>
        </rdfs:subClassOf>
        <owl:disjointWith rdf:resource="https://github.com/sustainable-processes/ontology/OntoCAPE/model/numerical_solution_strategy.owl#SolutionStrategyForImplicitODEs"/>
        <rdfs:comment>A SolutionStrategyForExplixcitODEs is used to solve ordinary differential equation systems that are given in an explicit_formulation. Examples are explicit Euler, explicit Runge-Kutta, etc.</rdfs:comment>
    </owl:Class>
    


    <!-- https://github.com/sustainable-processes/ontology/OntoCAPE/model/numerical_solution_strategy.owl#SolutionStrategyForImplicitODEs -->

    <owl:Class rdf:about="https://github.com/sustainable-processes/ontology/OntoCAPE/model/numerical_solution_strategy.owl#SolutionStrategyForImplicitODEs">
        <rdfs:subClassOf rdf:resource="https://github.com/sustainable-processes/ontology/OntoCAPE/model/numerical_solution_strategy.owl#ODE_SolutionStrategy"/>
        <rdfs:subClassOf>
            <owl:Restriction>
                <owl:onProperty rdf:resource="https://github.com/sustainable-processes/ontology/OntoCAPE/model/numerical_solution_strategy.owl#solves"/>
                <owl:allValuesFrom>
                    <owl:Class>
                        <owl:intersectionOf rdf:parseType="Collection">
                            <rdf:Description rdf:about="https://github.com/sustainable-processes/ontology/OntoCAPE/model/equation_system.owl#OrdinaryDifferentialEquationSystem"/>
                            <owl:Restriction>
                                <owl:onProperty rdf:resource="https://github.com/sustainable-processes/ontology/OntoCAPE/model/equation_system.owl#hasODE_explicitness"/>
                                <owl:hasValue rdf:resource="https://github.com/sustainable-processes/ontology/OntoCAPE/model/equation_system.owl#implicit_formulation"/>
                            </owl:Restriction>
                        </owl:intersectionOf>
                    </owl:Class>
                </owl:allValuesFrom>
            </owl:Restriction>
        </rdfs:subClassOf>
        <rdfs:comment>A SolutionStrategyForIImplicitODEs is used to solve OrdinaryDifferentialEquationSystems that are given in an implicit_formulation. Examples are implicit Euler, implicit Runge-Kutta, etc.</rdfs:comment>
    </owl:Class>
    


    <!-- https://github.com/sustainable-processes/ontology/OntoCAPE/model/numerical_solution_strategy.owl#TypeOfInvolvedSteps -->

    <owl:Class rdf:about="https://github.com/sustainable-processes/ontology/OntoCAPE/model/numerical_solution_strategy.owl#TypeOfInvolvedSteps">
        <owl:equivalentClass>
            <owl:Class>
                <owl:oneOf rdf:parseType="Collection">
                    <rdf:Description rdf:about="https://github.com/sustainable-processes/ontology/OntoCAPE/model/numerical_solution_strategy.owl#multi-step_method"/>
                    <rdf:Description rdf:about="https://github.com/sustainable-processes/ontology/OntoCAPE/model/numerical_solution_strategy.owl#one-step_method"/>
                </owl:oneOf>
            </owl:Class>
        </owl:equivalentClass>
        <rdfs:subClassOf rdf:resource="https://github.com/sustainable-processes/ontology/OntoCAPE/upper_level/system.owl#FixedValueSet"/>
        <rdfs:comment>A type of involved step denotes whether an ordinary differential equation solution strategy is of one-step nature or multi-step nature.
- A one-step_method characterizes an ODESolutionStrategy that uses information of one integration step. Examples are various Runge-Kutta methods.
- A multi-step_method characterizes an ODESolutionStrategy that uses information of multiple integration steps. Examples are Adams, BDF, etc.</rdfs:comment>
    </owl:Class>
    


    <!-- 
    ///////////////////////////////////////////////////////////////////////////////////////
    //
    // Individuals
    //
    ///////////////////////////////////////////////////////////////////////////////////////
     -->

    


    <!-- https://github.com/sustainable-processes/ontology/OntoCAPE/model/numerical_solution_strategy.owl#multi-step_method -->

    <owl:NamedIndividual rdf:about="https://github.com/sustainable-processes/ontology/OntoCAPE/model/numerical_solution_strategy.owl#multi-step_method">
        <rdf:type rdf:resource="https://github.com/sustainable-processes/ontology/OntoCAPE/model/numerical_solution_strategy.owl#TypeOfInvolvedSteps"/>
        <owl:differentFrom rdf:resource="https://github.com/sustainable-processes/ontology/OntoCAPE/model/numerical_solution_strategy.owl#one-step_method"/>
        <rdfs:comment>A multi-step_method characterizes an ODE_SolutionStrategy that uses information of multiple integration steps. Examples are Adams, BDF, etc.</rdfs:comment>
    </owl:NamedIndividual>
    


    <!-- https://github.com/sustainable-processes/ontology/OntoCAPE/model/numerical_solution_strategy.owl#one-step_method -->

    <owl:NamedIndividual rdf:about="https://github.com/sustainable-processes/ontology/OntoCAPE/model/numerical_solution_strategy.owl#one-step_method">
        <rdf:type rdf:resource="https://github.com/sustainable-processes/ontology/OntoCAPE/model/numerical_solution_strategy.owl#TypeOfInvolvedSteps"/>
        <rdfs:comment>A one-step_method characterizes an ODE_SolutionStrategy that uses information of one integration step. Examples are various Runge-Kutta methods.</rdfs:comment>
    </owl:NamedIndividual>
</rdf:RDF>



<!-- Generated by the OWL API (version 4.5.26.2023-07-17T20:34:13Z) https://github.com/owlcs/owlapi -->

