<?xml version="1.0"?>
<rdf:RDF xmlns="https://github.com/sustainable-processes/ontology/OntoCAPE/model/property_models.owl#"
     xml:base="https://github.com/sustainable-processes/ontology/OntoCAPE/model/property_models.owl"
     xmlns:owl="http://www.w3.org/2002/07/owl#"
     xmlns:rdf="http://www.w3.org/1999/02/22-rdf-syntax-ns#"
     xmlns:xml="http://www.w3.org/XML/1998/namespace"
     xmlns:xsd="http://www.w3.org/2001/XMLSchema#"
     xmlns:rdfs="http://www.w3.org/2000/01/rdf-schema#"
     xmlns:root="https://github.com/sustainable-processes/ontology/OntoCAPE/"
     xmlns:array="https://github.com/sustainable-processes/ontology/meta_model/data_structures/array.owl#"
     xmlns:terms="http://purl.org/dc/terms/"
     xmlns:multiset="https://github.com/sustainable-processes/ontology/meta_model/data_structures/multiset.owl#"
     xmlns:phase_system="https://github.com/sustainable-processes/ontology/OntoCAPE/material/phase_system/phase_system.owl"
     xmlns:process_model="https://github.com/sustainable-processes/ontology/OntoCAPE/model/process_model.owl#"
     xmlns:property_models="https://github.com/sustainable-processes/ontology/OntoCAPE/model/property_models.owl"
     xmlns:mathematical_model="https://github.com/sustainable-processes/ontology/OntoCAPE/model/mathematical_model.owl"
     xmlns:fundamental_concepts="https://github.com/sustainable-processes/ontology/meta_model/fundamental_concepts/fundamental_concepts.owl#"
     xmlns:mathematical_relation="https://github.com/sustainable-processes/ontology/OntoCAPE/supporting_concepts/mathematical_relation/mathematical_relation.owl#">
    <owl:Ontology rdf:about="https://github.com/sustainable-processes/ontology/OntoCAPE/model/property_models.owl">
        <owl:imports rdf:resource="https://github.com/sustainable-processes/ontology/OntoCAPE/model/process_model.owl"/>
        <terms:license>Copyright (C) [2009] [Andreas Wiesner]
                This program is free software; you can redistribute it and/or modify it under the terms of the GNU General Public License as published by the Free Software Foundation; either version 3 of the License, or (at your option) any later version.
                This program is distributed in the hope that it will be useful, but WITHOUT ANY WARRANTY; without even the implied warranty of MERCHANTABILITY or FITNESS FOR A PARTICULAR PURPOSE. See the GNU General Public License for more details.
                You should have received a copy of the GNU General Public License along with this program; if not, see &lt;http://www.gnu.org/licenses/&gt;.
</terms:license>
        <rdfs:comment>The ontolog module &apos;property_models&apos; represents  mathematical correlations for the compuation of certain PhysicalQuantities, such as vapor pressure correlations or activity coefficient models.    
The following classes and relations from other ontology modules are used within &apos;property_models&apos;:
 
&lt;owl:Class rdf:about=&quot;https://github.com/sustainable-processes/ontology/OntoCAPE/model/mathematical_model.owl#ModelVariable&quot;/&gt;
&lt;owl:Class rdf:about=&quot;https://github.com/sustainable-processes/ontology/OntoCAPE/material/phase_system/phase_system.owl#ActivityCoefficient&quot;/&gt;
&lt;owl:Class rdf:about=&quot;https://github.com/sustainable-processes/ontology/OntoCAPE/material/phase_system/phase_system.owl#Density&quot;/&gt;
&lt;owl:Class rdf:about=&quot;https://github.com/sustainable-processes/ontology/OntoCAPE/material/phase_system/phase_system.owl#DiffusionCoefficient&quot;/&gt;
&lt;owl:Class rdf:about=&quot;https://github.com/sustainable-processes/ontology/OntoCAPE/material/phase_system/phase_system.owl#DynamicViscosity&quot;/&gt;
&lt;owl:Class rdf:about=&quot;https://github.com/sustainable-processes/ontology/OntoCAPE/material/phase_system/phase_system.owl#FugacityCoefficient&quot;/&gt;
&lt;owl:Class rdf:about=&quot;https://github.com/sustainable-processes/ontology/OntoCAPE/material/phase_system/phase_system.owl#PartialMolarEnthalpy&quot;/&gt;
&lt;owl:Class rdf:about=&quot;https://github.com/sustainable-processes/ontology/OntoCAPE/material/phase_system/phase_system.owl#PartialMolarVolume&quot;/&gt;
&lt;owl:Class rdf:about=&quot;https://github.com/sustainable-processes/ontology/OntoCAPE/material/phase_system/phase_system.owl#PhaseEquilibriumRatio&quot;/&gt;
&lt;owl:Class rdf:about=&quot;https://github.com/sustainable-processes/ontology/OntoCAPE/material/phase_system/phase_system.owl#PhaseSystemProperty&quot;/&gt;
&lt;owl:Class rdf:about=&quot;https://github.com/sustainable-processes/ontology/OntoCAPE/material/phase_system/phase_system.owl#SpecificEnthalpy&quot;/&gt;
&lt;owl:Class rdf:about=&quot;https://github.com/sustainable-processes/ontology/OntoCAPE/material/phase_system/phase_system.owl#ThermalConductivity&quot;/&gt;
&lt;owl:Class rdf:about=&quot;https://github.com/sustainable-processes/ontology/OntoCAPE/material/phase_system/phase_system.owl#TransportPhenomenaProperty&quot;/&gt;
&lt;owl:Class rdf:about=&quot;https://github.com/sustainable-processes/ontology/OntoCAPE/material/phase_system/phase_system.owl#IntensiveThermodynamicStateVariable&quot;/&gt;
&lt;owl:Class rdf:about=&quot;https://github.com/sustainable-processes/ontology/OntoCAPE/material/phase_system/phase_system.owl#SurfaceTension&quot;/&gt;
&lt;owl:Class rdf:about=&quot;https://github.com/sustainable-processes/ontology/OntoCAPE/model/process_model.owl#PropertyModel&quot;/&gt;

&lt;owl:ObjectProperty rdf:about=&quot;https://github.com/sustainable-processes/ontology/OntoCAPE/model/mathematical_model.owl#correspondsToQuantity&quot;/&gt;
&lt;owl:ObjectProperty rdf:about=&quot;https://github.com/sustainable-processes/ontology/OntoCAPE/model/mathematical_model.owl#hasModelVariable&quot;/&gt;
</rdfs:comment>
        <owl:versionInfo>2.0</owl:versionInfo>
    </owl:Ontology>
    


    <!-- 
    ///////////////////////////////////////////////////////////////////////////////////////
    //
    // Classes
    //
    ///////////////////////////////////////////////////////////////////////////////////////
     -->

    


    <!-- https://github.com/sustainable-processes/ontology/OntoCAPE/model/property_models.owl#ActivityCoefficientModel -->

    <owl:Class rdf:about="https://github.com/sustainable-processes/ontology/OntoCAPE/model/property_models.owl#ActivityCoefficientModel">
        <rdfs:subClassOf rdf:resource="https://github.com/sustainable-processes/ontology/OntoCAPE/model/property_models.owl#IntensiveThermodynamicStateModel"/>
        <rdfs:subClassOf>
            <owl:Restriction>
                <owl:onProperty rdf:resource="https://github.com/sustainable-processes/ontology/OntoCAPE/model/mathematical_model.owl#hasModelVariable"/>
                <owl:someValuesFrom>
                    <owl:Class>
                        <owl:intersectionOf rdf:parseType="Collection">
                            <rdf:Description rdf:about="https://github.com/sustainable-processes/ontology/OntoCAPE/model/mathematical_model.owl#ModelVariable"/>
                            <owl:Restriction>
                                <owl:onProperty rdf:resource="https://github.com/sustainable-processes/ontology/OntoCAPE/model/mathematical_model.owl#correspondsToQuantity"/>
                                <owl:someValuesFrom rdf:resource="https://github.com/sustainable-processes/ontology/OntoCAPE/material/phase_system/phase_system.owl#ActivityCoefficient"/>
                            </owl:Restriction>
                        </owl:intersectionOf>
                    </owl:Class>
                </owl:someValuesFrom>
            </owl:Restriction>
        </rdfs:subClassOf>
        <owl:disjointWith rdf:resource="https://github.com/sustainable-processes/ontology/OntoCAPE/model/property_models.owl#AdsorptionEquilibriumConstantModel"/>
        <owl:disjointWith rdf:resource="https://github.com/sustainable-processes/ontology/OntoCAPE/model/property_models.owl#DensityModel"/>
        <owl:disjointWith rdf:resource="https://github.com/sustainable-processes/ontology/OntoCAPE/model/property_models.owl#FugacityCoefficientModel"/>
        <owl:disjointWith rdf:resource="https://github.com/sustainable-processes/ontology/OntoCAPE/model/property_models.owl#HeatCapacityModel"/>
        <owl:disjointWith rdf:resource="https://github.com/sustainable-processes/ontology/OntoCAPE/model/property_models.owl#PartialMolarEnthalpyModel"/>
        <owl:disjointWith rdf:resource="https://github.com/sustainable-processes/ontology/OntoCAPE/model/property_models.owl#PartialMolarVolumeModel"/>
        <owl:disjointWith rdf:resource="https://github.com/sustainable-processes/ontology/OntoCAPE/model/property_models.owl#PhaseEquilibriumRatioModel"/>
        <owl:disjointWith rdf:resource="https://github.com/sustainable-processes/ontology/OntoCAPE/model/property_models.owl#ReactionEquilibriumConstantModel"/>
        <owl:disjointWith rdf:resource="https://github.com/sustainable-processes/ontology/OntoCAPE/model/property_models.owl#SpecificEnthalpyModel"/>
        <owl:disjointWith rdf:resource="https://github.com/sustainable-processes/ontology/OntoCAPE/model/property_models.owl#VapourPressureModel"/>
        <rdfs:comment>A PropertyModel that provides a correlation for an ActivityCoefficient.</rdfs:comment>
    </owl:Class>
    


    <!-- https://github.com/sustainable-processes/ontology/OntoCAPE/model/property_models.owl#AdsorptionEquilibriumConstantModel -->

    <owl:Class rdf:about="https://github.com/sustainable-processes/ontology/OntoCAPE/model/property_models.owl#AdsorptionEquilibriumConstantModel">
        <rdfs:subClassOf rdf:resource="https://github.com/sustainable-processes/ontology/OntoCAPE/model/property_models.owl#IntensiveThermodynamicStateModel"/>
        <owl:disjointWith rdf:resource="https://github.com/sustainable-processes/ontology/OntoCAPE/model/property_models.owl#DensityModel"/>
        <owl:disjointWith rdf:resource="https://github.com/sustainable-processes/ontology/OntoCAPE/model/property_models.owl#FugacityCoefficientModel"/>
        <owl:disjointWith rdf:resource="https://github.com/sustainable-processes/ontology/OntoCAPE/model/property_models.owl#HeatCapacityModel"/>
        <owl:disjointWith rdf:resource="https://github.com/sustainable-processes/ontology/OntoCAPE/model/property_models.owl#PartialMolarEnthalpyModel"/>
        <owl:disjointWith rdf:resource="https://github.com/sustainable-processes/ontology/OntoCAPE/model/property_models.owl#PartialMolarVolumeModel"/>
        <owl:disjointWith rdf:resource="https://github.com/sustainable-processes/ontology/OntoCAPE/model/property_models.owl#PhaseEquilibriumRatioModel"/>
        <owl:disjointWith rdf:resource="https://github.com/sustainable-processes/ontology/OntoCAPE/model/property_models.owl#ReactionEquilibriumConstantModel"/>
        <owl:disjointWith rdf:resource="https://github.com/sustainable-processes/ontology/OntoCAPE/model/property_models.owl#SpecificEnthalpyModel"/>
        <owl:disjointWith rdf:resource="https://github.com/sustainable-processes/ontology/OntoCAPE/model/property_models.owl#VapourPressureModel"/>
        <rdfs:comment>A PropertyModel that provides a correlation for an adsorption equilibrium constant.</rdfs:comment>
    </owl:Class>
    


    <!-- https://github.com/sustainable-processes/ontology/OntoCAPE/model/property_models.owl#AdsorptionRateCoefficientModel -->

    <owl:Class rdf:about="https://github.com/sustainable-processes/ontology/OntoCAPE/model/property_models.owl#AdsorptionRateCoefficientModel">
        <rdfs:subClassOf rdf:resource="https://github.com/sustainable-processes/ontology/OntoCAPE/model/property_models.owl#ChemicalKineticsPropertyModel"/>
        <owl:disjointWith rdf:resource="https://github.com/sustainable-processes/ontology/OntoCAPE/model/property_models.owl#HeterogeneousReactionRateCoefficientModel"/>
        <owl:disjointWith rdf:resource="https://github.com/sustainable-processes/ontology/OntoCAPE/model/property_models.owl#HomogeneousReactionRateCoefficientModel"/>
        <rdfs:comment>A PropertyModel that provides a correlation for a surface reaction rate coefficient.</rdfs:comment>
    </owl:Class>
    


    <!-- https://github.com/sustainable-processes/ontology/OntoCAPE/model/property_models.owl#ChemicalKineticsPropertyModel -->

    <owl:Class rdf:about="https://github.com/sustainable-processes/ontology/OntoCAPE/model/property_models.owl#ChemicalKineticsPropertyModel">
        <rdfs:subClassOf rdf:resource="https://github.com/sustainable-processes/ontology/OntoCAPE/model/process_model.owl#PropertyModel"/>
        <owl:disjointWith rdf:resource="https://github.com/sustainable-processes/ontology/OntoCAPE/model/property_models.owl#PhaseInterfaceTransportPropertyModel"/>
        <owl:disjointWith rdf:resource="https://github.com/sustainable-processes/ontology/OntoCAPE/model/property_models.owl#ThermoModel"/>
        <rdfs:comment>A PropertyModel that provides a correlation for a chemical kinetics coefficient.</rdfs:comment>
    </owl:Class>
    


    <!-- https://github.com/sustainable-processes/ontology/OntoCAPE/model/property_models.owl#DensityModel -->

    <owl:Class rdf:about="https://github.com/sustainable-processes/ontology/OntoCAPE/model/property_models.owl#DensityModel">
        <rdfs:subClassOf rdf:resource="https://github.com/sustainable-processes/ontology/OntoCAPE/model/property_models.owl#IntensiveThermodynamicStateModel"/>
        <rdfs:subClassOf>
            <owl:Restriction>
                <owl:onProperty rdf:resource="https://github.com/sustainable-processes/ontology/OntoCAPE/model/mathematical_model.owl#hasModelVariable"/>
                <owl:someValuesFrom>
                    <owl:Class>
                        <owl:intersectionOf rdf:parseType="Collection">
                            <rdf:Description rdf:about="https://github.com/sustainable-processes/ontology/OntoCAPE/model/mathematical_model.owl#ModelVariable"/>
                            <owl:Restriction>
                                <owl:onProperty rdf:resource="https://github.com/sustainable-processes/ontology/OntoCAPE/model/mathematical_model.owl#correspondsToQuantity"/>
                                <owl:someValuesFrom rdf:resource="https://github.com/sustainable-processes/ontology/OntoCAPE/material/phase_system/phase_system.owl#Density"/>
                            </owl:Restriction>
                        </owl:intersectionOf>
                    </owl:Class>
                </owl:someValuesFrom>
            </owl:Restriction>
        </rdfs:subClassOf>
        <owl:disjointWith rdf:resource="https://github.com/sustainable-processes/ontology/OntoCAPE/model/property_models.owl#FugacityCoefficientModel"/>
        <owl:disjointWith rdf:resource="https://github.com/sustainable-processes/ontology/OntoCAPE/model/property_models.owl#HeatCapacityModel"/>
        <owl:disjointWith rdf:resource="https://github.com/sustainable-processes/ontology/OntoCAPE/model/property_models.owl#PartialMolarEnthalpyModel"/>
        <owl:disjointWith rdf:resource="https://github.com/sustainable-processes/ontology/OntoCAPE/model/property_models.owl#PartialMolarVolumeModel"/>
        <owl:disjointWith rdf:resource="https://github.com/sustainable-processes/ontology/OntoCAPE/model/property_models.owl#PhaseEquilibriumRatioModel"/>
        <owl:disjointWith rdf:resource="https://github.com/sustainable-processes/ontology/OntoCAPE/model/property_models.owl#ReactionEquilibriumConstantModel"/>
        <owl:disjointWith rdf:resource="https://github.com/sustainable-processes/ontology/OntoCAPE/model/property_models.owl#SpecificEnthalpyModel"/>
        <owl:disjointWith rdf:resource="https://github.com/sustainable-processes/ontology/OntoCAPE/model/property_models.owl#VapourPressureModel"/>
        <rdfs:comment>A PropertyModel that provides a correlation for the computation of Density.</rdfs:comment>
    </owl:Class>
    


    <!-- https://github.com/sustainable-processes/ontology/OntoCAPE/model/property_models.owl#FugacityCoefficientModel -->

    <owl:Class rdf:about="https://github.com/sustainable-processes/ontology/OntoCAPE/model/property_models.owl#FugacityCoefficientModel">
        <rdfs:subClassOf rdf:resource="https://github.com/sustainable-processes/ontology/OntoCAPE/model/property_models.owl#IntensiveThermodynamicStateModel"/>
        <rdfs:subClassOf>
            <owl:Restriction>
                <owl:onProperty rdf:resource="https://github.com/sustainable-processes/ontology/OntoCAPE/model/mathematical_model.owl#hasModelVariable"/>
                <owl:someValuesFrom>
                    <owl:Class>
                        <owl:intersectionOf rdf:parseType="Collection">
                            <rdf:Description rdf:about="https://github.com/sustainable-processes/ontology/OntoCAPE/model/mathematical_model.owl#ModelVariable"/>
                            <owl:Restriction>
                                <owl:onProperty rdf:resource="https://github.com/sustainable-processes/ontology/OntoCAPE/model/mathematical_model.owl#correspondsToQuantity"/>
                                <owl:someValuesFrom rdf:resource="https://github.com/sustainable-processes/ontology/OntoCAPE/material/phase_system/phase_system.owl#FugacityCoefficient"/>
                            </owl:Restriction>
                        </owl:intersectionOf>
                    </owl:Class>
                </owl:someValuesFrom>
            </owl:Restriction>
        </rdfs:subClassOf>
        <owl:disjointWith rdf:resource="https://github.com/sustainable-processes/ontology/OntoCAPE/model/property_models.owl#HeatCapacityModel"/>
        <owl:disjointWith rdf:resource="https://github.com/sustainable-processes/ontology/OntoCAPE/model/property_models.owl#PartialMolarEnthalpyModel"/>
        <owl:disjointWith rdf:resource="https://github.com/sustainable-processes/ontology/OntoCAPE/model/property_models.owl#PartialMolarVolumeModel"/>
        <owl:disjointWith rdf:resource="https://github.com/sustainable-processes/ontology/OntoCAPE/model/property_models.owl#PhaseEquilibriumRatioModel"/>
        <owl:disjointWith rdf:resource="https://github.com/sustainable-processes/ontology/OntoCAPE/model/property_models.owl#ReactionEquilibriumConstantModel"/>
        <owl:disjointWith rdf:resource="https://github.com/sustainable-processes/ontology/OntoCAPE/model/property_models.owl#SpecificEnthalpyModel"/>
        <owl:disjointWith rdf:resource="https://github.com/sustainable-processes/ontology/OntoCAPE/model/property_models.owl#VapourPressureModel"/>
        <rdfs:comment>A PropertyModel that provides a correlation for the computation of FugacityCoefficient.</rdfs:comment>
    </owl:Class>
    


    <!-- https://github.com/sustainable-processes/ontology/OntoCAPE/model/property_models.owl#HeatCapacityModel -->

    <owl:Class rdf:about="https://github.com/sustainable-processes/ontology/OntoCAPE/model/property_models.owl#HeatCapacityModel">
        <rdfs:subClassOf rdf:resource="https://github.com/sustainable-processes/ontology/OntoCAPE/model/property_models.owl#IntensiveThermodynamicStateModel"/>
        <owl:disjointWith rdf:resource="https://github.com/sustainable-processes/ontology/OntoCAPE/model/property_models.owl#PartialMolarEnthalpyModel"/>
        <owl:disjointWith rdf:resource="https://github.com/sustainable-processes/ontology/OntoCAPE/model/property_models.owl#PartialMolarVolumeModel"/>
        <owl:disjointWith rdf:resource="https://github.com/sustainable-processes/ontology/OntoCAPE/model/property_models.owl#PhaseEquilibriumRatioModel"/>
        <owl:disjointWith rdf:resource="https://github.com/sustainable-processes/ontology/OntoCAPE/model/property_models.owl#ReactionEquilibriumConstantModel"/>
        <owl:disjointWith rdf:resource="https://github.com/sustainable-processes/ontology/OntoCAPE/model/property_models.owl#SpecificEnthalpyModel"/>
        <owl:disjointWith rdf:resource="https://github.com/sustainable-processes/ontology/OntoCAPE/model/property_models.owl#VapourPressureModel"/>
        <rdfs:comment>A PropertyModel that provides a correlation for the computation of the heat capacity.</rdfs:comment>
    </owl:Class>
    


    <!-- https://github.com/sustainable-processes/ontology/OntoCAPE/model/property_models.owl#HeatTransferCoefficientModel -->

    <owl:Class rdf:about="https://github.com/sustainable-processes/ontology/OntoCAPE/model/property_models.owl#HeatTransferCoefficientModel">
        <rdfs:subClassOf rdf:resource="https://github.com/sustainable-processes/ontology/OntoCAPE/model/property_models.owl#PhaseInterfaceTransportPropertyModel"/>
        <owl:disjointWith rdf:resource="https://github.com/sustainable-processes/ontology/OntoCAPE/model/property_models.owl#MassTransferCoefficientModel"/>
        <rdfs:comment>A PropertyModel that provides a correlation for a heat transfer coefficient.</rdfs:comment>
    </owl:Class>
    


    <!-- https://github.com/sustainable-processes/ontology/OntoCAPE/model/property_models.owl#HeterogeneousReactionRateCoefficientModel -->

    <owl:Class rdf:about="https://github.com/sustainable-processes/ontology/OntoCAPE/model/property_models.owl#HeterogeneousReactionRateCoefficientModel">
        <rdfs:subClassOf rdf:resource="https://github.com/sustainable-processes/ontology/OntoCAPE/model/property_models.owl#ChemicalKineticsPropertyModel"/>
        <owl:disjointWith rdf:resource="https://github.com/sustainable-processes/ontology/OntoCAPE/model/property_models.owl#HomogeneousReactionRateCoefficientModel"/>
        <rdfs:comment>A PropertyModel that provides a correlation for an adsorption equilibrium constant.</rdfs:comment>
    </owl:Class>
    


    <!-- https://github.com/sustainable-processes/ontology/OntoCAPE/model/property_models.owl#HomogeneousReactionRateCoefficientModel -->

    <owl:Class rdf:about="https://github.com/sustainable-processes/ontology/OntoCAPE/model/property_models.owl#HomogeneousReactionRateCoefficientModel">
        <rdfs:subClassOf rdf:resource="https://github.com/sustainable-processes/ontology/OntoCAPE/model/property_models.owl#ChemicalKineticsPropertyModel"/>
        <rdfs:comment>A PropertyModel that provides a correlation for a chemical reaction rate coefficient</rdfs:comment>
    </owl:Class>
    


    <!-- https://github.com/sustainable-processes/ontology/OntoCAPE/model/property_models.owl#IntensiveThermodynamicStateModel -->

    <owl:Class rdf:about="https://github.com/sustainable-processes/ontology/OntoCAPE/model/property_models.owl#IntensiveThermodynamicStateModel">
        <rdfs:subClassOf rdf:resource="https://github.com/sustainable-processes/ontology/OntoCAPE/model/property_models.owl#ThermoModel"/>
        <rdfs:subClassOf>
            <owl:Restriction>
                <owl:onProperty rdf:resource="https://github.com/sustainable-processes/ontology/OntoCAPE/model/mathematical_model.owl#hasModelVariable"/>
                <owl:someValuesFrom>
                    <owl:Class>
                        <owl:intersectionOf rdf:parseType="Collection">
                            <rdf:Description rdf:about="https://github.com/sustainable-processes/ontology/OntoCAPE/model/mathematical_model.owl#ModelVariable"/>
                            <owl:Restriction>
                                <owl:onProperty rdf:resource="https://github.com/sustainable-processes/ontology/OntoCAPE/model/mathematical_model.owl#correspondsToQuantity"/>
                                <owl:someValuesFrom rdf:resource="https://github.com/sustainable-processes/ontology/OntoCAPE/material/phase_system/phase_system.owl#IntensiveThermodynamicStateVariable"/>
                            </owl:Restriction>
                        </owl:intersectionOf>
                    </owl:Class>
                </owl:someValuesFrom>
            </owl:Restriction>
        </rdfs:subClassOf>
        <owl:disjointWith rdf:resource="https://github.com/sustainable-processes/ontology/OntoCAPE/model/property_models.owl#IntraPhaseTransportPropertyModel"/>
        <owl:disjointWith rdf:resource="https://github.com/sustainable-processes/ontology/OntoCAPE/model/property_models.owl#SurfaceTensionModel"/>
        <rdfs:comment>A PropertyModel that provides a correlation for an IntensiveThermodynamicStateVariable.</rdfs:comment>
    </owl:Class>
    


    <!-- https://github.com/sustainable-processes/ontology/OntoCAPE/model/property_models.owl#IntraPhaseTransportPropertyModel -->

    <owl:Class rdf:about="https://github.com/sustainable-processes/ontology/OntoCAPE/model/property_models.owl#IntraPhaseTransportPropertyModel">
        <rdfs:subClassOf rdf:resource="https://github.com/sustainable-processes/ontology/OntoCAPE/model/property_models.owl#ThermoModel"/>
        <rdfs:subClassOf>
            <owl:Restriction>
                <owl:onProperty rdf:resource="https://github.com/sustainable-processes/ontology/OntoCAPE/model/mathematical_model.owl#hasModelVariable"/>
                <owl:someValuesFrom>
                    <owl:Class>
                        <owl:intersectionOf rdf:parseType="Collection">
                            <rdf:Description rdf:about="https://github.com/sustainable-processes/ontology/OntoCAPE/model/mathematical_model.owl#ModelVariable"/>
                            <owl:Restriction>
                                <owl:onProperty rdf:resource="https://github.com/sustainable-processes/ontology/OntoCAPE/model/mathematical_model.owl#correspondsToQuantity"/>
                                <owl:someValuesFrom rdf:resource="https://github.com/sustainable-processes/ontology/OntoCAPE/material/phase_system/phase_system.owl#TransportPhenomenaProperty"/>
                            </owl:Restriction>
                        </owl:intersectionOf>
                    </owl:Class>
                </owl:someValuesFrom>
            </owl:Restriction>
        </rdfs:subClassOf>
        <owl:disjointWith rdf:resource="https://github.com/sustainable-processes/ontology/OntoCAPE/model/property_models.owl#SurfaceTensionModel"/>
        <rdfs:comment>A PropertyModel that provides a correlation for a TransportPhenomenaProperty</rdfs:comment>
    </owl:Class>
    


    <!-- https://github.com/sustainable-processes/ontology/OntoCAPE/model/property_models.owl#MassDiffusionCoefficientModel -->

    <owl:Class rdf:about="https://github.com/sustainable-processes/ontology/OntoCAPE/model/property_models.owl#MassDiffusionCoefficientModel">
        <rdfs:subClassOf rdf:resource="https://github.com/sustainable-processes/ontology/OntoCAPE/model/property_models.owl#IntraPhaseTransportPropertyModel"/>
        <rdfs:subClassOf>
            <owl:Restriction>
                <owl:onProperty rdf:resource="https://github.com/sustainable-processes/ontology/OntoCAPE/model/mathematical_model.owl#hasModelVariable"/>
                <owl:someValuesFrom>
                    <owl:Class>
                        <owl:intersectionOf rdf:parseType="Collection">
                            <rdf:Description rdf:about="https://github.com/sustainable-processes/ontology/OntoCAPE/model/mathematical_model.owl#ModelVariable"/>
                            <owl:Restriction>
                                <owl:onProperty rdf:resource="https://github.com/sustainable-processes/ontology/OntoCAPE/model/mathematical_model.owl#correspondsToQuantity"/>
                                <owl:someValuesFrom rdf:resource="https://github.com/sustainable-processes/ontology/OntoCAPE/material/phase_system/phase_system.owl#DiffusionCoefficient"/>
                            </owl:Restriction>
                        </owl:intersectionOf>
                    </owl:Class>
                </owl:someValuesFrom>
            </owl:Restriction>
        </rdfs:subClassOf>
        <owl:disjointWith rdf:resource="https://github.com/sustainable-processes/ontology/OntoCAPE/model/property_models.owl#ThermalConductivityModel"/>
        <owl:disjointWith rdf:resource="https://github.com/sustainable-processes/ontology/OntoCAPE/model/property_models.owl#ViscosityModel"/>
        <rdfs:comment>A PropertyModel that provides a correlation for an intra-phase mass DiffusionCoefficient.</rdfs:comment>
    </owl:Class>
    


    <!-- https://github.com/sustainable-processes/ontology/OntoCAPE/model/property_models.owl#MassTransferCoefficientModel -->

    <owl:Class rdf:about="https://github.com/sustainable-processes/ontology/OntoCAPE/model/property_models.owl#MassTransferCoefficientModel">
        <rdfs:subClassOf rdf:resource="https://github.com/sustainable-processes/ontology/OntoCAPE/model/property_models.owl#PhaseInterfaceTransportPropertyModel"/>
        <rdfs:comment>A PropertyModel that provides a correlation for a phase interface mass transfer coefficient.</rdfs:comment>
    </owl:Class>
    


    <!-- https://github.com/sustainable-processes/ontology/OntoCAPE/model/property_models.owl#PartialMolarEnthalpyModel -->

    <owl:Class rdf:about="https://github.com/sustainable-processes/ontology/OntoCAPE/model/property_models.owl#PartialMolarEnthalpyModel">
        <rdfs:subClassOf rdf:resource="https://github.com/sustainable-processes/ontology/OntoCAPE/model/property_models.owl#IntensiveThermodynamicStateModel"/>
        <rdfs:subClassOf>
            <owl:Restriction>
                <owl:onProperty rdf:resource="https://github.com/sustainable-processes/ontology/OntoCAPE/model/mathematical_model.owl#hasModelVariable"/>
                <owl:someValuesFrom>
                    <owl:Class>
                        <owl:intersectionOf rdf:parseType="Collection">
                            <rdf:Description rdf:about="https://github.com/sustainable-processes/ontology/OntoCAPE/model/mathematical_model.owl#ModelVariable"/>
                            <owl:Restriction>
                                <owl:onProperty rdf:resource="https://github.com/sustainable-processes/ontology/OntoCAPE/model/mathematical_model.owl#correspondsToQuantity"/>
                                <owl:someValuesFrom rdf:resource="https://github.com/sustainable-processes/ontology/OntoCAPE/material/phase_system/phase_system.owl#PartialMolarEnthalpy"/>
                            </owl:Restriction>
                        </owl:intersectionOf>
                    </owl:Class>
                </owl:someValuesFrom>
            </owl:Restriction>
        </rdfs:subClassOf>
        <owl:disjointWith rdf:resource="https://github.com/sustainable-processes/ontology/OntoCAPE/model/property_models.owl#PartialMolarVolumeModel"/>
        <owl:disjointWith rdf:resource="https://github.com/sustainable-processes/ontology/OntoCAPE/model/property_models.owl#PhaseEquilibriumRatioModel"/>
        <owl:disjointWith rdf:resource="https://github.com/sustainable-processes/ontology/OntoCAPE/model/property_models.owl#ReactionEquilibriumConstantModel"/>
        <owl:disjointWith rdf:resource="https://github.com/sustainable-processes/ontology/OntoCAPE/model/property_models.owl#SpecificEnthalpyModel"/>
        <owl:disjointWith rdf:resource="https://github.com/sustainable-processes/ontology/OntoCAPE/model/property_models.owl#VapourPressureModel"/>
        <rdfs:comment>A PropertyModel that provides a correlation for the computation of the PartialMolarEnthalpy.</rdfs:comment>
    </owl:Class>
    


    <!-- https://github.com/sustainable-processes/ontology/OntoCAPE/model/property_models.owl#PartialMolarVolumeModel -->

    <owl:Class rdf:about="https://github.com/sustainable-processes/ontology/OntoCAPE/model/property_models.owl#PartialMolarVolumeModel">
        <rdfs:subClassOf rdf:resource="https://github.com/sustainable-processes/ontology/OntoCAPE/model/property_models.owl#IntensiveThermodynamicStateModel"/>
        <rdfs:subClassOf>
            <owl:Restriction>
                <owl:onProperty rdf:resource="https://github.com/sustainable-processes/ontology/OntoCAPE/model/mathematical_model.owl#hasModelVariable"/>
                <owl:someValuesFrom>
                    <owl:Class>
                        <owl:intersectionOf rdf:parseType="Collection">
                            <rdf:Description rdf:about="https://github.com/sustainable-processes/ontology/OntoCAPE/model/mathematical_model.owl#ModelVariable"/>
                            <owl:Restriction>
                                <owl:onProperty rdf:resource="https://github.com/sustainable-processes/ontology/OntoCAPE/model/mathematical_model.owl#correspondsToQuantity"/>
                                <owl:someValuesFrom rdf:resource="https://github.com/sustainable-processes/ontology/OntoCAPE/material/phase_system/phase_system.owl#PartialMolarVolume"/>
                            </owl:Restriction>
                        </owl:intersectionOf>
                    </owl:Class>
                </owl:someValuesFrom>
            </owl:Restriction>
        </rdfs:subClassOf>
        <owl:disjointWith rdf:resource="https://github.com/sustainable-processes/ontology/OntoCAPE/model/property_models.owl#PhaseEquilibriumRatioModel"/>
        <owl:disjointWith rdf:resource="https://github.com/sustainable-processes/ontology/OntoCAPE/model/property_models.owl#ReactionEquilibriumConstantModel"/>
        <owl:disjointWith rdf:resource="https://github.com/sustainable-processes/ontology/OntoCAPE/model/property_models.owl#SpecificEnthalpyModel"/>
        <owl:disjointWith rdf:resource="https://github.com/sustainable-processes/ontology/OntoCAPE/model/property_models.owl#VapourPressureModel"/>
        <rdfs:comment>A PropertyModel that provides a correlation for the computation of the PartialMolarVolume.</rdfs:comment>
    </owl:Class>
    


    <!-- https://github.com/sustainable-processes/ontology/OntoCAPE/model/property_models.owl#PhaseEquilibriumRatioModel -->

    <owl:Class rdf:about="https://github.com/sustainable-processes/ontology/OntoCAPE/model/property_models.owl#PhaseEquilibriumRatioModel">
        <rdfs:subClassOf rdf:resource="https://github.com/sustainable-processes/ontology/OntoCAPE/model/property_models.owl#IntensiveThermodynamicStateModel"/>
        <rdfs:subClassOf>
            <owl:Restriction>
                <owl:onProperty rdf:resource="https://github.com/sustainable-processes/ontology/OntoCAPE/model/mathematical_model.owl#hasModelVariable"/>
                <owl:someValuesFrom>
                    <owl:Class>
                        <owl:intersectionOf rdf:parseType="Collection">
                            <rdf:Description rdf:about="https://github.com/sustainable-processes/ontology/OntoCAPE/model/mathematical_model.owl#ModelVariable"/>
                            <owl:Restriction>
                                <owl:onProperty rdf:resource="https://github.com/sustainable-processes/ontology/OntoCAPE/model/mathematical_model.owl#correspondsToQuantity"/>
                                <owl:someValuesFrom rdf:resource="https://github.com/sustainable-processes/ontology/OntoCAPE/material/phase_system/phase_system.owl#PhaseEquilibriumRatio"/>
                            </owl:Restriction>
                        </owl:intersectionOf>
                    </owl:Class>
                </owl:someValuesFrom>
            </owl:Restriction>
        </rdfs:subClassOf>
        <owl:disjointWith rdf:resource="https://github.com/sustainable-processes/ontology/OntoCAPE/model/property_models.owl#ReactionEquilibriumConstantModel"/>
        <owl:disjointWith rdf:resource="https://github.com/sustainable-processes/ontology/OntoCAPE/model/property_models.owl#SpecificEnthalpyModel"/>
        <owl:disjointWith rdf:resource="https://github.com/sustainable-processes/ontology/OntoCAPE/model/property_models.owl#VapourPressureModel"/>
        <rdfs:comment>A PropertyModel that provides a correlation for the computation of a PhaseEquilibriumRatio.</rdfs:comment>
    </owl:Class>
    


    <!-- https://github.com/sustainable-processes/ontology/OntoCAPE/model/property_models.owl#PhaseInterfaceTransportPropertyModel -->

    <owl:Class rdf:about="https://github.com/sustainable-processes/ontology/OntoCAPE/model/property_models.owl#PhaseInterfaceTransportPropertyModel">
        <rdfs:subClassOf rdf:resource="https://github.com/sustainable-processes/ontology/OntoCAPE/model/process_model.owl#PropertyModel"/>
        <owl:disjointWith rdf:resource="https://github.com/sustainable-processes/ontology/OntoCAPE/model/property_models.owl#ThermoModel"/>
        <rdfs:comment>A PropertyModel that provides a correlation for a phase interface transport coefficient.</rdfs:comment>
    </owl:Class>
    


    <!-- https://github.com/sustainable-processes/ontology/OntoCAPE/model/property_models.owl#ReactionEquilibriumConstantModel -->

    <owl:Class rdf:about="https://github.com/sustainable-processes/ontology/OntoCAPE/model/property_models.owl#ReactionEquilibriumConstantModel">
        <rdfs:subClassOf rdf:resource="https://github.com/sustainable-processes/ontology/OntoCAPE/model/property_models.owl#IntensiveThermodynamicStateModel"/>
        <owl:disjointWith rdf:resource="https://github.com/sustainable-processes/ontology/OntoCAPE/model/property_models.owl#SpecificEnthalpyModel"/>
        <owl:disjointWith rdf:resource="https://github.com/sustainable-processes/ontology/OntoCAPE/model/property_models.owl#VapourPressureModel"/>
        <rdfs:comment>A PropertyModel that provides a correlation for a reaction equilibrium constant.</rdfs:comment>
    </owl:Class>
    


    <!-- https://github.com/sustainable-processes/ontology/OntoCAPE/model/property_models.owl#SpecificEnthalpyModel -->

    <owl:Class rdf:about="https://github.com/sustainable-processes/ontology/OntoCAPE/model/property_models.owl#SpecificEnthalpyModel">
        <rdfs:subClassOf rdf:resource="https://github.com/sustainable-processes/ontology/OntoCAPE/model/property_models.owl#IntensiveThermodynamicStateModel"/>
        <rdfs:subClassOf>
            <owl:Restriction>
                <owl:onProperty rdf:resource="https://github.com/sustainable-processes/ontology/OntoCAPE/model/mathematical_model.owl#hasModelVariable"/>
                <owl:someValuesFrom>
                    <owl:Class>
                        <owl:intersectionOf rdf:parseType="Collection">
                            <rdf:Description rdf:about="https://github.com/sustainable-processes/ontology/OntoCAPE/model/mathematical_model.owl#ModelVariable"/>
                            <owl:Restriction>
                                <owl:onProperty rdf:resource="https://github.com/sustainable-processes/ontology/OntoCAPE/model/mathematical_model.owl#correspondsToQuantity"/>
                                <owl:someValuesFrom rdf:resource="https://github.com/sustainable-processes/ontology/OntoCAPE/material/phase_system/phase_system.owl#SpecificEnthalpy"/>
                            </owl:Restriction>
                        </owl:intersectionOf>
                    </owl:Class>
                </owl:someValuesFrom>
            </owl:Restriction>
        </rdfs:subClassOf>
        <owl:disjointWith rdf:resource="https://github.com/sustainable-processes/ontology/OntoCAPE/model/property_models.owl#VapourPressureModel"/>
        <rdfs:comment>A PropertyModel that provides a correlation for the computation of the SpecificEnthalpy.</rdfs:comment>
    </owl:Class>
    


    <!-- https://github.com/sustainable-processes/ontology/OntoCAPE/model/property_models.owl#SpecificGibbsFreeEnergyModel -->

    <owl:Class rdf:about="https://github.com/sustainable-processes/ontology/OntoCAPE/model/property_models.owl#SpecificGibbsFreeEnergyModel">
        <rdfs:subClassOf rdf:resource="https://github.com/sustainable-processes/ontology/OntoCAPE/model/property_models.owl#IntensiveThermodynamicStateModel"/>
        <rdfs:comment>A PropertyModel that provides a correlation for the computation of the SpecificGibbsFreeEnergy.</rdfs:comment>
    </owl:Class>
    


    <!-- https://github.com/sustainable-processes/ontology/OntoCAPE/model/property_models.owl#SurfaceTensionModel -->

    <owl:Class rdf:about="https://github.com/sustainable-processes/ontology/OntoCAPE/model/property_models.owl#SurfaceTensionModel">
        <rdfs:subClassOf rdf:resource="https://github.com/sustainable-processes/ontology/OntoCAPE/model/property_models.owl#ThermoModel"/>
        <rdfs:subClassOf>
            <owl:Restriction>
                <owl:onProperty rdf:resource="https://github.com/sustainable-processes/ontology/OntoCAPE/model/mathematical_model.owl#hasModelVariable"/>
                <owl:someValuesFrom>
                    <owl:Class>
                        <owl:intersectionOf rdf:parseType="Collection">
                            <rdf:Description rdf:about="https://github.com/sustainable-processes/ontology/OntoCAPE/model/mathematical_model.owl#ModelVariable"/>
                            <owl:Restriction>
                                <owl:onProperty rdf:resource="https://github.com/sustainable-processes/ontology/OntoCAPE/model/mathematical_model.owl#correspondsToQuantity"/>
                                <owl:someValuesFrom rdf:resource="https://github.com/sustainable-processes/ontology/OntoCAPE/material/phase_system/phase_system.owl#SurfaceTension"/>
                            </owl:Restriction>
                        </owl:intersectionOf>
                    </owl:Class>
                </owl:someValuesFrom>
            </owl:Restriction>
        </rdfs:subClassOf>
        <rdfs:comment>A PropertyModel that provides a correlation for computation of the SurfaceTension.</rdfs:comment>
    </owl:Class>
    


    <!-- https://github.com/sustainable-processes/ontology/OntoCAPE/model/property_models.owl#ThermalConductivityModel -->

    <owl:Class rdf:about="https://github.com/sustainable-processes/ontology/OntoCAPE/model/property_models.owl#ThermalConductivityModel">
        <rdfs:subClassOf rdf:resource="https://github.com/sustainable-processes/ontology/OntoCAPE/model/property_models.owl#IntraPhaseTransportPropertyModel"/>
        <rdfs:subClassOf>
            <owl:Restriction>
                <owl:onProperty rdf:resource="https://github.com/sustainable-processes/ontology/OntoCAPE/model/mathematical_model.owl#hasModelVariable"/>
                <owl:someValuesFrom>
                    <owl:Class>
                        <owl:intersectionOf rdf:parseType="Collection">
                            <rdf:Description rdf:about="https://github.com/sustainable-processes/ontology/OntoCAPE/model/mathematical_model.owl#ModelVariable"/>
                            <owl:Restriction>
                                <owl:onProperty rdf:resource="https://github.com/sustainable-processes/ontology/OntoCAPE/model/mathematical_model.owl#correspondsToQuantity"/>
                                <owl:someValuesFrom rdf:resource="https://github.com/sustainable-processes/ontology/OntoCAPE/material/phase_system/phase_system.owl#ThermalConductivity"/>
                            </owl:Restriction>
                        </owl:intersectionOf>
                    </owl:Class>
                </owl:someValuesFrom>
            </owl:Restriction>
        </rdfs:subClassOf>
        <owl:disjointWith rdf:resource="https://github.com/sustainable-processes/ontology/OntoCAPE/model/property_models.owl#ViscosityModel"/>
        <rdfs:comment>A PropertyModel that provides a correlation for the ThermalConductivity.</rdfs:comment>
    </owl:Class>
    


    <!-- https://github.com/sustainable-processes/ontology/OntoCAPE/model/property_models.owl#ThermoModel -->

    <owl:Class rdf:about="https://github.com/sustainable-processes/ontology/OntoCAPE/model/property_models.owl#ThermoModel">
        <rdfs:subClassOf rdf:resource="https://github.com/sustainable-processes/ontology/OntoCAPE/model/process_model.owl#PropertyModel"/>
        <rdfs:subClassOf>
            <owl:Restriction>
                <owl:onProperty rdf:resource="https://github.com/sustainable-processes/ontology/OntoCAPE/model/mathematical_model.owl#hasModelVariable"/>
                <owl:someValuesFrom>
                    <owl:Class>
                        <owl:intersectionOf rdf:parseType="Collection">
                            <rdf:Description rdf:about="https://github.com/sustainable-processes/ontology/OntoCAPE/model/mathematical_model.owl#ModelVariable"/>
                            <owl:Restriction>
                                <owl:onProperty rdf:resource="https://github.com/sustainable-processes/ontology/OntoCAPE/model/mathematical_model.owl#correspondsToQuantity"/>
                                <owl:someValuesFrom rdf:resource="https://github.com/sustainable-processes/ontology/OntoCAPE/material/phase_system/phase_system.owl#PhaseSystemProperty"/>
                            </owl:Restriction>
                        </owl:intersectionOf>
                    </owl:Class>
                </owl:someValuesFrom>
            </owl:Restriction>
        </rdfs:subClassOf>
        <rdfs:comment>A PropertyModel that provides a correlation for a PhaseSystemProperty not relevant to rates.</rdfs:comment>
    </owl:Class>
    


    <!-- https://github.com/sustainable-processes/ontology/OntoCAPE/model/property_models.owl#VapourPressureModel -->

    <owl:Class rdf:about="https://github.com/sustainable-processes/ontology/OntoCAPE/model/property_models.owl#VapourPressureModel">
        <rdfs:subClassOf rdf:resource="https://github.com/sustainable-processes/ontology/OntoCAPE/model/property_models.owl#IntensiveThermodynamicStateModel"/>
        <rdfs:comment>A PropertyModel that provides a correlation for the computation of the vapor pressure.</rdfs:comment>
    </owl:Class>
    


    <!-- https://github.com/sustainable-processes/ontology/OntoCAPE/model/property_models.owl#ViscosityModel -->

    <owl:Class rdf:about="https://github.com/sustainable-processes/ontology/OntoCAPE/model/property_models.owl#ViscosityModel">
        <rdfs:subClassOf rdf:resource="https://github.com/sustainable-processes/ontology/OntoCAPE/model/property_models.owl#IntraPhaseTransportPropertyModel"/>
        <rdfs:subClassOf>
            <owl:Restriction>
                <owl:onProperty rdf:resource="https://github.com/sustainable-processes/ontology/OntoCAPE/model/mathematical_model.owl#hasModelVariable"/>
                <owl:someValuesFrom>
                    <owl:Class>
                        <owl:intersectionOf rdf:parseType="Collection">
                            <rdf:Description rdf:about="https://github.com/sustainable-processes/ontology/OntoCAPE/model/mathematical_model.owl#ModelVariable"/>
                            <owl:Restriction>
                                <owl:onProperty rdf:resource="https://github.com/sustainable-processes/ontology/OntoCAPE/model/mathematical_model.owl#correspondsToQuantity"/>
                                <owl:someValuesFrom rdf:resource="https://github.com/sustainable-processes/ontology/OntoCAPE/material/phase_system/phase_system.owl#DynamicViscosity"/>
                            </owl:Restriction>
                        </owl:intersectionOf>
                    </owl:Class>
                </owl:someValuesFrom>
            </owl:Restriction>
        </rdfs:subClassOf>
        <rdfs:comment>A PropertyModel that provides a correlation for the DynamicViscosity.</rdfs:comment>
    </owl:Class>
    


    <!-- 
    ///////////////////////////////////////////////////////////////////////////////////////
    //
    // Individuals
    //
    ///////////////////////////////////////////////////////////////////////////////////////
     -->

    


    <!-- https://github.com/sustainable-processes/ontology/OntoCAPE/model/property_models.owl#Antoine -->

    <owl:NamedIndividual rdf:about="https://github.com/sustainable-processes/ontology/OntoCAPE/model/property_models.owl#Antoine">
        <rdf:type rdf:resource="https://github.com/sustainable-processes/ontology/OntoCAPE/model/property_models.owl#VapourPressureModel"/>
    </owl:NamedIndividual>
    


    <!-- https://github.com/sustainable-processes/ontology/OntoCAPE/model/property_models.owl#NRTL -->

    <owl:NamedIndividual rdf:about="https://github.com/sustainable-processes/ontology/OntoCAPE/model/property_models.owl#NRTL">
        <rdf:type rdf:resource="https://github.com/sustainable-processes/ontology/OntoCAPE/model/property_models.owl#ActivityCoefficientModel"/>
    </owl:NamedIndividual>
    


    <!-- https://github.com/sustainable-processes/ontology/OntoCAPE/model/property_models.owl#UNIFAC -->

    <owl:NamedIndividual rdf:about="https://github.com/sustainable-processes/ontology/OntoCAPE/model/property_models.owl#UNIFAC">
        <rdf:type rdf:resource="https://github.com/sustainable-processes/ontology/OntoCAPE/model/property_models.owl#ActivityCoefficientModel"/>
    </owl:NamedIndividual>
    


    <!-- https://github.com/sustainable-processes/ontology/OntoCAPE/model/property_models.owl#WILSON -->

    <owl:NamedIndividual rdf:about="https://github.com/sustainable-processes/ontology/OntoCAPE/model/property_models.owl#WILSON">
        <rdf:type rdf:resource="https://github.com/sustainable-processes/ontology/OntoCAPE/model/property_models.owl#ActivityCoefficientModel"/>
    </owl:NamedIndividual>
</rdf:RDF>



<!-- Generated by the OWL API (version 4.5.26.2023-07-17T20:34:13Z) https://github.com/owlcs/owlapi -->

