<?xml version="1.0"?>
<rdf:RDF xmlns="https://github.com/sustainable-processes/ontology/OntoCAPE/supporting_concepts/physical_dimension/derived_dimensions.owl#"
     xml:base="https://github.com/sustainable-processes/ontology/OntoCAPE/supporting_concepts/physical_dimension/derived_dimensions.owl"
     xmlns:owl="http://www.w3.org/2002/07/owl#"
     xmlns:rdf="http://www.w3.org/1999/02/22-rdf-syntax-ns#"
     xmlns:xml="http://www.w3.org/XML/1998/namespace"
     xmlns:xsd="http://www.w3.org/2001/XMLSchema#"
     xmlns:rdfs="http://www.w3.org/2000/01/rdf-schema#"
     xmlns:maths="https://github.com/sustainable-processes/ontology/OntoCAPE/supporting_concepts/mathematical_relation/mathematical_relation.owl#"
     xmlns:terms="http://purl.org/dc/terms/"
     xmlns:system="https://github.com/sustainable-processes/ontology/OntoCAPE/upper_level/system.owl#"
     xmlns:owl2xml="http://www.w3.org/2006/12/owl2-xml#"
     xmlns:phys_dim="https://github.com/sustainable-processes/ontology/OntoCAPE/supporting_concepts/physical_dimension/physical_dimension.owl#"
     xmlns:binary_tree="https://github.com/sustainable-processes/ontology/meta_model/data_structures/binary_tree.owl#"
     xmlns:derived_dimensions="https://github.com/sustainable-processes/ontology/OntoCAPE/supporting_concepts/physical_dimension/derived_dimensions.owl#">
    <owl:Ontology rdf:about="https://github.com/sustainable-processes/ontology/OntoCAPE/supporting_concepts/physical_dimension/derived_dimensions.owl">
        <owl:imports rdf:resource="https://github.com/sustainable-processes/ontology/OntoCAPE/supporting_concepts/physical_dimension/physical_dimension.owl"/>
        <terms:license>Copyright (C) [2009] [Andreas Wiesner]
                This program is free software; you can redistribute it and/or modify it under the terms of the GNU General Public License as published by the Free Software Foundation; either version 3 of the License, or (at your option) any later version.
                This program is distributed in the hope that it will be useful, but WITHOUT ANY WARRANTY; without even the implied warranty of MERCHANTABILITY or FITNESS FOR A PARTICULAR PURPOSE. See the GNU General Public License for more details.
                You should have received a copy of the GNU General Public License along with this program; if not, see &lt;http://www.gnu.org/licenses/&gt;.
</terms:license>
        <rdfs:comment>The ontology module &apos;derived_dimensions&apos; introduces a number of physical dimensions and their mathematical definitions. 
The following classes, relations, and individuals from other ontology modules are used within &apos;derived_dimensions&apos;:

&lt;owl:Class rdf:about=&quot;https://github.com/sustainable-processes/ontology/OntoCAPE/supporting_concepts/physical_dimension/physical_dimension.owl#DerivedDimension&quot;/&gt;
&lt;owl:Class rdf:about=&quot;https://github.com/sustainable-processes/ontology/OntoCAPE/supporting_concepts/mathematical_relation/mathematical_relation.owl#BinaryOperator&quot;/&gt;
&lt;owl:Class rdf:about=&quot;https://github.com/sustainable-processes/ontology/OntoCAPE/supporting_concepts/mathematical_relation/mathematical_relation.owl#Leaf&quot;/&gt;
&lt;owl:Class rdf:about=&quot;https://github.com/sustainable-processes/ontology/OntoCAPE/supporting_concepts/mathematical_relation/mathematical_relation.owl#Node&quot;/&gt;

&lt;owl:ObjectProperty rdf:about=&quot;https://github.com/sustainable-processes/ontology/OntoCAPE/supporting_concepts/mathematical_relation/mathematical_relation.owl#hasLeftChild&quot;/&gt;
&lt;owl:ObjectProperty rdf:about=&quot;https://github.com/sustainable-processes/ontology/OntoCAPE/supporting_concepts/mathematical_relation/mathematical_relation.owl#hasNodeValue&quot;/&gt;
&lt;owl:ObjectProperty rdf:about=&quot;https://github.com/sustainable-processes/ontology/OntoCAPE/supporting_concepts/mathematical_relation/mathematical_relation.owl#hasRightChild&quot;/&gt;
&lt;owl:ObjectProperty rdf:about=&quot;https://github.com/sustainable-processes/ontology/OntoCAPE/supporting_concepts/mathematical_relation/mathematical_relation.owl#isLeftChildOf&quot;/&gt;
&lt;owl:ObjectProperty rdf:about=&quot;https://github.com/sustainable-processes/ontology/OntoCAPE/supporting_concepts/mathematical_relation/mathematical_relation.owl#isRightChildOf&quot;/&gt;
&lt;owl:ObjectProperty rdf:about=&quot;https://github.com/sustainable-processes/ontology/OntoCAPE/supporting_concepts/mathematical_relation/mathematical_relation.owl#rightChildNodeValue&quot;/&gt;
&lt;owl:ObjectProperty rdf:about=&quot;https://github.com/sustainable-processes/ontology/OntoCAPE/supporting_concepts/physical_dimension/physical_dimension.owl#isDefinedBy&quot;/&gt;

&lt;maths:BinaryOperator rdf:about=&quot;https://github.com/sustainable-processes/ontology/OntoCAPE/supporting_concepts/mathematical_relation/mathematical_relation.owl#divide&quot;/&gt;
&lt;maths:BinaryOperator rdf:about=&quot;https://github.com/sustainable-processes/ontology/OntoCAPE/supporting_concepts/mathematical_relation/mathematical_relation.owl#power&quot;/&gt;
&lt;maths:BinaryOperator rdf:about=&quot;https://github.com/sustainable-processes/ontology/OntoCAPE/supporting_concepts/mathematical_relation/mathematical_relation.owl#times&quot;/&gt;
&lt;maths:Leaf rdf:about=&quot;https://github.com/sustainable-processes/ontology/OntoCAPE/supporting_concepts/physical_dimension/physical_dimension.owl#AMOUNT_OF_SUBSTANCE&quot;/&gt;
&lt;maths:Leaf rdf:about=&quot;https://github.com/sustainable-processes/ontology/OntoCAPE/supporting_concepts/physical_dimension/physical_dimension.owl#ELECTRIC_CURRENT&quot;&gt;
&lt;maths:Leaf rdf:about=&quot;https://github.com/sustainable-processes/ontology/OntoCAPE/supporting_concepts/physical_dimension/physical_dimension.owl#LENGTH&quot;/&gt;
&lt;maths:Leaf rdf:about=&quot;https://github.com/sustainable-processes/ontology/OntoCAPE/supporting_concepts/physical_dimension/physical_dimension.owl#MASS&quot;/&gt;
&lt;maths:Leaf rdf:about=&quot;https://github.com/sustainable-processes/ontology/OntoCAPE/supporting_concepts/physical_dimension/physical_dimension.owl#TIME&quot;&gt;</rdfs:comment>
        <owl:versionInfo>2.0</owl:versionInfo>
    </owl:Ontology>
    


    <!-- 
    ///////////////////////////////////////////////////////////////////////////////////////
    //
    // Object Properties
    //
    ///////////////////////////////////////////////////////////////////////////////////////
     -->

    


    <!-- https://github.com/sustainable-processes/ontology/OntoCAPE/supporting_concepts/mathematical_relation/mathematical_relation.owl#hasLeftChild -->

    <owl:ObjectProperty rdf:about="https://github.com/sustainable-processes/ontology/OntoCAPE/supporting_concepts/mathematical_relation/mathematical_relation.owl#hasLeftChild"/>
    


    <!-- https://github.com/sustainable-processes/ontology/OntoCAPE/supporting_concepts/mathematical_relation/mathematical_relation.owl#hasNodeValue -->

    <owl:ObjectProperty rdf:about="https://github.com/sustainable-processes/ontology/OntoCAPE/supporting_concepts/mathematical_relation/mathematical_relation.owl#hasNodeValue"/>
    


    <!-- https://github.com/sustainable-processes/ontology/OntoCAPE/supporting_concepts/mathematical_relation/mathematical_relation.owl#hasRightChild -->

    <owl:ObjectProperty rdf:about="https://github.com/sustainable-processes/ontology/OntoCAPE/supporting_concepts/mathematical_relation/mathematical_relation.owl#hasRightChild"/>
    


    <!-- https://github.com/sustainable-processes/ontology/OntoCAPE/supporting_concepts/mathematical_relation/mathematical_relation.owl#isLeftChildOf -->

    <owl:ObjectProperty rdf:about="https://github.com/sustainable-processes/ontology/OntoCAPE/supporting_concepts/mathematical_relation/mathematical_relation.owl#isLeftChildOf"/>
    


    <!-- https://github.com/sustainable-processes/ontology/OntoCAPE/supporting_concepts/mathematical_relation/mathematical_relation.owl#isRightChildOf -->

    <owl:ObjectProperty rdf:about="https://github.com/sustainable-processes/ontology/OntoCAPE/supporting_concepts/mathematical_relation/mathematical_relation.owl#isRightChildOf"/>
    


    <!-- https://github.com/sustainable-processes/ontology/OntoCAPE/supporting_concepts/physical_dimension/physical_dimension.owl#isDefinedBy -->

    <owl:ObjectProperty rdf:about="https://github.com/sustainable-processes/ontology/OntoCAPE/supporting_concepts/physical_dimension/physical_dimension.owl#isDefinedBy"/>
    


    <!-- 
    ///////////////////////////////////////////////////////////////////////////////////////
    //
    // Data properties
    //
    ///////////////////////////////////////////////////////////////////////////////////////
     -->

    


    <!-- https://github.com/sustainable-processes/ontology/OntoCAPE/supporting_concepts/mathematical_relation/mathematical_relation.owl#rightChildNodeValue -->

    <owl:DatatypeProperty rdf:about="https://github.com/sustainable-processes/ontology/OntoCAPE/supporting_concepts/mathematical_relation/mathematical_relation.owl#rightChildNodeValue"/>
    


    <!-- 
    ///////////////////////////////////////////////////////////////////////////////////////
    //
    // Classes
    //
    ///////////////////////////////////////////////////////////////////////////////////////
     -->

    


    <!-- https://github.com/sustainable-processes/ontology/OntoCAPE/supporting_concepts/mathematical_relation/mathematical_relation.owl#Node -->

    <owl:Class rdf:about="https://github.com/sustainable-processes/ontology/OntoCAPE/supporting_concepts/mathematical_relation/mathematical_relation.owl#Node"/>
    


    <!-- https://github.com/sustainable-processes/ontology/OntoCAPE/supporting_concepts/physical_dimension/derived_dimensions.owl#ElectricityAndMagnetism -->

    <owl:Class rdf:about="https://github.com/sustainable-processes/ontology/OntoCAPE/supporting_concepts/physical_dimension/derived_dimensions.owl#ElectricityAndMagnetism">
        <rdfs:subClassOf rdf:resource="https://github.com/sustainable-processes/ontology/OntoCAPE/supporting_concepts/physical_dimension/physical_dimension.owl#DerivedDimension"/>
        <owl:disjointWith rdf:resource="https://github.com/sustainable-processes/ontology/OntoCAPE/supporting_concepts/physical_dimension/derived_dimensions.owl#Mechanics"/>
        <owl:disjointWith rdf:resource="https://github.com/sustainable-processes/ontology/OntoCAPE/supporting_concepts/physical_dimension/derived_dimensions.owl#PeriodicPhenomena"/>
        <owl:disjointWith rdf:resource="https://github.com/sustainable-processes/ontology/OntoCAPE/supporting_concepts/physical_dimension/derived_dimensions.owl#SpaceAndTime"/>
        <owl:disjointWith rdf:resource="https://github.com/sustainable-processes/ontology/OntoCAPE/supporting_concepts/physical_dimension/derived_dimensions.owl#Thermodynamics"/>
        <rdfs:comment>The class ElectricityAndMagnetism subsumes DerivedDimensions that are connected with the phenomena of electricity or magnetism.</rdfs:comment>
    </owl:Class>
    


    <!-- https://github.com/sustainable-processes/ontology/OntoCAPE/supporting_concepts/physical_dimension/derived_dimensions.owl#Mechanics -->

    <owl:Class rdf:about="https://github.com/sustainable-processes/ontology/OntoCAPE/supporting_concepts/physical_dimension/derived_dimensions.owl#Mechanics">
        <rdfs:subClassOf rdf:resource="https://github.com/sustainable-processes/ontology/OntoCAPE/supporting_concepts/physical_dimension/physical_dimension.owl#DerivedDimension"/>
        <owl:disjointWith rdf:resource="https://github.com/sustainable-processes/ontology/OntoCAPE/supporting_concepts/physical_dimension/derived_dimensions.owl#PeriodicPhenomena"/>
        <owl:disjointWith rdf:resource="https://github.com/sustainable-processes/ontology/OntoCAPE/supporting_concepts/physical_dimension/derived_dimensions.owl#SpaceAndTime"/>
        <owl:disjointWith rdf:resource="https://github.com/sustainable-processes/ontology/OntoCAPE/supporting_concepts/physical_dimension/derived_dimensions.owl#Thermodynamics"/>
        <rdfs:comment>The class Mechanics subsumes DerivedDimensions that are of relevance for the field of mechanics.</rdfs:comment>
    </owl:Class>
    


    <!-- https://github.com/sustainable-processes/ontology/OntoCAPE/supporting_concepts/physical_dimension/derived_dimensions.owl#PeriodicPhenomena -->

    <owl:Class rdf:about="https://github.com/sustainable-processes/ontology/OntoCAPE/supporting_concepts/physical_dimension/derived_dimensions.owl#PeriodicPhenomena">
        <rdfs:subClassOf rdf:resource="https://github.com/sustainable-processes/ontology/OntoCAPE/supporting_concepts/physical_dimension/physical_dimension.owl#DerivedDimension"/>
        <owl:disjointWith rdf:resource="https://github.com/sustainable-processes/ontology/OntoCAPE/supporting_concepts/physical_dimension/derived_dimensions.owl#SpaceAndTime"/>
        <owl:disjointWith rdf:resource="https://github.com/sustainable-processes/ontology/OntoCAPE/supporting_concepts/physical_dimension/derived_dimensions.owl#Thermodynamics"/>
        <rdfs:comment>The class PeriodicPhenomena subsumes DerivedDimensions with a periodic character, such as frequency or period.</rdfs:comment>
    </owl:Class>
    


    <!-- https://github.com/sustainable-processes/ontology/OntoCAPE/supporting_concepts/physical_dimension/derived_dimensions.owl#SpaceAndTime -->

    <owl:Class rdf:about="https://github.com/sustainable-processes/ontology/OntoCAPE/supporting_concepts/physical_dimension/derived_dimensions.owl#SpaceAndTime">
        <rdfs:subClassOf rdf:resource="https://github.com/sustainable-processes/ontology/OntoCAPE/supporting_concepts/physical_dimension/physical_dimension.owl#DerivedDimension"/>
        <owl:disjointWith rdf:resource="https://github.com/sustainable-processes/ontology/OntoCAPE/supporting_concepts/physical_dimension/derived_dimensions.owl#Thermodynamics"/>
        <rdfs:comment>The class SpaceAndTime subsumes DerivedDimensions that can be derived from the base dimensions length and time.</rdfs:comment>
    </owl:Class>
    


    <!-- https://github.com/sustainable-processes/ontology/OntoCAPE/supporting_concepts/physical_dimension/derived_dimensions.owl#Thermodynamics -->

    <owl:Class rdf:about="https://github.com/sustainable-processes/ontology/OntoCAPE/supporting_concepts/physical_dimension/derived_dimensions.owl#Thermodynamics">
        <rdfs:subClassOf rdf:resource="https://github.com/sustainable-processes/ontology/OntoCAPE/supporting_concepts/physical_dimension/physical_dimension.owl#DerivedDimension"/>
        <rdfs:comment>The class Thermodynamics subsumes DerivedDimensions that are of relevance in the area of heat transfer and thermodynamics.</rdfs:comment>
    </owl:Class>
    


    <!-- https://github.com/sustainable-processes/ontology/OntoCAPE/supporting_concepts/physical_dimension/physical_dimension.owl#DerivedDimension -->

    <owl:Class rdf:about="https://github.com/sustainable-processes/ontology/OntoCAPE/supporting_concepts/physical_dimension/physical_dimension.owl#DerivedDimension"/>
    


    <!-- 
    ///////////////////////////////////////////////////////////////////////////////////////
    //
    // Individuals
    //
    ///////////////////////////////////////////////////////////////////////////////////////
     -->

    


    <!-- https://github.com/sustainable-processes/ontology/OntoCAPE/supporting_concepts/mathematical_relation/mathematical_relation.owl#divide -->

    <owl:NamedIndividual rdf:about="https://github.com/sustainable-processes/ontology/OntoCAPE/supporting_concepts/mathematical_relation/mathematical_relation.owl#divide"/>
    


    <!-- https://github.com/sustainable-processes/ontology/OntoCAPE/supporting_concepts/mathematical_relation/mathematical_relation.owl#power -->

    <owl:NamedIndividual rdf:about="https://github.com/sustainable-processes/ontology/OntoCAPE/supporting_concepts/mathematical_relation/mathematical_relation.owl#power"/>
    


    <!-- https://github.com/sustainable-processes/ontology/OntoCAPE/supporting_concepts/mathematical_relation/mathematical_relation.owl#times -->

    <owl:NamedIndividual rdf:about="https://github.com/sustainable-processes/ontology/OntoCAPE/supporting_concepts/mathematical_relation/mathematical_relation.owl#times"/>
    


    <!-- https://github.com/sustainable-processes/ontology/OntoCAPE/supporting_concepts/physical_dimension/derived_dimensions.owl#ACCELERATION -->

    <owl:NamedIndividual rdf:about="https://github.com/sustainable-processes/ontology/OntoCAPE/supporting_concepts/physical_dimension/derived_dimensions.owl#ACCELERATION">
        <rdf:type rdf:resource="https://github.com/sustainable-processes/ontology/OntoCAPE/supporting_concepts/mathematical_relation/mathematical_relation.owl#Node"/>
        <maths:hasLeftChild rdf:resource="https://github.com/sustainable-processes/ontology/OntoCAPE/supporting_concepts/physical_dimension/derived_dimensions.owl#VELOCITY"/>
        <maths:hasNodeValue rdf:resource="https://github.com/sustainable-processes/ontology/OntoCAPE/supporting_concepts/mathematical_relation/mathematical_relation.owl#divide"/>
        <maths:hasRightChild rdf:resource="https://github.com/sustainable-processes/ontology/OntoCAPE/supporting_concepts/physical_dimension/physical_dimension.owl#TIME"/>
        <rdfs:comment>velocity/time</rdfs:comment>
    </owl:NamedIndividual>
    


    <!-- https://github.com/sustainable-processes/ontology/OntoCAPE/supporting_concepts/physical_dimension/derived_dimensions.owl#AREA -->

    <owl:NamedIndividual rdf:about="https://github.com/sustainable-processes/ontology/OntoCAPE/supporting_concepts/physical_dimension/derived_dimensions.owl#AREA">
        <rdf:type rdf:resource="https://github.com/sustainable-processes/ontology/OntoCAPE/supporting_concepts/mathematical_relation/mathematical_relation.owl#Node"/>
        <maths:hasLeftChild rdf:resource="https://github.com/sustainable-processes/ontology/OntoCAPE/supporting_concepts/physical_dimension/physical_dimension.owl#LENGTH"/>
        <maths:hasNodeValue rdf:resource="https://github.com/sustainable-processes/ontology/OntoCAPE/supporting_concepts/mathematical_relation/mathematical_relation.owl#power"/>
        <maths:rightChildNodeValue rdf:datatype="http://www.w3.org/2001/XMLSchema#decimal">2</maths:rightChildNodeValue>
        <rdfs:comment>length^2</rdfs:comment>
    </owl:NamedIndividual>
    


    <!-- https://github.com/sustainable-processes/ontology/OntoCAPE/supporting_concepts/physical_dimension/derived_dimensions.owl#ELECTRIC_CHARGE -->

    <owl:NamedIndividual rdf:about="https://github.com/sustainable-processes/ontology/OntoCAPE/supporting_concepts/physical_dimension/derived_dimensions.owl#ELECTRIC_CHARGE">
        <rdf:type rdf:resource="https://github.com/sustainable-processes/ontology/OntoCAPE/supporting_concepts/mathematical_relation/mathematical_relation.owl#Node"/>
        <maths:hasLeftChild rdf:resource="https://github.com/sustainable-processes/ontology/OntoCAPE/supporting_concepts/physical_dimension/physical_dimension.owl#ELECTRIC_CURRENT"/>
        <maths:hasNodeValue rdf:resource="https://github.com/sustainable-processes/ontology/OntoCAPE/supporting_concepts/mathematical_relation/mathematical_relation.owl#times"/>
        <maths:hasRightChild rdf:resource="https://github.com/sustainable-processes/ontology/OntoCAPE/supporting_concepts/physical_dimension/physical_dimension.owl#TIME"/>
    </owl:NamedIndividual>
    


    <!-- https://github.com/sustainable-processes/ontology/OntoCAPE/supporting_concepts/physical_dimension/derived_dimensions.owl#MOLAR_VOLUME -->

    <owl:NamedIndividual rdf:about="https://github.com/sustainable-processes/ontology/OntoCAPE/supporting_concepts/physical_dimension/derived_dimensions.owl#MOLAR_VOLUME">
        <rdf:type rdf:resource="https://github.com/sustainable-processes/ontology/OntoCAPE/supporting_concepts/mathematical_relation/mathematical_relation.owl#Node"/>
        <maths:hasLeftChild rdf:resource="https://github.com/sustainable-processes/ontology/OntoCAPE/supporting_concepts/physical_dimension/derived_dimensions.owl#VOLUME"/>
        <maths:hasNodeValue rdf:resource="https://github.com/sustainable-processes/ontology/OntoCAPE/supporting_concepts/mathematical_relation/mathematical_relation.owl#divide"/>
        <maths:hasRightChild rdf:resource="https://github.com/sustainable-processes/ontology/OntoCAPE/supporting_concepts/physical_dimension/physical_dimension.owl#AMOUNT_OF_SUBSTANCE"/>
        <rdfs:comment>volume/amount_of_substance</rdfs:comment>
    </owl:NamedIndividual>
    


    <!-- https://github.com/sustainable-processes/ontology/OntoCAPE/supporting_concepts/physical_dimension/derived_dimensions.owl#MOLECULAR_MASS -->

    <owl:NamedIndividual rdf:about="https://github.com/sustainable-processes/ontology/OntoCAPE/supporting_concepts/physical_dimension/derived_dimensions.owl#MOLECULAR_MASS">
        <rdf:type rdf:resource="https://github.com/sustainable-processes/ontology/OntoCAPE/supporting_concepts/mathematical_relation/mathematical_relation.owl#Node"/>
        <maths:hasLeftChild rdf:resource="https://github.com/sustainable-processes/ontology/OntoCAPE/supporting_concepts/physical_dimension/physical_dimension.owl#MASS"/>
        <maths:hasNodeValue rdf:resource="https://github.com/sustainable-processes/ontology/OntoCAPE/supporting_concepts/mathematical_relation/mathematical_relation.owl#divide"/>
        <maths:hasRightChild rdf:resource="https://github.com/sustainable-processes/ontology/OntoCAPE/supporting_concepts/physical_dimension/physical_dimension.owl#AMOUNT_OF_SUBSTANCE"/>
        <rdfs:comment>mass/amount_of_substance</rdfs:comment>
    </owl:NamedIndividual>
    


    <!-- https://github.com/sustainable-processes/ontology/OntoCAPE/supporting_concepts/physical_dimension/derived_dimensions.owl#VELOCITY -->

    <owl:NamedIndividual rdf:about="https://github.com/sustainable-processes/ontology/OntoCAPE/supporting_concepts/physical_dimension/derived_dimensions.owl#VELOCITY">
        <rdf:type rdf:resource="https://github.com/sustainable-processes/ontology/OntoCAPE/supporting_concepts/mathematical_relation/mathematical_relation.owl#Node"/>
        <maths:hasLeftChild rdf:resource="https://github.com/sustainable-processes/ontology/OntoCAPE/supporting_concepts/physical_dimension/physical_dimension.owl#LENGTH"/>
        <maths:hasNodeValue rdf:resource="https://github.com/sustainable-processes/ontology/OntoCAPE/supporting_concepts/mathematical_relation/mathematical_relation.owl#divide"/>
        <maths:hasRightChild rdf:resource="https://github.com/sustainable-processes/ontology/OntoCAPE/supporting_concepts/physical_dimension/physical_dimension.owl#TIME"/>
        <rdfs:comment>length/time</rdfs:comment>
    </owl:NamedIndividual>
    


    <!-- https://github.com/sustainable-processes/ontology/OntoCAPE/supporting_concepts/physical_dimension/derived_dimensions.owl#VOLUME -->

    <owl:NamedIndividual rdf:about="https://github.com/sustainable-processes/ontology/OntoCAPE/supporting_concepts/physical_dimension/derived_dimensions.owl#VOLUME">
        <rdf:type rdf:resource="https://github.com/sustainable-processes/ontology/OntoCAPE/supporting_concepts/mathematical_relation/mathematical_relation.owl#Node"/>
        <maths:hasLeftChild rdf:resource="https://github.com/sustainable-processes/ontology/OntoCAPE/supporting_concepts/physical_dimension/physical_dimension.owl#LENGTH"/>
        <maths:hasNodeValue rdf:resource="https://github.com/sustainable-processes/ontology/OntoCAPE/supporting_concepts/mathematical_relation/mathematical_relation.owl#power"/>
        <maths:isLeftChildOf rdf:resource="https://github.com/sustainable-processes/ontology/OntoCAPE/supporting_concepts/physical_dimension/derived_dimensions.owl#MOLAR_VOLUME"/>
        <maths:rightChildNodeValue rdf:datatype="http://www.w3.org/2001/XMLSchema#decimal">3</maths:rightChildNodeValue>
        <rdfs:comment>length^3</rdfs:comment>
    </owl:NamedIndividual>
    


    <!-- https://github.com/sustainable-processes/ontology/OntoCAPE/supporting_concepts/physical_dimension/derived_dimensions.owl#acceleration -->

    <owl:NamedIndividual rdf:about="https://github.com/sustainable-processes/ontology/OntoCAPE/supporting_concepts/physical_dimension/derived_dimensions.owl#acceleration">
        <rdf:type rdf:resource="https://github.com/sustainable-processes/ontology/OntoCAPE/supporting_concepts/physical_dimension/derived_dimensions.owl#SpaceAndTime"/>
        <phys_dim:isDefinedBy rdf:resource="https://github.com/sustainable-processes/ontology/OntoCAPE/supporting_concepts/physical_dimension/derived_dimensions.owl#ACCELERATION"/>
        <phys_dim:isDefinedBy rdf:resource="https://github.com/sustainable-processes/ontology/OntoCAPE/supporting_concepts/physical_dimension/derived_dimensions.owl#AREA"/>
        <rdfs:comment>the first time derivative from velocity [Chertov, 1997]</rdfs:comment>
    </owl:NamedIndividual>
    


    <!-- https://github.com/sustainable-processes/ontology/OntoCAPE/supporting_concepts/physical_dimension/derived_dimensions.owl#angular_acceleration -->

    <owl:NamedIndividual rdf:about="https://github.com/sustainable-processes/ontology/OntoCAPE/supporting_concepts/physical_dimension/derived_dimensions.owl#angular_acceleration">
        <rdf:type rdf:resource="https://github.com/sustainable-processes/ontology/OntoCAPE/supporting_concepts/physical_dimension/derived_dimensions.owl#SpaceAndTime"/>
        <rdfs:comment>the first time derivative from the angular velocity [Chertov, 1997]</rdfs:comment>
    </owl:NamedIndividual>
    


    <!-- https://github.com/sustainable-processes/ontology/OntoCAPE/supporting_concepts/physical_dimension/derived_dimensions.owl#angular_velocity -->

    <owl:NamedIndividual rdf:about="https://github.com/sustainable-processes/ontology/OntoCAPE/supporting_concepts/physical_dimension/derived_dimensions.owl#angular_velocity">
        <rdf:type rdf:resource="https://github.com/sustainable-processes/ontology/OntoCAPE/supporting_concepts/physical_dimension/derived_dimensions.owl#SpaceAndTime"/>
        <rdfs:comment>the first time derivative from the deflection angle [Chertov, 1997]</rdfs:comment>
    </owl:NamedIndividual>
    


    <!-- https://github.com/sustainable-processes/ontology/OntoCAPE/supporting_concepts/physical_dimension/derived_dimensions.owl#area -->

    <owl:NamedIndividual rdf:about="https://github.com/sustainable-processes/ontology/OntoCAPE/supporting_concepts/physical_dimension/derived_dimensions.owl#area">
        <rdf:type rdf:resource="https://github.com/sustainable-processes/ontology/OntoCAPE/supporting_concepts/physical_dimension/derived_dimensions.owl#SpaceAndTime"/>
        <phys_dim:isDefinedBy rdf:resource="https://github.com/sustainable-processes/ontology/OntoCAPE/supporting_concepts/physical_dimension/derived_dimensions.owl#AREA"/>
        <rdfs:comment>characterizes the plane and curved surfaces of a physical body [Chertov, 1997]</rdfs:comment>
    </owl:NamedIndividual>
    


    <!-- https://github.com/sustainable-processes/ontology/OntoCAPE/supporting_concepts/physical_dimension/derived_dimensions.owl#damping_coefficient -->

    <owl:NamedIndividual rdf:about="https://github.com/sustainable-processes/ontology/OntoCAPE/supporting_concepts/physical_dimension/derived_dimensions.owl#damping_coefficient">
        <rdf:type rdf:resource="https://github.com/sustainable-processes/ontology/OntoCAPE/supporting_concepts/physical_dimension/derived_dimensions.owl#PeriodicPhenomena"/>
        <rdfs:comment>the inverse to the time interval during which the amplitude decrease e times [Chertov, 1997]</rdfs:comment>
    </owl:NamedIndividual>
    


    <!-- https://github.com/sustainable-processes/ontology/OntoCAPE/supporting_concepts/physical_dimension/derived_dimensions.owl#density -->

    <owl:NamedIndividual rdf:about="https://github.com/sustainable-processes/ontology/OntoCAPE/supporting_concepts/physical_dimension/derived_dimensions.owl#density">
        <rdf:type rdf:resource="https://github.com/sustainable-processes/ontology/OntoCAPE/supporting_concepts/physical_dimension/derived_dimensions.owl#Mechanics"/>
        <rdfs:comment>the ratio of the mass to the volume of a body´s element [Chertov, 1997]</rdfs:comment>
    </owl:NamedIndividual>
    


    <!-- https://github.com/sustainable-processes/ontology/OntoCAPE/supporting_concepts/physical_dimension/derived_dimensions.owl#dynamic_viscosity -->

    <owl:NamedIndividual rdf:about="https://github.com/sustainable-processes/ontology/OntoCAPE/supporting_concepts/physical_dimension/derived_dimensions.owl#dynamic_viscosity">
        <rdf:type rdf:resource="https://github.com/sustainable-processes/ontology/OntoCAPE/supporting_concepts/physical_dimension/derived_dimensions.owl#Mechanics"/>
        <rdfs:comment>the coefficient of proportinality in the internal friction force formula [Chertov, 1997]</rdfs:comment>
    </owl:NamedIndividual>
    


    <!-- https://github.com/sustainable-processes/ontology/OntoCAPE/supporting_concepts/physical_dimension/derived_dimensions.owl#electric_charge -->

    <owl:NamedIndividual rdf:about="https://github.com/sustainable-processes/ontology/OntoCAPE/supporting_concepts/physical_dimension/derived_dimensions.owl#electric_charge">
        <rdf:type rdf:resource="https://github.com/sustainable-processes/ontology/OntoCAPE/supporting_concepts/physical_dimension/derived_dimensions.owl#ElectricityAndMagnetism"/>
        <phys_dim:isDefinedBy rdf:resource="https://github.com/sustainable-processes/ontology/OntoCAPE/supporting_concepts/physical_dimension/derived_dimensions.owl#ELECTRIC_CHARGE"/>
        <rdfs:comment>The measure equal to the product of electic current into time during which the current flows [Chertov]</rdfs:comment>
    </owl:NamedIndividual>
    


    <!-- https://github.com/sustainable-processes/ontology/OntoCAPE/supporting_concepts/physical_dimension/derived_dimensions.owl#entropy -->

    <owl:NamedIndividual rdf:about="https://github.com/sustainable-processes/ontology/OntoCAPE/supporting_concepts/physical_dimension/derived_dimensions.owl#entropy">
        <rdf:type rdf:resource="https://github.com/sustainable-processes/ontology/OntoCAPE/supporting_concepts/physical_dimension/derived_dimensions.owl#Thermodynamics"/>
        <rdfs:comment>the ratio of an infinitely small quantity of heat transmitted to a system to the temperature [Chertov, 1997]</rdfs:comment>
    </owl:NamedIndividual>
    


    <!-- https://github.com/sustainable-processes/ontology/OntoCAPE/supporting_concepts/physical_dimension/derived_dimensions.owl#force -->

    <owl:NamedIndividual rdf:about="https://github.com/sustainable-processes/ontology/OntoCAPE/supporting_concepts/physical_dimension/derived_dimensions.owl#force">
        <rdf:type rdf:resource="https://github.com/sustainable-processes/ontology/OntoCAPE/supporting_concepts/physical_dimension/derived_dimensions.owl#Mechanics"/>
        <rdfs:comment>the degree of mechanical influence exerted on a body by other bodies [Chertov, 1997]</rdfs:comment>
    </owl:NamedIndividual>
    


    <!-- https://github.com/sustainable-processes/ontology/OntoCAPE/supporting_concepts/physical_dimension/derived_dimensions.owl#frequency -->

    <owl:NamedIndividual rdf:about="https://github.com/sustainable-processes/ontology/OntoCAPE/supporting_concepts/physical_dimension/derived_dimensions.owl#frequency">
        <rdf:type rdf:resource="https://github.com/sustainable-processes/ontology/OntoCAPE/supporting_concepts/physical_dimension/derived_dimensions.owl#PeriodicPhenomena"/>
        <rdfs:comment>the inverse to the period [Chertov, 1997]</rdfs:comment>
    </owl:NamedIndividual>
    


    <!-- https://github.com/sustainable-processes/ontology/OntoCAPE/supporting_concepts/physical_dimension/derived_dimensions.owl#heat_capacity -->

    <owl:NamedIndividual rdf:about="https://github.com/sustainable-processes/ontology/OntoCAPE/supporting_concepts/physical_dimension/derived_dimensions.owl#heat_capacity">
        <rdf:type rdf:resource="https://github.com/sustainable-processes/ontology/OntoCAPE/supporting_concepts/physical_dimension/derived_dimensions.owl#Thermodynamics"/>
        <rdfs:comment>the ratio of heat required to warm a physical body to the difference in temperature [Chertov, 1997]</rdfs:comment>
    </owl:NamedIndividual>
    


    <!-- https://github.com/sustainable-processes/ontology/OntoCAPE/supporting_concepts/physical_dimension/derived_dimensions.owl#heat_flow_rate -->

    <owl:NamedIndividual rdf:about="https://github.com/sustainable-processes/ontology/OntoCAPE/supporting_concepts/physical_dimension/derived_dimensions.owl#heat_flow_rate">
        <rdf:type rdf:resource="https://github.com/sustainable-processes/ontology/OntoCAPE/supporting_concepts/physical_dimension/derived_dimensions.owl#Thermodynamics"/>
        <rdfs:comment>the ratio of the quantity of heat which passes a surface to time [Chertov, 1997]</rdfs:comment>
    </owl:NamedIndividual>
    


    <!-- https://github.com/sustainable-processes/ontology/OntoCAPE/supporting_concepts/physical_dimension/derived_dimensions.owl#internal_energy -->

    <owl:NamedIndividual rdf:about="https://github.com/sustainable-processes/ontology/OntoCAPE/supporting_concepts/physical_dimension/derived_dimensions.owl#internal_energy">
        <rdf:type rdf:resource="https://github.com/sustainable-processes/ontology/OntoCAPE/supporting_concepts/physical_dimension/derived_dimensions.owl#Thermodynamics"/>
        <rdfs:comment>the energy from the random thermal movement of all microparticles in a system [Chertov, 1997]</rdfs:comment>
    </owl:NamedIndividual>
    


    <!-- https://github.com/sustainable-processes/ontology/OntoCAPE/supporting_concepts/physical_dimension/derived_dimensions.owl#kinematic_viscosity -->

    <owl:NamedIndividual rdf:about="https://github.com/sustainable-processes/ontology/OntoCAPE/supporting_concepts/physical_dimension/derived_dimensions.owl#kinematic_viscosity">
        <rdf:type rdf:resource="https://github.com/sustainable-processes/ontology/OntoCAPE/supporting_concepts/physical_dimension/derived_dimensions.owl#Mechanics"/>
        <rdfs:comment>the ratio of the dynamic viscosity of a medium to its density [Chertov, 1997]</rdfs:comment>
    </owl:NamedIndividual>
    


    <!-- https://github.com/sustainable-processes/ontology/OntoCAPE/supporting_concepts/physical_dimension/derived_dimensions.owl#mass_fraction -->

    <owl:NamedIndividual rdf:about="https://github.com/sustainable-processes/ontology/OntoCAPE/supporting_concepts/physical_dimension/derived_dimensions.owl#mass_fraction">
        <rdf:type rdf:resource="https://github.com/sustainable-processes/ontology/OntoCAPE/supporting_concepts/physical_dimension/physical_dimension.owl#DerivedDimension"/>
        <rdfs:comment>The mass of some particular substance per total mass</rdfs:comment>
    </owl:NamedIndividual>
    


    <!-- https://github.com/sustainable-processes/ontology/OntoCAPE/supporting_concepts/physical_dimension/derived_dimensions.owl#molar_fraction -->

    <owl:NamedIndividual rdf:about="https://github.com/sustainable-processes/ontology/OntoCAPE/supporting_concepts/physical_dimension/derived_dimensions.owl#molar_fraction">
        <rdf:type rdf:resource="https://github.com/sustainable-processes/ontology/OntoCAPE/supporting_concepts/physical_dimension/physical_dimension.owl#DerivedDimension"/>
        <rdfs:comment>The amount of some particular substance per total amount of substance</rdfs:comment>
    </owl:NamedIndividual>
    


    <!-- https://github.com/sustainable-processes/ontology/OntoCAPE/supporting_concepts/physical_dimension/derived_dimensions.owl#molar_volume -->

    <owl:NamedIndividual rdf:about="https://github.com/sustainable-processes/ontology/OntoCAPE/supporting_concepts/physical_dimension/derived_dimensions.owl#molar_volume">
        <rdf:type rdf:resource="https://github.com/sustainable-processes/ontology/OntoCAPE/supporting_concepts/physical_dimension/physical_dimension.owl#DerivedDimension"/>
        <phys_dim:isDefinedBy rdf:resource="https://github.com/sustainable-processes/ontology/OntoCAPE/supporting_concepts/physical_dimension/derived_dimensions.owl#MOLAR_VOLUME"/>
        <rdfs:comment>the volume of one mole of material</rdfs:comment>
    </owl:NamedIndividual>
    


    <!-- https://github.com/sustainable-processes/ontology/OntoCAPE/supporting_concepts/physical_dimension/derived_dimensions.owl#molecular_mass -->

    <owl:NamedIndividual rdf:about="https://github.com/sustainable-processes/ontology/OntoCAPE/supporting_concepts/physical_dimension/derived_dimensions.owl#molecular_mass">
        <rdf:type rdf:resource="https://github.com/sustainable-processes/ontology/OntoCAPE/supporting_concepts/physical_dimension/physical_dimension.owl#DerivedDimension"/>
        <phys_dim:isDefinedBy rdf:resource="https://github.com/sustainable-processes/ontology/OntoCAPE/supporting_concepts/physical_dimension/derived_dimensions.owl#MOLECULAR_MASS"/>
        <rdfs:comment>The molecular mass of a substance (less accurately called molecular weight) is the mass of one molecule of that substance, relative to the unified atomic mass unit u (equal to 1/12 the mass of one atom of carbon-12). [Wikipedia]</rdfs:comment>
    </owl:NamedIndividual>
    


    <!-- https://github.com/sustainable-processes/ontology/OntoCAPE/supporting_concepts/physical_dimension/derived_dimensions.owl#moment_of_force -->

    <owl:NamedIndividual rdf:about="https://github.com/sustainable-processes/ontology/OntoCAPE/supporting_concepts/physical_dimension/derived_dimensions.owl#moment_of_force">
        <rdf:type rdf:resource="https://github.com/sustainable-processes/ontology/OntoCAPE/supporting_concepts/physical_dimension/derived_dimensions.owl#Mechanics"/>
        <rdfs:comment>in relation to a certain point, the product of the force and the arm, i.e. the distance between the direction of the force and the point [Chertov, 1997]</rdfs:comment>
    </owl:NamedIndividual>
    


    <!-- https://github.com/sustainable-processes/ontology/OntoCAPE/supporting_concepts/physical_dimension/derived_dimensions.owl#moment_of_inertia -->

    <owl:NamedIndividual rdf:about="https://github.com/sustainable-processes/ontology/OntoCAPE/supporting_concepts/physical_dimension/derived_dimensions.owl#moment_of_inertia">
        <rdf:type rdf:resource="https://github.com/sustainable-processes/ontology/OntoCAPE/supporting_concepts/physical_dimension/derived_dimensions.owl#Mechanics"/>
        <rdfs:comment>the mass of a material point per square distance to the axis of rotation [Chertov, 1997]</rdfs:comment>
    </owl:NamedIndividual>
    


    <!-- https://github.com/sustainable-processes/ontology/OntoCAPE/supporting_concepts/physical_dimension/derived_dimensions.owl#momentum -->

    <owl:NamedIndividual rdf:about="https://github.com/sustainable-processes/ontology/OntoCAPE/supporting_concepts/physical_dimension/derived_dimensions.owl#momentum">
        <rdf:type rdf:resource="https://github.com/sustainable-processes/ontology/OntoCAPE/supporting_concepts/physical_dimension/derived_dimensions.owl#Mechanics"/>
        <rdfs:comment>the mass of a physical body at its velocity [Chertov, 1997]</rdfs:comment>
    </owl:NamedIndividual>
    


    <!-- https://github.com/sustainable-processes/ontology/OntoCAPE/supporting_concepts/physical_dimension/derived_dimensions.owl#oscillation_phase -->

    <owl:NamedIndividual rdf:about="https://github.com/sustainable-processes/ontology/OntoCAPE/supporting_concepts/physical_dimension/derived_dimensions.owl#oscillation_phase">
        <rdf:type rdf:resource="https://github.com/sustainable-processes/ontology/OntoCAPE/supporting_concepts/physical_dimension/derived_dimensions.owl#PeriodicPhenomena"/>
        <rdfs:comment>independent variable of a function describing the quantity which changes according the law of harmonic vibrations [Chertov, 1997]</rdfs:comment>
    </owl:NamedIndividual>
    


    <!-- https://github.com/sustainable-processes/ontology/OntoCAPE/supporting_concepts/physical_dimension/derived_dimensions.owl#period -->

    <owl:NamedIndividual rdf:about="https://github.com/sustainable-processes/ontology/OntoCAPE/supporting_concepts/physical_dimension/derived_dimensions.owl#period">
        <rdf:type rdf:resource="https://github.com/sustainable-processes/ontology/OntoCAPE/supporting_concepts/physical_dimension/derived_dimensions.owl#PeriodicPhenomena"/>
        <rdfs:comment>the time interval during which a cycle of periodic process is completed [Chertov, 1997]</rdfs:comment>
    </owl:NamedIndividual>
    


    <!-- https://github.com/sustainable-processes/ontology/OntoCAPE/supporting_concepts/physical_dimension/derived_dimensions.owl#plane_angle -->

    <owl:NamedIndividual rdf:about="https://github.com/sustainable-processes/ontology/OntoCAPE/supporting_concepts/physical_dimension/derived_dimensions.owl#plane_angle">
        <rdf:type rdf:resource="https://github.com/sustainable-processes/ontology/OntoCAPE/supporting_concepts/physical_dimension/derived_dimensions.owl#SpaceAndTime"/>
        <rdfs:comment>geometric figure formed by two rays (sides of the angle) extending from one point [Chertov, 1997]</rdfs:comment>
    </owl:NamedIndividual>
    


    <!-- https://github.com/sustainable-processes/ontology/OntoCAPE/supporting_concepts/physical_dimension/derived_dimensions.owl#power -->

    <owl:NamedIndividual rdf:about="https://github.com/sustainable-processes/ontology/OntoCAPE/supporting_concepts/physical_dimension/derived_dimensions.owl#power">
        <rdf:type rdf:resource="https://github.com/sustainable-processes/ontology/OntoCAPE/supporting_concepts/physical_dimension/derived_dimensions.owl#Mechanics"/>
        <rdfs:comment>the ratio of work to time interval during which the work is completed [Chertov, 1997]</rdfs:comment>
    </owl:NamedIndividual>
    


    <!-- https://github.com/sustainable-processes/ontology/OntoCAPE/supporting_concepts/physical_dimension/derived_dimensions.owl#pressure -->

    <owl:NamedIndividual rdf:about="https://github.com/sustainable-processes/ontology/OntoCAPE/supporting_concepts/physical_dimension/derived_dimensions.owl#pressure">
        <rdf:type rdf:resource="https://github.com/sustainable-processes/ontology/OntoCAPE/supporting_concepts/physical_dimension/derived_dimensions.owl#Mechanics"/>
        <rdfs:comment>the ratio between the perpendicular force acting on a surface element to the area of the element [Chertov, 1997]</rdfs:comment>
    </owl:NamedIndividual>
    


    <!-- https://github.com/sustainable-processes/ontology/OntoCAPE/supporting_concepts/physical_dimension/derived_dimensions.owl#quantity_of_heat -->

    <owl:NamedIndividual rdf:about="https://github.com/sustainable-processes/ontology/OntoCAPE/supporting_concepts/physical_dimension/derived_dimensions.owl#quantity_of_heat">
        <rdf:type rdf:resource="https://github.com/sustainable-processes/ontology/OntoCAPE/supporting_concepts/physical_dimension/derived_dimensions.owl#Thermodynamics"/>
        <rdfs:comment>the part of internal energy which is transferred spontaneously, with no external influence from more to less heated physical body [Chertov, 1997]</rdfs:comment>
    </owl:NamedIndividual>
    


    <!-- https://github.com/sustainable-processes/ontology/OntoCAPE/supporting_concepts/physical_dimension/derived_dimensions.owl#rotational_frequency -->

    <owl:NamedIndividual rdf:about="https://github.com/sustainable-processes/ontology/OntoCAPE/supporting_concepts/physical_dimension/derived_dimensions.owl#rotational_frequency">
        <rdf:type rdf:resource="https://github.com/sustainable-processes/ontology/OntoCAPE/supporting_concepts/physical_dimension/derived_dimensions.owl#PeriodicPhenomena"/>
        <rdfs:comment>the number of rotations completed in a second [Chertov, 1997]</rdfs:comment>
    </owl:NamedIndividual>
    


    <!-- https://github.com/sustainable-processes/ontology/OntoCAPE/supporting_concepts/physical_dimension/derived_dimensions.owl#solid_angle -->

    <owl:NamedIndividual rdf:about="https://github.com/sustainable-processes/ontology/OntoCAPE/supporting_concepts/physical_dimension/derived_dimensions.owl#solid_angle">
        <rdf:type rdf:resource="https://github.com/sustainable-processes/ontology/OntoCAPE/supporting_concepts/physical_dimension/derived_dimensions.owl#SpaceAndTime"/>
        <rdfs:comment>the part of space enclosed within one cavity of conical surface with a closed directrix [Chertov, 1997]</rdfs:comment>
    </owl:NamedIndividual>
    


    <!-- https://github.com/sustainable-processes/ontology/OntoCAPE/supporting_concepts/physical_dimension/derived_dimensions.owl#specific_entropy -->

    <owl:NamedIndividual rdf:about="https://github.com/sustainable-processes/ontology/OntoCAPE/supporting_concepts/physical_dimension/derived_dimensions.owl#specific_entropy">
        <rdf:type rdf:resource="https://github.com/sustainable-processes/ontology/OntoCAPE/supporting_concepts/physical_dimension/derived_dimensions.owl#Thermodynamics"/>
        <rdfs:comment>the ratio of entropy to the mass of a system [Chertov, 1997]</rdfs:comment>
    </owl:NamedIndividual>
    


    <!-- https://github.com/sustainable-processes/ontology/OntoCAPE/supporting_concepts/physical_dimension/derived_dimensions.owl#specific_heat_capacity -->

    <owl:NamedIndividual rdf:about="https://github.com/sustainable-processes/ontology/OntoCAPE/supporting_concepts/physical_dimension/derived_dimensions.owl#specific_heat_capacity">
        <rdf:type rdf:resource="https://github.com/sustainable-processes/ontology/OntoCAPE/supporting_concepts/physical_dimension/derived_dimensions.owl#Thermodynamics"/>
        <rdfs:comment>the ratio of the heat capacity of a uniform physical body to its mass [Chertov, 1997]</rdfs:comment>
    </owl:NamedIndividual>
    


    <!-- https://github.com/sustainable-processes/ontology/OntoCAPE/supporting_concepts/physical_dimension/derived_dimensions.owl#specific_volume -->

    <owl:NamedIndividual rdf:about="https://github.com/sustainable-processes/ontology/OntoCAPE/supporting_concepts/physical_dimension/derived_dimensions.owl#specific_volume">
        <rdf:type rdf:resource="https://github.com/sustainable-processes/ontology/OntoCAPE/supporting_concepts/physical_dimension/derived_dimensions.owl#Mechanics"/>
        <rdfs:comment>the ratio of the volume to the mass of a body´s element [Chertov, 1997]</rdfs:comment>
    </owl:NamedIndividual>
    


    <!-- https://github.com/sustainable-processes/ontology/OntoCAPE/supporting_concepts/physical_dimension/derived_dimensions.owl#surface_tension -->

    <owl:NamedIndividual rdf:about="https://github.com/sustainable-processes/ontology/OntoCAPE/supporting_concepts/physical_dimension/derived_dimensions.owl#surface_tension">
        <rdf:type rdf:resource="https://github.com/sustainable-processes/ontology/OntoCAPE/supporting_concepts/physical_dimension/derived_dimensions.owl#Mechanics"/>
        <rdfs:comment>the ratio of between the force, acting on a segment of the free surface contour perpendicular to the contour and tangentially to the surface, and the length of the segment [Chertov, 1997]</rdfs:comment>
    </owl:NamedIndividual>
    


    <!-- https://github.com/sustainable-processes/ontology/OntoCAPE/supporting_concepts/physical_dimension/derived_dimensions.owl#temperature_coefficient -->

    <owl:NamedIndividual rdf:about="https://github.com/sustainable-processes/ontology/OntoCAPE/supporting_concepts/physical_dimension/derived_dimensions.owl#temperature_coefficient">
        <rdf:type rdf:resource="https://github.com/sustainable-processes/ontology/OntoCAPE/supporting_concepts/physical_dimension/derived_dimensions.owl#Thermodynamics"/>
        <rdfs:comment>the ratio of the relative change in a physical quantity to the temperature change reckoned from the initial temperature [Chertov, 1997]</rdfs:comment>
    </owl:NamedIndividual>
    


    <!-- https://github.com/sustainable-processes/ontology/OntoCAPE/supporting_concepts/physical_dimension/derived_dimensions.owl#thermal_conductivity -->

    <owl:NamedIndividual rdf:about="https://github.com/sustainable-processes/ontology/OntoCAPE/supporting_concepts/physical_dimension/derived_dimensions.owl#thermal_conductivity">
        <rdf:type rdf:resource="https://github.com/sustainable-processes/ontology/OntoCAPE/supporting_concepts/physical_dimension/derived_dimensions.owl#Thermodynamics"/>
        <rdfs:comment>the density of heat flux produced by heat conductivity at temperature gradient [Chertov, 1997]</rdfs:comment>
    </owl:NamedIndividual>
    


    <!-- https://github.com/sustainable-processes/ontology/OntoCAPE/supporting_concepts/physical_dimension/derived_dimensions.owl#velocity -->

    <owl:NamedIndividual rdf:about="https://github.com/sustainable-processes/ontology/OntoCAPE/supporting_concepts/physical_dimension/derived_dimensions.owl#velocity">
        <rdf:type rdf:resource="https://github.com/sustainable-processes/ontology/OntoCAPE/supporting_concepts/physical_dimension/derived_dimensions.owl#SpaceAndTime"/>
        <phys_dim:isDefinedBy rdf:resource="https://github.com/sustainable-processes/ontology/OntoCAPE/supporting_concepts/physical_dimension/derived_dimensions.owl#VELOCITY"/>
        <rdfs:comment>the first time derivative from movement [Chertov, 1997]</rdfs:comment>
    </owl:NamedIndividual>
    


    <!-- https://github.com/sustainable-processes/ontology/OntoCAPE/supporting_concepts/physical_dimension/derived_dimensions.owl#volume -->

    <owl:NamedIndividual rdf:about="https://github.com/sustainable-processes/ontology/OntoCAPE/supporting_concepts/physical_dimension/derived_dimensions.owl#volume">
        <rdf:type rdf:resource="https://github.com/sustainable-processes/ontology/OntoCAPE/supporting_concepts/physical_dimension/derived_dimensions.owl#SpaceAndTime"/>
        <phys_dim:isDefinedBy rdf:resource="https://github.com/sustainable-processes/ontology/OntoCAPE/supporting_concepts/physical_dimension/derived_dimensions.owl#VOLUME"/>
        <rdfs:comment>characterizes physical bodies [Chertov, 1997]</rdfs:comment>
    </owl:NamedIndividual>
    


    <!-- https://github.com/sustainable-processes/ontology/OntoCAPE/supporting_concepts/physical_dimension/derived_dimensions.owl#volume_fraction -->

    <owl:NamedIndividual rdf:about="https://github.com/sustainable-processes/ontology/OntoCAPE/supporting_concepts/physical_dimension/derived_dimensions.owl#volume_fraction">
        <rdf:type rdf:resource="https://github.com/sustainable-processes/ontology/OntoCAPE/supporting_concepts/physical_dimension/physical_dimension.owl#DerivedDimension"/>
        <rdfs:comment>The volume of some particular substance per total volume</rdfs:comment>
    </owl:NamedIndividual>
    


    <!-- https://github.com/sustainable-processes/ontology/OntoCAPE/supporting_concepts/physical_dimension/derived_dimensions.owl#work -->

    <owl:NamedIndividual rdf:about="https://github.com/sustainable-processes/ontology/OntoCAPE/supporting_concepts/physical_dimension/derived_dimensions.owl#work">
        <rdf:type rdf:resource="https://github.com/sustainable-processes/ontology/OntoCAPE/supporting_concepts/physical_dimension/derived_dimensions.owl#Mechanics"/>
        <rdfs:comment>the scalar product of force into an elementary displacement [Chertov, 1997]</rdfs:comment>
    </owl:NamedIndividual>
    


    <!-- https://github.com/sustainable-processes/ontology/OntoCAPE/supporting_concepts/physical_dimension/physical_dimension.owl#ELECTRIC_CURRENT -->

    <rdf:Description rdf:about="https://github.com/sustainable-processes/ontology/OntoCAPE/supporting_concepts/physical_dimension/physical_dimension.owl#ELECTRIC_CURRENT">
        <maths:isLeftChildOf rdf:resource="https://github.com/sustainable-processes/ontology/OntoCAPE/supporting_concepts/physical_dimension/derived_dimensions.owl#ELECTRIC_CHARGE"/>
    </rdf:Description>
    


    <!-- https://github.com/sustainable-processes/ontology/OntoCAPE/supporting_concepts/physical_dimension/physical_dimension.owl#TIME -->

    <rdf:Description rdf:about="https://github.com/sustainable-processes/ontology/OntoCAPE/supporting_concepts/physical_dimension/physical_dimension.owl#TIME">
        <maths:isRightChildOf rdf:resource="https://github.com/sustainable-processes/ontology/OntoCAPE/supporting_concepts/physical_dimension/derived_dimensions.owl#ELECTRIC_CHARGE"/>
    </rdf:Description>
    


    <!-- 
    ///////////////////////////////////////////////////////////////////////////////////////
    //
    // General axioms
    //
    ///////////////////////////////////////////////////////////////////////////////////////
     -->

    <rdf:Description>
        <rdf:type rdf:resource="http://www.w3.org/2002/07/owl#AllDifferent"/>
        <owl:distinctMembers rdf:parseType="Collection">
            <rdf:Description rdf:about="https://github.com/sustainable-processes/ontology/OntoCAPE/supporting_concepts/physical_dimension/derived_dimensions.owl#ACCELERATION"/>
            <rdf:Description rdf:about="https://github.com/sustainable-processes/ontology/OntoCAPE/supporting_concepts/physical_dimension/derived_dimensions.owl#AREA"/>
            <rdf:Description rdf:about="https://github.com/sustainable-processes/ontology/OntoCAPE/supporting_concepts/physical_dimension/derived_dimensions.owl#MOLAR_VOLUME"/>
            <rdf:Description rdf:about="https://github.com/sustainable-processes/ontology/OntoCAPE/supporting_concepts/physical_dimension/derived_dimensions.owl#MOLECULAR_MASS"/>
            <rdf:Description rdf:about="https://github.com/sustainable-processes/ontology/OntoCAPE/supporting_concepts/physical_dimension/derived_dimensions.owl#VELOCITY"/>
            <rdf:Description rdf:about="https://github.com/sustainable-processes/ontology/OntoCAPE/supporting_concepts/physical_dimension/derived_dimensions.owl#VOLUME"/>
        </owl:distinctMembers>
    </rdf:Description>
    <rdf:Description>
        <rdf:type rdf:resource="http://www.w3.org/2002/07/owl#AllDifferent"/>
        <owl:distinctMembers rdf:parseType="Collection">
            <rdf:Description rdf:about="https://github.com/sustainable-processes/ontology/OntoCAPE/supporting_concepts/physical_dimension/derived_dimensions.owl#acceleration"/>
            <rdf:Description rdf:about="https://github.com/sustainable-processes/ontology/OntoCAPE/supporting_concepts/physical_dimension/derived_dimensions.owl#angular_acceleration"/>
            <rdf:Description rdf:about="https://github.com/sustainable-processes/ontology/OntoCAPE/supporting_concepts/physical_dimension/derived_dimensions.owl#angular_velocity"/>
            <rdf:Description rdf:about="https://github.com/sustainable-processes/ontology/OntoCAPE/supporting_concepts/physical_dimension/derived_dimensions.owl#area"/>
            <rdf:Description rdf:about="https://github.com/sustainable-processes/ontology/OntoCAPE/supporting_concepts/physical_dimension/derived_dimensions.owl#plane_angle"/>
            <rdf:Description rdf:about="https://github.com/sustainable-processes/ontology/OntoCAPE/supporting_concepts/physical_dimension/derived_dimensions.owl#solid_angle"/>
            <rdf:Description rdf:about="https://github.com/sustainable-processes/ontology/OntoCAPE/supporting_concepts/physical_dimension/derived_dimensions.owl#velocity"/>
            <rdf:Description rdf:about="https://github.com/sustainable-processes/ontology/OntoCAPE/supporting_concepts/physical_dimension/derived_dimensions.owl#volume"/>
        </owl:distinctMembers>
    </rdf:Description>
    <rdf:Description>
        <rdf:type rdf:resource="http://www.w3.org/2002/07/owl#AllDifferent"/>
        <owl:distinctMembers rdf:parseType="Collection">
            <rdf:Description rdf:about="https://github.com/sustainable-processes/ontology/OntoCAPE/supporting_concepts/physical_dimension/derived_dimensions.owl#damping_coefficient"/>
            <rdf:Description rdf:about="https://github.com/sustainable-processes/ontology/OntoCAPE/supporting_concepts/physical_dimension/derived_dimensions.owl#frequency"/>
            <rdf:Description rdf:about="https://github.com/sustainable-processes/ontology/OntoCAPE/supporting_concepts/physical_dimension/derived_dimensions.owl#oscillation_phase"/>
            <rdf:Description rdf:about="https://github.com/sustainable-processes/ontology/OntoCAPE/supporting_concepts/physical_dimension/derived_dimensions.owl#period"/>
            <rdf:Description rdf:about="https://github.com/sustainable-processes/ontology/OntoCAPE/supporting_concepts/physical_dimension/derived_dimensions.owl#rotational_frequency"/>
        </owl:distinctMembers>
    </rdf:Description>
    <rdf:Description>
        <rdf:type rdf:resource="http://www.w3.org/2002/07/owl#AllDifferent"/>
        <owl:distinctMembers rdf:parseType="Collection">
            <rdf:Description rdf:about="https://github.com/sustainable-processes/ontology/OntoCAPE/supporting_concepts/physical_dimension/derived_dimensions.owl#density"/>
            <rdf:Description rdf:about="https://github.com/sustainable-processes/ontology/OntoCAPE/supporting_concepts/physical_dimension/derived_dimensions.owl#dynamic_viscosity"/>
            <rdf:Description rdf:about="https://github.com/sustainable-processes/ontology/OntoCAPE/supporting_concepts/physical_dimension/derived_dimensions.owl#force"/>
            <rdf:Description rdf:about="https://github.com/sustainable-processes/ontology/OntoCAPE/supporting_concepts/physical_dimension/derived_dimensions.owl#kinematic_viscosity"/>
            <rdf:Description rdf:about="https://github.com/sustainable-processes/ontology/OntoCAPE/supporting_concepts/physical_dimension/derived_dimensions.owl#moment_of_force"/>
            <rdf:Description rdf:about="https://github.com/sustainable-processes/ontology/OntoCAPE/supporting_concepts/physical_dimension/derived_dimensions.owl#moment_of_inertia"/>
            <rdf:Description rdf:about="https://github.com/sustainable-processes/ontology/OntoCAPE/supporting_concepts/physical_dimension/derived_dimensions.owl#momentum"/>
            <rdf:Description rdf:about="https://github.com/sustainable-processes/ontology/OntoCAPE/supporting_concepts/physical_dimension/derived_dimensions.owl#power"/>
            <rdf:Description rdf:about="https://github.com/sustainable-processes/ontology/OntoCAPE/supporting_concepts/physical_dimension/derived_dimensions.owl#pressure"/>
            <rdf:Description rdf:about="https://github.com/sustainable-processes/ontology/OntoCAPE/supporting_concepts/physical_dimension/derived_dimensions.owl#specific_volume"/>
            <rdf:Description rdf:about="https://github.com/sustainable-processes/ontology/OntoCAPE/supporting_concepts/physical_dimension/derived_dimensions.owl#surface_tension"/>
            <rdf:Description rdf:about="https://github.com/sustainable-processes/ontology/OntoCAPE/supporting_concepts/physical_dimension/derived_dimensions.owl#work"/>
        </owl:distinctMembers>
    </rdf:Description>
    <rdf:Description>
        <rdf:type rdf:resource="http://www.w3.org/2002/07/owl#AllDifferent"/>
        <owl:distinctMembers rdf:parseType="Collection">
            <rdf:Description rdf:about="https://github.com/sustainable-processes/ontology/OntoCAPE/supporting_concepts/physical_dimension/derived_dimensions.owl#entropy"/>
            <rdf:Description rdf:about="https://github.com/sustainable-processes/ontology/OntoCAPE/supporting_concepts/physical_dimension/derived_dimensions.owl#heat_capacity"/>
            <rdf:Description rdf:about="https://github.com/sustainable-processes/ontology/OntoCAPE/supporting_concepts/physical_dimension/derived_dimensions.owl#heat_flow_rate"/>
            <rdf:Description rdf:about="https://github.com/sustainable-processes/ontology/OntoCAPE/supporting_concepts/physical_dimension/derived_dimensions.owl#internal_energy"/>
            <rdf:Description rdf:about="https://github.com/sustainable-processes/ontology/OntoCAPE/supporting_concepts/physical_dimension/derived_dimensions.owl#quantity_of_heat"/>
            <rdf:Description rdf:about="https://github.com/sustainable-processes/ontology/OntoCAPE/supporting_concepts/physical_dimension/derived_dimensions.owl#specific_entropy"/>
            <rdf:Description rdf:about="https://github.com/sustainable-processes/ontology/OntoCAPE/supporting_concepts/physical_dimension/derived_dimensions.owl#specific_heat_capacity"/>
            <rdf:Description rdf:about="https://github.com/sustainable-processes/ontology/OntoCAPE/supporting_concepts/physical_dimension/derived_dimensions.owl#temperature_coefficient"/>
            <rdf:Description rdf:about="https://github.com/sustainable-processes/ontology/OntoCAPE/supporting_concepts/physical_dimension/derived_dimensions.owl#thermal_conductivity"/>
        </owl:distinctMembers>
    </rdf:Description>
    <rdf:Description>
        <rdf:type rdf:resource="http://www.w3.org/2002/07/owl#AllDifferent"/>
        <owl:distinctMembers rdf:parseType="Collection">
            <rdf:Description rdf:about="https://github.com/sustainable-processes/ontology/OntoCAPE/supporting_concepts/physical_dimension/derived_dimensions.owl#mass_fraction"/>
            <rdf:Description rdf:about="https://github.com/sustainable-processes/ontology/OntoCAPE/supporting_concepts/physical_dimension/derived_dimensions.owl#molar_fraction"/>
            <rdf:Description rdf:about="https://github.com/sustainable-processes/ontology/OntoCAPE/supporting_concepts/physical_dimension/derived_dimensions.owl#molar_volume"/>
            <rdf:Description rdf:about="https://github.com/sustainable-processes/ontology/OntoCAPE/supporting_concepts/physical_dimension/derived_dimensions.owl#molecular_mass"/>
            <rdf:Description rdf:about="https://github.com/sustainable-processes/ontology/OntoCAPE/supporting_concepts/physical_dimension/derived_dimensions.owl#volume_fraction"/>
        </owl:distinctMembers>
    </rdf:Description>
</rdf:RDF>



<!-- Generated by the OWL API (version 4.5.26.2023-07-17T20:34:13Z) https://github.com/owlcs/owlapi -->

