<?xml version="1.0"?>
<rdf:RDF xmlns="https://github.com/sustainable-processes/ontology/OntoCAPE/chemical_process_system/CPS_realization/plant_equipment/machine.owl#"
     xml:base="https://github.com/sustainable-processes/ontology/OntoCAPE/chemical_process_system/CPS_realization/plant_equipment/machine.owl"
     xmlns:p1="https://github.com/sustainable-processes/ontology/OntoCAPE/chemical_process_system/CPS_realization/apparatus/machine.owl#"
     xmlns:owl="http://www.w3.org/2002/07/owl#"
     xmlns:rdf="http://www.w3.org/1999/02/22-rdf-syntax-ns#"
     xmlns:xml="http://www.w3.org/XML/1998/namespace"
     xmlns:xsd="http://www.w3.org/2001/XMLSchema#"
     xmlns:rdfs="http://www.w3.org/2000/01/rdf-schema#"
     xmlns:root="https://github.com/sustainable-processes/ontology/OntoCAPE/"
     xmlns:plant="https://github.com/sustainable-processes/ontology/OntoCAPE/chemical_process_system/CPS_realization/plant.owl#"
     xmlns:terms="http://purl.org/dc/terms/"
     xmlns:system="https://github.com/sustainable-processes/ontology/OntoCAPE/upper_level/system.owl"
     xmlns:fixture="https://github.com/sustainable-processes/ontology/OntoCAPE/chemical_process_system/CPS_realization/plant_equipment/fixture.owl"
     xmlns:machine="https://github.com/sustainable-processes/ontology/OntoCAPE/chemical_process_system/CPS_realization/plant_equipment/machine.owl">
    <owl:Ontology rdf:about="https://github.com/sustainable-processes/ontology/OntoCAPE/chemical_process_system/CPS_realization/plant_equipment/machine.owl">
        <owl:imports rdf:resource="https://github.com/sustainable-processes/ontology/OntoCAPE/chemical_process_system/CPS_realization/plant_equipment/fixture.owl"/>
        <terms:license>Copyright (C) [2009] [Andreas Wiesner]
                This program is free software; you can redistribute it and/or modify it under the terms of the GNU General Public License as published by the Free Software Foundation; either version 3 of the License, or (at your option) any later version.
                This program is distributed in the hope that it will be useful, but WITHOUT ANY WARRANTY; without even the implied warranty of MERCHANTABILITY or FITNESS FOR A PARTICULAR PURPOSE. See the GNU General Public License for more details.
                You should have received a copy of the GNU General Public License along with this program; if not, see &lt;http://www.gnu.org/licenses/&gt;.
    </terms:license>
        <rdfs:comment>The ontology module &apos;machine&apos; provides specializations of machines applicable to a chemical process system.
The following classes and relations from other ontology modules are used within &apos;machine&apos;:

&lt;owl:Class rdf:about=&quot;https://github.com/sustainable-processes/ontology/OntoCAPE/upper_level/system.owl#QuantitativeValue&quot;/&gt;
&lt;owl:Class rdf:about=&quot;https://github.com/sustainable-processes/ontology/OntoCAPE/chemical_process_system/CPS_realization/plant.owl#Machine&quot;/&gt;

&lt;owl:ObjectProperty rdf:about=&quot;https://github.com/sustainable-processes/ontology/OntoCAPE/upper_level/system.owl#hasCharacteristic&quot;/&gt;
    </rdfs:comment>
        <owl:versionInfo>2.0</owl:versionInfo>
    </owl:Ontology>
    


    <!-- 
    ///////////////////////////////////////////////////////////////////////////////////////
    //
    // Object Properties
    //
    ///////////////////////////////////////////////////////////////////////////////////////
     -->

    


    <!-- https://github.com/sustainable-processes/ontology/OntoCAPE/chemical_process_system/CPS_realization/apparatus/machine.owl#hasPumpHead -->

    <owl:ObjectProperty rdf:about="https://github.com/sustainable-processes/ontology/OntoCAPE/chemical_process_system/CPS_realization/apparatus/machine.owl#hasPumpHead">
        <rdfs:subPropertyOf rdf:resource="https://github.com/sustainable-processes/ontology/OntoCAPE/upper_level/system.owl#hasCharacteristic"/>
        <rdfs:domain rdf:resource="https://github.com/sustainable-processes/ontology/OntoCAPE/chemical_process_system/CPS_realization/apparatus/machine.owl#Pump"/>
    </owl:ObjectProperty>
    


    <!-- https://github.com/sustainable-processes/ontology/OntoCAPE/chemical_process_system/CPS_realization/plant_equipment/machine.owl#hasPumpHead -->

    <owl:ObjectProperty rdf:about="https://github.com/sustainable-processes/ontology/OntoCAPE/chemical_process_system/CPS_realization/plant_equipment/machine.owl#hasPumpHead">
        <rdfs:comment>The relation hasPumpHead refers the pump head a pump is design for.</rdfs:comment>
    </owl:ObjectProperty>
    


    <!-- 
    ///////////////////////////////////////////////////////////////////////////////////////
    //
    // Classes
    //
    ///////////////////////////////////////////////////////////////////////////////////////
     -->

    


    <!-- https://github.com/sustainable-processes/ontology/OntoCAPE/chemical_process_system/CPS_realization/apparatus/machine.owl#Pump -->

    <owl:Class rdf:about="https://github.com/sustainable-processes/ontology/OntoCAPE/chemical_process_system/CPS_realization/apparatus/machine.owl#Pump"/>
    


    <!-- https://github.com/sustainable-processes/ontology/OntoCAPE/chemical_process_system/CPS_realization/plant.owl#Machine -->

    <owl:Class rdf:about="https://github.com/sustainable-processes/ontology/OntoCAPE/chemical_process_system/CPS_realization/plant.owl#Machine"/>
    


    <!-- https://github.com/sustainable-processes/ontology/OntoCAPE/chemical_process_system/CPS_realization/plant_equipment/machine.owl#Pump -->

    <owl:Class rdf:about="https://github.com/sustainable-processes/ontology/OntoCAPE/chemical_process_system/CPS_realization/plant_equipment/machine.owl#Pump">
        <rdfs:subClassOf rdf:resource="https://github.com/sustainable-processes/ontology/OntoCAPE/chemical_process_system/CPS_realization/plant.owl#Machine"/>
        <rdfs:subClassOf>
            <owl:Restriction>
                <owl:onProperty rdf:resource="https://github.com/sustainable-processes/ontology/OntoCAPE/chemical_process_system/CPS_realization/plant_equipment/machine.owl#hasPumpHead"/>
                <owl:someValuesFrom rdf:resource="https://github.com/sustainable-processes/ontology/OntoCAPE/upper_level/system.owl#QuantitativeValue"/>
            </owl:Restriction>
        </rdfs:subClassOf>
    </owl:Class>
    


    <!-- 
    ///////////////////////////////////////////////////////////////////////////////////////
    //
    // Annotations
    //
    ///////////////////////////////////////////////////////////////////////////////////////
     -->

    <rdf:Description rdf:about="http://www.w3.org/2002/07/owl#Thing">
        <rdfs:comment>A Pump is a Machine which is used to compress or move fluid materials. 
A further classification of pumps is beyond the current scope of OntoCAPE.</rdfs:comment>
    </rdf:Description>
</rdf:RDF>



<!-- Generated by the OWL API (version 4.5.26.2023-07-17T20:34:13Z) https://github.com/owlcs/owlapi -->

