<?xml version="1.0"?>
<rdf:RDF xmlns="https://github.com/sustainable-processes/ontology/OntoCAPE/chemical_process_system/CPS_realization/plant.owl#"
     xml:base="https://github.com/sustainable-processes/ontology/OntoCAPE/chemical_process_system/CPS_realization/plant.owl"
     xmlns:fc="https://github.com/sustainable-processes/ontology/meta_model/fundamental_concepts/fundamental_concepts.owl"
     xmlns:owl="http://www.w3.org/2002/07/owl#"
     xmlns:rdf="http://www.w3.org/1999/02/22-rdf-syntax-ns#"
     xmlns:xml="http://www.w3.org/XML/1998/namespace"
     xmlns:xsd="http://www.w3.org/2001/XMLSchema#"
     xmlns:rdfs="http://www.w3.org/2000/01/rdf-schema#"
     xmlns:root="https://github.com/sustainable-processes/ontology/OntoCAPE/"
     xmlns:array="https://github.com/sustainable-processes/ontology/meta_model/data_structures/array.owl#"
     xmlns:plant="https://github.com/sustainable-processes/ontology/OntoCAPE/chemical_process_system/CPS_realization/plant.owl"
     xmlns:terms="http://purl.org/dc/terms/"
     xmlns:system="https://github.com/sustainable-processes/ontology/OntoCAPE/upper_level/system.owl#"
     xmlns:geometry="https://github.com/sustainable-processes/ontology/OntoCAPE/supporting_concepts/geometry/geometry.owl#"
     xmlns:multiset="https://github.com/sustainable-processes/ontology/meta_model/data_structures/multiset.owl"
     xmlns:multiset1="https://github.com/sustainable-processes/ontology/meta_model/data_structures/multiset.owl#"
     xmlns:substance="https://github.com/sustainable-processes/ontology/OntoCAPE/material/substance/substance.owl#"
     xmlns:fundamental_concepts="https://github.com/sustainable-processes/ontology/meta_model/fundamental_concepts/fundamental_concepts.owl#"
     xmlns:mathematical_relation="https://github.com/sustainable-processes/ontology/OntoCAPE/supporting_concepts/mathematical_relation/mathematical_relation.owl#">
    <owl:Ontology rdf:about="https://github.com/sustainable-processes/ontology/OntoCAPE/chemical_process_system/CPS_realization/plant.owl">
        <owl:imports rdf:resource="https://github.com/sustainable-processes/ontology/OntoCAPE/material/substance/substance.owl"/>
        <owl:imports rdf:resource="https://github.com/sustainable-processes/ontology/OntoCAPE/supporting_concepts/geometry/geometry.owl"/>
        <terms:license>Copyright (C) [2009] [Andreas Wiesner]
                This program is free software; you can redistribute it and/or modify it under the terms of the GNU General Public License as published by the Free Software Foundation; either version 3 of the License, or (at your option) any later version.
                This program is distributed in the hope that it will be useful, but WITHOUT ANY WARRANTY; without even the implied warranty of MERCHANTABILITY or FITNESS FOR A PARTICULAR PURPOSE. See the GNU General Public License for more details.
                You should have received a copy of the GNU General Public License along with this program; if not, see &lt;http://www.gnu.org/licenses/&gt;.
    </terms:license>
        <rdfs:comment>The ontology module &apos;plant&apos; realizes a chemical process system in terms of technical equipment for production.
The following classes and relations from other ontology modules are used within &apos;plant&apos;:

&lt;owl:Class rdf:about=&quot;https://github.com/sustainable-processes/ontology/OntoCAPE/material/substance/substance.owl#Substance&quot;/&gt;
&lt;owl:Class rdf:about=&quot;https://github.com/sustainable-processes/ontology/OntoCAPE/supporting_concepts/geometry/geometry.owl#Cylinder&quot;/&gt;
&lt;owl:Class rdf:about=&quot;https://github.com/sustainable-processes/ontology/meta_model/data_structures/multiset.owl#Multiplicity&quot;/&gt;
&lt;owl:Class rdf:about=&quot;https://github.com/sustainable-processes/ontology/OntoCAPE/supporting_concepts/geometry/geometry.owl#Diameter&quot;/&gt;
&lt;owl:Class rdf:about=&quot;https://github.com/sustainable-processes/ontology/OntoCAPE/supporting_concepts/geometry/geometry.owl#Solid&quot;/&gt;
&lt;owl:Class rdf:about=&quot;https://github.com/sustainable-processes/ontology/OntoCAPE/upper_level/system.owl#System&quot;/&gt;
&lt;owl:Class rdf:about=&quot;https://github.com/sustainable-processes/ontology/OntoCAPE/supporting_concepts/geometry/geometry.owl#EdgeLength&quot;/&gt;
&lt;owl:Class rdf:about=&quot;https://github.com/sustainable-processes/ontology/OntoCAPE/upper_level/system.owl#SystemInterface&quot;/&gt;
&lt;owl:Class rdf:about=&quot;https://github.com/sustainable-processes/ontology/OntoCAPE/upper_level/system.owl#Property&quot;/&gt;
&lt;owl:Class rdf:about=&quot;https://github.com/sustainable-processes/ontology/OntoCAPE/supporting_concepts/geometry/geometry.owl#Height&quot;/&gt;
&lt;owl:Class rdf:about=&quot;https://github.com/sustainable-processes/ontology/OntoCAPE/upper_level/system.owl#QuantitativeValue&quot;/&gt;

&lt;owl:Class rdf:about=&quot;https://github.com/sustainable-processes/ontology/OntoCAPE/supporting_concepts/geometry/geometry.owl#ShapeRepresentation&quot;/&gt;
&lt;owl:ObjectProperty rdf:about=&quot;https://github.com/sustainable-processes/ontology/OntoCAPE/upper_level/system.owl#hasProperty&quot;/&gt;
&lt;owl:ObjectProperty rdf:about=&quot;https://github.com/sustainable-processes/ontology/OntoCAPE/upper_level/system.owl#isDirectlyConnectedTo&quot;/&gt;
&lt;owl:ObjectProperty rdf:about=&quot;https://github.com/sustainable-processes/ontology/OntoCAPE/upper_level/system.owl#hasDirectSubsystem&quot;/&gt;
&lt;owl:ObjectProperty rdf:about=&quot;https://github.com/sustainable-processes/ontology/OntoCAPE/upper_level/system.owl#hasSubsystem&quot;/&gt;
&lt;owl:ObjectProperty rdf:about=&quot;https://github.com/sustainable-processes/ontology/OntoCAPE/upper_level/system.owl#isExclusivelySubsystemOf&quot;/&gt;
&lt;owl:ObjectProperty rdf:about=&quot;https://github.com/sustainable-processes/ontology/OntoCAPE/upper_level/system.owl#hasCharacteristic&quot;/&gt;
&lt;owl:ObjectProperty rdf:about=&quot;https://github.com/sustainable-processes/ontology/meta_model/data_structures/multiset.owl#hasMultiplicity&quot;/&gt;
&lt;owl:ObjectProperty rdf:about=&quot;https://github.com/sustainable-processes/ontology/OntoCAPE/upper_level/system.owl#isComposedOfSubsystem&quot;/&gt;

The following classes and relations from the Meta Model are refined within &apos;plant&apos;:

&lt;owl:ObjectProperty rdf:about=&quot;https://github.com/sustainable-processes/ontology/meta_model/fundamental_concepts/fundamental_concepts.owl#isInvolvedInN-aryRelation&quot;/&gt;
&lt;owl:ObjectProperty rdf:about=&quot;https://github.com/sustainable-processes/ontology/meta_model/data_structures/multiset.owl#indicatesMultiplicityOf&quot;/&gt;
&lt;owl:ObjectProperty rdf:about=&quot;https://github.com/sustainable-processes/ontology/meta_model/fundamental_concepts/fundamental_concepts.owl#inter-objectRelation&quot;/&gt;
&lt;owl:ObjectProperty rdf:about=&quot;https://github.com/sustainable-processes/ontology/meta_model/data_structures/multiset.owl#multiplicity&quot;/&gt;

    </rdfs:comment>
        <owl:versionInfo>2.0</owl:versionInfo>
    </owl:Ontology>
    


    <!-- 
    ///////////////////////////////////////////////////////////////////////////////////////
    //
    // Object Properties
    //
    ///////////////////////////////////////////////////////////////////////////////////////
     -->

    


    <!-- https://github.com/sustainable-processes/ontology/OntoCAPE/chemical_process_system/CPS_realization/plant.owl#hasCapacity -->

    <owl:ObjectProperty rdf:about="https://github.com/sustainable-processes/ontology/OntoCAPE/chemical_process_system/CPS_realization/plant.owl#hasCapacity">
        <rdfs:subPropertyOf rdf:resource="https://github.com/sustainable-processes/ontology/OntoCAPE/upper_level/system.owl#hasCharacteristic"/>
        <rdfs:domain rdf:resource="https://github.com/sustainable-processes/ontology/OntoCAPE/chemical_process_system/CPS_realization/plant.owl#Equipment"/>
        <rdfs:comment>The relation hasCapacity indicates equipment’s capacity.</rdfs:comment>
    </owl:ObjectProperty>
    


    <!-- https://github.com/sustainable-processes/ontology/OntoCAPE/chemical_process_system/CPS_realization/plant.owl#hasConnector -->

    <owl:ObjectProperty rdf:about="https://github.com/sustainable-processes/ontology/OntoCAPE/chemical_process_system/CPS_realization/plant.owl#hasConnector">
        <rdfs:subPropertyOf rdf:resource="https://github.com/sustainable-processes/ontology/OntoCAPE/upper_level/system.owl#isComposedOfSubsystem"/>
        <owl:inverseOf rdf:resource="https://github.com/sustainable-processes/ontology/OntoCAPE/chemical_process_system/CPS_realization/plant.owl#isConnectorOf"/>
        <rdfs:domain>
            <owl:Class>
                <owl:unionOf rdf:parseType="Collection">
                    <rdf:Description rdf:about="https://github.com/sustainable-processes/ontology/OntoCAPE/chemical_process_system/CPS_realization/plant.owl#Instrument"/>
                    <rdf:Description rdf:about="https://github.com/sustainable-processes/ontology/OntoCAPE/chemical_process_system/CPS_realization/plant.owl#PieceOfEquipment"/>
                    <rdf:Description rdf:about="https://github.com/sustainable-processes/ontology/OntoCAPE/chemical_process_system/CPS_realization/plant.owl#PipeSegment"/>
                </owl:unionOf>
            </owl:Class>
        </rdfs:domain>
        <rdfs:range rdf:resource="https://github.com/sustainable-processes/ontology/OntoCAPE/chemical_process_system/CPS_realization/plant.owl#PlantItemInterface"/>
        <rdfs:comment>The relation hasConnector refers from a PieceOfEquipment or a PipeSegment or an Instrument to the corresponding PlantItemInterface.</rdfs:comment>
    </owl:ObjectProperty>
    


    <!-- https://github.com/sustainable-processes/ontology/OntoCAPE/chemical_process_system/CPS_realization/plant.owl#hasConstructionMaterial -->

    <owl:ObjectProperty rdf:about="https://github.com/sustainable-processes/ontology/OntoCAPE/chemical_process_system/CPS_realization/plant.owl#hasConstructionMaterial">
        <rdfs:subPropertyOf rdf:resource="https://github.com/sustainable-processes/ontology/meta_model/fundamental_concepts/fundamental_concepts.owl#inter-objectRelation"/>
        <rdfs:domain rdf:resource="https://github.com/sustainable-processes/ontology/OntoCAPE/chemical_process_system/CPS_realization/plant.owl#PlantItem"/>
        <rdfs:range rdf:resource="https://github.com/sustainable-processes/ontology/OntoCAPE/material/substance/substance.owl#Substance"/>
        <rdfs:comment>The relation hasConstructionMaterial refers to the Material chosen for construction of PlantItems.</rdfs:comment>
    </owl:ObjectProperty>
    


    <!-- https://github.com/sustainable-processes/ontology/OntoCAPE/chemical_process_system/CPS_realization/plant.owl#hasEfficiency -->

    <owl:ObjectProperty rdf:about="https://github.com/sustainable-processes/ontology/OntoCAPE/chemical_process_system/CPS_realization/plant.owl#hasEfficiency">
        <rdfs:subPropertyOf rdf:resource="https://github.com/sustainable-processes/ontology/OntoCAPE/upper_level/system.owl#hasCharacteristic"/>
        <rdfs:domain rdf:resource="https://github.com/sustainable-processes/ontology/OntoCAPE/chemical_process_system/CPS_realization/plant.owl#Equipment"/>
        <rdfs:comment>The relation hasPumpEfficiency indicates a machine’s efficiency</rdfs:comment>
    </owl:ObjectProperty>
    


    <!-- https://github.com/sustainable-processes/ontology/OntoCAPE/chemical_process_system/CPS_realization/plant.owl#hasFixture -->

    <owl:ObjectProperty rdf:about="https://github.com/sustainable-processes/ontology/OntoCAPE/chemical_process_system/CPS_realization/plant.owl#hasFixture">
        <rdfs:subPropertyOf rdf:resource="https://github.com/sustainable-processes/ontology/OntoCAPE/upper_level/system.owl#isComposedOfSubsystem"/>
        <owl:inverseOf rdf:resource="https://github.com/sustainable-processes/ontology/OntoCAPE/chemical_process_system/CPS_realization/plant.owl#isFixtureOf"/>
        <rdfs:domain rdf:resource="https://github.com/sustainable-processes/ontology/OntoCAPE/chemical_process_system/CPS_realization/plant.owl#Equipment"/>
        <rdfs:range rdf:resource="https://github.com/sustainable-processes/ontology/OntoCAPE/chemical_process_system/CPS_realization/plant.owl#Fixture"/>
        <rdfs:comment>The relation hasFixture refers from a Equipment to the corresponding Fixture.</rdfs:comment>
    </owl:ObjectProperty>
    


    <!-- https://github.com/sustainable-processes/ontology/OntoCAPE/chemical_process_system/CPS_realization/plant.owl#hasHeight -->

    <owl:ObjectProperty rdf:about="https://github.com/sustainable-processes/ontology/OntoCAPE/chemical_process_system/CPS_realization/plant.owl#hasHeight">
        <rdfs:subPropertyOf rdf:resource="https://github.com/sustainable-processes/ontology/OntoCAPE/upper_level/system.owl#hasCharacteristic"/>
        <rdfs:domain rdf:resource="https://github.com/sustainable-processes/ontology/OntoCAPE/chemical_process_system/CPS_realization/plant.owl#PieceOfEquipment"/>
        <rdfs:comment>The relation hasHeight refers the height of equipment.</rdfs:comment>
    </owl:ObjectProperty>
    


    <!-- https://github.com/sustainable-processes/ontology/OntoCAPE/chemical_process_system/CPS_realization/plant.owl#hasInsideDiameter -->

    <owl:ObjectProperty rdf:about="https://github.com/sustainable-processes/ontology/OntoCAPE/chemical_process_system/CPS_realization/plant.owl#hasInsideDiameter">
        <rdfs:subPropertyOf rdf:resource="https://github.com/sustainable-processes/ontology/OntoCAPE/upper_level/system.owl#hasCharacteristic"/>
        <rdfs:domain>
            <owl:Class>
                <owl:unionOf rdf:parseType="Collection">
                    <rdf:Description rdf:about="https://github.com/sustainable-processes/ontology/OntoCAPE/chemical_process_system/CPS_realization/plant.owl#Instrument"/>
                    <rdf:Description rdf:about="https://github.com/sustainable-processes/ontology/OntoCAPE/chemical_process_system/CPS_realization/plant.owl#PieceOfEquipment"/>
                    <rdf:Description rdf:about="https://github.com/sustainable-processes/ontology/OntoCAPE/chemical_process_system/CPS_realization/plant.owl#Pipe"/>
                </owl:unionOf>
            </owl:Class>
        </rdfs:domain>
        <rdfs:comment>The relation hasDiameter indicates an equipment’s inside diameter.</rdfs:comment>
    </owl:ObjectProperty>
    


    <!-- https://github.com/sustainable-processes/ontology/OntoCAPE/chemical_process_system/CPS_realization/plant.owl#hasMultiplicity -->

    <owl:ObjectProperty rdf:about="https://github.com/sustainable-processes/ontology/OntoCAPE/chemical_process_system/CPS_realization/plant.owl#hasMultiplicity">
        <rdfs:subPropertyOf rdf:resource="https://github.com/sustainable-processes/ontology/meta_model/data_structures/multiset.owl#hasMultiplicity"/>
        <owl:inverseOf rdf:resource="https://github.com/sustainable-processes/ontology/OntoCAPE/chemical_process_system/CPS_realization/plant.owl#indicatesMultiplicityOf"/>
        <rdfs:domain rdf:resource="https://github.com/sustainable-processes/ontology/OntoCAPE/chemical_process_system/CPS_realization/plant.owl#PlantItem"/>
        <rdfs:range rdf:resource="https://github.com/sustainable-processes/ontology/OntoCAPE/chemical_process_system/CPS_realization/plant.owl#Multiplicity"/>
    </owl:ObjectProperty>
    


    <!-- https://github.com/sustainable-processes/ontology/OntoCAPE/chemical_process_system/CPS_realization/plant.owl#hasNumberOfPlantItems -->

    <owl:ObjectProperty rdf:about="https://github.com/sustainable-processes/ontology/OntoCAPE/chemical_process_system/CPS_realization/plant.owl#hasNumberOfPlantItems">
        <rdfs:subPropertyOf rdf:resource="https://github.com/sustainable-processes/ontology/meta_model/fundamental_concepts/fundamental_concepts.owl#isInvolvedInN-aryRelation"/>
        <rdfs:domain rdf:resource="https://github.com/sustainable-processes/ontology/OntoCAPE/chemical_process_system/CPS_realization/plant.owl#PlantItem"/>
        <rdfs:range rdf:resource="https://github.com/sustainable-processes/ontology/OntoCAPE/chemical_process_system/CPS_realization/plant.owl#Multiplicity"/>
    </owl:ObjectProperty>
    


    <!-- https://github.com/sustainable-processes/ontology/OntoCAPE/chemical_process_system/CPS_realization/plant.owl#hasOutsideDiameter -->

    <owl:ObjectProperty rdf:about="https://github.com/sustainable-processes/ontology/OntoCAPE/chemical_process_system/CPS_realization/plant.owl#hasOutsideDiameter">
        <rdfs:subPropertyOf rdf:resource="https://github.com/sustainable-processes/ontology/OntoCAPE/upper_level/system.owl#hasCharacteristic"/>
        <rdfs:domain rdf:resource="https://github.com/sustainable-processes/ontology/OntoCAPE/chemical_process_system/CPS_realization/plant.owl#PlantItem"/>
    </owl:ObjectProperty>
    


    <!-- https://github.com/sustainable-processes/ontology/OntoCAPE/chemical_process_system/CPS_realization/plant.owl#hasPowerOutput -->

    <owl:ObjectProperty rdf:about="https://github.com/sustainable-processes/ontology/OntoCAPE/chemical_process_system/CPS_realization/plant.owl#hasPowerOutput">
        <rdfs:subPropertyOf rdf:resource="https://github.com/sustainable-processes/ontology/OntoCAPE/upper_level/system.owl#hasCharacteristic"/>
        <rdfs:domain rdf:resource="https://github.com/sustainable-processes/ontology/OntoCAPE/chemical_process_system/CPS_realization/plant.owl#Machine"/>
        <rdfs:comment>The relation hasPowerOutput indicates a machine’s magnitude of power output.</rdfs:comment>
    </owl:ObjectProperty>
    


    <!-- https://github.com/sustainable-processes/ontology/OntoCAPE/chemical_process_system/CPS_realization/plant.owl#hasTEMAClass -->

    <owl:ObjectProperty rdf:about="https://github.com/sustainable-processes/ontology/OntoCAPE/chemical_process_system/CPS_realization/plant.owl#hasTEMAClass">
        <rdfs:subPropertyOf rdf:resource="https://github.com/sustainable-processes/ontology/OntoCAPE/upper_level/system.owl#hasCharacteristic"/>
    </owl:ObjectProperty>
    


    <!-- https://github.com/sustainable-processes/ontology/OntoCAPE/chemical_process_system/CPS_realization/plant.owl#hasTrayNumberingConvention -->

    <owl:ObjectProperty rdf:about="https://github.com/sustainable-processes/ontology/OntoCAPE/chemical_process_system/CPS_realization/plant.owl#hasTrayNumberingConvention">
        <rdfs:subPropertyOf rdf:resource="https://github.com/sustainable-processes/ontology/OntoCAPE/upper_level/system.owl#hasCharacteristic"/>
    </owl:ObjectProperty>
    


    <!-- https://github.com/sustainable-processes/ontology/OntoCAPE/chemical_process_system/CPS_realization/plant.owl#indicatesMultiplicityOf -->

    <owl:ObjectProperty rdf:about="https://github.com/sustainable-processes/ontology/OntoCAPE/chemical_process_system/CPS_realization/plant.owl#indicatesMultiplicityOf">
        <rdfs:subPropertyOf rdf:resource="https://github.com/sustainable-processes/ontology/meta_model/data_structures/multiset.owl#indicatesMultiplicityOf"/>
        <rdfs:domain rdf:resource="https://github.com/sustainable-processes/ontology/OntoCAPE/chemical_process_system/CPS_realization/plant.owl#Multiplicity"/>
        <rdfs:range rdf:resource="https://github.com/sustainable-processes/ontology/OntoCAPE/chemical_process_system/CPS_realization/plant.owl#PlantItem"/>
    </owl:ObjectProperty>
    


    <!-- https://github.com/sustainable-processes/ontology/OntoCAPE/chemical_process_system/CPS_realization/plant.owl#isConnectorOf -->

    <owl:ObjectProperty rdf:about="https://github.com/sustainable-processes/ontology/OntoCAPE/chemical_process_system/CPS_realization/plant.owl#isConnectorOf">
        <rdfs:subPropertyOf rdf:resource="https://github.com/sustainable-processes/ontology/OntoCAPE/upper_level/system.owl#isExclusivelySubsystemOf"/>
        <rdfs:domain rdf:resource="https://github.com/sustainable-processes/ontology/OntoCAPE/chemical_process_system/CPS_realization/plant.owl#PlantItemInterface"/>
        <rdfs:range>
            <owl:Class>
                <owl:unionOf rdf:parseType="Collection">
                    <rdf:Description rdf:about="https://github.com/sustainable-processes/ontology/OntoCAPE/chemical_process_system/CPS_realization/plant.owl#Instrument"/>
                    <rdf:Description rdf:about="https://github.com/sustainable-processes/ontology/OntoCAPE/chemical_process_system/CPS_realization/plant.owl#PieceOfEquipment"/>
                    <rdf:Description rdf:about="https://github.com/sustainable-processes/ontology/OntoCAPE/chemical_process_system/CPS_realization/plant.owl#PipeSegment"/>
                </owl:unionOf>
            </owl:Class>
        </rdfs:range>
        <rdfs:comment>The relation isConnectorOf refers from a PlantItemInterface to the corresponding piece of EquipmentOrPipeSegmentOrInstrument.</rdfs:comment>
    </owl:ObjectProperty>
    


    <!-- https://github.com/sustainable-processes/ontology/OntoCAPE/chemical_process_system/CPS_realization/plant.owl#isFixtureOf -->

    <owl:ObjectProperty rdf:about="https://github.com/sustainable-processes/ontology/OntoCAPE/chemical_process_system/CPS_realization/plant.owl#isFixtureOf">
        <rdfs:subPropertyOf rdf:resource="https://github.com/sustainable-processes/ontology/OntoCAPE/upper_level/system.owl#isExclusivelySubsystemOf"/>
        <rdfs:domain rdf:resource="https://github.com/sustainable-processes/ontology/OntoCAPE/chemical_process_system/CPS_realization/plant.owl#Fixture"/>
        <rdfs:range rdf:resource="https://github.com/sustainable-processes/ontology/OntoCAPE/chemical_process_system/CPS_realization/plant.owl#Equipment"/>
        <rdfs:comment>The relation isFixtureOf refers from a Fixture to the corresponding Equipment.</rdfs:comment>
    </owl:ObjectProperty>
    


    <!-- 
    ///////////////////////////////////////////////////////////////////////////////////////
    //
    // Data properties
    //
    ///////////////////////////////////////////////////////////////////////////////////////
     -->

    


    <!-- https://github.com/sustainable-processes/ontology/OntoCAPE/chemical_process_system/CPS_realization/plant.owl#has_number_of_tube_passes_per_shell -->

    <owl:DatatypeProperty rdf:about="https://github.com/sustainable-processes/ontology/OntoCAPE/chemical_process_system/CPS_realization/plant.owl#has_number_of_tube_passes_per_shell">
        <rdfs:range rdf:resource="http://www.w3.org/2001/XMLSchema#int"/>
    </owl:DatatypeProperty>
    


    <!-- https://github.com/sustainable-processes/ontology/OntoCAPE/chemical_process_system/CPS_realization/plant.owl#multiplicity -->

    <owl:DatatypeProperty rdf:about="https://github.com/sustainable-processes/ontology/OntoCAPE/chemical_process_system/CPS_realization/plant.owl#multiplicity">
        <rdfs:subPropertyOf rdf:resource="https://github.com/sustainable-processes/ontology/meta_model/data_structures/multiset.owl#multiplicity"/>
        <rdfs:domain rdf:resource="https://github.com/sustainable-processes/ontology/OntoCAPE/chemical_process_system/CPS_realization/plant.owl#Multiplicity"/>
        <rdfs:range rdf:resource="http://www.w3.org/2001/XMLSchema#int"/>
    </owl:DatatypeProperty>
    


    <!-- 
    ///////////////////////////////////////////////////////////////////////////////////////
    //
    // Classes
    //
    ///////////////////////////////////////////////////////////////////////////////////////
     -->

    


    <!-- https://github.com/sustainable-processes/ontology/OntoCAPE/chemical_process_system/CPS_realization/plant.owl#Apparatus -->

    <owl:Class rdf:about="https://github.com/sustainable-processes/ontology/OntoCAPE/chemical_process_system/CPS_realization/plant.owl#Apparatus">
        <rdfs:subClassOf rdf:resource="https://github.com/sustainable-processes/ontology/OntoCAPE/chemical_process_system/CPS_realization/plant.owl#PieceOfEquipment"/>
        <owl:disjointWith rdf:resource="https://github.com/sustainable-processes/ontology/OntoCAPE/chemical_process_system/CPS_realization/plant.owl#Machine"/>
        <rdfs:comment>An Apparatus is a PieceOfEquipment which mainly consists of non-moving parts and provides space for materials to be processed.</rdfs:comment>
    </owl:Class>
    


    <!-- https://github.com/sustainable-processes/ontology/OntoCAPE/chemical_process_system/CPS_realization/plant.owl#Equipment -->

    <owl:Class rdf:about="https://github.com/sustainable-processes/ontology/OntoCAPE/chemical_process_system/CPS_realization/plant.owl#Equipment">
        <owl:equivalentClass>
            <owl:Class>
                <owl:unionOf rdf:parseType="Collection">
                    <rdf:Description rdf:about="https://github.com/sustainable-processes/ontology/OntoCAPE/chemical_process_system/CPS_realization/plant.owl#GroupOfEquipment"/>
                    <rdf:Description rdf:about="https://github.com/sustainable-processes/ontology/OntoCAPE/chemical_process_system/CPS_realization/plant.owl#PieceOfEquipment"/>
                </owl:unionOf>
            </owl:Class>
        </owl:equivalentClass>
        <rdfs:subClassOf rdf:resource="https://github.com/sustainable-processes/ontology/OntoCAPE/chemical_process_system/CPS_realization/plant.owl#PlantItem"/>
        <owl:disjointWith rdf:resource="https://github.com/sustainable-processes/ontology/OntoCAPE/chemical_process_system/CPS_realization/plant.owl#Fixture"/>
        <owl:disjointWith rdf:resource="https://github.com/sustainable-processes/ontology/OntoCAPE/chemical_process_system/CPS_realization/plant.owl#Instrumentation"/>
        <owl:disjointWith rdf:resource="https://github.com/sustainable-processes/ontology/OntoCAPE/chemical_process_system/CPS_realization/plant.owl#Piping"/>
        <rdfs:comment>Equipment is a PlantIitem that is capable of independently realizing one or more Process Steps.</rdfs:comment>
    </owl:Class>
    


    <!-- https://github.com/sustainable-processes/ontology/OntoCAPE/chemical_process_system/CPS_realization/plant.owl#Fixture -->

    <owl:Class rdf:about="https://github.com/sustainable-processes/ontology/OntoCAPE/chemical_process_system/CPS_realization/plant.owl#Fixture">
        <rdfs:subClassOf rdf:resource="https://github.com/sustainable-processes/ontology/OntoCAPE/chemical_process_system/CPS_realization/plant.owl#PlantItem"/>
        <owl:disjointWith rdf:resource="https://github.com/sustainable-processes/ontology/OntoCAPE/chemical_process_system/CPS_realization/plant.owl#Instrumentation"/>
        <owl:disjointWith rdf:resource="https://github.com/sustainable-processes/ontology/OntoCAPE/chemical_process_system/CPS_realization/plant.owl#Piping"/>
        <rdfs:comment>A Fixture is a PlantItem that is part of Equipment and therefore not capable of independently realizing a ProcessStep. The function of a PlantItem essentially depends on the required Fixtures.</rdfs:comment>
    </owl:Class>
    


    <!-- https://github.com/sustainable-processes/ontology/OntoCAPE/chemical_process_system/CPS_realization/plant.owl#GroupOfEquipment -->

    <owl:Class rdf:about="https://github.com/sustainable-processes/ontology/OntoCAPE/chemical_process_system/CPS_realization/plant.owl#GroupOfEquipment">
        <owl:equivalentClass>
            <owl:Class>
                <owl:intersectionOf rdf:parseType="Collection">
                    <rdf:Description rdf:about="https://github.com/sustainable-processes/ontology/OntoCAPE/chemical_process_system/CPS_realization/plant.owl#Equipment"/>
                    <owl:Restriction>
                        <owl:onProperty rdf:resource="https://github.com/sustainable-processes/ontology/OntoCAPE/upper_level/system.owl#hasSubsystem"/>
                        <owl:someValuesFrom rdf:resource="https://github.com/sustainable-processes/ontology/OntoCAPE/chemical_process_system/CPS_realization/plant.owl#Equipment"/>
                    </owl:Restriction>
                    <owl:Restriction>
                        <owl:onProperty rdf:resource="https://github.com/sustainable-processes/ontology/OntoCAPE/upper_level/system.owl#hasSubsystem"/>
                        <owl:someValuesFrom rdf:resource="https://github.com/sustainable-processes/ontology/OntoCAPE/chemical_process_system/CPS_realization/plant.owl#Instrumentation"/>
                    </owl:Restriction>
                    <owl:Restriction>
                        <owl:onProperty rdf:resource="https://github.com/sustainable-processes/ontology/OntoCAPE/upper_level/system.owl#hasSubsystem"/>
                        <owl:someValuesFrom rdf:resource="https://github.com/sustainable-processes/ontology/OntoCAPE/chemical_process_system/CPS_realization/plant.owl#Piping"/>
                    </owl:Restriction>
                </owl:intersectionOf>
            </owl:Class>
        </owl:equivalentClass>
        <owl:disjointWith rdf:resource="https://github.com/sustainable-processes/ontology/OntoCAPE/chemical_process_system/CPS_realization/plant.owl#PieceOfEquipment"/>
        <rdfs:comment>A GroupOfEquipment is a Supersystem of Equipment that comprises of a number of Equipment, Piping and Instrumentation that realizes one or more CompositeProcessSteps.</rdfs:comment>
    </owl:Class>
    


    <!-- https://github.com/sustainable-processes/ontology/OntoCAPE/chemical_process_system/CPS_realization/plant.owl#HeatedLength -->

    <owl:Class rdf:about="https://github.com/sustainable-processes/ontology/OntoCAPE/chemical_process_system/CPS_realization/plant.owl#HeatedLength">
        <rdfs:subClassOf rdf:resource="https://github.com/sustainable-processes/ontology/OntoCAPE/supporting_concepts/geometry/geometry.owl#EdgeLength"/>
    </owl:Class>
    


    <!-- https://github.com/sustainable-processes/ontology/OntoCAPE/chemical_process_system/CPS_realization/plant.owl#HoleDiameter -->

    <owl:Class rdf:about="https://github.com/sustainable-processes/ontology/OntoCAPE/chemical_process_system/CPS_realization/plant.owl#HoleDiameter">
        <rdfs:subClassOf rdf:resource="https://github.com/sustainable-processes/ontology/OntoCAPE/supporting_concepts/geometry/geometry.owl#Diameter"/>
    </owl:Class>
    


    <!-- https://github.com/sustainable-processes/ontology/OntoCAPE/chemical_process_system/CPS_realization/plant.owl#InsideDiameter -->

    <owl:Class rdf:about="https://github.com/sustainable-processes/ontology/OntoCAPE/chemical_process_system/CPS_realization/plant.owl#InsideDiameter">
        <rdfs:subClassOf rdf:resource="https://github.com/sustainable-processes/ontology/OntoCAPE/supporting_concepts/geometry/geometry.owl#Diameter"/>
        <owl:disjointWith rdf:resource="https://github.com/sustainable-processes/ontology/OntoCAPE/chemical_process_system/CPS_realization/plant.owl#OutsideDiameter"/>
    </owl:Class>
    


    <!-- https://github.com/sustainable-processes/ontology/OntoCAPE/chemical_process_system/CPS_realization/plant.owl#Instrument -->

    <owl:Class rdf:about="https://github.com/sustainable-processes/ontology/OntoCAPE/chemical_process_system/CPS_realization/plant.owl#Instrument">
        <rdfs:subClassOf rdf:resource="https://github.com/sustainable-processes/ontology/OntoCAPE/chemical_process_system/CPS_realization/plant.owl#Instrumentation"/>
        <rdfs:subClassOf>
            <owl:Restriction>
                <owl:onProperty rdf:resource="https://github.com/sustainable-processes/ontology/OntoCAPE/chemical_process_system/CPS_realization/plant.owl#hasConnector"/>
                <owl:allValuesFrom rdf:resource="https://github.com/sustainable-processes/ontology/OntoCAPE/chemical_process_system/CPS_realization/plant.owl#InstrumentationConnection"/>
            </owl:Restriction>
        </rdfs:subClassOf>
        <rdfs:subClassOf>
            <owl:Restriction>
                <owl:onProperty rdf:resource="https://github.com/sustainable-processes/ontology/OntoCAPE/chemical_process_system/CPS_realization/plant.owl#hasConnector"/>
                <owl:maxCardinality rdf:datatype="http://www.w3.org/2001/XMLSchema#nonNegativeInteger">2</owl:maxCardinality>
            </owl:Restriction>
        </rdfs:subClassOf>
        <rdfs:comment>An Instrument is a devices used to measure or control multiple or complex material Properties.</rdfs:comment>
    </owl:Class>
    


    <!-- https://github.com/sustainable-processes/ontology/OntoCAPE/chemical_process_system/CPS_realization/plant.owl#Instrumentation -->

    <owl:Class rdf:about="https://github.com/sustainable-processes/ontology/OntoCAPE/chemical_process_system/CPS_realization/plant.owl#Instrumentation">
        <owl:equivalentClass>
            <owl:Class>
                <owl:unionOf rdf:parseType="Collection">
                    <rdf:Description rdf:about="https://github.com/sustainable-processes/ontology/OntoCAPE/chemical_process_system/CPS_realization/plant.owl#Instrument"/>
                    <rdf:Description rdf:about="https://github.com/sustainable-processes/ontology/OntoCAPE/chemical_process_system/CPS_realization/plant.owl#Loop"/>
                </owl:unionOf>
            </owl:Class>
        </owl:equivalentClass>
        <rdfs:subClassOf rdf:resource="https://github.com/sustainable-processes/ontology/OntoCAPE/chemical_process_system/CPS_realization/plant.owl#PlantItem"/>
        <owl:disjointWith rdf:resource="https://github.com/sustainable-processes/ontology/OntoCAPE/chemical_process_system/CPS_realization/plant.owl#Piping"/>
        <rdfs:comment>Instrumentation is about measuring and control. Instrumentation may comprise instruments as well as loops.</rdfs:comment>
    </owl:Class>
    


    <!-- https://github.com/sustainable-processes/ontology/OntoCAPE/chemical_process_system/CPS_realization/plant.owl#InstrumentationConnection -->

    <owl:Class rdf:about="https://github.com/sustainable-processes/ontology/OntoCAPE/chemical_process_system/CPS_realization/plant.owl#InstrumentationConnection">
        <rdfs:subClassOf rdf:resource="https://github.com/sustainable-processes/ontology/OntoCAPE/chemical_process_system/CPS_realization/plant.owl#PlantItemInterface"/>
        <rdfs:subClassOf>
            <owl:Restriction>
                <owl:onProperty rdf:resource="https://github.com/sustainable-processes/ontology/OntoCAPE/upper_level/system.owl#isDirectlyConnectedTo"/>
                <owl:allValuesFrom>
                    <owl:Class>
                        <owl:unionOf rdf:parseType="Collection">
                            <rdf:Description rdf:about="https://github.com/sustainable-processes/ontology/OntoCAPE/chemical_process_system/CPS_realization/plant.owl#Nozzle"/>
                            <rdf:Description rdf:about="https://github.com/sustainable-processes/ontology/OntoCAPE/chemical_process_system/CPS_realization/plant.owl#PipeSegmentEnd"/>
                        </owl:unionOf>
                    </owl:Class>
                </owl:allValuesFrom>
            </owl:Restriction>
        </rdfs:subClassOf>
        <rdfs:subClassOf>
            <owl:Restriction>
                <owl:onProperty rdf:resource="https://github.com/sustainable-processes/ontology/OntoCAPE/upper_level/system.owl#isDirectlyConnectedTo"/>
                <owl:maxCardinality rdf:datatype="http://www.w3.org/2001/XMLSchema#nonNegativeInteger">1</owl:maxCardinality>
            </owl:Restriction>
        </rdfs:subClassOf>
        <owl:disjointWith rdf:resource="https://github.com/sustainable-processes/ontology/OntoCAPE/chemical_process_system/CPS_realization/plant.owl#Nozzle"/>
        <owl:disjointWith rdf:resource="https://github.com/sustainable-processes/ontology/OntoCAPE/chemical_process_system/CPS_realization/plant.owl#PipeSegmentEnd"/>
    </owl:Class>
    


    <!-- https://github.com/sustainable-processes/ontology/OntoCAPE/chemical_process_system/CPS_realization/plant.owl#Loop -->

    <owl:Class rdf:about="https://github.com/sustainable-processes/ontology/OntoCAPE/chemical_process_system/CPS_realization/plant.owl#Loop">
        <rdfs:subClassOf rdf:resource="https://github.com/sustainable-processes/ontology/OntoCAPE/chemical_process_system/CPS_realization/plant.owl#Instrumentation"/>
        <rdfs:subClassOf>
            <owl:Restriction>
                <owl:onProperty rdf:resource="https://github.com/sustainable-processes/ontology/OntoCAPE/upper_level/system.owl#hasSubsystem"/>
                <owl:someValuesFrom rdf:resource="https://github.com/sustainable-processes/ontology/OntoCAPE/chemical_process_system/CPS_realization/plant.owl#Instrumentation"/>
            </owl:Restriction>
        </rdfs:subClassOf>
        <rdfs:comment>A Loop, including instruments, is arranged in such a fashion as to try to regulate a variable of a certain controlled system.</rdfs:comment>
    </owl:Class>
    


    <!-- https://github.com/sustainable-processes/ontology/OntoCAPE/chemical_process_system/CPS_realization/plant.owl#Machine -->

    <owl:Class rdf:about="https://github.com/sustainable-processes/ontology/OntoCAPE/chemical_process_system/CPS_realization/plant.owl#Machine">
        <rdfs:subClassOf rdf:resource="https://github.com/sustainable-processes/ontology/OntoCAPE/chemical_process_system/CPS_realization/plant.owl#PieceOfEquipment"/>
        <rdfs:subClassOf>
            <owl:Restriction>
                <owl:onProperty rdf:resource="https://github.com/sustainable-processes/ontology/OntoCAPE/chemical_process_system/CPS_realization/plant.owl#hasEfficiency"/>
                <owl:allValuesFrom rdf:resource="https://github.com/sustainable-processes/ontology/OntoCAPE/upper_level/system.owl#QuantitativeValue"/>
            </owl:Restriction>
        </rdfs:subClassOf>
        <rdfs:subClassOf>
            <owl:Restriction>
                <owl:onProperty rdf:resource="https://github.com/sustainable-processes/ontology/OntoCAPE/chemical_process_system/CPS_realization/plant.owl#hasPowerOutput"/>
                <owl:allValuesFrom rdf:resource="https://github.com/sustainable-processes/ontology/OntoCAPE/upper_level/system.owl#QuantitativeValue"/>
            </owl:Restriction>
        </rdfs:subClassOf>
        <rdfs:comment>A Machine is any mechanical or electrical device that transmits or modifies energy to perform or assist in the desired performance</rdfs:comment>
    </owl:Class>
    


    <!-- https://github.com/sustainable-processes/ontology/OntoCAPE/chemical_process_system/CPS_realization/plant.owl#Multiplicity -->

    <owl:Class rdf:about="https://github.com/sustainable-processes/ontology/OntoCAPE/chemical_process_system/CPS_realization/plant.owl#Multiplicity">
        <rdfs:subClassOf rdf:resource="https://github.com/sustainable-processes/ontology/meta_model/data_structures/multiset.owl#Multiplicity"/>
        <rdfs:subClassOf>
            <owl:Restriction>
                <owl:onProperty rdf:resource="https://github.com/sustainable-processes/ontology/OntoCAPE/chemical_process_system/CPS_realization/plant.owl#indicatesMultiplicityOf"/>
                <owl:someValuesFrom rdf:resource="https://github.com/sustainable-processes/ontology/OntoCAPE/chemical_process_system/CPS_realization/plant.owl#PlantItem"/>
            </owl:Restriction>
        </rdfs:subClassOf>
        <rdfs:subClassOf>
            <owl:Restriction>
                <owl:onProperty rdf:resource="https://github.com/sustainable-processes/ontology/OntoCAPE/chemical_process_system/CPS_realization/plant.owl#indicatesMultiplicityOf"/>
                <owl:allValuesFrom rdf:resource="https://github.com/sustainable-processes/ontology/OntoCAPE/chemical_process_system/CPS_realization/plant.owl#PlantItem"/>
            </owl:Restriction>
        </rdfs:subClassOf>
        <rdfs:subClassOf>
            <owl:Restriction>
                <owl:onProperty rdf:resource="https://github.com/sustainable-processes/ontology/OntoCAPE/chemical_process_system/CPS_realization/plant.owl#indicatesMultiplicityOf"/>
                <owl:cardinality rdf:datatype="http://www.w3.org/2001/XMLSchema#nonNegativeInteger">1</owl:cardinality>
            </owl:Restriction>
        </rdfs:subClassOf>
        <rdfs:subClassOf>
            <owl:Restriction>
                <owl:onProperty rdf:resource="https://github.com/sustainable-processes/ontology/OntoCAPE/chemical_process_system/CPS_realization/plant.owl#multiplicity"/>
                <owl:cardinality rdf:datatype="http://www.w3.org/2001/XMLSchema#nonNegativeInteger">1</owl:cardinality>
            </owl:Restriction>
        </rdfs:subClassOf>
    </owl:Class>
    


    <!-- https://github.com/sustainable-processes/ontology/OntoCAPE/chemical_process_system/CPS_realization/plant.owl#Nozzle -->

    <owl:Class rdf:about="https://github.com/sustainable-processes/ontology/OntoCAPE/chemical_process_system/CPS_realization/plant.owl#Nozzle">
        <rdfs:subClassOf rdf:resource="https://github.com/sustainable-processes/ontology/OntoCAPE/chemical_process_system/CPS_realization/plant.owl#PlantItemInterface"/>
        <rdfs:subClassOf>
            <owl:Restriction>
                <owl:onProperty rdf:resource="https://github.com/sustainable-processes/ontology/OntoCAPE/upper_level/system.owl#isDirectlyConnectedTo"/>
                <owl:allValuesFrom>
                    <owl:Class>
                        <owl:unionOf rdf:parseType="Collection">
                            <rdf:Description rdf:about="https://github.com/sustainable-processes/ontology/OntoCAPE/chemical_process_system/CPS_realization/plant.owl#InstrumentationConnection"/>
                            <rdf:Description rdf:about="https://github.com/sustainable-processes/ontology/OntoCAPE/chemical_process_system/CPS_realization/plant.owl#PipeSegmentEnd"/>
                        </owl:unionOf>
                    </owl:Class>
                </owl:allValuesFrom>
            </owl:Restriction>
        </rdfs:subClassOf>
        <rdfs:subClassOf>
            <owl:Restriction>
                <owl:onProperty rdf:resource="https://github.com/sustainable-processes/ontology/OntoCAPE/upper_level/system.owl#isDirectlyConnectedTo"/>
                <owl:maxCardinality rdf:datatype="http://www.w3.org/2001/XMLSchema#nonNegativeInteger">1</owl:maxCardinality>
            </owl:Restriction>
        </rdfs:subClassOf>
        <owl:disjointWith rdf:resource="https://github.com/sustainable-processes/ontology/OntoCAPE/chemical_process_system/CPS_realization/plant.owl#PipeSegmentEnd"/>
        <rdfs:comment>A Nozzle represents the interface through which a plant item that owns it can be connected to another PlantItem or to the environment of a Plant.</rdfs:comment>
    </owl:Class>
    


    <!-- https://github.com/sustainable-processes/ontology/OntoCAPE/chemical_process_system/CPS_realization/plant.owl#OutsideDiameter -->

    <owl:Class rdf:about="https://github.com/sustainable-processes/ontology/OntoCAPE/chemical_process_system/CPS_realization/plant.owl#OutsideDiameter">
        <rdfs:subClassOf rdf:resource="https://github.com/sustainable-processes/ontology/OntoCAPE/supporting_concepts/geometry/geometry.owl#Diameter"/>
    </owl:Class>
    


    <!-- https://github.com/sustainable-processes/ontology/OntoCAPE/chemical_process_system/CPS_realization/plant.owl#PieceOfEquipment -->

    <owl:Class rdf:about="https://github.com/sustainable-processes/ontology/OntoCAPE/chemical_process_system/CPS_realization/plant.owl#PieceOfEquipment">
        <rdfs:subClassOf rdf:resource="https://github.com/sustainable-processes/ontology/OntoCAPE/chemical_process_system/CPS_realization/plant.owl#Equipment"/>
        <rdfs:subClassOf>
            <owl:Restriction>
                <owl:onProperty rdf:resource="https://github.com/sustainable-processes/ontology/OntoCAPE/chemical_process_system/CPS_realization/plant.owl#hasConnector"/>
                <owl:allValuesFrom rdf:resource="https://github.com/sustainable-processes/ontology/OntoCAPE/chemical_process_system/CPS_realization/plant.owl#Nozzle"/>
            </owl:Restriction>
        </rdfs:subClassOf>
        <rdfs:subClassOf>
            <owl:Restriction>
                <owl:onProperty rdf:resource="https://github.com/sustainable-processes/ontology/OntoCAPE/chemical_process_system/CPS_realization/plant.owl#hasFixture"/>
                <owl:allValuesFrom rdf:resource="https://github.com/sustainable-processes/ontology/OntoCAPE/chemical_process_system/CPS_realization/plant.owl#Fixture"/>
            </owl:Restriction>
        </rdfs:subClassOf>
        <rdfs:comment>A PieceOfEquipment is an elementary unit in the sense that it does not include other Equipments or Pipes.</rdfs:comment>
    </owl:Class>
    


    <!-- https://github.com/sustainable-processes/ontology/OntoCAPE/chemical_process_system/CPS_realization/plant.owl#Pipe -->

    <owl:Class rdf:about="https://github.com/sustainable-processes/ontology/OntoCAPE/chemical_process_system/CPS_realization/plant.owl#Pipe">
        <owl:equivalentClass>
            <owl:Class>
                <owl:intersectionOf rdf:parseType="Collection">
                    <rdf:Description rdf:about="https://github.com/sustainable-processes/ontology/OntoCAPE/chemical_process_system/CPS_realization/plant.owl#Piping"/>
                    <owl:Class>
                        <owl:unionOf rdf:parseType="Collection">
                            <owl:Class>
                                <owl:intersectionOf rdf:parseType="Collection">
                                    <owl:Restriction>
                                        <owl:onProperty rdf:resource="https://github.com/sustainable-processes/ontology/OntoCAPE/upper_level/system.owl#hasDirectSubsystem"/>
                                        <owl:someValuesFrom rdf:resource="https://github.com/sustainable-processes/ontology/OntoCAPE/chemical_process_system/CPS_realization/plant.owl#PipeSegment"/>
                                    </owl:Restriction>
                                    <owl:Restriction>
                                        <owl:onProperty rdf:resource="https://github.com/sustainable-processes/ontology/OntoCAPE/upper_level/system.owl#hasSubsystem"/>
                                        <owl:someValuesFrom rdf:resource="https://github.com/sustainable-processes/ontology/OntoCAPE/chemical_process_system/CPS_realization/plant.owl#Instrument"/>
                                    </owl:Restriction>
                                </owl:intersectionOf>
                            </owl:Class>
                            <owl:Restriction>
                                <owl:onProperty rdf:resource="https://github.com/sustainable-processes/ontology/OntoCAPE/upper_level/system.owl#hasDirectSubsystem"/>
                                <owl:someValuesFrom rdf:resource="https://github.com/sustainable-processes/ontology/OntoCAPE/chemical_process_system/CPS_realization/plant.owl#PipeSegment"/>
                            </owl:Restriction>
                        </owl:unionOf>
                    </owl:Class>
                </owl:intersectionOf>
            </owl:Class>
        </owl:equivalentClass>
        <owl:disjointWith rdf:resource="https://github.com/sustainable-processes/ontology/OntoCAPE/chemical_process_system/CPS_realization/plant.owl#PipeFitting"/>
        <owl:disjointWith rdf:resource="https://github.com/sustainable-processes/ontology/OntoCAPE/chemical_process_system/CPS_realization/plant.owl#PipeSegment"/>
        <owl:disjointWith rdf:resource="https://github.com/sustainable-processes/ontology/OntoCAPE/chemical_process_system/CPS_realization/plant.owl#PipingNetwork"/>
        <rdfs:comment>A Pipe can be used to connect one PlantItem to another PlantItem or to the environment of a Plant.</rdfs:comment>
    </owl:Class>
    


    <!-- https://github.com/sustainable-processes/ontology/OntoCAPE/chemical_process_system/CPS_realization/plant.owl#PipeFitting -->

    <owl:Class rdf:about="https://github.com/sustainable-processes/ontology/OntoCAPE/chemical_process_system/CPS_realization/plant.owl#PipeFitting">
        <rdfs:subClassOf rdf:resource="https://github.com/sustainable-processes/ontology/OntoCAPE/chemical_process_system/CPS_realization/plant.owl#Piping"/>
        <owl:disjointWith rdf:resource="https://github.com/sustainable-processes/ontology/OntoCAPE/chemical_process_system/CPS_realization/plant.owl#PipeSegment"/>
        <owl:disjointWith rdf:resource="https://github.com/sustainable-processes/ontology/OntoCAPE/chemical_process_system/CPS_realization/plant.owl#PipingNetwork"/>
        <rdfs:comment>Fittings are used in PipingNetworks to connect straight Pipe sections, to adapt to different sizes or shapes or forking of Piping.</rdfs:comment>
    </owl:Class>
    


    <!-- https://github.com/sustainable-processes/ontology/OntoCAPE/chemical_process_system/CPS_realization/plant.owl#PipeSegment -->

    <owl:Class rdf:about="https://github.com/sustainable-processes/ontology/OntoCAPE/chemical_process_system/CPS_realization/plant.owl#PipeSegment">
        <rdfs:subClassOf rdf:resource="https://github.com/sustainable-processes/ontology/OntoCAPE/chemical_process_system/CPS_realization/plant.owl#Piping"/>
        <rdfs:subClassOf>
            <owl:Restriction>
                <owl:onProperty rdf:resource="https://github.com/sustainable-processes/ontology/OntoCAPE/chemical_process_system/CPS_realization/plant.owl#hasConnector"/>
                <owl:allValuesFrom rdf:resource="https://github.com/sustainable-processes/ontology/OntoCAPE/chemical_process_system/CPS_realization/plant.owl#PipeSegmentEnd"/>
            </owl:Restriction>
        </rdfs:subClassOf>
        <rdfs:subClassOf>
            <owl:Restriction>
                <owl:onProperty rdf:resource="https://github.com/sustainable-processes/ontology/OntoCAPE/chemical_process_system/CPS_realization/plant.owl#hasConnector"/>
                <owl:cardinality rdf:datatype="http://www.w3.org/2001/XMLSchema#nonNegativeInteger">2</owl:cardinality>
            </owl:Restriction>
        </rdfs:subClassOf>
        <owl:disjointWith rdf:resource="https://github.com/sustainable-processes/ontology/OntoCAPE/chemical_process_system/CPS_realization/plant.owl#PipingNetwork"/>
        <rdfs:comment>A PipeSegment is the elementary part of Piping. A Pipe is assembled of a number of PipeSegments.</rdfs:comment>
    </owl:Class>
    


    <!-- https://github.com/sustainable-processes/ontology/OntoCAPE/chemical_process_system/CPS_realization/plant.owl#PipeSegmentEnd -->

    <owl:Class rdf:about="https://github.com/sustainable-processes/ontology/OntoCAPE/chemical_process_system/CPS_realization/plant.owl#PipeSegmentEnd">
        <rdfs:subClassOf rdf:resource="https://github.com/sustainable-processes/ontology/OntoCAPE/chemical_process_system/CPS_realization/plant.owl#PlantItemInterface"/>
        <rdfs:subClassOf>
            <owl:Restriction>
                <owl:onProperty rdf:resource="https://github.com/sustainable-processes/ontology/OntoCAPE/upper_level/system.owl#isDirectlyConnectedTo"/>
                <owl:allValuesFrom>
                    <owl:Class>
                        <owl:unionOf rdf:parseType="Collection">
                            <rdf:Description rdf:about="https://github.com/sustainable-processes/ontology/OntoCAPE/chemical_process_system/CPS_realization/plant.owl#InstrumentationConnection"/>
                            <rdf:Description rdf:about="https://github.com/sustainable-processes/ontology/OntoCAPE/chemical_process_system/CPS_realization/plant.owl#Nozzle"/>
                            <rdf:Description rdf:about="https://github.com/sustainable-processes/ontology/OntoCAPE/chemical_process_system/CPS_realization/plant.owl#PipeSegmentEnd"/>
                        </owl:unionOf>
                    </owl:Class>
                </owl:allValuesFrom>
            </owl:Restriction>
        </rdfs:subClassOf>
        <rdfs:subClassOf>
            <owl:Restriction>
                <owl:onProperty rdf:resource="https://github.com/sustainable-processes/ontology/OntoCAPE/upper_level/system.owl#isDirectlyConnectedTo"/>
                <owl:maxCardinality rdf:datatype="http://www.w3.org/2001/XMLSchema#nonNegativeInteger">1</owl:maxCardinality>
            </owl:Restriction>
        </rdfs:subClassOf>
        <rdfs:comment>A PipeSegmentEnd is an on or off-page Connector  to an other Pipe, PieceOfEquipment or Instrumentation.</rdfs:comment>
    </owl:Class>
    


    <!-- https://github.com/sustainable-processes/ontology/OntoCAPE/chemical_process_system/CPS_realization/plant.owl#Piping -->

    <owl:Class rdf:about="https://github.com/sustainable-processes/ontology/OntoCAPE/chemical_process_system/CPS_realization/plant.owl#Piping">
        <owl:equivalentClass>
            <owl:Class>
                <owl:unionOf rdf:parseType="Collection">
                    <rdf:Description rdf:about="https://github.com/sustainable-processes/ontology/OntoCAPE/chemical_process_system/CPS_realization/plant.owl#Pipe"/>
                    <rdf:Description rdf:about="https://github.com/sustainable-processes/ontology/OntoCAPE/chemical_process_system/CPS_realization/plant.owl#PipeFitting"/>
                    <rdf:Description rdf:about="https://github.com/sustainable-processes/ontology/OntoCAPE/chemical_process_system/CPS_realization/plant.owl#PipeSegment"/>
                    <rdf:Description rdf:about="https://github.com/sustainable-processes/ontology/OntoCAPE/chemical_process_system/CPS_realization/plant.owl#PipingNetwork"/>
                </owl:unionOf>
            </owl:Class>
        </owl:equivalentClass>
        <rdfs:subClassOf rdf:resource="https://github.com/sustainable-processes/ontology/OntoCAPE/chemical_process_system/CPS_realization/plant.owl#PlantItem"/>
        <rdfs:comment>A Piping is a plant item which is used for fluid transport. It may connect Equipment or/and Instruments.</rdfs:comment>
    </owl:Class>
    


    <!-- https://github.com/sustainable-processes/ontology/OntoCAPE/chemical_process_system/CPS_realization/plant.owl#PipingNetwork -->

    <owl:Class rdf:about="https://github.com/sustainable-processes/ontology/OntoCAPE/chemical_process_system/CPS_realization/plant.owl#PipingNetwork">
        <owl:equivalentClass>
            <owl:Class>
                <owl:intersectionOf rdf:parseType="Collection">
                    <rdf:Description rdf:about="https://github.com/sustainable-processes/ontology/OntoCAPE/chemical_process_system/CPS_realization/plant.owl#Piping"/>
                    <owl:Class>
                        <owl:unionOf rdf:parseType="Collection">
                            <owl:Class>
                                <owl:intersectionOf rdf:parseType="Collection">
                                    <owl:Restriction>
                                        <owl:onProperty rdf:resource="https://github.com/sustainable-processes/ontology/OntoCAPE/upper_level/system.owl#hasSubsystem"/>
                                        <owl:someValuesFrom rdf:resource="https://github.com/sustainable-processes/ontology/OntoCAPE/chemical_process_system/CPS_realization/plant.owl#Pipe"/>
                                    </owl:Restriction>
                                    <owl:Restriction>
                                        <owl:onProperty rdf:resource="https://github.com/sustainable-processes/ontology/OntoCAPE/upper_level/system.owl#hasSubsystem"/>
                                        <owl:someValuesFrom rdf:resource="https://github.com/sustainable-processes/ontology/OntoCAPE/chemical_process_system/CPS_realization/plant.owl#PipeFitting"/>
                                    </owl:Restriction>
                                </owl:intersectionOf>
                            </owl:Class>
                            <owl:Restriction>
                                <owl:onProperty rdf:resource="https://github.com/sustainable-processes/ontology/OntoCAPE/upper_level/system.owl#hasSubsystem"/>
                                <owl:someValuesFrom rdf:resource="https://github.com/sustainable-processes/ontology/OntoCAPE/chemical_process_system/CPS_realization/plant.owl#Pipe"/>
                            </owl:Restriction>
                        </owl:unionOf>
                    </owl:Class>
                </owl:intersectionOf>
            </owl:Class>
        </owl:equivalentClass>
        <rdfs:subClassOf>
            <owl:Restriction>
                <owl:onProperty rdf:resource="https://github.com/sustainable-processes/ontology/OntoCAPE/upper_level/system.owl#hasSubsystem"/>
                <owl:someValuesFrom rdf:resource="https://github.com/sustainable-processes/ontology/OntoCAPE/chemical_process_system/CPS_realization/plant.owl#PipingNetwork"/>
            </owl:Restriction>
        </rdfs:subClassOf>
        <rdfs:comment>A PipingNetwork is an agglomeration of Pipes and PipeFittings used to connect multiple PiecesOfEquipment.</rdfs:comment>
    </owl:Class>
    


    <!-- https://github.com/sustainable-processes/ontology/OntoCAPE/chemical_process_system/CPS_realization/plant.owl#Plant -->

    <owl:Class rdf:about="https://github.com/sustainable-processes/ontology/OntoCAPE/chemical_process_system/CPS_realization/plant.owl#Plant">
        <rdfs:subClassOf rdf:resource="https://github.com/sustainable-processes/ontology/OntoCAPE/chemical_process_system/CPS_realization/plant.owl#GroupOfEquipment"/>
        <rdfs:subClassOf>
            <owl:Restriction>
                <owl:onProperty rdf:resource="https://github.com/sustainable-processes/ontology/OntoCAPE/upper_level/system.owl#isExclusivelySubsystemOf"/>
                <owl:cardinality rdf:datatype="http://www.w3.org/2001/XMLSchema#nonNegativeInteger">0</owl:cardinality>
            </owl:Restriction>
        </rdfs:subClassOf>
        <rdfs:label>Plant</rdfs:label>
    </owl:Class>
    


    <!-- https://github.com/sustainable-processes/ontology/OntoCAPE/chemical_process_system/CPS_realization/plant.owl#PlantItem -->

    <owl:Class rdf:about="https://github.com/sustainable-processes/ontology/OntoCAPE/chemical_process_system/CPS_realization/plant.owl#PlantItem">
        <rdfs:subClassOf rdf:resource="https://github.com/sustainable-processes/ontology/OntoCAPE/upper_level/system.owl#System"/>
        <rdfs:subClassOf>
            <owl:Restriction>
                <owl:onProperty rdf:resource="https://github.com/sustainable-processes/ontology/OntoCAPE/chemical_process_system/CPS_realization/plant.owl#hasConstructionMaterial"/>
                <owl:someValuesFrom rdf:resource="https://github.com/sustainable-processes/ontology/OntoCAPE/material/substance/substance.owl#Substance"/>
            </owl:Restriction>
        </rdfs:subClassOf>
        <rdfs:subClassOf>
            <owl:Restriction>
                <owl:onProperty rdf:resource="https://github.com/sustainable-processes/ontology/OntoCAPE/supporting_concepts/geometry/geometry.owl#hasShapeRepresentation"/>
                <owl:allValuesFrom rdf:resource="https://github.com/sustainable-processes/ontology/OntoCAPE/supporting_concepts/geometry/geometry.owl#Solid"/>
            </owl:Restriction>
        </rdfs:subClassOf>
        <rdfs:subClassOf>
            <owl:Restriction>
                <owl:onProperty rdf:resource="https://github.com/sustainable-processes/ontology/OntoCAPE/upper_level/system.owl#isDirectlyConnectedTo"/>
                <owl:allValuesFrom rdf:resource="https://github.com/sustainable-processes/ontology/OntoCAPE/chemical_process_system/CPS_realization/plant.owl#PlantItem"/>
            </owl:Restriction>
        </rdfs:subClassOf>
        <rdfs:comment>A PlantItem is an object which exists, in a material form, in a ChemicalProcessSystem and in which one or more ProcessSteps could be performed.</rdfs:comment>
    </owl:Class>
    


    <!-- https://github.com/sustainable-processes/ontology/OntoCAPE/chemical_process_system/CPS_realization/plant.owl#PlantItemInterface -->

    <owl:Class rdf:about="https://github.com/sustainable-processes/ontology/OntoCAPE/chemical_process_system/CPS_realization/plant.owl#PlantItemInterface">
        <rdfs:subClassOf rdf:resource="https://github.com/sustainable-processes/ontology/OntoCAPE/upper_level/system.owl#SystemInterface"/>
    </owl:Class>
    


    <!-- https://github.com/sustainable-processes/ontology/OntoCAPE/chemical_process_system/CPS_realization/plant.owl#PlantItemProperty -->

    <owl:Class rdf:about="https://github.com/sustainable-processes/ontology/OntoCAPE/chemical_process_system/CPS_realization/plant.owl#PlantItemProperty">
        <rdfs:subClassOf rdf:resource="https://github.com/sustainable-processes/ontology/OntoCAPE/upper_level/system.owl#Property"/>
    </owl:Class>
    


    <!-- https://github.com/sustainable-processes/ontology/OntoCAPE/chemical_process_system/CPS_realization/plant.owl#WeirHeight -->

    <owl:Class rdf:about="https://github.com/sustainable-processes/ontology/OntoCAPE/chemical_process_system/CPS_realization/plant.owl#WeirHeight">
        <rdfs:subClassOf rdf:resource="https://github.com/sustainable-processes/ontology/OntoCAPE/supporting_concepts/geometry/geometry.owl#Height"/>
    </owl:Class>
</rdf:RDF>



<!-- Generated by the OWL API (version 4.5.26.2023-07-17T20:34:13Z) https://github.com/owlcs/owlapi -->

