<?xml version="1.0"?>
<rdf:RDF xmlns="https://github.com/sustainable-processes/ontology/OntoCAPE/chemical_process_system/CPS_realization/process_control_equipment/measuring_instrument.owl#"
     xml:base="https://github.com/sustainable-processes/ontology/OntoCAPE/chemical_process_system/CPS_realization/process_control_equipment/measuring_instrument.owl"
     xmlns:owl="http://www.w3.org/2002/07/owl#"
     xmlns:rdf="http://www.w3.org/1999/02/22-rdf-syntax-ns#"
     xmlns:xml="http://www.w3.org/XML/1998/namespace"
     xmlns:xsd="http://www.w3.org/2001/XMLSchema#"
     xmlns:rdfs="http://www.w3.org/2000/01/rdf-schema#"
     xmlns:root="https://github.com/sustainable-processes/ontology/OntoCAPE/"
     xmlns:terms="http://purl.org/dc/terms/"
     xmlns:pro_con_sys="https://github.com/sustainable-processes/ontology/OntoCAPE/chemical_process_system/CPS_realization/process_control_system.owl#">
    <owl:Ontology rdf:about="https://github.com/sustainable-processes/ontology/OntoCAPE/chemical_process_system/CPS_realization/process_control_equipment/measuring_instrument.owl">
        <owl:imports rdf:resource="https://github.com/sustainable-processes/ontology/OntoCAPE/chemical_process_system/CPS_realization/process_control_system.owl"/>
        <terms:license>Copyright (C) [2009] [Andreas Wiesner]
                This program is free software; you can redistribute it and/or modify it under the terms of the GNU General Public License as published by the Free Software Foundation; either version 3 of the License, or (at your option) any later version.
                This program is distributed in the hope that it will be useful, but WITHOUT ANY WARRANTY; without even the implied warranty of MERCHANTABILITY or FITNESS FOR A PARTICULAR PURPOSE. See the GNU General Public License for more details.
                You should have received a copy of the GNU General Public License along with this program; if not, see &lt;http://www.gnu.org/licenses/&gt;.
    </terms:license>
        <rdfs:comment>The ontology module &apos;measuring_instrument&apos; provides specializations for measuring instruments that are applicable to chemical process systems.
The following classes and relations from other ontology modules are used within &apos;measuring_instrument&apos;:

&lt;owl:Class rdf:about=&quot;https://github.com/sustainable-processes/ontology/OntoCAPE/chemical_process_system/CPS_realization/process_control_system.owl#MeasuringInstrument&quot;/&gt;
    </rdfs:comment>
        <owl:versionInfo>2.0</owl:versionInfo>
    </owl:Ontology>
    


    <!-- 
    ///////////////////////////////////////////////////////////////////////////////////////
    //
    // Annotation properties
    //
    ///////////////////////////////////////////////////////////////////////////////////////
     -->

    


    <!-- http://purl.org/dc/terms/license -->

    <owl:AnnotationProperty rdf:about="http://purl.org/dc/terms/license"/>
    


    <!-- 
    ///////////////////////////////////////////////////////////////////////////////////////
    //
    // Classes
    //
    ///////////////////////////////////////////////////////////////////////////////////////
     -->

    


    <!-- https://github.com/sustainable-processes/ontology/OntoCAPE/chemical_process_system/CPS_realization/process_control_equipment/measuring_instrument.owl#BimetalT-Sensor -->

    <owl:Class rdf:about="https://github.com/sustainable-processes/ontology/OntoCAPE/chemical_process_system/CPS_realization/process_control_equipment/measuring_instrument.owl#BimetalT-Sensor">
        <rdfs:subClassOf rdf:resource="https://github.com/sustainable-processes/ontology/OntoCAPE/chemical_process_system/CPS_realization/process_control_equipment/measuring_instrument.owl#T-Sensor"/>
        <rdfs:comment>BimetalT-sensor is a specific type of temperature measuring sensor.</rdfs:comment>
    </owl:Class>
    


    <!-- https://github.com/sustainable-processes/ontology/OntoCAPE/chemical_process_system/CPS_realization/process_control_equipment/measuring_instrument.owl#ExpansionT-Sensor -->

    <owl:Class rdf:about="https://github.com/sustainable-processes/ontology/OntoCAPE/chemical_process_system/CPS_realization/process_control_equipment/measuring_instrument.owl#ExpansionT-Sensor">
        <rdfs:subClassOf rdf:resource="https://github.com/sustainable-processes/ontology/OntoCAPE/chemical_process_system/CPS_realization/process_control_equipment/measuring_instrument.owl#T-Sensor"/>
        <rdfs:comment>ExpansionT-sensor is a specific type of temperature measuring sensor.</rdfs:comment>
    </owl:Class>
    


    <!-- https://github.com/sustainable-processes/ontology/OntoCAPE/chemical_process_system/CPS_realization/process_control_equipment/measuring_instrument.owl#F-Sensor -->

    <owl:Class rdf:about="https://github.com/sustainable-processes/ontology/OntoCAPE/chemical_process_system/CPS_realization/process_control_equipment/measuring_instrument.owl#F-Sensor">
        <rdfs:subClassOf rdf:resource="https://github.com/sustainable-processes/ontology/OntoCAPE/chemical_process_system/CPS_realization/process_control_system.owl#MeasuringInstrument"/>
        <rdfs:comment>F-sensor is applied for flow measuring.</rdfs:comment>
    </owl:Class>
    


    <!-- https://github.com/sustainable-processes/ontology/OntoCAPE/chemical_process_system/CPS_realization/process_control_equipment/measuring_instrument.owl#L-Sensor -->

    <owl:Class rdf:about="https://github.com/sustainable-processes/ontology/OntoCAPE/chemical_process_system/CPS_realization/process_control_equipment/measuring_instrument.owl#L-Sensor">
        <rdfs:subClassOf rdf:resource="https://github.com/sustainable-processes/ontology/OntoCAPE/chemical_process_system/CPS_realization/process_control_system.owl#MeasuringInstrument"/>
        <rdfs:comment>L-sensor is applied for level measuring.</rdfs:comment>
    </owl:Class>
    


    <!-- https://github.com/sustainable-processes/ontology/OntoCAPE/chemical_process_system/CPS_realization/process_control_equipment/measuring_instrument.owl#P-Sensor -->

    <owl:Class rdf:about="https://github.com/sustainable-processes/ontology/OntoCAPE/chemical_process_system/CPS_realization/process_control_equipment/measuring_instrument.owl#P-Sensor">
        <rdfs:subClassOf rdf:resource="https://github.com/sustainable-processes/ontology/OntoCAPE/chemical_process_system/CPS_realization/process_control_system.owl#MeasuringInstrument"/>
        <rdfs:comment>P-sensor is applied for preasure measuring.</rdfs:comment>
    </owl:Class>
    


    <!-- https://github.com/sustainable-processes/ontology/OntoCAPE/chemical_process_system/CPS_realization/process_control_equipment/measuring_instrument.owl#Pt100 -->

    <owl:Class rdf:about="https://github.com/sustainable-processes/ontology/OntoCAPE/chemical_process_system/CPS_realization/process_control_equipment/measuring_instrument.owl#Pt100">
        <rdfs:subClassOf rdf:resource="https://github.com/sustainable-processes/ontology/OntoCAPE/chemical_process_system/CPS_realization/process_control_equipment/measuring_instrument.owl#T-Sensor"/>
        <rdfs:comment>Pt100 is a specific type of temperature measuring sensor.</rdfs:comment>
    </owl:Class>
    


    <!-- https://github.com/sustainable-processes/ontology/OntoCAPE/chemical_process_system/CPS_realization/process_control_equipment/measuring_instrument.owl#Pyrometer -->

    <owl:Class rdf:about="https://github.com/sustainable-processes/ontology/OntoCAPE/chemical_process_system/CPS_realization/process_control_equipment/measuring_instrument.owl#Pyrometer">
        <rdfs:subClassOf rdf:resource="https://github.com/sustainable-processes/ontology/OntoCAPE/chemical_process_system/CPS_realization/process_control_equipment/measuring_instrument.owl#T-Sensor"/>
        <rdfs:comment>Pyrometer is a specific type of temperature measuring sensor.</rdfs:comment>
    </owl:Class>
    


    <!-- https://github.com/sustainable-processes/ontology/OntoCAPE/chemical_process_system/CPS_realization/process_control_equipment/measuring_instrument.owl#Q-Sensor -->

    <owl:Class rdf:about="https://github.com/sustainable-processes/ontology/OntoCAPE/chemical_process_system/CPS_realization/process_control_equipment/measuring_instrument.owl#Q-Sensor">
        <rdfs:subClassOf rdf:resource="https://github.com/sustainable-processes/ontology/OntoCAPE/chemical_process_system/CPS_realization/process_control_system.owl#MeasuringInstrument"/>
        <rdfs:comment>Q-sensor is applied for quality measuring (quality quantity, like concentration, conductivity).</rdfs:comment>
    </owl:Class>
    


    <!-- https://github.com/sustainable-processes/ontology/OntoCAPE/chemical_process_system/CPS_realization/process_control_equipment/measuring_instrument.owl#QuartzCristalT-Sensor -->

    <owl:Class rdf:about="https://github.com/sustainable-processes/ontology/OntoCAPE/chemical_process_system/CPS_realization/process_control_equipment/measuring_instrument.owl#QuartzCristalT-Sensor">
        <rdfs:subClassOf rdf:resource="https://github.com/sustainable-processes/ontology/OntoCAPE/chemical_process_system/CPS_realization/process_control_equipment/measuring_instrument.owl#T-Sensor"/>
        <rdfs:comment>QuartzCrystalT-sensor is a specific type of temperature measuring sensor.</rdfs:comment>
    </owl:Class>
    


    <!-- https://github.com/sustainable-processes/ontology/OntoCAPE/chemical_process_system/CPS_realization/process_control_equipment/measuring_instrument.owl#SegerCone -->

    <owl:Class rdf:about="https://github.com/sustainable-processes/ontology/OntoCAPE/chemical_process_system/CPS_realization/process_control_equipment/measuring_instrument.owl#SegerCone">
        <rdfs:subClassOf rdf:resource="https://github.com/sustainable-processes/ontology/OntoCAPE/chemical_process_system/CPS_realization/process_control_equipment/measuring_instrument.owl#T-Sensor"/>
        <rdfs:comment>SegerCone is a specific type of temperature measuring sensor.</rdfs:comment>
    </owl:Class>
    


    <!-- https://github.com/sustainable-processes/ontology/OntoCAPE/chemical_process_system/CPS_realization/process_control_equipment/measuring_instrument.owl#T-Sensor -->

    <owl:Class rdf:about="https://github.com/sustainable-processes/ontology/OntoCAPE/chemical_process_system/CPS_realization/process_control_equipment/measuring_instrument.owl#T-Sensor">
        <rdfs:subClassOf rdf:resource="https://github.com/sustainable-processes/ontology/OntoCAPE/chemical_process_system/CPS_realization/process_control_system.owl#MeasuringInstrument"/>
        <rdfs:comment>T-sensor is applied for temperature measuring.</rdfs:comment>
    </owl:Class>
    


    <!-- https://github.com/sustainable-processes/ontology/OntoCAPE/chemical_process_system/CPS_realization/process_control_equipment/measuring_instrument.owl#Thermocouple -->

    <owl:Class rdf:about="https://github.com/sustainable-processes/ontology/OntoCAPE/chemical_process_system/CPS_realization/process_control_equipment/measuring_instrument.owl#Thermocouple">
        <rdfs:subClassOf rdf:resource="https://github.com/sustainable-processes/ontology/OntoCAPE/chemical_process_system/CPS_realization/process_control_equipment/measuring_instrument.owl#T-Sensor"/>
        <rdfs:comment>Thermocouple is a specific type of temperature measuring sensor.</rdfs:comment>
    </owl:Class>
    


    <!-- https://github.com/sustainable-processes/ontology/OntoCAPE/chemical_process_system/CPS_realization/process_control_system.owl#MeasuringInstrument -->

    <owl:Class rdf:about="https://github.com/sustainable-processes/ontology/OntoCAPE/chemical_process_system/CPS_realization/process_control_system.owl#MeasuringInstrument"/>
</rdf:RDF>



<!-- Generated by the OWL API (version 4.5.26.2023-07-17T20:34:13Z) https://github.com/owlcs/owlapi -->

