<?xml version="1.0"?>
<rdf:RDF xmlns="https://raw.githubusercontent.com/sustainable-processes/ontology/refs/heads/main/OntoCAPE/chemical_process_system/CPS_function/process_control.owl#"
     xml:base="https://raw.githubusercontent.com/sustainable-processes/ontology/refs/heads/main/OntoCAPE/chemical_process_system/CPS_function/process_control.owl"
     xmlns:fc="https://raw.githubusercontent.com/sustainable-processes/ontology/refs/heads/main/meta_model/fundamental_concepts/fundamental_concepts.owl"
     xmlns:owl="http://www.w3.org/2002/07/owl#"
     xmlns:rdf="http://www.w3.org/1999/02/22-rdf-syntax-ns#"
     xmlns:xml="http://www.w3.org/XML/1998/namespace"
     xmlns:xsd="http://www.w3.org/2001/XMLSchema#"
     xmlns:rdfs="http://www.w3.org/2000/01/rdf-schema#"
     xmlns:root="https://raw.githubusercontent.com/sustainable-processes/ontology/refs/heads/main/OntoCAPE/"
     xmlns:array="https://raw.githubusercontent.com/sustainable-processes/ontology/refs/heads/main/meta_model/data_structures/array.owl#"
     xmlns:terms="http://purl.org/dc/terms/"
     xmlns:system="https://raw.githubusercontent.com/sustainable-processes/ontology/refs/heads/main/OntoCAPE/upper_level/system.owl#"
     xmlns:process="https://raw.githubusercontent.com/sustainable-processes/ontology/refs/heads/main/OntoCAPE/chemical_process_system/CPS_function/process.owl#"
     xmlns:multiset="https://raw.githubusercontent.com/sustainable-processes/ontology/refs/heads/main/meta_model/data_structures/multiset.owl#"
     xmlns:network_system="https://raw.githubusercontent.com/sustainable-processes/ontology/refs/heads/main/OntoCAPE/upper_level/network_system.owl#"
     xmlns:process_control="https://raw.githubusercontent.com/sustainable-processes/ontology/refs/heads/main/OntoCAPE/chemical_process_system/CPS_function/process_control.owl"
     xmlns:fundamental_concepts="https://raw.githubusercontent.com/sustainable-processes/ontology/refs/heads/main/meta_model/fundamental_concepts/fundamental_concepts.owl#"
     xmlns:mathematical_relation="https://raw.githubusercontent.com/sustainable-processes/ontology/refs/heads/main/OntoCAPE/supporting_concepts/mathematical_relation/mathematical_relation.owl#">
    <owl:Ontology rdf:about="https://raw.githubusercontent.com/sustainable-processes/ontology/refs/heads/main/OntoCAPE/chemical_process_system/CPS_function/process_control.owl">
        <owl:imports rdf:resource="https://raw.githubusercontent.com/sustainable-processes/ontology/refs/heads/main/OntoCAPE/chemical_process_system/CPS_function/process.owl"/>
        <terms:license>Copyright (C) [2009] [Andreas Wiesner]
                This program is free software; you can redistribute it and/or modify it under the terms of the GNU General Public License as published by the Free Software Foundation; either version 3 of the License, or (at your option) any later version.
                This program is distributed in the hope that it will be useful, but WITHOUT ANY WARRANTY; without even the implied warranty of MERCHANTABILITY or FITNESS FOR A PARTICULAR PURPOSE. See the GNU General Public License for more details.
                You should have received a copy of the GNU General Public License along with this program; if not, see &lt;http://www.gnu.org/licenses/&gt;.
   </terms:license>
        <rdfs:comment>The ontology module &apos;process_control&apos; provides concepts based on control theory for process control architectures for a chemical process system.
The following classes and relations from other ontology modules are used within &apos;process_control&apos;:

&lt;owl:Class rdf:about=&quot;https://raw.githubusercontent.com/sustainable-processes/ontology/refs/heads/main/OntoCAPE/upper_level/system.owl#System&quot;/&gt;
&lt;owl:Class rdf:about=&quot;https://raw.githubusercontent.com/sustainable-processes/ontology/refs/heads/main/OntoCAPE/upper_level/network_system.owl#Device&quot;/&gt;
&lt;owl:Class rdf:about=&quot;https://raw.githubusercontent.com/sustainable-processes/ontology/refs/heads/main/OntoCAPE/upper_level/network_system.owl#Connection&quot;/&gt;
&lt;owl:Class rdf:about=&quot;https://raw.githubusercontent.com/sustainable-processes/ontology/refs/heads/main/OntoCAPE/chemical_process_system/CPS_function/process.owl#ProcessStep&quot;/&gt;

&lt;owl:ObjectProperty rdf:about=&quot;https://raw.githubusercontent.com/sustainable-processes/ontology/refs/heads/main/OntoCAPE/upper_level/system.owl#hasSubsystem&quot;/&gt;
&lt;owl:ObjectProperty rdf:about=&quot;https://raw.githubusercontent.com/sustainable-processes/ontology/refs/heads/main/OntoCAPE/upper_level/system.owl#isDirectlyConnectedTo&quot;/&gt;
&lt;owl:ObjectProperty rdf:about=&quot;https://raw.githubusercontent.com/sustainable-processes/ontology/refs/heads/main/OntoCAPE/upper_level/network_system.owl#hasOutput&quot;/&gt;
&lt;owl:ObjectProperty rdf:about=&quot;https://raw.githubusercontent.com/sustainable-processes/ontology/refs/heads/main/OntoCAPE/upper_level/network_system.owl#hasInput&quot;/&gt;
&lt;owl:ObjectProperty rdf:about=&quot;https://raw.githubusercontent.com/sustainable-processes/ontology/refs/heads/main/OntoCAPE/upper_level/system.owl#isDirectSubsystemOf&quot;/&gt;
&lt;owl:ObjectProperty rdf:about=&quot;https://raw.githubusercontent.com/sustainable-processes/ontology/refs/heads/main/OntoCAPE/upper_level/system.owl#hasDirectSubsystem&quot;/&gt;
&lt;owl:ObjectProperty rdf:about=&quot;https://raw.githubusercontent.com/sustainable-processes/ontology/refs/heads/main/OntoCAPE/upper_level/network_system.owl#enters&quot;/&gt;
&lt;owl:ObjectProperty rdf:about=&quot;https://raw.githubusercontent.com/sustainable-processes/ontology/refs/heads/main/OntoCAPE/upper_level/network_system.owl#leaves&quot;/&gt;
&lt;owl:ObjectProperty rdf:about=&quot;https://raw.githubusercontent.com/sustainable-processes/ontology/refs/heads/main/OntoCAPE/upper_level/system.owl#isRelatedTo&quot;/&gt;

The following classes and relations from the Meta Model are refined within &apos;process_control&apos;:

&lt;owl:Class rdf:about=&quot;https://raw.githubusercontent.com/sustainable-processes/ontology/refs/heads/main/meta_model/fundamental_concepts/fundamental_concepts.owl#ValueSet&quot;/&gt;
&lt;owl:Class rdf:about=&quot;https://raw.githubusercontent.com/sustainable-processes/ontology/refs/heads/main/meta_model/fundamental_concepts/fundamental_concepts.owl#NonExhaustiveValueSet&quot;/&gt;

&lt;owl:ObjectProperty rdf:about=&quot;https://raw.githubusercontent.com/sustainable-processes/ontology/refs/heads/main/meta_model/fundamental_concepts/fundamental_concepts.owl#isOfType&quot;/&gt;

   </rdfs:comment>
        <owl:versionInfo>2.0</owl:versionInfo>
    </owl:Ontology>
    


    <!-- 
    ///////////////////////////////////////////////////////////////////////////////////////
    //
    // Object Properties
    //
    ///////////////////////////////////////////////////////////////////////////////////////
     -->

    


    <!-- https://raw.githubusercontent.com/sustainable-processes/ontology/refs/heads/main/OntoCAPE/chemical_process_system/CPS_function/process_control.owl#hasControlLoopArchitecture -->

    <owl:ObjectProperty rdf:about="https://raw.githubusercontent.com/sustainable-processes/ontology/refs/heads/main/OntoCAPE/chemical_process_system/CPS_function/process_control.owl#hasControlLoopArchitecture">
        <rdfs:subPropertyOf rdf:resource="https://raw.githubusercontent.com/sustainable-processes/ontology/refs/heads/main/meta_model/fundamental_concepts/fundamental_concepts.owl#isOfType"/>
        <rdf:type rdf:resource="http://www.w3.org/2002/07/owl#FunctionalProperty"/>
        <rdfs:domain rdf:resource="https://raw.githubusercontent.com/sustainable-processes/ontology/refs/heads/main/OntoCAPE/chemical_process_system/CPS_function/process_control.owl#ControlLoop"/>
        <rdfs:range rdf:resource="https://raw.githubusercontent.com/sustainable-processes/ontology/refs/heads/main/OntoCAPE/chemical_process_system/CPS_function/process_control.owl#ControlLoopArchitectureVT"/>
        <rdfs:comment>The relation hasControlLoopArchitecture refers from a equipment to the corresponding fixture.</rdfs:comment>
    </owl:ObjectProperty>
    


    <!-- https://raw.githubusercontent.com/sustainable-processes/ontology/refs/heads/main/OntoCAPE/chemical_process_system/CPS_function/process_control.owl#hasLinearity -->

    <owl:ObjectProperty rdf:about="https://raw.githubusercontent.com/sustainable-processes/ontology/refs/heads/main/OntoCAPE/chemical_process_system/CPS_function/process_control.owl#hasLinearity">
        <rdfs:subPropertyOf rdf:resource="https://raw.githubusercontent.com/sustainable-processes/ontology/refs/heads/main/meta_model/fundamental_concepts/fundamental_concepts.owl#isOfType"/>
        <rdf:type rdf:resource="http://www.w3.org/2002/07/owl#FunctionalProperty"/>
        <rdfs:domain rdf:resource="https://raw.githubusercontent.com/sustainable-processes/ontology/refs/heads/main/OntoCAPE/chemical_process_system/CPS_function/process_control.owl#FunctionBlock"/>
        <rdfs:range rdf:resource="https://raw.githubusercontent.com/sustainable-processes/ontology/refs/heads/main/OntoCAPE/chemical_process_system/CPS_function/process_control.owl#LinearityVT"/>
        <rdfs:comment>The relation hasLinearity refers from a FunctionBlock to its LinearityValueType.</rdfs:comment>
    </owl:ObjectProperty>
    


    <!-- https://raw.githubusercontent.com/sustainable-processes/ontology/refs/heads/main/OntoCAPE/chemical_process_system/CPS_function/process_control.owl#hasResponseCharacteristics -->

    <owl:ObjectProperty rdf:about="https://raw.githubusercontent.com/sustainable-processes/ontology/refs/heads/main/OntoCAPE/chemical_process_system/CPS_function/process_control.owl#hasResponseCharacteristics">
        <rdfs:subPropertyOf rdf:resource="https://raw.githubusercontent.com/sustainable-processes/ontology/refs/heads/main/meta_model/fundamental_concepts/fundamental_concepts.owl#isOfType"/>
        <rdf:type rdf:resource="http://www.w3.org/2002/07/owl#FunctionalProperty"/>
        <rdfs:domain rdf:resource="https://raw.githubusercontent.com/sustainable-processes/ontology/refs/heads/main/OntoCAPE/chemical_process_system/CPS_function/process_control.owl#FunctionBlock"/>
        <rdfs:range rdf:resource="https://raw.githubusercontent.com/sustainable-processes/ontology/refs/heads/main/OntoCAPE/chemical_process_system/CPS_function/process_control.owl#ResponseCharacteristicsVT"/>
        <rdfs:comment>The relation hasResponseCharacteristics refers from the function block to its ResponseCharacteristicsValueType.</rdfs:comment>
    </owl:ObjectProperty>
    


    <!-- https://raw.githubusercontent.com/sustainable-processes/ontology/refs/heads/main/OntoCAPE/chemical_process_system/CPS_function/process_control.owl#refersToProcessStep -->

    <owl:ObjectProperty rdf:about="https://raw.githubusercontent.com/sustainable-processes/ontology/refs/heads/main/OntoCAPE/chemical_process_system/CPS_function/process_control.owl#refersToProcessStep">
        <rdfs:subPropertyOf rdf:resource="https://raw.githubusercontent.com/sustainable-processes/ontology/refs/heads/main/OntoCAPE/upper_level/system.owl#isRelatedTo"/>
        <rdfs:domain rdf:resource="https://raw.githubusercontent.com/sustainable-processes/ontology/refs/heads/main/OntoCAPE/chemical_process_system/CPS_function/process_control.owl#ControlledSystem"/>
        <rdfs:range rdf:resource="https://raw.githubusercontent.com/sustainable-processes/ontology/refs/heads/main/OntoCAPE/chemical_process_system/CPS_function/process.owl#ProcessStep"/>
    </owl:ObjectProperty>
    


    <!-- 
    ///////////////////////////////////////////////////////////////////////////////////////
    //
    // Classes
    //
    ///////////////////////////////////////////////////////////////////////////////////////
     -->

    


    <!-- https://raw.githubusercontent.com/sustainable-processes/ontology/refs/heads/main/OntoCAPE/chemical_process_system/CPS_function/process_control.owl#Actionline -->

    <owl:Class rdf:about="https://raw.githubusercontent.com/sustainable-processes/ontology/refs/heads/main/OntoCAPE/chemical_process_system/CPS_function/process_control.owl#Actionline">
        <rdfs:subClassOf rdf:resource="https://raw.githubusercontent.com/sustainable-processes/ontology/refs/heads/main/OntoCAPE/upper_level/network_system.owl#Connection"/>
        <rdfs:subClassOf>
            <owl:Restriction>
                <owl:onProperty rdf:resource="https://raw.githubusercontent.com/sustainable-processes/ontology/refs/heads/main/OntoCAPE/upper_level/system.owl#hasDirectSubsystem"/>
                <owl:allValuesFrom>
                    <owl:Class>
                        <owl:unionOf rdf:parseType="Collection">
                            <rdf:Description rdf:about="https://raw.githubusercontent.com/sustainable-processes/ontology/refs/heads/main/OntoCAPE/chemical_process_system/CPS_function/process_control.owl#Actionline"/>
                            <rdf:Description rdf:about="https://raw.githubusercontent.com/sustainable-processes/ontology/refs/heads/main/OntoCAPE/chemical_process_system/CPS_function/process_control.owl#ControlComponent"/>
                        </owl:unionOf>
                    </owl:Class>
                </owl:allValuesFrom>
            </owl:Restriction>
        </rdfs:subClassOf>
        <rdfs:subClassOf>
            <owl:Restriction>
                <owl:onProperty rdf:resource="https://raw.githubusercontent.com/sustainable-processes/ontology/refs/heads/main/OntoCAPE/upper_level/system.owl#hasSubsystem"/>
                <owl:allValuesFrom>
                    <owl:Class>
                        <owl:unionOf rdf:parseType="Collection">
                            <rdf:Description rdf:about="https://raw.githubusercontent.com/sustainable-processes/ontology/refs/heads/main/OntoCAPE/chemical_process_system/CPS_function/process_control.owl#Actionline"/>
                            <rdf:Description rdf:about="https://raw.githubusercontent.com/sustainable-processes/ontology/refs/heads/main/OntoCAPE/chemical_process_system/CPS_function/process_control.owl#ControlComponent"/>
                        </owl:unionOf>
                    </owl:Class>
                </owl:allValuesFrom>
            </owl:Restriction>
        </rdfs:subClassOf>
        <rdfs:subClassOf>
            <owl:Restriction>
                <owl:onProperty rdf:resource="https://raw.githubusercontent.com/sustainable-processes/ontology/refs/heads/main/OntoCAPE/upper_level/system.owl#isDirectSubsystemOf"/>
                <owl:allValuesFrom>
                    <owl:Class>
                        <owl:unionOf rdf:parseType="Collection">
                            <rdf:Description rdf:about="https://raw.githubusercontent.com/sustainable-processes/ontology/refs/heads/main/OntoCAPE/chemical_process_system/CPS_function/process_control.owl#Actionline"/>
                            <rdf:Description rdf:about="https://raw.githubusercontent.com/sustainable-processes/ontology/refs/heads/main/OntoCAPE/chemical_process_system/CPS_function/process_control.owl#ControlComponent"/>
                        </owl:unionOf>
                    </owl:Class>
                </owl:allValuesFrom>
            </owl:Restriction>
        </rdfs:subClassOf>
        <rdfs:subClassOf>
            <owl:Restriction>
                <owl:onProperty rdf:resource="https://raw.githubusercontent.com/sustainable-processes/ontology/refs/heads/main/OntoCAPE/upper_level/system.owl#isDirectlyConnectedTo"/>
                <owl:allValuesFrom rdf:resource="https://raw.githubusercontent.com/sustainable-processes/ontology/refs/heads/main/OntoCAPE/chemical_process_system/CPS_function/process_control.owl#ControlComponent"/>
            </owl:Restriction>
        </rdfs:subClassOf>
        <rdfs:subClassOf>
            <owl:Restriction>
                <owl:onProperty rdf:resource="https://raw.githubusercontent.com/sustainable-processes/ontology/refs/heads/main/OntoCAPE/upper_level/system.owl#isDirectlyConnectedTo"/>
                <owl:maxCardinality rdf:datatype="http://www.w3.org/2001/XMLSchema#nonNegativeInteger">2</owl:maxCardinality>
            </owl:Restriction>
        </rdfs:subClassOf>
        <rdfs:comment>Control Components are connected by actionlines, which represents a specific type of information collection. Actionlines are treated analogous to topological arcs.</rdfs:comment>
    </owl:Class>
    


    <!-- https://raw.githubusercontent.com/sustainable-processes/ontology/refs/heads/main/OntoCAPE/chemical_process_system/CPS_function/process_control.owl#ActuatorFunction -->

    <owl:Class rdf:about="https://raw.githubusercontent.com/sustainable-processes/ontology/refs/heads/main/OntoCAPE/chemical_process_system/CPS_function/process_control.owl#ActuatorFunction">
        <rdfs:subClassOf rdf:resource="https://raw.githubusercontent.com/sustainable-processes/ontology/refs/heads/main/OntoCAPE/chemical_process_system/CPS_function/process_control.owl#FunctionBlock"/>
        <rdfs:comment>ActuatorFunction transforms the output of the Controller into the input of the ControlledSystem.</rdfs:comment>
    </owl:Class>
    


    <!-- https://raw.githubusercontent.com/sustainable-processes/ontology/refs/heads/main/OntoCAPE/chemical_process_system/CPS_function/process_control.owl#BranchingPoint -->

    <owl:Class rdf:about="https://raw.githubusercontent.com/sustainable-processes/ontology/refs/heads/main/OntoCAPE/chemical_process_system/CPS_function/process_control.owl#BranchingPoint">
        <rdfs:subClassOf rdf:resource="https://raw.githubusercontent.com/sustainable-processes/ontology/refs/heads/main/OntoCAPE/chemical_process_system/CPS_function/process_control.owl#ControlComponent"/>
        <rdfs:comment>BranchingPoint describes the splitting of a controlled system.</rdfs:comment>
    </owl:Class>
    


    <!-- https://raw.githubusercontent.com/sustainable-processes/ontology/refs/heads/main/OntoCAPE/chemical_process_system/CPS_function/process_control.owl#ComparingElement -->

    <owl:Class rdf:about="https://raw.githubusercontent.com/sustainable-processes/ontology/refs/heads/main/OntoCAPE/chemical_process_system/CPS_function/process_control.owl#ComparingElement">
        <rdfs:subClassOf rdf:resource="https://raw.githubusercontent.com/sustainable-processes/ontology/refs/heads/main/OntoCAPE/chemical_process_system/CPS_function/process_control.owl#ControlComponent"/>
        <rdfs:comment>ComparingElement indicates whether a action line influence as a feed back or directly.</rdfs:comment>
    </owl:Class>
    


    <!-- https://raw.githubusercontent.com/sustainable-processes/ontology/refs/heads/main/OntoCAPE/chemical_process_system/CPS_function/process_control.owl#ControlComponent -->

    <owl:Class rdf:about="https://raw.githubusercontent.com/sustainable-processes/ontology/refs/heads/main/OntoCAPE/chemical_process_system/CPS_function/process_control.owl#ControlComponent">
        <rdfs:subClassOf rdf:resource="https://raw.githubusercontent.com/sustainable-processes/ontology/refs/heads/main/OntoCAPE/upper_level/network_system.owl#Device"/>
        <rdfs:subClassOf>
            <owl:Restriction>
                <owl:onProperty rdf:resource="https://raw.githubusercontent.com/sustainable-processes/ontology/refs/heads/main/OntoCAPE/upper_level/network_system.owl#hasInput"/>
                <owl:allValuesFrom rdf:resource="https://raw.githubusercontent.com/sustainable-processes/ontology/refs/heads/main/OntoCAPE/chemical_process_system/CPS_function/process_control.owl#DirectedActionline"/>
            </owl:Restriction>
        </rdfs:subClassOf>
        <rdfs:subClassOf>
            <owl:Restriction>
                <owl:onProperty rdf:resource="https://raw.githubusercontent.com/sustainable-processes/ontology/refs/heads/main/OntoCAPE/upper_level/network_system.owl#hasOutput"/>
                <owl:allValuesFrom rdf:resource="https://raw.githubusercontent.com/sustainable-processes/ontology/refs/heads/main/OntoCAPE/chemical_process_system/CPS_function/process_control.owl#DirectedActionline"/>
            </owl:Restriction>
        </rdfs:subClassOf>
        <rdfs:subClassOf>
            <owl:Restriction>
                <owl:onProperty rdf:resource="https://raw.githubusercontent.com/sustainable-processes/ontology/refs/heads/main/OntoCAPE/upper_level/system.owl#hasDirectSubsystem"/>
                <owl:allValuesFrom>
                    <owl:Class>
                        <owl:unionOf rdf:parseType="Collection">
                            <rdf:Description rdf:about="https://raw.githubusercontent.com/sustainable-processes/ontology/refs/heads/main/OntoCAPE/chemical_process_system/CPS_function/process_control.owl#Actionline"/>
                            <rdf:Description rdf:about="https://raw.githubusercontent.com/sustainable-processes/ontology/refs/heads/main/OntoCAPE/chemical_process_system/CPS_function/process_control.owl#ControlComponent"/>
                        </owl:unionOf>
                    </owl:Class>
                </owl:allValuesFrom>
            </owl:Restriction>
        </rdfs:subClassOf>
        <rdfs:subClassOf>
            <owl:Restriction>
                <owl:onProperty rdf:resource="https://raw.githubusercontent.com/sustainable-processes/ontology/refs/heads/main/OntoCAPE/upper_level/system.owl#hasSubsystem"/>
                <owl:allValuesFrom>
                    <owl:Class>
                        <owl:unionOf rdf:parseType="Collection">
                            <rdf:Description rdf:about="https://raw.githubusercontent.com/sustainable-processes/ontology/refs/heads/main/OntoCAPE/chemical_process_system/CPS_function/process_control.owl#Actionline"/>
                            <rdf:Description rdf:about="https://raw.githubusercontent.com/sustainable-processes/ontology/refs/heads/main/OntoCAPE/chemical_process_system/CPS_function/process_control.owl#ControlComponent"/>
                        </owl:unionOf>
                    </owl:Class>
                </owl:allValuesFrom>
            </owl:Restriction>
        </rdfs:subClassOf>
        <rdfs:subClassOf>
            <owl:Restriction>
                <owl:onProperty rdf:resource="https://raw.githubusercontent.com/sustainable-processes/ontology/refs/heads/main/OntoCAPE/upper_level/system.owl#isDirectSubsystemOf"/>
                <owl:allValuesFrom>
                    <owl:Class>
                        <owl:unionOf rdf:parseType="Collection">
                            <rdf:Description rdf:about="https://raw.githubusercontent.com/sustainable-processes/ontology/refs/heads/main/OntoCAPE/chemical_process_system/CPS_function/process_control.owl#Actionline"/>
                            <rdf:Description rdf:about="https://raw.githubusercontent.com/sustainable-processes/ontology/refs/heads/main/OntoCAPE/chemical_process_system/CPS_function/process_control.owl#ControlComponent"/>
                        </owl:unionOf>
                    </owl:Class>
                </owl:allValuesFrom>
            </owl:Restriction>
        </rdfs:subClassOf>
        <rdfs:subClassOf>
            <owl:Restriction>
                <owl:onProperty rdf:resource="https://raw.githubusercontent.com/sustainable-processes/ontology/refs/heads/main/OntoCAPE/upper_level/system.owl#isDirectlyConnectedTo"/>
                <owl:allValuesFrom rdf:resource="https://raw.githubusercontent.com/sustainable-processes/ontology/refs/heads/main/OntoCAPE/chemical_process_system/CPS_function/process_control.owl#Actionline"/>
            </owl:Restriction>
        </rdfs:subClassOf>
        <rdfs:comment>ControlComponent comprises the different features required for describing control.</rdfs:comment>
    </owl:Class>
    


    <!-- https://raw.githubusercontent.com/sustainable-processes/ontology/refs/heads/main/OntoCAPE/chemical_process_system/CPS_function/process_control.owl#ControlLoop -->

    <owl:Class rdf:about="https://raw.githubusercontent.com/sustainable-processes/ontology/refs/heads/main/OntoCAPE/chemical_process_system/CPS_function/process_control.owl#ControlLoop">
        <rdfs:subClassOf rdf:resource="https://raw.githubusercontent.com/sustainable-processes/ontology/refs/heads/main/OntoCAPE/upper_level/system.owl#System"/>
        <rdfs:subClassOf>
            <owl:Restriction>
                <owl:onProperty rdf:resource="https://raw.githubusercontent.com/sustainable-processes/ontology/refs/heads/main/OntoCAPE/chemical_process_system/CPS_function/process_control.owl#hasControlLoopArchitecture"/>
                <owl:someValuesFrom rdf:resource="https://raw.githubusercontent.com/sustainable-processes/ontology/refs/heads/main/OntoCAPE/chemical_process_system/CPS_function/process_control.owl#ControlLoopArchitectureVT"/>
            </owl:Restriction>
        </rdfs:subClassOf>
        <rdfs:subClassOf>
            <owl:Restriction>
                <owl:onProperty rdf:resource="https://raw.githubusercontent.com/sustainable-processes/ontology/refs/heads/main/OntoCAPE/upper_level/system.owl#hasSubsystem"/>
                <owl:someValuesFrom rdf:resource="https://raw.githubusercontent.com/sustainable-processes/ontology/refs/heads/main/OntoCAPE/chemical_process_system/CPS_function/process_control.owl#Actionline"/>
            </owl:Restriction>
        </rdfs:subClassOf>
        <rdfs:subClassOf>
            <owl:Restriction>
                <owl:onProperty rdf:resource="https://raw.githubusercontent.com/sustainable-processes/ontology/refs/heads/main/OntoCAPE/upper_level/system.owl#hasSubsystem"/>
                <owl:someValuesFrom rdf:resource="https://raw.githubusercontent.com/sustainable-processes/ontology/refs/heads/main/OntoCAPE/chemical_process_system/CPS_function/process_control.owl#ControlComponent"/>
            </owl:Restriction>
        </rdfs:subClassOf>
        <rdfs:subClassOf>
            <owl:Restriction>
                <owl:onProperty rdf:resource="https://raw.githubusercontent.com/sustainable-processes/ontology/refs/heads/main/OntoCAPE/chemical_process_system/CPS_function/process_control.owl#hasControlLoopArchitecture"/>
                <owl:allValuesFrom rdf:resource="https://raw.githubusercontent.com/sustainable-processes/ontology/refs/heads/main/OntoCAPE/chemical_process_system/CPS_function/process_control.owl#ControlLoopArchitectureVT"/>
            </owl:Restriction>
        </rdfs:subClassOf>
        <rdfs:subClassOf>
            <owl:Restriction>
                <owl:onProperty rdf:resource="https://raw.githubusercontent.com/sustainable-processes/ontology/refs/heads/main/OntoCAPE/upper_level/system.owl#hasSubsystem"/>
                <owl:allValuesFrom>
                    <owl:Class>
                        <owl:unionOf rdf:parseType="Collection">
                            <rdf:Description rdf:about="https://raw.githubusercontent.com/sustainable-processes/ontology/refs/heads/main/OntoCAPE/chemical_process_system/CPS_function/process_control.owl#Actionline"/>
                            <rdf:Description rdf:about="https://raw.githubusercontent.com/sustainable-processes/ontology/refs/heads/main/OntoCAPE/chemical_process_system/CPS_function/process_control.owl#ControlComponent"/>
                        </owl:unionOf>
                    </owl:Class>
                </owl:allValuesFrom>
            </owl:Restriction>
        </rdfs:subClassOf>
        <rdfs:subClassOf>
            <owl:Restriction>
                <owl:onProperty rdf:resource="https://raw.githubusercontent.com/sustainable-processes/ontology/refs/heads/main/OntoCAPE/chemical_process_system/CPS_function/process_control.owl#hasControlLoopArchitecture"/>
                <owl:cardinality rdf:datatype="http://www.w3.org/2001/XMLSchema#nonNegativeInteger">1</owl:cardinality>
            </owl:Restriction>
        </rdfs:subClassOf>
        <rdfs:comment>ControlSystem is a functional subsystem of ProcessControlSystem and deals with functional describtion of the control system</rdfs:comment>
    </owl:Class>
    


    <!-- https://raw.githubusercontent.com/sustainable-processes/ontology/refs/heads/main/OntoCAPE/chemical_process_system/CPS_function/process_control.owl#ControlLoopArchitectureVT -->

    <owl:Class rdf:about="https://raw.githubusercontent.com/sustainable-processes/ontology/refs/heads/main/OntoCAPE/chemical_process_system/CPS_function/process_control.owl#ControlLoopArchitectureVT">
        <rdfs:subClassOf rdf:resource="https://raw.githubusercontent.com/sustainable-processes/ontology/refs/heads/main/meta_model/fundamental_concepts/fundamental_concepts.owl#NonExhaustiveValueSet"/>
        <owl:disjointWith rdf:resource="https://raw.githubusercontent.com/sustainable-processes/ontology/refs/heads/main/OntoCAPE/chemical_process_system/CPS_function/process_control.owl#LinearityVT"/>
        <owl:disjointWith rdf:resource="https://raw.githubusercontent.com/sustainable-processes/ontology/refs/heads/main/OntoCAPE/chemical_process_system/CPS_function/process_control.owl#ResponseCharacteristicsVT"/>
        <rdfs:comment>ControlLoopArchitectureValue type comprises the different types of control loop structures. ControlLoopType  is an enumeration of its instances OpenLoopControl, FeedForwardControl, StateFeedbackControl, OutputFeedbackControl and ComplexControlLoop.</rdfs:comment>
    </owl:Class>
    


    <!-- https://raw.githubusercontent.com/sustainable-processes/ontology/refs/heads/main/OntoCAPE/chemical_process_system/CPS_function/process_control.owl#ControlledSystem -->

    <owl:Class rdf:about="https://raw.githubusercontent.com/sustainable-processes/ontology/refs/heads/main/OntoCAPE/chemical_process_system/CPS_function/process_control.owl#ControlledSystem">
        <rdfs:subClassOf rdf:resource="https://raw.githubusercontent.com/sustainable-processes/ontology/refs/heads/main/OntoCAPE/chemical_process_system/CPS_function/process_control.owl#FunctionBlock"/>
        <rdfs:comment>ControlledSystem describes the functionality of the system to be controlled.</rdfs:comment>
    </owl:Class>
    


    <!-- https://raw.githubusercontent.com/sustainable-processes/ontology/refs/heads/main/OntoCAPE/chemical_process_system/CPS_function/process_control.owl#Controller -->

    <owl:Class rdf:about="https://raw.githubusercontent.com/sustainable-processes/ontology/refs/heads/main/OntoCAPE/chemical_process_system/CPS_function/process_control.owl#Controller">
        <rdfs:subClassOf rdf:resource="https://raw.githubusercontent.com/sustainable-processes/ontology/refs/heads/main/OntoCAPE/chemical_process_system/CPS_function/process_control.owl#FunctionBlock"/>
        <rdfs:comment>Controller represents the different types of controller.</rdfs:comment>
    </owl:Class>
    


    <!-- https://raw.githubusercontent.com/sustainable-processes/ontology/refs/heads/main/OntoCAPE/chemical_process_system/CPS_function/process_control.owl#DirectedActionline -->

    <owl:Class rdf:about="https://raw.githubusercontent.com/sustainable-processes/ontology/refs/heads/main/OntoCAPE/chemical_process_system/CPS_function/process_control.owl#DirectedActionline">
        <rdfs:subClassOf rdf:resource="https://raw.githubusercontent.com/sustainable-processes/ontology/refs/heads/main/OntoCAPE/chemical_process_system/CPS_function/process_control.owl#Actionline"/>
        <rdfs:subClassOf>
            <owl:Restriction>
                <owl:onProperty rdf:resource="https://raw.githubusercontent.com/sustainable-processes/ontology/refs/heads/main/OntoCAPE/upper_level/system.owl#isDirectlyConnectedTo"/>
                <owl:cardinality rdf:datatype="http://www.w3.org/2001/XMLSchema#nonNegativeInteger">0</owl:cardinality>
            </owl:Restriction>
        </rdfs:subClassOf>
        <rdfs:subClassOf>
            <owl:Restriction>
                <owl:onProperty rdf:resource="https://raw.githubusercontent.com/sustainable-processes/ontology/refs/heads/main/OntoCAPE/upper_level/network_system.owl#enters"/>
                <owl:maxCardinality rdf:datatype="http://www.w3.org/2001/XMLSchema#nonNegativeInteger">1</owl:maxCardinality>
            </owl:Restriction>
        </rdfs:subClassOf>
        <rdfs:subClassOf>
            <owl:Restriction>
                <owl:onProperty rdf:resource="https://raw.githubusercontent.com/sustainable-processes/ontology/refs/heads/main/OntoCAPE/upper_level/network_system.owl#leaves"/>
                <owl:maxCardinality rdf:datatype="http://www.w3.org/2001/XMLSchema#nonNegativeInteger">1</owl:maxCardinality>
            </owl:Restriction>
        </rdfs:subClassOf>
        <rdfs:comment>DirectedActionline is a specialization of Actionline and likewise the connecting element between ControlComponents. However, the usage of DirectedActionline implies the indication of a directed connection.</rdfs:comment>
    </owl:Class>
    


    <!-- https://raw.githubusercontent.com/sustainable-processes/ontology/refs/heads/main/OntoCAPE/chemical_process_system/CPS_function/process_control.owl#FunctionBlock -->

    <owl:Class rdf:about="https://raw.githubusercontent.com/sustainable-processes/ontology/refs/heads/main/OntoCAPE/chemical_process_system/CPS_function/process_control.owl#FunctionBlock">
        <rdfs:subClassOf rdf:resource="https://raw.githubusercontent.com/sustainable-processes/ontology/refs/heads/main/OntoCAPE/chemical_process_system/CPS_function/process_control.owl#ControlComponent"/>
        <rdfs:subClassOf>
            <owl:Restriction>
                <owl:onProperty rdf:resource="https://raw.githubusercontent.com/sustainable-processes/ontology/refs/heads/main/OntoCAPE/chemical_process_system/CPS_function/process_control.owl#hasLinearity"/>
                <owl:someValuesFrom rdf:resource="https://raw.githubusercontent.com/sustainable-processes/ontology/refs/heads/main/OntoCAPE/chemical_process_system/CPS_function/process_control.owl#LinearityVT"/>
            </owl:Restriction>
        </rdfs:subClassOf>
        <rdfs:subClassOf>
            <owl:Restriction>
                <owl:onProperty rdf:resource="https://raw.githubusercontent.com/sustainable-processes/ontology/refs/heads/main/OntoCAPE/chemical_process_system/CPS_function/process_control.owl#hasResponseCharacteristics"/>
                <owl:someValuesFrom rdf:resource="https://raw.githubusercontent.com/sustainable-processes/ontology/refs/heads/main/OntoCAPE/chemical_process_system/CPS_function/process_control.owl#ResponseCharacteristicsVT"/>
            </owl:Restriction>
        </rdfs:subClassOf>
        <rdfs:subClassOf>
            <owl:Restriction>
                <owl:onProperty rdf:resource="https://raw.githubusercontent.com/sustainable-processes/ontology/refs/heads/main/OntoCAPE/chemical_process_system/CPS_function/process_control.owl#hasLinearity"/>
                <owl:allValuesFrom rdf:resource="https://raw.githubusercontent.com/sustainable-processes/ontology/refs/heads/main/OntoCAPE/chemical_process_system/CPS_function/process_control.owl#LinearityVT"/>
            </owl:Restriction>
        </rdfs:subClassOf>
        <rdfs:subClassOf>
            <owl:Restriction>
                <owl:onProperty rdf:resource="https://raw.githubusercontent.com/sustainable-processes/ontology/refs/heads/main/OntoCAPE/chemical_process_system/CPS_function/process_control.owl#hasResponseCharacteristics"/>
                <owl:allValuesFrom rdf:resource="https://raw.githubusercontent.com/sustainable-processes/ontology/refs/heads/main/OntoCAPE/chemical_process_system/CPS_function/process_control.owl#ResponseCharacteristicsVT"/>
            </owl:Restriction>
        </rdfs:subClassOf>
        <rdfs:subClassOf>
            <owl:Restriction>
                <owl:onProperty rdf:resource="https://raw.githubusercontent.com/sustainable-processes/ontology/refs/heads/main/OntoCAPE/chemical_process_system/CPS_function/process_control.owl#hasLinearity"/>
                <owl:cardinality rdf:datatype="http://www.w3.org/2001/XMLSchema#nonNegativeInteger">1</owl:cardinality>
            </owl:Restriction>
        </rdfs:subClassOf>
        <rdfs:comment>FunctionBlock have a distinct transfer function, which can be used to characterize them.</rdfs:comment>
    </owl:Class>
    


    <!-- https://raw.githubusercontent.com/sustainable-processes/ontology/refs/heads/main/OntoCAPE/chemical_process_system/CPS_function/process_control.owl#FunctionBlockLinearType -->

    <owl:Class rdf:about="https://raw.githubusercontent.com/sustainable-processes/ontology/refs/heads/main/OntoCAPE/chemical_process_system/CPS_function/process_control.owl#FunctionBlockLinearType">
        <owl:equivalentClass>
            <owl:Class>
                <owl:intersectionOf rdf:parseType="Collection">
                    <rdf:Description rdf:about="https://raw.githubusercontent.com/sustainable-processes/ontology/refs/heads/main/OntoCAPE/chemical_process_system/CPS_function/process_control.owl#FunctionBlock"/>
                    <owl:Restriction>
                        <owl:onProperty rdf:resource="https://raw.githubusercontent.com/sustainable-processes/ontology/refs/heads/main/OntoCAPE/chemical_process_system/CPS_function/process_control.owl#hasLinearity"/>
                        <owl:hasValue rdf:resource="https://raw.githubusercontent.com/sustainable-processes/ontology/refs/heads/main/OntoCAPE/chemical_process_system/CPS_function/process_control.owl#linear"/>
                    </owl:Restriction>
                </owl:intersectionOf>
            </owl:Class>
        </owl:equivalentClass>
    </owl:Class>
    


    <!-- https://raw.githubusercontent.com/sustainable-processes/ontology/refs/heads/main/OntoCAPE/chemical_process_system/CPS_function/process_control.owl#LinearControlLoop -->

    <owl:Class rdf:about="https://raw.githubusercontent.com/sustainable-processes/ontology/refs/heads/main/OntoCAPE/chemical_process_system/CPS_function/process_control.owl#LinearControlLoop">
        <owl:equivalentClass>
            <owl:Class>
                <owl:intersectionOf rdf:parseType="Collection">
                    <rdf:Description rdf:about="https://raw.githubusercontent.com/sustainable-processes/ontology/refs/heads/main/OntoCAPE/chemical_process_system/CPS_function/process_control.owl#ControlLoop"/>
                    <owl:Restriction>
                        <owl:onProperty rdf:resource="https://raw.githubusercontent.com/sustainable-processes/ontology/refs/heads/main/OntoCAPE/upper_level/system.owl#hasSubsystem"/>
                        <owl:someValuesFrom rdf:resource="https://raw.githubusercontent.com/sustainable-processes/ontology/refs/heads/main/OntoCAPE/chemical_process_system/CPS_function/process_control.owl#FunctionBlockLinearType"/>
                    </owl:Restriction>
                    <owl:Restriction>
                        <owl:onProperty rdf:resource="https://raw.githubusercontent.com/sustainable-processes/ontology/refs/heads/main/OntoCAPE/upper_level/system.owl#hasSubsystem"/>
                        <owl:allValuesFrom>
                            <owl:Class>
                                <owl:unionOf rdf:parseType="Collection">
                                    <rdf:Description rdf:about="https://raw.githubusercontent.com/sustainable-processes/ontology/refs/heads/main/OntoCAPE/chemical_process_system/CPS_function/process_control.owl#Actionline"/>
                                    <rdf:Description rdf:about="https://raw.githubusercontent.com/sustainable-processes/ontology/refs/heads/main/OntoCAPE/chemical_process_system/CPS_function/process_control.owl#FunctionBlockLinearType"/>
                                </owl:unionOf>
                            </owl:Class>
                        </owl:allValuesFrom>
                    </owl:Restriction>
                </owl:intersectionOf>
            </owl:Class>
        </owl:equivalentClass>
    </owl:Class>
    


    <!-- https://raw.githubusercontent.com/sustainable-processes/ontology/refs/heads/main/OntoCAPE/chemical_process_system/CPS_function/process_control.owl#LinearityVT -->

    <owl:Class rdf:about="https://raw.githubusercontent.com/sustainable-processes/ontology/refs/heads/main/OntoCAPE/chemical_process_system/CPS_function/process_control.owl#LinearityVT">
        <owl:equivalentClass>
            <owl:Class>
                <owl:oneOf rdf:parseType="Collection">
                    <rdf:Description rdf:about="https://raw.githubusercontent.com/sustainable-processes/ontology/refs/heads/main/OntoCAPE/chemical_process_system/CPS_function/process_control.owl#linear"/>
                    <rdf:Description rdf:about="https://raw.githubusercontent.com/sustainable-processes/ontology/refs/heads/main/OntoCAPE/chemical_process_system/CPS_function/process_control.owl#nonlinear"/>
                </owl:oneOf>
            </owl:Class>
        </owl:equivalentClass>
        <rdfs:subClassOf rdf:resource="https://raw.githubusercontent.com/sustainable-processes/ontology/refs/heads/main/meta_model/fundamental_concepts/fundamental_concepts.owl#ValueSet"/>
        <owl:disjointWith rdf:resource="https://raw.githubusercontent.com/sustainable-processes/ontology/refs/heads/main/OntoCAPE/chemical_process_system/CPS_function/process_control.owl#ResponseCharacteristicsVT"/>
        <rdfs:comment>Linearity is an enumeration of its instances linear and Non-linear.</rdfs:comment>
    </owl:Class>
    


    <!-- https://raw.githubusercontent.com/sustainable-processes/ontology/refs/heads/main/OntoCAPE/chemical_process_system/CPS_function/process_control.owl#ResponseCharacteristicsVT -->

    <owl:Class rdf:about="https://raw.githubusercontent.com/sustainable-processes/ontology/refs/heads/main/OntoCAPE/chemical_process_system/CPS_function/process_control.owl#ResponseCharacteristicsVT">
        <rdfs:subClassOf rdf:resource="https://raw.githubusercontent.com/sustainable-processes/ontology/refs/heads/main/meta_model/fundamental_concepts/fundamental_concepts.owl#NonExhaustiveValueSet"/>
        <rdfs:comment>ResponseCharacteristics describe the several characteristics how a controlled system may react on a manipulation.</rdfs:comment>
    </owl:Class>
    


    <!-- https://raw.githubusercontent.com/sustainable-processes/ontology/refs/heads/main/OntoCAPE/chemical_process_system/CPS_function/process_control.owl#ReversingElement -->

    <owl:Class rdf:about="https://raw.githubusercontent.com/sustainable-processes/ontology/refs/heads/main/OntoCAPE/chemical_process_system/CPS_function/process_control.owl#ReversingElement">
        <rdfs:subClassOf rdf:resource="https://raw.githubusercontent.com/sustainable-processes/ontology/refs/heads/main/OntoCAPE/chemical_process_system/CPS_function/process_control.owl#ControlComponent"/>
        <rdfs:comment>ReversingElement describes the functionality of lead.</rdfs:comment>
    </owl:Class>
    


    <!-- https://raw.githubusercontent.com/sustainable-processes/ontology/refs/heads/main/OntoCAPE/chemical_process_system/CPS_function/process_control.owl#SensorFunction -->

    <owl:Class rdf:about="https://raw.githubusercontent.com/sustainable-processes/ontology/refs/heads/main/OntoCAPE/chemical_process_system/CPS_function/process_control.owl#SensorFunction">
        <rdfs:subClassOf rdf:resource="https://raw.githubusercontent.com/sustainable-processes/ontology/refs/heads/main/OntoCAPE/chemical_process_system/CPS_function/process_control.owl#FunctionBlock"/>
        <rdfs:comment>The SensorFunction comprises the entire function of recording, relaying, and writing out ProcessQuantities within other ControlComponents.</rdfs:comment>
    </owl:Class>
    


    <!-- 
    ///////////////////////////////////////////////////////////////////////////////////////
    //
    // Individuals
    //
    ///////////////////////////////////////////////////////////////////////////////////////
     -->

    


    <!-- https://raw.githubusercontent.com/sustainable-processes/ontology/refs/heads/main/OntoCAPE/chemical_process_system/CPS_function/process_control.owl#ComplexControlLoop -->

    <owl:NamedIndividual rdf:about="https://raw.githubusercontent.com/sustainable-processes/ontology/refs/heads/main/OntoCAPE/chemical_process_system/CPS_function/process_control.owl#ComplexControlLoop">
        <rdf:type rdf:resource="https://raw.githubusercontent.com/sustainable-processes/ontology/refs/heads/main/OntoCAPE/chemical_process_system/CPS_function/process_control.owl#ControlLoopArchitectureVT"/>
        <rdfs:comment>ComplexControlLoop is not yet specifically defined control loop which may be composed of other control loop elements.</rdfs:comment>
    </owl:NamedIndividual>
    


    <!-- https://raw.githubusercontent.com/sustainable-processes/ontology/refs/heads/main/OntoCAPE/chemical_process_system/CPS_function/process_control.owl#D-Element -->

    <owl:NamedIndividual rdf:about="https://raw.githubusercontent.com/sustainable-processes/ontology/refs/heads/main/OntoCAPE/chemical_process_system/CPS_function/process_control.owl#D-Element">
        <rdf:type rdf:resource="https://raw.githubusercontent.com/sustainable-processes/ontology/refs/heads/main/OntoCAPE/chemical_process_system/CPS_function/process_control.owl#ResponseCharacteristicsVT"/>
        <rdfs:comment>D-Element is a derivative part of a controller which is applied for smoother control trajectories since it reduces the magnitude of the overshoot produced by the integral component.</rdfs:comment>
    </owl:NamedIndividual>
    


    <!-- https://raw.githubusercontent.com/sustainable-processes/ontology/refs/heads/main/OntoCAPE/chemical_process_system/CPS_function/process_control.owl#FeedForwardControl -->

    <owl:NamedIndividual rdf:about="https://raw.githubusercontent.com/sustainable-processes/ontology/refs/heads/main/OntoCAPE/chemical_process_system/CPS_function/process_control.owl#FeedForwardControl">
        <rdf:type rdf:resource="https://raw.githubusercontent.com/sustainable-processes/ontology/refs/heads/main/OntoCAPE/chemical_process_system/CPS_function/process_control.owl#ControlLoopArchitectureVT"/>
        <rdfs:comment>A system which exhibits FeedForwardControl responds to a measured disturbance in a pre-defined way before the disturbance effects the control variable.</rdfs:comment>
    </owl:NamedIndividual>
    


    <!-- https://raw.githubusercontent.com/sustainable-processes/ontology/refs/heads/main/OntoCAPE/chemical_process_system/CPS_function/process_control.owl#I-Element -->

    <owl:NamedIndividual rdf:about="https://raw.githubusercontent.com/sustainable-processes/ontology/refs/heads/main/OntoCAPE/chemical_process_system/CPS_function/process_control.owl#I-Element">
        <rdf:type rdf:resource="https://raw.githubusercontent.com/sustainable-processes/ontology/refs/heads/main/OntoCAPE/chemical_process_system/CPS_function/process_control.owl#ResponseCharacteristicsVT"/>
        <rdfs:comment>I-Element is a integrative part of a controller which force the signal to approach the setpoint quicker than a proportional controller alone and eliminate steady state error.</rdfs:comment>
    </owl:NamedIndividual>
    


    <!-- https://raw.githubusercontent.com/sustainable-processes/ontology/refs/heads/main/OntoCAPE/chemical_process_system/CPS_function/process_control.owl#OpenLoopControl -->

    <owl:NamedIndividual rdf:about="https://raw.githubusercontent.com/sustainable-processes/ontology/refs/heads/main/OntoCAPE/chemical_process_system/CPS_function/process_control.owl#OpenLoopControl">
        <rdf:type rdf:resource="https://raw.githubusercontent.com/sustainable-processes/ontology/refs/heads/main/OntoCAPE/chemical_process_system/CPS_function/process_control.owl#ControlLoopArchitectureVT"/>
        <rdfs:comment>OpenLoopControl is a type of architecture which computes its input into a system using only the current state and its model of the system.</rdfs:comment>
    </owl:NamedIndividual>
    


    <!-- https://raw.githubusercontent.com/sustainable-processes/ontology/refs/heads/main/OntoCAPE/chemical_process_system/CPS_function/process_control.owl#OutputFeedbackControl -->

    <owl:NamedIndividual rdf:about="https://raw.githubusercontent.com/sustainable-processes/ontology/refs/heads/main/OntoCAPE/chemical_process_system/CPS_function/process_control.owl#OutputFeedbackControl">
        <rdf:type rdf:resource="https://raw.githubusercontent.com/sustainable-processes/ontology/refs/heads/main/OntoCAPE/chemical_process_system/CPS_function/process_control.owl#ControlLoopArchitectureVT"/>
        <rdfs:comment>OutputFeedbackControl is applied when the output of the system is fed back into the system as part of its input.</rdfs:comment>
    </owl:NamedIndividual>
    


    <!-- https://raw.githubusercontent.com/sustainable-processes/ontology/refs/heads/main/OntoCAPE/chemical_process_system/CPS_function/process_control.owl#P-Element -->

    <owl:NamedIndividual rdf:about="https://raw.githubusercontent.com/sustainable-processes/ontology/refs/heads/main/OntoCAPE/chemical_process_system/CPS_function/process_control.owl#P-Element">
        <rdf:type rdf:resource="https://raw.githubusercontent.com/sustainable-processes/ontology/refs/heads/main/OntoCAPE/chemical_process_system/CPS_function/process_control.owl#ResponseCharacteristicsVT"/>
        <rdfs:comment>P-Element is a proportional part of a controller which responds to a change in the process variable proportional to the current measured error value.</rdfs:comment>
    </owl:NamedIndividual>
    


    <!-- https://raw.githubusercontent.com/sustainable-processes/ontology/refs/heads/main/OntoCAPE/chemical_process_system/CPS_function/process_control.owl#PID-Element -->

    <owl:NamedIndividual rdf:about="https://raw.githubusercontent.com/sustainable-processes/ontology/refs/heads/main/OntoCAPE/chemical_process_system/CPS_function/process_control.owl#PID-Element">
        <rdf:type rdf:resource="https://raw.githubusercontent.com/sustainable-processes/ontology/refs/heads/main/OntoCAPE/chemical_process_system/CPS_function/process_control.owl#ResponseCharacteristicsVT"/>
        <rdfs:comment>PID-Element combines all features provided by the P-, I- and D-Element of a controller.</rdfs:comment>
    </owl:NamedIndividual>
    


    <!-- https://raw.githubusercontent.com/sustainable-processes/ontology/refs/heads/main/OntoCAPE/chemical_process_system/CPS_function/process_control.owl#PT1-Element -->

    <owl:NamedIndividual rdf:about="https://raw.githubusercontent.com/sustainable-processes/ontology/refs/heads/main/OntoCAPE/chemical_process_system/CPS_function/process_control.owl#PT1-Element">
        <rdf:type rdf:resource="https://raw.githubusercontent.com/sustainable-processes/ontology/refs/heads/main/OntoCAPE/chemical_process_system/CPS_function/process_control.owl#ResponseCharacteristicsVT"/>
        <rdfs:comment>PT1-Element deals with time-delay in controlled system to avoid instability.</rdfs:comment>
    </owl:NamedIndividual>
    


    <!-- https://raw.githubusercontent.com/sustainable-processes/ontology/refs/heads/main/OntoCAPE/chemical_process_system/CPS_function/process_control.owl#StateFeedbackControl -->

    <owl:NamedIndividual rdf:about="https://raw.githubusercontent.com/sustainable-processes/ontology/refs/heads/main/OntoCAPE/chemical_process_system/CPS_function/process_control.owl#StateFeedbackControl">
        <rdf:type rdf:resource="https://raw.githubusercontent.com/sustainable-processes/ontology/refs/heads/main/OntoCAPE/chemical_process_system/CPS_function/process_control.owl#ControlLoopArchitectureVT"/>
        <rdfs:comment>StateFeedbackControl is a method employed in feedback control.</rdfs:comment>
    </owl:NamedIndividual>
    


    <!-- https://raw.githubusercontent.com/sustainable-processes/ontology/refs/heads/main/OntoCAPE/chemical_process_system/CPS_function/process_control.owl#linear -->

    <owl:NamedIndividual rdf:about="https://raw.githubusercontent.com/sustainable-processes/ontology/refs/heads/main/OntoCAPE/chemical_process_system/CPS_function/process_control.owl#linear">
        <rdf:type rdf:resource="https://raw.githubusercontent.com/sustainable-processes/ontology/refs/heads/main/OntoCAPE/chemical_process_system/CPS_function/process_control.owl#LinearityVT"/>
        <owl:differentFrom rdf:resource="https://raw.githubusercontent.com/sustainable-processes/ontology/refs/heads/main/OntoCAPE/chemical_process_system/CPS_function/process_control.owl#nonlinear"/>
        <rdfs:comment>Linear refers to the behavior of the ControlledSystem.</rdfs:comment>
    </owl:NamedIndividual>
    


    <!-- https://raw.githubusercontent.com/sustainable-processes/ontology/refs/heads/main/OntoCAPE/chemical_process_system/CPS_function/process_control.owl#nonlinear -->

    <owl:NamedIndividual rdf:about="https://raw.githubusercontent.com/sustainable-processes/ontology/refs/heads/main/OntoCAPE/chemical_process_system/CPS_function/process_control.owl#nonlinear">
        <rdf:type rdf:resource="https://raw.githubusercontent.com/sustainable-processes/ontology/refs/heads/main/OntoCAPE/chemical_process_system/CPS_function/process_control.owl#LinearityVT"/>
        <rdfs:comment>Nonlinear refers to the behavior of the ControlledSystem which cannot be described as a linear function of the state of that system.</rdfs:comment>
    </owl:NamedIndividual>
    


    <!-- 
    ///////////////////////////////////////////////////////////////////////////////////////
    //
    // General axioms
    //
    ///////////////////////////////////////////////////////////////////////////////////////
     -->

    <rdf:Description>
        <rdf:type rdf:resource="http://www.w3.org/2002/07/owl#AllDifferent"/>
        <owl:distinctMembers rdf:parseType="Collection">
            <rdf:Description rdf:about="https://raw.githubusercontent.com/sustainable-processes/ontology/refs/heads/main/OntoCAPE/chemical_process_system/CPS_function/process_control.owl#ComplexControlLoop"/>
            <rdf:Description rdf:about="https://raw.githubusercontent.com/sustainable-processes/ontology/refs/heads/main/OntoCAPE/chemical_process_system/CPS_function/process_control.owl#FeedForwardControl"/>
            <rdf:Description rdf:about="https://raw.githubusercontent.com/sustainable-processes/ontology/refs/heads/main/OntoCAPE/chemical_process_system/CPS_function/process_control.owl#OpenLoopControl"/>
            <rdf:Description rdf:about="https://raw.githubusercontent.com/sustainable-processes/ontology/refs/heads/main/OntoCAPE/chemical_process_system/CPS_function/process_control.owl#OutputFeedbackControl"/>
            <rdf:Description rdf:about="https://raw.githubusercontent.com/sustainable-processes/ontology/refs/heads/main/OntoCAPE/chemical_process_system/CPS_function/process_control.owl#StateFeedbackControl"/>
        </owl:distinctMembers>
    </rdf:Description>
    <rdf:Description>
        <rdf:type rdf:resource="http://www.w3.org/2002/07/owl#AllDifferent"/>
        <owl:distinctMembers rdf:parseType="Collection">
            <rdf:Description rdf:about="https://raw.githubusercontent.com/sustainable-processes/ontology/refs/heads/main/OntoCAPE/chemical_process_system/CPS_function/process_control.owl#D-Element"/>
            <rdf:Description rdf:about="https://raw.githubusercontent.com/sustainable-processes/ontology/refs/heads/main/OntoCAPE/chemical_process_system/CPS_function/process_control.owl#I-Element"/>
            <rdf:Description rdf:about="https://raw.githubusercontent.com/sustainable-processes/ontology/refs/heads/main/OntoCAPE/chemical_process_system/CPS_function/process_control.owl#P-Element"/>
            <rdf:Description rdf:about="https://raw.githubusercontent.com/sustainable-processes/ontology/refs/heads/main/OntoCAPE/chemical_process_system/CPS_function/process_control.owl#PID-Element"/>
            <rdf:Description rdf:about="https://raw.githubusercontent.com/sustainable-processes/ontology/refs/heads/main/OntoCAPE/chemical_process_system/CPS_function/process_control.owl#PT1-Element"/>
        </owl:distinctMembers>
    </rdf:Description>
</rdf:RDF>



<!-- Generated by the OWL API (version 4.5.26.2023-07-17T20:34:13Z) https://github.com/owlcs/owlapi -->

