<?xml version="1.0"?>
<rdf:RDF xmlns="https://github.com/sustainable-processes/ontology/OntoCAPE/chemical_process_system/CPS_function/process_extensionTGL25001.owl#"
     xml:base="https://github.com/sustainable-processes/ontology/OntoCAPE/chemical_process_system/CPS_function/process_extensionTGL25001.owl"
     xmlns:owl="http://www.w3.org/2002/07/owl#"
     xmlns:rdf="http://www.w3.org/1999/02/22-rdf-syntax-ns#"
     xmlns:xml="http://www.w3.org/XML/1998/namespace"
     xmlns:xsd="http://www.w3.org/2001/XMLSchema#"
     xmlns:rdfs="http://www.w3.org/2000/01/rdf-schema#"
     xmlns:root="https://github.com/sustainable-processes/ontology/OntoCAPE/"
     xmlns:terms="http://purl.org/dc/terms/"
     xmlns:process="https://github.com/sustainable-processes/ontology/OntoCAPE/chemical_process_system/CPS_function/process.owl#"
     xmlns:process_ext="https://github.com/sustainable-processes/ontology/OntoCAPE/chemical_process_system/CPS_function/process_extensionTGL25001.owl">
    <owl:Ontology rdf:about="https://github.com/sustainable-processes/ontology/OntoCAPE/chemical_process_system/CPS_function/process_extensionTGL25001.owl">
        <owl:imports rdf:resource="https://github.com/sustainable-processes/ontology/OntoCAPE/chemical_process_system/CPS_function/process.owl"/>
        <terms:license>Copyright (C) [2009] [Andreas Wiesner]
                This program is free software; you can redistribute it and/or modify it under the terms of the GNU General Public License as published by the Free Software Foundation; either version 3 of the License, or (at your option) any later version.
                This program is distributed in the hope that it will be useful, but WITHOUT ANY WARRANTY; without even the implied warranty of MERCHANTABILITY or FITNESS FOR A PARTICULAR PURPOSE. See the GNU General Public License for more details.
                You should have received a copy of the GNU General Public License along with this program; if not, see &lt;http://www.gnu.org/licenses/&gt;.
    </terms:license>
        <rdfs:comment>Extension of partial model process; classification of ProcessSteps according to TGL 25001</rdfs:comment>
        <rdfs:comment>The following classes and relations from other ontology modules are used within &apos;process_extensionTGL25001&apos;:

&lt;owl:Class rdf:about=&quot;https://github.com/sustainable-processes/ontology/OntoCAPE/chemical_process_system/CPS_function/process.owl#PhaseChange&quot;/&gt;
&lt;owl:Class rdf:about=&quot;https://github.com/sustainable-processes/ontology/OntoCAPE/chemical_process_system/CPS_function/process.owl#Separation&quot;/&gt;
&lt;owl:Class rdf:about=&quot;https://github.com/sustainable-processes/ontology/OntoCAPE/chemical_process_system/CPS_function/process.owl#Combination&quot;/&gt;
&lt;owl:Class rdf:about=&quot;https://github.com/sustainable-processes/ontology/OntoCAPE/chemical_process_system/CPS_function/process.owl#TemperatureChange&quot;/&gt;
&lt;owl:Class rdf:about=&quot;https://github.com/sustainable-processes/ontology/OntoCAPE/chemical_process_system/CPS_function/process.owl#Fragmentation&quot;/&gt;
&lt;owl:Class rdf:about=&quot;https://github.com/sustainable-processes/ontology/OntoCAPE/chemical_process_system/CPS_function/process.owl#Mixing&quot;/&gt;

    </rdfs:comment>
        <owl:versionInfo>2.0</owl:versionInfo>
    </owl:Ontology>
    


    <!-- 
    ///////////////////////////////////////////////////////////////////////////////////////
    //
    // Classes
    //
    ///////////////////////////////////////////////////////////////////////////////////////
     -->

    


    <!-- https://github.com/sustainable-processes/ontology/OntoCAPE/chemical_process_system/CPS_function/process_extensionTGL25001.owl#Abrasion -->

    <owl:Class rdf:about="https://github.com/sustainable-processes/ontology/OntoCAPE/chemical_process_system/CPS_function/process_extensionTGL25001.owl#Abrasion">
        <rdfs:subClassOf rdf:resource="https://github.com/sustainable-processes/ontology/OntoCAPE/chemical_process_system/CPS_function/process.owl#Fragmentation"/>
        <rdfs:comment>Granulation of a solid by frictional action using an abrading medium.</rdfs:comment>
    </owl:Class>
    


    <!-- https://github.com/sustainable-processes/ontology/OntoCAPE/chemical_process_system/CPS_function/process_extensionTGL25001.owl#Absorption -->

    <owl:Class rdf:about="https://github.com/sustainable-processes/ontology/OntoCAPE/chemical_process_system/CPS_function/process_extensionTGL25001.owl#Absorption">
        <rdfs:subClassOf rdf:resource="https://github.com/sustainable-processes/ontology/OntoCAPE/chemical_process_system/CPS_function/process.owl#Separation"/>
        <rdfs:comment>Absorption is the transfer of a soluble component in a gas-phase mixture into a liquid absorbent whose volatility is low under process conditions. (Perry)</rdfs:comment>
    </owl:Class>
    


    <!-- https://github.com/sustainable-processes/ontology/OntoCAPE/chemical_process_system/CPS_function/process_extensionTGL25001.owl#Adsorption -->

    <owl:Class rdf:about="https://github.com/sustainable-processes/ontology/OntoCAPE/chemical_process_system/CPS_function/process_extensionTGL25001.owl#Adsorption">
        <rdfs:subClassOf rdf:resource="https://github.com/sustainable-processes/ontology/OntoCAPE/chemical_process_system/CPS_function/process.owl#Separation"/>
        <rdfs:comment>Adsorption is the selcective transfer of molecules or fine-granular particles from a fluid (gas or liquid) to the interface of the adsorbents.</rdfs:comment>
    </owl:Class>
    


    <!-- https://github.com/sustainable-processes/ontology/OntoCAPE/chemical_process_system/CPS_function/process_extensionTGL25001.owl#BoilingDown -->

    <owl:Class rdf:about="https://github.com/sustainable-processes/ontology/OntoCAPE/chemical_process_system/CPS_function/process_extensionTGL25001.owl#BoilingDown">
        <rdfs:subClassOf rdf:resource="https://github.com/sustainable-processes/ontology/OntoCAPE/chemical_process_system/CPS_function/process.owl#Separation"/>
        <rdfs:comment>Boiling down refers to the separation of a solution into gaseous and solid substances by evaporating the volatile components completely. </rdfs:comment>
    </owl:Class>
    


    <!-- https://github.com/sustainable-processes/ontology/OntoCAPE/chemical_process_system/CPS_function/process_extensionTGL25001.owl#Briquetting -->

    <owl:Class rdf:about="https://github.com/sustainable-processes/ontology/OntoCAPE/chemical_process_system/CPS_function/process_extensionTGL25001.owl#Briquetting">
        <rdfs:subClassOf rdf:resource="https://github.com/sustainable-processes/ontology/OntoCAPE/chemical_process_system/CPS_function/process.owl#Combination"/>
        <rdfs:comment>The agglomeration of a fine-granular powder to coarse-granular pieces by mechanical pressure.</rdfs:comment>
    </owl:Class>
    


    <!-- https://github.com/sustainable-processes/ontology/OntoCAPE/chemical_process_system/CPS_function/process_extensionTGL25001.owl#Centrifugation -->

    <owl:Class rdf:about="https://github.com/sustainable-processes/ontology/OntoCAPE/chemical_process_system/CPS_function/process_extensionTGL25001.owl#Centrifugation">
        <rdfs:subClassOf rdf:resource="https://github.com/sustainable-processes/ontology/OntoCAPE/chemical_process_system/CPS_function/process.owl#Separation"/>
        <rdfs:comment>A process of separating the lighter portions of a solution, mixture, or suspension from the heavier portions by centrifugal force.</rdfs:comment>
    </owl:Class>
    


    <!-- https://github.com/sustainable-processes/ontology/OntoCAPE/chemical_process_system/CPS_function/process_extensionTGL25001.owl#Compacting -->

    <owl:Class rdf:about="https://github.com/sustainable-processes/ontology/OntoCAPE/chemical_process_system/CPS_function/process_extensionTGL25001.owl#Compacting">
        <rdfs:subClassOf rdf:resource="https://github.com/sustainable-processes/ontology/OntoCAPE/chemical_process_system/CPS_function/process.owl#Combination"/>
        <rdfs:comment>The compression of a loose, voluminous powder to a more dense, closely packed powder by mechanical pressure.</rdfs:comment>
    </owl:Class>
    


    <!-- https://github.com/sustainable-processes/ontology/OntoCAPE/chemical_process_system/CPS_function/process_extensionTGL25001.owl#ConcentrationByEvaporation -->

    <owl:Class rdf:about="https://github.com/sustainable-processes/ontology/OntoCAPE/chemical_process_system/CPS_function/process_extensionTGL25001.owl#ConcentrationByEvaporation">
        <rdfs:subClassOf rdf:resource="https://github.com/sustainable-processes/ontology/OntoCAPE/chemical_process_system/CPS_function/process.owl#Separation"/>
        <rdfs:comment>In evaporization, the vapor from a boiling liquid is removed and a more concentrated solution remains. (Geankoplis: Transport processes and unit operations)</rdfs:comment>
    </owl:Class>
    


    <!-- https://github.com/sustainable-processes/ontology/OntoCAPE/chemical_process_system/CPS_function/process_extensionTGL25001.owl#Condensation -->

    <owl:Class rdf:about="https://github.com/sustainable-processes/ontology/OntoCAPE/chemical_process_system/CPS_function/process_extensionTGL25001.owl#Condensation">
        <rdfs:subClassOf rdf:resource="https://github.com/sustainable-processes/ontology/OntoCAPE/chemical_process_system/CPS_function/process_extensionTGL25001.owl#PhaseChangeOfGases"/>
        <rdfs:comment>The phase transition from gas to liquid.</rdfs:comment>
    </owl:Class>
    


    <!-- https://github.com/sustainable-processes/ontology/OntoCAPE/chemical_process_system/CPS_function/process_extensionTGL25001.owl#CoolingOfGases -->

    <owl:Class rdf:about="https://github.com/sustainable-processes/ontology/OntoCAPE/chemical_process_system/CPS_function/process_extensionTGL25001.owl#CoolingOfGases">
        <rdfs:subClassOf rdf:resource="https://github.com/sustainable-processes/ontology/OntoCAPE/chemical_process_system/CPS_function/process_extensionTGL25001.owl#TemperatureChangeOfGases"/>
        <rdfs:comment>Reducing the temperature of a gas without changing ist state of aggregation</rdfs:comment>
    </owl:Class>
    


    <!-- https://github.com/sustainable-processes/ontology/OntoCAPE/chemical_process_system/CPS_function/process_extensionTGL25001.owl#CoolingOfLiquids -->

    <owl:Class rdf:about="https://github.com/sustainable-processes/ontology/OntoCAPE/chemical_process_system/CPS_function/process_extensionTGL25001.owl#CoolingOfLiquids">
        <rdfs:subClassOf rdf:resource="https://github.com/sustainable-processes/ontology/OntoCAPE/chemical_process_system/CPS_function/process_extensionTGL25001.owl#TemperatureChangeOfLiquids"/>
        <rdfs:comment>Reducing the temperature of a liquid without changing ist state of aggregation</rdfs:comment>
    </owl:Class>
    


    <!-- https://github.com/sustainable-processes/ontology/OntoCAPE/chemical_process_system/CPS_function/process_extensionTGL25001.owl#CoolingOfSolids -->

    <owl:Class rdf:about="https://github.com/sustainable-processes/ontology/OntoCAPE/chemical_process_system/CPS_function/process_extensionTGL25001.owl#CoolingOfSolids">
        <rdfs:subClassOf rdf:resource="https://github.com/sustainable-processes/ontology/OntoCAPE/chemical_process_system/CPS_function/process_extensionTGL25001.owl#TemperatureChangeOfSolids"/>
        <rdfs:comment>Reducing the temperature of a solid.</rdfs:comment>
    </owl:Class>
    


    <!-- https://github.com/sustainable-processes/ontology/OntoCAPE/chemical_process_system/CPS_function/process_extensionTGL25001.owl#Cutting -->

    <owl:Class rdf:about="https://github.com/sustainable-processes/ontology/OntoCAPE/chemical_process_system/CPS_function/process_extensionTGL25001.owl#Cutting">
        <rdfs:subClassOf rdf:resource="https://github.com/sustainable-processes/ontology/OntoCAPE/chemical_process_system/CPS_function/process.owl#Fragmentation"/>
        <rdfs:comment>Fragmentation of solid material by the effect of shear forces</rdfs:comment>
    </owl:Class>
    


    <!-- https://github.com/sustainable-processes/ontology/OntoCAPE/chemical_process_system/CPS_function/process_extensionTGL25001.owl#CyclonicSeparation -->

    <owl:Class rdf:about="https://github.com/sustainable-processes/ontology/OntoCAPE/chemical_process_system/CPS_function/process_extensionTGL25001.owl#CyclonicSeparation">
        <rdfs:subClassOf rdf:resource="https://github.com/sustainable-processes/ontology/OntoCAPE/chemical_process_system/CPS_function/process.owl#Separation"/>
        <rdfs:comment>Cyclonic separation is a method of removing particles from a gas stream by means of centrifugal forces. </rdfs:comment>
    </owl:Class>
    


    <!-- https://github.com/sustainable-processes/ontology/OntoCAPE/chemical_process_system/CPS_function/process_extensionTGL25001.owl#Desublimation -->

    <owl:Class rdf:about="https://github.com/sustainable-processes/ontology/OntoCAPE/chemical_process_system/CPS_function/process_extensionTGL25001.owl#Desublimation">
        <rdfs:subClassOf rdf:resource="https://github.com/sustainable-processes/ontology/OntoCAPE/chemical_process_system/CPS_function/process_extensionTGL25001.owl#PhaseChangeOfGases"/>
        <rdfs:comment>The phase transition from gas to solid without passing through an intermediate liquid state.</rdfs:comment>
    </owl:Class>
    


    <!-- https://github.com/sustainable-processes/ontology/OntoCAPE/chemical_process_system/CPS_function/process_extensionTGL25001.owl#DiffusionSeparation -->

    <owl:Class rdf:about="https://github.com/sustainable-processes/ontology/OntoCAPE/chemical_process_system/CPS_function/process_extensionTGL25001.owl#DiffusionSeparation">
        <rdfs:subClassOf rdf:resource="https://github.com/sustainable-processes/ontology/OntoCAPE/chemical_process_system/CPS_function/process.owl#Separation"/>
        <rdfs:comment>Process to separate a gas mixture into its components by means of differences in the diffusion rates of the component molecules</rdfs:comment>
    </owl:Class>
    


    <!-- https://github.com/sustainable-processes/ontology/OntoCAPE/chemical_process_system/CPS_function/process_extensionTGL25001.owl#Dissolution -->

    <owl:Class rdf:about="https://github.com/sustainable-processes/ontology/OntoCAPE/chemical_process_system/CPS_function/process_extensionTGL25001.owl#Dissolution">
        <rdfs:subClassOf rdf:resource="https://github.com/sustainable-processes/ontology/OntoCAPE/chemical_process_system/CPS_function/process.owl#Combination"/>
        <rdfs:comment>The mixing of a solid and a liquid with the formation of one new homogeneous phase (i.e. the solution).</rdfs:comment>
    </owl:Class>
    


    <!-- https://github.com/sustainable-processes/ontology/OntoCAPE/chemical_process_system/CPS_function/process_extensionTGL25001.owl#Distillation -->

    <owl:Class rdf:about="https://github.com/sustainable-processes/ontology/OntoCAPE/chemical_process_system/CPS_function/process_extensionTGL25001.owl#Distillation">
        <rdfs:subClassOf rdf:resource="https://github.com/sustainable-processes/ontology/OntoCAPE/chemical_process_system/CPS_function/process.owl#Separation"/>
        <rdfs:comment>Distillation is the seperation of the constituents of liquid mixture via partial vaporization of the mixture and separate recovery of vapor and residue. (Perry)</rdfs:comment>
    </owl:Class>
    


    <!-- https://github.com/sustainable-processes/ontology/OntoCAPE/chemical_process_system/CPS_function/process_extensionTGL25001.owl#ElectricalGasCleaning -->

    <owl:Class rdf:about="https://github.com/sustainable-processes/ontology/OntoCAPE/chemical_process_system/CPS_function/process_extensionTGL25001.owl#ElectricalGasCleaning">
        <rdfs:subClassOf rdf:resource="https://github.com/sustainable-processes/ontology/OntoCAPE/chemical_process_system/CPS_function/process.owl#Separation"/>
        <rdfs:comment>The separation of dispersed particles from a gas phase by means of an electric field.</rdfs:comment>
    </owl:Class>
    


    <!-- https://github.com/sustainable-processes/ontology/OntoCAPE/chemical_process_system/CPS_function/process_extensionTGL25001.owl#Electrodialysis -->

    <owl:Class rdf:about="https://github.com/sustainable-processes/ontology/OntoCAPE/chemical_process_system/CPS_function/process_extensionTGL25001.owl#Electrodialysis">
        <rdfs:subClassOf rdf:resource="https://github.com/sustainable-processes/ontology/OntoCAPE/chemical_process_system/CPS_function/process.owl#Separation"/>
        <rdfs:comment>A process which uses an electric field and two semipermeable membranes to separate dissociated species from undissociated species in a solvent. The electric field forces the dissociated ions through the membranes, while the nonpolar species remain in the solvent.</rdfs:comment>
    </owl:Class>
    


    <!-- https://github.com/sustainable-processes/ontology/OntoCAPE/chemical_process_system/CPS_function/process_extensionTGL25001.owl#ElectromagneticCrushing -->

    <owl:Class rdf:about="https://github.com/sustainable-processes/ontology/OntoCAPE/chemical_process_system/CPS_function/process_extensionTGL25001.owl#ElectromagneticCrushing">
        <rdfs:subClassOf rdf:resource="https://github.com/sustainable-processes/ontology/OntoCAPE/chemical_process_system/CPS_function/process.owl#Fragmentation"/>
        <rdfs:comment>The process of crushing solid material by applying electromagnetic fields that cause internal stresses.</rdfs:comment>
    </owl:Class>
    


    <!-- https://github.com/sustainable-processes/ontology/OntoCAPE/chemical_process_system/CPS_function/process_extensionTGL25001.owl#Electrophoresis -->

    <owl:Class rdf:about="https://github.com/sustainable-processes/ontology/OntoCAPE/chemical_process_system/CPS_function/process_extensionTGL25001.owl#Electrophoresis">
        <rdfs:subClassOf rdf:resource="https://github.com/sustainable-processes/ontology/OntoCAPE/chemical_process_system/CPS_function/process.owl#Separation"/>
        <rdfs:comment>Electrophoresis is the technique of separating electrically charged particles, particularly proteins, in a solution by passing an electric current through the solution. The rate of movement of the different components depends upon their charge, so that they gradually separate into bands. [neurolab.jsc.nasa.gov/glosseh.htm]</rdfs:comment>
    </owl:Class>
    


    <!-- https://github.com/sustainable-processes/ontology/OntoCAPE/chemical_process_system/CPS_function/process_extensionTGL25001.owl#Emulsification -->

    <owl:Class rdf:about="https://github.com/sustainable-processes/ontology/OntoCAPE/chemical_process_system/CPS_function/process_extensionTGL25001.owl#Emulsification">
        <rdfs:subClassOf rdf:resource="https://github.com/sustainable-processes/ontology/OntoCAPE/chemical_process_system/CPS_function/process.owl#Combination"/>
        <rdfs:comment>The formation of a mixture of two liquids, such as oil and water, in which one of the liquids is in the form of fine droplets and is dispersed in the other.</rdfs:comment>
    </owl:Class>
    


    <!-- https://github.com/sustainable-processes/ontology/OntoCAPE/chemical_process_system/CPS_function/process_extensionTGL25001.owl#Extraction -->

    <owl:Class rdf:about="https://github.com/sustainable-processes/ontology/OntoCAPE/chemical_process_system/CPS_function/process_extensionTGL25001.owl#Extraction">
        <rdfs:subClassOf rdf:resource="https://github.com/sustainable-processes/ontology/OntoCAPE/chemical_process_system/CPS_function/process.owl#Separation"/>
        <rdfs:comment>Extraction refers to both liquid-liquid extraction and leaching:
Liquid-liquid extraction is a process for separationg components in solution by their distribution between two immiscible liquid phases. Such a process can also be simply referred to as liquid extraction or solvent extraction; however, the latter term my be confusing because it also applies to the leaching of soluble substance from a solid. (Perry&apos;s) 
Leaching is the removal of a soluble fraction, in the form of a solution, from an insoluble, permeable solid phase with which it is associated. The separation usually involves selective dissolution. The soluble constituent may be solid or liquid (Perry&apos;s)
    </rdfs:comment>
    </owl:Class>
    


    <!-- https://github.com/sustainable-processes/ontology/OntoCAPE/chemical_process_system/CPS_function/process_extensionTGL25001.owl#FoamFormation -->

    <owl:Class rdf:about="https://github.com/sustainable-processes/ontology/OntoCAPE/chemical_process_system/CPS_function/process_extensionTGL25001.owl#FoamFormation">
        <rdfs:subClassOf rdf:resource="https://github.com/sustainable-processes/ontology/OntoCAPE/chemical_process_system/CPS_function/process.owl#Combination"/>
        <rdfs:comment>The combination of a liquid and a gas phase to a foam.</rdfs:comment>
    </owl:Class>
    


    <!-- https://github.com/sustainable-processes/ontology/OntoCAPE/chemical_process_system/CPS_function/process_extensionTGL25001.owl#FoamFractionation -->

    <owl:Class rdf:about="https://github.com/sustainable-processes/ontology/OntoCAPE/chemical_process_system/CPS_function/process_extensionTGL25001.owl#FoamFractionation">
        <rdfs:subClassOf rdf:resource="https://github.com/sustainable-processes/ontology/OntoCAPE/chemical_process_system/CPS_function/process.owl#Separation"/>
        <rdfs:comment>A method of separation in which a component of the bulk liquid is preferentially adsorbed at the liquid/vapour (L/V) interface and is removed by foaming. (IUPAC Compendium of Chemical Terminology)</rdfs:comment>
    </owl:Class>
    


    <!-- https://github.com/sustainable-processes/ontology/OntoCAPE/chemical_process_system/CPS_function/process_extensionTGL25001.owl#Fusion -->

    <owl:Class rdf:about="https://github.com/sustainable-processes/ontology/OntoCAPE/chemical_process_system/CPS_function/process_extensionTGL25001.owl#Fusion">
        <rdfs:subClassOf rdf:resource="https://github.com/sustainable-processes/ontology/OntoCAPE/chemical_process_system/CPS_function/process.owl#Combination"/>
        <rdfs:comment>The merging of two or more solid components by melting.</rdfs:comment>
    </owl:Class>
    


    <!-- https://github.com/sustainable-processes/ontology/OntoCAPE/chemical_process_system/CPS_function/process_extensionTGL25001.owl#GasCentrifugation -->

    <owl:Class rdf:about="https://github.com/sustainable-processes/ontology/OntoCAPE/chemical_process_system/CPS_function/process_extensionTGL25001.owl#GasCentrifugation">
        <rdfs:subClassOf rdf:resource="https://github.com/sustainable-processes/ontology/OntoCAPE/chemical_process_system/CPS_function/process.owl#Separation"/>
        <rdfs:comment>The separation of a mixture of gases of different densities by centrifugal force. </rdfs:comment>
    </owl:Class>
    


    <!-- https://github.com/sustainable-processes/ontology/OntoCAPE/chemical_process_system/CPS_function/process_extensionTGL25001.owl#GasFiltration -->

    <owl:Class rdf:about="https://github.com/sustainable-processes/ontology/OntoCAPE/chemical_process_system/CPS_function/process_extensionTGL25001.owl#GasFiltration">
        <rdfs:subClassOf rdf:resource="https://github.com/sustainable-processes/ontology/OntoCAPE/chemical_process_system/CPS_function/process.owl#Separation"/>
        <rdfs:comment>Gas filtration is the separation of a gas-solids mixture by forcing the mixture through a porous barrier which retains most of the solid particulates contained in the mixture.</rdfs:comment>
    </owl:Class>
    


    <!-- https://github.com/sustainable-processes/ontology/OntoCAPE/chemical_process_system/CPS_function/process_extensionTGL25001.owl#Grinding -->

    <owl:Class rdf:about="https://github.com/sustainable-processes/ontology/OntoCAPE/chemical_process_system/CPS_function/process_extensionTGL25001.owl#Grinding">
        <rdfs:subClassOf rdf:resource="https://github.com/sustainable-processes/ontology/OntoCAPE/chemical_process_system/CPS_function/process.owl#Fragmentation"/>
        <rdfs:comment>The process of pulverizing solid material to fine-granular particles by applying mechanical forces</rdfs:comment>
    </owl:Class>
    


    <!-- https://github.com/sustainable-processes/ontology/OntoCAPE/chemical_process_system/CPS_function/process_extensionTGL25001.owl#HeatingOfGases -->

    <owl:Class rdf:about="https://github.com/sustainable-processes/ontology/OntoCAPE/chemical_process_system/CPS_function/process_extensionTGL25001.owl#HeatingOfGases">
        <rdfs:subClassOf rdf:resource="https://github.com/sustainable-processes/ontology/OntoCAPE/chemical_process_system/CPS_function/process_extensionTGL25001.owl#TemperatureChangeOfGases"/>
        <rdfs:comment>Increasing the temperature of a gas</rdfs:comment>
    </owl:Class>
    


    <!-- https://github.com/sustainable-processes/ontology/OntoCAPE/chemical_process_system/CPS_function/process_extensionTGL25001.owl#HeatingOfLiquids -->

    <owl:Class rdf:about="https://github.com/sustainable-processes/ontology/OntoCAPE/chemical_process_system/CPS_function/process_extensionTGL25001.owl#HeatingOfLiquids">
        <rdfs:subClassOf rdf:resource="https://github.com/sustainable-processes/ontology/OntoCAPE/chemical_process_system/CPS_function/process_extensionTGL25001.owl#TemperatureChangeOfLiquids"/>
        <rdfs:comment>Increasing the temperature of a liquid without changing ist state of aggregation</rdfs:comment>
    </owl:Class>
    


    <!-- https://github.com/sustainable-processes/ontology/OntoCAPE/chemical_process_system/CPS_function/process_extensionTGL25001.owl#HeatingOfSolids -->

    <owl:Class rdf:about="https://github.com/sustainable-processes/ontology/OntoCAPE/chemical_process_system/CPS_function/process_extensionTGL25001.owl#HeatingOfSolids">
        <rdfs:subClassOf rdf:resource="https://github.com/sustainable-processes/ontology/OntoCAPE/chemical_process_system/CPS_function/process_extensionTGL25001.owl#TemperatureChangeOfSolids"/>
        <rdfs:comment>Increasing the temperature of a solid without changing ist state of aggregation.</rdfs:comment>
    </owl:Class>
    


    <!-- https://github.com/sustainable-processes/ontology/OntoCAPE/chemical_process_system/CPS_function/process_extensionTGL25001.owl#Humidification -->

    <owl:Class rdf:about="https://github.com/sustainable-processes/ontology/OntoCAPE/chemical_process_system/CPS_function/process_extensionTGL25001.owl#Humidification">
        <rdfs:subClassOf rdf:resource="https://github.com/sustainable-processes/ontology/OntoCAPE/chemical_process_system/CPS_function/process.owl#Combination"/>
        <rdfs:comment>The mixing of a gas and the vapor of a liquid with the formation of a new homogeneous phase.</rdfs:comment>
    </owl:Class>
    


    <!-- https://github.com/sustainable-processes/ontology/OntoCAPE/chemical_process_system/CPS_function/process_extensionTGL25001.owl#HydrocyclonicSeparation -->

    <owl:Class rdf:about="https://github.com/sustainable-processes/ontology/OntoCAPE/chemical_process_system/CPS_function/process_extensionTGL25001.owl#HydrocyclonicSeparation">
        <rdfs:subClassOf rdf:resource="https://github.com/sustainable-processes/ontology/OntoCAPE/chemical_process_system/CPS_function/process.owl#Separation"/>
        <rdfs:comment>Hydrocyclonic separation is a method of removing particles from a liquid stream by means of centrifugal forces. </rdfs:comment>
    </owl:Class>
    


    <!-- https://github.com/sustainable-processes/ontology/OntoCAPE/chemical_process_system/CPS_function/process_extensionTGL25001.owl#ImpingementSeparation -->

    <owl:Class rdf:about="https://github.com/sustainable-processes/ontology/OntoCAPE/chemical_process_system/CPS_function/process_extensionTGL25001.owl#ImpingementSeparation">
        <rdfs:subClassOf rdf:resource="https://github.com/sustainable-processes/ontology/OntoCAPE/chemical_process_system/CPS_function/process.owl#Separation"/>
        <rdfs:comment>Particles are separated from gas by impingement on collected bodies arrayed across the path of the gas stream.(Perry)</rdfs:comment>
    </owl:Class>
    


    <!-- https://github.com/sustainable-processes/ontology/OntoCAPE/chemical_process_system/CPS_function/process_extensionTGL25001.owl#Impregnation -->

    <owl:Class rdf:about="https://github.com/sustainable-processes/ontology/OntoCAPE/chemical_process_system/CPS_function/process_extensionTGL25001.owl#Impregnation">
        <rdfs:subClassOf rdf:resource="https://github.com/sustainable-processes/ontology/OntoCAPE/chemical_process_system/CPS_function/process.owl#Combination"/>
        <rdfs:comment>The process of soaking a porous material with a liquid.</rdfs:comment>
    </owl:Class>
    


    <!-- https://github.com/sustainable-processes/ontology/OntoCAPE/chemical_process_system/CPS_function/process_extensionTGL25001.owl#Kneading -->

    <owl:Class rdf:about="https://github.com/sustainable-processes/ontology/OntoCAPE/chemical_process_system/CPS_function/process_extensionTGL25001.owl#Kneading">
        <rdfs:subClassOf rdf:resource="https://github.com/sustainable-processes/ontology/OntoCAPE/chemical_process_system/CPS_function/process.owl#Combination"/>
        <rdfs:comment>The blending of solid and liquid components into a uniform mass, as by folding, pressing, and stretching.</rdfs:comment>
    </owl:Class>
    


    <!-- https://github.com/sustainable-processes/ontology/OntoCAPE/chemical_process_system/CPS_function/process_extensionTGL25001.owl#LiquidFiltration -->

    <owl:Class rdf:about="https://github.com/sustainable-processes/ontology/OntoCAPE/chemical_process_system/CPS_function/process_extensionTGL25001.owl#LiquidFiltration">
        <rdfs:subClassOf rdf:resource="https://github.com/sustainable-processes/ontology/OntoCAPE/chemical_process_system/CPS_function/process.owl#Separation"/>
        <rdfs:comment>Liquid filtration is the separation of a liquid-solids mixture by forcing the mixture through a porous barrier which retains most of the solid particulates contained in the mixture.</rdfs:comment>
    </owl:Class>
    


    <!-- https://github.com/sustainable-processes/ontology/OntoCAPE/chemical_process_system/CPS_function/process_extensionTGL25001.owl#MechanicalCrushing -->

    <owl:Class rdf:about="https://github.com/sustainable-processes/ontology/OntoCAPE/chemical_process_system/CPS_function/process_extensionTGL25001.owl#MechanicalCrushing">
        <rdfs:subClassOf rdf:resource="https://github.com/sustainable-processes/ontology/OntoCAPE/chemical_process_system/CPS_function/process.owl#Fragmentation"/>
        <rdfs:comment>The process of breaking solid material into coarse-granular pieces by applying mechanical forces</rdfs:comment>
    </owl:Class>
    


    <!-- https://github.com/sustainable-processes/ontology/OntoCAPE/chemical_process_system/CPS_function/process_extensionTGL25001.owl#Melting -->

    <owl:Class rdf:about="https://github.com/sustainable-processes/ontology/OntoCAPE/chemical_process_system/CPS_function/process_extensionTGL25001.owl#Melting">
        <rdfs:subClassOf rdf:resource="https://github.com/sustainable-processes/ontology/OntoCAPE/chemical_process_system/CPS_function/process_extensionTGL25001.owl#PhaseChangeOfSolids"/>
        <rdfs:comment>The phase transition from solid to the liquid.</rdfs:comment>
    </owl:Class>
    


    <!-- https://github.com/sustainable-processes/ontology/OntoCAPE/chemical_process_system/CPS_function/process_extensionTGL25001.owl#MixingOfLiquids -->

    <owl:Class rdf:about="https://github.com/sustainable-processes/ontology/OntoCAPE/chemical_process_system/CPS_function/process_extensionTGL25001.owl#MixingOfLiquids">
        <rdfs:subClassOf rdf:resource="https://github.com/sustainable-processes/ontology/OntoCAPE/chemical_process_system/CPS_function/process.owl#Mixing"/>
        <rdfs:comment>The combination of two or more liquids of different composition to a homogeneous system.</rdfs:comment>
    </owl:Class>
    


    <!-- https://github.com/sustainable-processes/ontology/OntoCAPE/chemical_process_system/CPS_function/process_extensionTGL25001.owl#MixingOfSolids -->

    <owl:Class rdf:about="https://github.com/sustainable-processes/ontology/OntoCAPE/chemical_process_system/CPS_function/process_extensionTGL25001.owl#MixingOfSolids">
        <rdfs:subClassOf rdf:resource="https://github.com/sustainable-processes/ontology/OntoCAPE/chemical_process_system/CPS_function/process.owl#Mixing"/>
        <rdfs:comment>The blending of different solid components to a granular mixture</rdfs:comment>
    </owl:Class>
    


    <!-- https://github.com/sustainable-processes/ontology/OntoCAPE/chemical_process_system/CPS_function/process_extensionTGL25001.owl#MixingofGases -->

    <owl:Class rdf:about="https://github.com/sustainable-processes/ontology/OntoCAPE/chemical_process_system/CPS_function/process_extensionTGL25001.owl#MixingofGases">
        <rdfs:subClassOf rdf:resource="https://github.com/sustainable-processes/ontology/OntoCAPE/chemical_process_system/CPS_function/process.owl#Mixing"/>
        <rdfs:comment>The mixing of two ore more gases of different compositions.</rdfs:comment>
    </owl:Class>
    


    <!-- https://github.com/sustainable-processes/ontology/OntoCAPE/chemical_process_system/CPS_function/process_extensionTGL25001.owl#PhaseChangeOfGases -->

    <owl:Class rdf:about="https://github.com/sustainable-processes/ontology/OntoCAPE/chemical_process_system/CPS_function/process_extensionTGL25001.owl#PhaseChangeOfGases">
        <rdfs:subClassOf rdf:resource="https://github.com/sustainable-processes/ontology/OntoCAPE/chemical_process_system/CPS_function/process.owl#PhaseChange"/>
    </owl:Class>
    


    <!-- https://github.com/sustainable-processes/ontology/OntoCAPE/chemical_process_system/CPS_function/process_extensionTGL25001.owl#PhaseChangeOfLiquids -->

    <owl:Class rdf:about="https://github.com/sustainable-processes/ontology/OntoCAPE/chemical_process_system/CPS_function/process_extensionTGL25001.owl#PhaseChangeOfLiquids">
        <rdfs:subClassOf rdf:resource="https://github.com/sustainable-processes/ontology/OntoCAPE/chemical_process_system/CPS_function/process.owl#PhaseChange"/>
    </owl:Class>
    


    <!-- https://github.com/sustainable-processes/ontology/OntoCAPE/chemical_process_system/CPS_function/process_extensionTGL25001.owl#PhaseChangeOfSolids -->

    <owl:Class rdf:about="https://github.com/sustainable-processes/ontology/OntoCAPE/chemical_process_system/CPS_function/process_extensionTGL25001.owl#PhaseChangeOfSolids">
        <rdfs:subClassOf rdf:resource="https://github.com/sustainable-processes/ontology/OntoCAPE/chemical_process_system/CPS_function/process.owl#PhaseChange"/>
    </owl:Class>
    


    <!-- https://github.com/sustainable-processes/ontology/OntoCAPE/chemical_process_system/CPS_function/process_extensionTGL25001.owl#QuenchGranulation -->

    <owl:Class rdf:about="https://github.com/sustainable-processes/ontology/OntoCAPE/chemical_process_system/CPS_function/process_extensionTGL25001.owl#QuenchGranulation">
        <rdfs:subClassOf rdf:resource="https://github.com/sustainable-processes/ontology/OntoCAPE/chemical_process_system/CPS_function/process.owl#Fragmentation"/>
        <rdfs:comment>Fragmentation of a melt by rapid solidifaction, which causes internal stresses.</rdfs:comment>
    </owl:Class>
    


    <!-- https://github.com/sustainable-processes/ontology/OntoCAPE/chemical_process_system/CPS_function/process_extensionTGL25001.owl#Rectification -->

    <owl:Class rdf:about="https://github.com/sustainable-processes/ontology/OntoCAPE/chemical_process_system/CPS_function/process_extensionTGL25001.owl#Rectification">
        <rdfs:subClassOf rdf:resource="https://github.com/sustainable-processes/ontology/OntoCAPE/chemical_process_system/CPS_function/process.owl#Separation"/>
        <rdfs:comment>Rectification is the separation of the constituents of a liquid mixture by successive distillations (partial vaporizations and condensations) and is obtained via the use of an integral of differential process. (Perry)</rdfs:comment>
    </owl:Class>
    


    <!-- https://github.com/sustainable-processes/ontology/OntoCAPE/chemical_process_system/CPS_function/process_extensionTGL25001.owl#Scrubbing -->

    <owl:Class rdf:about="https://github.com/sustainable-processes/ontology/OntoCAPE/chemical_process_system/CPS_function/process_extensionTGL25001.owl#Scrubbing">
        <rdfs:subClassOf rdf:resource="https://github.com/sustainable-processes/ontology/OntoCAPE/chemical_process_system/CPS_function/process.owl#Separation"/>
        <rdfs:comment>The separation of dispersed particels from a gas phase by suspensing or solving the particles in a liquid phase.</rdfs:comment>
    </owl:Class>
    


    <!-- https://github.com/sustainable-processes/ontology/OntoCAPE/chemical_process_system/CPS_function/process_extensionTGL25001.owl#Shredding -->

    <owl:Class rdf:about="https://github.com/sustainable-processes/ontology/OntoCAPE/chemical_process_system/CPS_function/process_extensionTGL25001.owl#Shredding">
        <rdfs:subClassOf rdf:resource="https://github.com/sustainable-processes/ontology/OntoCAPE/chemical_process_system/CPS_function/process.owl#Fragmentation"/>
        <rdfs:comment>The fragmentation of fibrous materials by the effect of tensile forces.</rdfs:comment>
    </owl:Class>
    


    <!-- https://github.com/sustainable-processes/ontology/OntoCAPE/chemical_process_system/CPS_function/process_extensionTGL25001.owl#Sintering -->

    <owl:Class rdf:about="https://github.com/sustainable-processes/ontology/OntoCAPE/chemical_process_system/CPS_function/process_extensionTGL25001.owl#Sintering">
        <rdfs:subClassOf rdf:resource="https://github.com/sustainable-processes/ontology/OntoCAPE/chemical_process_system/CPS_function/process.owl#Combination"/>
        <rdfs:comment>The heating of a mass of fine particles below the melting point, causing agglomeration to form larger particles. 
(www.mim.com.au/glossary.html)</rdfs:comment>
    </owl:Class>
    


    <!-- https://github.com/sustainable-processes/ontology/OntoCAPE/chemical_process_system/CPS_function/process_extensionTGL25001.owl#Solidification -->

    <owl:Class rdf:about="https://github.com/sustainable-processes/ontology/OntoCAPE/chemical_process_system/CPS_function/process_extensionTGL25001.owl#Solidification">
        <rdfs:subClassOf rdf:resource="https://github.com/sustainable-processes/ontology/OntoCAPE/chemical_process_system/CPS_function/process_extensionTGL25001.owl#PhaseChangeOfLiquids"/>
        <rdfs:comment>The phase transition from liquid to solid.</rdfs:comment>
    </owl:Class>
    


    <!-- https://github.com/sustainable-processes/ontology/OntoCAPE/chemical_process_system/CPS_function/process_extensionTGL25001.owl#SonicGasCleaning -->

    <owl:Class rdf:about="https://github.com/sustainable-processes/ontology/OntoCAPE/chemical_process_system/CPS_function/process_extensionTGL25001.owl#SonicGasCleaning">
        <rdfs:subClassOf rdf:resource="https://github.com/sustainable-processes/ontology/OntoCAPE/chemical_process_system/CPS_function/process.owl#Separation"/>
        <rdfs:comment>Separation procedure based on the coagulation of small particles suspended in a fluid medium into larger aggregates by the action of sound waves.</rdfs:comment>
    </owl:Class>
    


    <!-- https://github.com/sustainable-processes/ontology/OntoCAPE/chemical_process_system/CPS_function/process_extensionTGL25001.owl#Spraying -->

    <owl:Class rdf:about="https://github.com/sustainable-processes/ontology/OntoCAPE/chemical_process_system/CPS_function/process_extensionTGL25001.owl#Spraying">
        <rdfs:subClassOf rdf:resource="https://github.com/sustainable-processes/ontology/OntoCAPE/chemical_process_system/CPS_function/process.owl#Fragmentation"/>
        <rdfs:comment>The process of dispersing liquid droplets in a gas phase.</rdfs:comment>
    </owl:Class>
    


    <!-- https://github.com/sustainable-processes/ontology/OntoCAPE/chemical_process_system/CPS_function/process_extensionTGL25001.owl#Sublimation -->

    <owl:Class rdf:about="https://github.com/sustainable-processes/ontology/OntoCAPE/chemical_process_system/CPS_function/process_extensionTGL25001.owl#Sublimation">
        <rdfs:subClassOf rdf:resource="https://github.com/sustainable-processes/ontology/OntoCAPE/chemical_process_system/CPS_function/process_extensionTGL25001.owl#PhaseChangeOfSolids"/>
        <rdfs:comment>The phase transition from solid to gas without passing through an intermediate liquid state.</rdfs:comment>
    </owl:Class>
    


    <!-- https://github.com/sustainable-processes/ontology/OntoCAPE/chemical_process_system/CPS_function/process_extensionTGL25001.owl#Suspending -->

    <owl:Class rdf:about="https://github.com/sustainable-processes/ontology/OntoCAPE/chemical_process_system/CPS_function/process_extensionTGL25001.owl#Suspending">
        <rdfs:subClassOf rdf:resource="https://github.com/sustainable-processes/ontology/OntoCAPE/chemical_process_system/CPS_function/process.owl#Combination"/>
        <rdfs:comment>The process of preparing a mixture in which fine particles are suspended in a fluid, where they are supported by buoyancy.</rdfs:comment>
    </owl:Class>
    


    <!-- https://github.com/sustainable-processes/ontology/OntoCAPE/chemical_process_system/CPS_function/process_extensionTGL25001.owl#Tabletting -->

    <owl:Class rdf:about="https://github.com/sustainable-processes/ontology/OntoCAPE/chemical_process_system/CPS_function/process_extensionTGL25001.owl#Tabletting">
        <rdfs:subClassOf rdf:resource="https://github.com/sustainable-processes/ontology/OntoCAPE/chemical_process_system/CPS_function/process.owl#Combination"/>
        <rdfs:comment>The process of preparing a small flat compressed cake of some powder by means of high pressure.</rdfs:comment>
    </owl:Class>
    


    <!-- https://github.com/sustainable-processes/ontology/OntoCAPE/chemical_process_system/CPS_function/process_extensionTGL25001.owl#TemperatureChangeOfGases -->

    <owl:Class rdf:about="https://github.com/sustainable-processes/ontology/OntoCAPE/chemical_process_system/CPS_function/process_extensionTGL25001.owl#TemperatureChangeOfGases">
        <rdfs:subClassOf rdf:resource="https://github.com/sustainable-processes/ontology/OntoCAPE/chemical_process_system/CPS_function/process.owl#TemperatureChange"/>
    </owl:Class>
    


    <!-- https://github.com/sustainable-processes/ontology/OntoCAPE/chemical_process_system/CPS_function/process_extensionTGL25001.owl#TemperatureChangeOfLiquids -->

    <owl:Class rdf:about="https://github.com/sustainable-processes/ontology/OntoCAPE/chemical_process_system/CPS_function/process_extensionTGL25001.owl#TemperatureChangeOfLiquids">
        <rdfs:subClassOf rdf:resource="https://github.com/sustainable-processes/ontology/OntoCAPE/chemical_process_system/CPS_function/process.owl#TemperatureChange"/>
    </owl:Class>
    


    <!-- https://github.com/sustainable-processes/ontology/OntoCAPE/chemical_process_system/CPS_function/process_extensionTGL25001.owl#TemperatureChangeOfSolids -->

    <owl:Class rdf:about="https://github.com/sustainable-processes/ontology/OntoCAPE/chemical_process_system/CPS_function/process_extensionTGL25001.owl#TemperatureChangeOfSolids">
        <rdfs:subClassOf rdf:resource="https://github.com/sustainable-processes/ontology/OntoCAPE/chemical_process_system/CPS_function/process.owl#TemperatureChange"/>
    </owl:Class>
    


    <!-- https://github.com/sustainable-processes/ontology/OntoCAPE/chemical_process_system/CPS_function/process_extensionTGL25001.owl#ThermalCrushing -->

    <owl:Class rdf:about="https://github.com/sustainable-processes/ontology/OntoCAPE/chemical_process_system/CPS_function/process_extensionTGL25001.owl#ThermalCrushing">
        <rdfs:subClassOf rdf:resource="https://github.com/sustainable-processes/ontology/OntoCAPE/chemical_process_system/CPS_function/process.owl#Fragmentation"/>
        <rdfs:comment>The process of crushing solid material by applying temperature differences that cause internal stresses.</rdfs:comment>
    </owl:Class>
    


    <!-- https://github.com/sustainable-processes/ontology/OntoCAPE/chemical_process_system/CPS_function/process_extensionTGL25001.owl#Vaporization -->

    <owl:Class rdf:about="https://github.com/sustainable-processes/ontology/OntoCAPE/chemical_process_system/CPS_function/process_extensionTGL25001.owl#Vaporization">
        <rdfs:subClassOf rdf:resource="https://github.com/sustainable-processes/ontology/OntoCAPE/chemical_process_system/CPS_function/process_extensionTGL25001.owl#PhaseChangeOfLiquids"/>
        <rdfs:comment>The phase transition from liquid to gas. </rdfs:comment>
    </owl:Class>
</rdf:RDF>



<!-- Generated by the OWL API (version 4.5.26.2023-07-17T20:34:13Z) https://github.com/owlcs/owlapi -->

